@prefix : <http://w3.id.org/def/BiomassOntology#> .
@prefix owl: <http://www.w3.org/2002/07/owl#> .
@prefix rdf: <http://www.w3.org/1999/02/22-rdf-syntax-ns#> .
@prefix xml: <http://www.w3.org/XML/1998/namespace> .
@prefix xsd: <http://www.w3.org/2001/XMLSchema#> .
@prefix rdfs: <http://www.w3.org/2000/01/rdf-schema#> .
@base <http://w3.id.org/def/BiomassOntology#> .

<http://w3.id.org/def/BiomassOntology> rdf:type owl:Ontology ;
                                        <http://purl.org/dc/elements/1.1/description> """Biomass Ontology has been created to model information about biomass, biofuels and their properties.

The general goal of the Biomass Ontology is to create a usable platform for storing information about the different biofuels on the market. Each biofuel comes from a type of biomass. Each Biofuel is the object of several Observations, where a Sensor measures one of the Observable Properties of the Biofuel. The values of the Observations are classified in a category of the Result class."""@en ;
                                        <http://purl.org/dc/terms/creator> "Álvaro González Berdasco"@en ;
                                        <http://purl.org/dc/terms/date> "16/06/2023"@en ;
                                        <http://purl.org/dc/terms/title> "Biomass Ontology"@en ;
                                        rdfs:comment "Biomass Ontology has been created as part of the \"Universidad Politécnica de Madrid\" Computational Biology Master Thesis."@en ;
                                        owl:versionInfo "Version 1.0 16 June 2023"@en .

#################################################################
#    Annotation properties
#################################################################

###  http://purl.org/dc/elements/1.1/description
<http://purl.org/dc/elements/1.1/description> rdf:type owl:AnnotationProperty .


###  http://purl.org/dc/terms/creator
<http://purl.org/dc/terms/creator> rdf:type owl:AnnotationProperty .


###  http://purl.org/dc/terms/date
<http://purl.org/dc/terms/date> rdf:type owl:AnnotationProperty .


###  http://purl.org/dc/terms/title
<http://purl.org/dc/terms/title> rdf:type owl:AnnotationProperty .


###  http://schema.org/domainIncludes
<http://schema.org/domainIncludes> rdf:type owl:AnnotationProperty .


###  http://schema.org/rangeIncludes
<http://schema.org/rangeIncludes> rdf:type owl:AnnotationProperty .


###  http://www.w3.org/2004/02/skos/core#altLabel
<http://www.w3.org/2004/02/skos/core#altLabel> rdf:type owl:AnnotationProperty ;
                                               rdfs:comment "The range of skos:altLabel is the class of RDF plain literals."@en ,
                                                            "skos:prefLabel, skos:altLabel and skos:hiddenLabel are pairwise disjoint properties."@en ;
                                               rdfs:isDefinedBy <http://www.w3.org/2004/02/skos/core> ;
                                               rdfs:label "alternative label"@en ;
                                               <http://www.w3.org/2004/02/skos/core#definition> "An alternative lexical label for a resource."@en ;
                                               <http://www.w3.org/2004/02/skos/core#example> "Acronyms, abbreviations, spelling variants, and irregular plural/singular forms may be included among the alternative labels for a concept. Mis-spelled terms are normally included as hidden labels (see skos:hiddenLabel)."@en ;
                                               rdfs:subPropertyOf rdfs:label .


###  http://www.w3.org/2004/02/skos/core#changeNote
<http://www.w3.org/2004/02/skos/core#changeNote> rdf:type owl:AnnotationProperty ;
                                                 rdfs:isDefinedBy <http://www.w3.org/2004/02/skos/core> ;
                                                 rdfs:label "change note"@en ;
                                                 <http://www.w3.org/2004/02/skos/core#definition> "A note about a modification to a concept."@en ;
                                                 rdfs:subPropertyOf <http://www.w3.org/2004/02/skos/core#note> .


###  http://www.w3.org/2004/02/skos/core#definition
<http://www.w3.org/2004/02/skos/core#definition> rdf:type owl:AnnotationProperty ;
                                                 rdfs:isDefinedBy <http://www.w3.org/2004/02/skos/core> ;
                                                 rdfs:label "definition"@en ;
                                                 <http://www.w3.org/2004/02/skos/core#definition> "A statement or formal explanation of the meaning of a concept."@en ;
                                                 rdfs:subPropertyOf <http://www.w3.org/2004/02/skos/core#note> .


###  http://www.w3.org/2004/02/skos/core#editorialNote
<http://www.w3.org/2004/02/skos/core#editorialNote> rdf:type owl:AnnotationProperty ;
                                                    rdfs:isDefinedBy <http://www.w3.org/2004/02/skos/core> ;
                                                    rdfs:label "editorial note"@en ;
                                                    <http://www.w3.org/2004/02/skos/core#definition> "A note for an editor, translator or maintainer of the vocabulary."@en ;
                                                    rdfs:subPropertyOf <http://www.w3.org/2004/02/skos/core#note> .


###  http://www.w3.org/2004/02/skos/core#example
<http://www.w3.org/2004/02/skos/core#example> rdf:type owl:AnnotationProperty ;
                                              rdfs:isDefinedBy <http://www.w3.org/2004/02/skos/core> ;
                                              rdfs:label "example"@en ;
                                              <http://www.w3.org/2004/02/skos/core#definition> "An example of the use of a concept."@en ;
                                              rdfs:subPropertyOf <http://www.w3.org/2004/02/skos/core#note> .


###  http://www.w3.org/2004/02/skos/core#hiddenLabel
<http://www.w3.org/2004/02/skos/core#hiddenLabel> rdf:type owl:AnnotationProperty ;
                                                  rdfs:comment "The range of skos:hiddenLabel is the class of RDF plain literals."@en ,
                                                               "skos:prefLabel, skos:altLabel and skos:hiddenLabel are pairwise disjoint properties."@en ;
                                                  rdfs:isDefinedBy <http://www.w3.org/2004/02/skos/core> ;
                                                  rdfs:label "hidden label"@en ;
                                                  <http://www.w3.org/2004/02/skos/core#definition> "A lexical label for a resource that should be hidden when generating visual displays of the resource, but should still be accessible to free text search operations."@en ;
                                                  rdfs:subPropertyOf rdfs:label .


###  http://www.w3.org/2004/02/skos/core#historyNote
<http://www.w3.org/2004/02/skos/core#historyNote> rdf:type owl:AnnotationProperty ;
                                                  rdfs:isDefinedBy <http://www.w3.org/2004/02/skos/core> ;
                                                  rdfs:label "history note"@en ;
                                                  <http://www.w3.org/2004/02/skos/core#definition> "A note about the past state/use/meaning of a concept."@en ;
                                                  rdfs:subPropertyOf <http://www.w3.org/2004/02/skos/core#note> .


###  http://www.w3.org/2004/02/skos/core#note
<http://www.w3.org/2004/02/skos/core#note> rdf:type owl:AnnotationProperty ;
                                           rdfs:isDefinedBy <http://www.w3.org/2004/02/skos/core> ;
                                           rdfs:label "note"@en ;
                                           <http://www.w3.org/2004/02/skos/core#definition> "A general note, for any purpose."@en ;
                                           <http://www.w3.org/2004/02/skos/core#scopeNote> "This property may be used directly, or as a super-property for more specific note types."@en .


###  http://www.w3.org/2004/02/skos/core#prefLabel
<http://www.w3.org/2004/02/skos/core#prefLabel> rdf:type owl:AnnotationProperty ;
                                                rdfs:comment "A resource has no more than one value of skos:prefLabel per language tag, and no more than one value of skos:prefLabel without language tag."@en ,
                                                             "The range of skos:prefLabel is the class of RDF plain literals."@en ,
                                                             """skos:prefLabel, skos:altLabel and skos:hiddenLabel are pairwise
      disjoint properties."""@en ;
                                                rdfs:isDefinedBy <http://www.w3.org/2004/02/skos/core> ;
                                                rdfs:label "preferred label"@en ;
                                                <http://www.w3.org/2004/02/skos/core#definition> "The preferred lexical label for a resource, in a given language."@en ;
                                                rdfs:subPropertyOf rdfs:label .


###  http://www.w3.org/2004/02/skos/core#scopeNote
<http://www.w3.org/2004/02/skos/core#scopeNote> rdf:type owl:AnnotationProperty ;
                                                rdfs:isDefinedBy <http://www.w3.org/2004/02/skos/core> ;
                                                rdfs:label "scope note"@en ;
                                                <http://www.w3.org/2004/02/skos/core#definition> "A note that helps to clarify the meaning and/or the use of a concept."@en ;
                                                rdfs:subPropertyOf <http://www.w3.org/2004/02/skos/core#note> .


#################################################################
#    Object Properties
#################################################################

###  http://w3.id.org/def/BiomassOntology#biomassOf
:biomassOf rdf:type owl:ObjectProperty ;
           owl:inverseOf :fromBiomass ;
           rdfs:domain <http://www.w3.org/2004/02/skos/core#Concept> ;
           rdfs:range :Biofuel ;
           rdfs:comment "Relation between a type of biomass and the Biofuel that was created from it. Should have a skos:Concept belonging to BiomassScheme as domain."@en ;
           rdfs:label "biomass of"@en .


###  http://w3.id.org/def/BiomassOntology#fromBiomass
:fromBiomass rdf:type owl:ObjectProperty ;
             rdfs:domain :Biofuel ;
             rdfs:range <http://www.w3.org/2004/02/skos/core#Concept> ;
             rdfs:comment "Relation between a Biofuel and the type of biomass it comes from. Should have a skos:Concept belonging to BiomassScheme as range."@en ;
             rdfs:label "from biomass"@en .


###  http://www.w3.org/2004/02/skos/core#broader
<http://www.w3.org/2004/02/skos/core#broader> rdf:type owl:ObjectProperty ;
                                              rdfs:subPropertyOf <http://www.w3.org/2004/02/skos/core#broaderTransitive> ;
                                              owl:inverseOf <http://www.w3.org/2004/02/skos/core#narrower> ;
                                              rdfs:domain <http://www.w3.org/2004/02/skos/core#Concept> ;
                                              rdfs:range <http://www.w3.org/2004/02/skos/core#Concept> ;
                                              rdfs:comment "Broader concepts are typically rendered as parents in a concept hierarchy (tree)."@en ;
                                              rdfs:isDefinedBy <http://www.w3.org/2004/02/skos/core> ;
                                              rdfs:label "has broader"@en ;
                                              <http://www.w3.org/2004/02/skos/core#definition> "Relates a concept to a concept that is more general in meaning."@en ;
                                              <http://www.w3.org/2004/02/skos/core#scopeNote> "By convention, skos:broader is only used to assert an immediate (i.e. direct) hierarchical link between two conceptual resources."@en .


###  http://www.w3.org/2004/02/skos/core#broaderTransitive
<http://www.w3.org/2004/02/skos/core#broaderTransitive> rdf:type owl:ObjectProperty ;
                                                        rdfs:subPropertyOf <http://www.w3.org/2004/02/skos/core#semanticRelation> ;
                                                        owl:inverseOf <http://www.w3.org/2004/02/skos/core#narrowerTransitive> ;
                                                        rdf:type owl:TransitiveProperty ;
                                                        rdfs:domain <http://www.w3.org/2004/02/skos/core#Concept> ;
                                                        rdfs:range <http://www.w3.org/2004/02/skos/core#Concept> ;
                                                        rdfs:isDefinedBy <http://www.w3.org/2004/02/skos/core> ;
                                                        rdfs:label "has broader transitive"@en ;
                                                        <http://www.w3.org/2004/02/skos/core#definition> "skos:broaderTransitive is a transitive superproperty of skos:broader." ;
                                                        <http://www.w3.org/2004/02/skos/core#scopeNote> "By convention, skos:broaderTransitive is not used to make assertions. Rather, the properties can be used to draw inferences about the transitive closure of the hierarchical relation, which is useful e.g. when implementing a simple query expansion algorithm in a search application."@en .


###  http://www.w3.org/2004/02/skos/core#hasTopConcept
<http://www.w3.org/2004/02/skos/core#hasTopConcept> rdf:type owl:ObjectProperty ;
                                                    owl:inverseOf <http://www.w3.org/2004/02/skos/core#topConceptOf> ;
                                                    rdfs:domain <http://www.w3.org/2004/02/skos/core#ConceptScheme> ;
                                                    rdfs:range <http://www.w3.org/2004/02/skos/core#Concept> ;
                                                    rdfs:isDefinedBy <http://www.w3.org/2004/02/skos/core> ;
                                                    rdfs:label "has top concept"@en ;
                                                    <http://www.w3.org/2004/02/skos/core#definition> "Relates, by convention, a concept scheme to a concept which is topmost in the broader/narrower concept hierarchies for that scheme, providing an entry point to these hierarchies."@en .


###  http://www.w3.org/2004/02/skos/core#inScheme
<http://www.w3.org/2004/02/skos/core#inScheme> rdf:type owl:ObjectProperty ;
                                               rdfs:range <http://www.w3.org/2004/02/skos/core#ConceptScheme> ;
                                               rdfs:isDefinedBy <http://www.w3.org/2004/02/skos/core> ;
                                               rdfs:label "is in scheme"@en ;
                                               <http://www.w3.org/2004/02/skos/core#definition> "Relates a resource (for example a concept) to a concept scheme in which it is included."@en ;
                                               <http://www.w3.org/2004/02/skos/core#scopeNote> "A concept may be a member of more than one concept scheme."@en .


###  http://www.w3.org/2004/02/skos/core#narrower
<http://www.w3.org/2004/02/skos/core#narrower> rdf:type owl:ObjectProperty ;
                                               rdfs:subPropertyOf <http://www.w3.org/2004/02/skos/core#narrowerTransitive> ;
                                               rdfs:domain <http://www.w3.org/2004/02/skos/core#Concept> ;
                                               rdfs:range <http://www.w3.org/2004/02/skos/core#Concept> ;
                                               rdfs:comment "Narrower concepts are typically rendered as children in a concept hierarchy (tree)."@en ;
                                               rdfs:isDefinedBy <http://www.w3.org/2004/02/skos/core> ;
                                               rdfs:label "has narrower"@en ;
                                               <http://www.w3.org/2004/02/skos/core#definition> "Relates a concept to a concept that is more specific in meaning."@en ;
                                               <http://www.w3.org/2004/02/skos/core#scopeNote> "By convention, skos:broader is only used to assert an immediate (i.e. direct) hierarchical link between two conceptual resources."@en .


###  http://www.w3.org/2004/02/skos/core#narrowerTransitive
<http://www.w3.org/2004/02/skos/core#narrowerTransitive> rdf:type owl:ObjectProperty ;
                                                         rdfs:subPropertyOf <http://www.w3.org/2004/02/skos/core#semanticRelation> ;
                                                         rdf:type owl:TransitiveProperty ;
                                                         rdfs:domain <http://www.w3.org/2004/02/skos/core#Concept> ;
                                                         rdfs:range <http://www.w3.org/2004/02/skos/core#Concept> ;
                                                         rdfs:isDefinedBy <http://www.w3.org/2004/02/skos/core> ;
                                                         rdfs:label "has narrower transitive"@en ;
                                                         <http://www.w3.org/2004/02/skos/core#definition> "skos:narrowerTransitive is a transitive superproperty of skos:narrower." ;
                                                         <http://www.w3.org/2004/02/skos/core#scopeNote> "By convention, skos:narrowerTransitive is not used to make assertions. Rather, the properties can be used to draw inferences about the transitive closure of the hierarchical relation, which is useful e.g. when implementing a simple query expansion algorithm in a search application."@en .


###  http://www.w3.org/2004/02/skos/core#semanticRelation
<http://www.w3.org/2004/02/skos/core#semanticRelation> rdf:type owl:ObjectProperty ;
                                                       rdfs:domain <http://www.w3.org/2004/02/skos/core#Concept> ;
                                                       rdfs:range <http://www.w3.org/2004/02/skos/core#Concept> ;
                                                       rdfs:isDefinedBy <http://www.w3.org/2004/02/skos/core> ;
                                                       rdfs:label "is in semantic relation with"@en ;
                                                       <http://www.w3.org/2004/02/skos/core#definition> "Links a concept to a concept related by meaning."@en ;
                                                       <http://www.w3.org/2004/02/skos/core#scopeNote> "This property should not be used directly, but as a super-property for all properties denoting a relationship of meaning between concepts."@en .


###  http://www.w3.org/2004/02/skos/core#topConceptOf
<http://www.w3.org/2004/02/skos/core#topConceptOf> rdf:type owl:ObjectProperty ;
                                                   rdfs:subPropertyOf <http://www.w3.org/2004/02/skos/core#inScheme> ;
                                                   rdfs:domain <http://www.w3.org/2004/02/skos/core#Concept> ;
                                                   rdfs:range <http://www.w3.org/2004/02/skos/core#ConceptScheme> ;
                                                   rdfs:isDefinedBy <http://www.w3.org/2004/02/skos/core> ;
                                                   rdfs:label "is top concept in scheme"@en ;
                                                   <http://www.w3.org/2004/02/skos/core#definition> "Relates a concept to the concept scheme that it is a top level concept of."@en .


###  http://www.w3.org/ns/sosa/hasFeatureOfInterest
<http://www.w3.org/ns/sosa/hasFeatureOfInterest> rdf:type owl:ObjectProperty ;
                                                 owl:inverseOf <http://www.w3.org/ns/sosa/isFeatureOfInterestOf> ;
                                                 rdfs:domain <http://www.w3.org/ns/sosa/Observation> ;
                                                 rdfs:range <http://www.w3.org/ns/sosa/FeatureOfInterest> ;
                                                 <http://schema.org/domainIncludes> <http://www.w3.org/ns/sosa/Actuation> ,
                                                                                    <http://www.w3.org/ns/sosa/Observation> ,
                                                                                    <http://www.w3.org/ns/sosa/Sampling> ;
                                                 <http://schema.org/rangeIncludes> <http://www.w3.org/ns/sosa/FeatureOfInterest> ;
                                                 rdfs:comment "A relation between an Observation and the entity whose quality was observed, or between an Actuation and the entity whose property was modified, or between an act of Sampling and the entity that was sampled."@en ;
                                                 rdfs:isDefinedBy <http://www.w3.org/ns/sosa/> ;
                                                 rdfs:label "has feature of interest"@en ;
                                                 <http://www.w3.org/2004/02/skos/core#definition> "A relation between an Observation and the entity whose quality was observed, or between an Actuation and the entity whose property was modified, or between an act of Sampling and the entity that was sampled."@en ;
                                                 <http://www.w3.org/2004/02/skos/core#example> "For example, in an Observation of the weight of a person, the FeatureOfInterest is the person and the property is its weight."@en .


###  http://www.w3.org/ns/sosa/hasResult
<http://www.w3.org/ns/sosa/hasResult> rdf:type owl:ObjectProperty ;
                                      owl:inverseOf <http://www.w3.org/ns/sosa/isResultOf> ;
                                      rdfs:domain <http://www.w3.org/ns/sosa/Observation> ;
                                      rdfs:range <http://www.w3.org/ns/sosa/Result> ;
                                      <http://schema.org/domainIncludes> <http://www.w3.org/ns/sosa/Actuation> ,
                                                                         <http://www.w3.org/ns/sosa/Observation> ,
                                                                         <http://www.w3.org/ns/sosa/Sampling> ;
                                      <http://schema.org/rangeIncludes> <http://www.w3.org/ns/sosa/Result> ;
                                      rdfs:comment "Relation linking an Observation or Actuation or act of Sampling and a Result or Sample."@en ;
                                      rdfs:isDefinedBy <http://www.w3.org/ns/sosa/> ;
                                      rdfs:label "has result"@en ;
                                      <http://www.w3.org/2004/02/skos/core#definition> "Relation linking an Observation or Actuation or act of Sampling and a Result or Sample."@en .


###  http://www.w3.org/ns/sosa/isFeatureOfInterestOf
<http://www.w3.org/ns/sosa/isFeatureOfInterestOf> rdf:type owl:ObjectProperty ;
                                                  rdfs:domain <http://www.w3.org/ns/sosa/FeatureOfInterest> ;
                                                  rdfs:range <http://www.w3.org/ns/sosa/Observation> ;
                                                  <http://schema.org/domainIncludes> <http://www.w3.org/ns/sosa/FeatureOfInterest> ;
                                                  <http://schema.org/rangeIncludes> <http://www.w3.org/ns/sosa/Actuation> ,
                                                                                    <http://www.w3.org/ns/sosa/Observation> ,
                                                                                    <http://www.w3.org/ns/sosa/Sampling> ;
                                                  rdfs:comment "A relation between a FeatureOfInterest and an Observation about it, an Actuation acting on it, or an act of Sampling that sampled it."@en ;
                                                  rdfs:isDefinedBy <http://www.w3.org/ns/sosa/> ;
                                                  rdfs:label "is feature of interest of"@en ;
                                                  <http://www.w3.org/2004/02/skos/core#definition> "A relation between a FeatureOfInterest and an Observation about it, an Actuation acting on it, or an act of Sampling that sampled it."@en .


###  http://www.w3.org/ns/sosa/isObservedBy
<http://www.w3.org/ns/sosa/isObservedBy> rdf:type owl:ObjectProperty ;
                                         owl:inverseOf <http://www.w3.org/ns/sosa/observes> ;
                                         rdfs:domain <http://www.w3.org/ns/sosa/ObservableProperty> ;
                                         rdfs:range <http://www.w3.org/ns/sosa/Sensor> ;
                                         <http://schema.org/domainIncludes> <http://www.w3.org/ns/sosa/ObservableProperty> ;
                                         <http://schema.org/rangeIncludes> <http://www.w3.org/ns/sosa/Sensor> ;
                                         rdfs:comment "Relation between an ObservableProperty and the Sensor able to observe it."@en ;
                                         rdfs:isDefinedBy <http://www.w3.org/ns/sosa/> ;
                                         rdfs:label "is observed by"@en ;
                                         <http://www.w3.org/2004/02/skos/core#definition> "Relation between an ObservableProperty and the Sensor able to observe it."@en .


###  http://www.w3.org/ns/sosa/isResultOf
<http://www.w3.org/ns/sosa/isResultOf> rdf:type owl:ObjectProperty ;
                                       rdfs:domain <http://www.w3.org/ns/sosa/Result> ;
                                       rdfs:range <http://www.w3.org/ns/sosa/Observation> ;
                                       <http://schema.org/domainIncludes> <http://www.w3.org/ns/sosa/Result> ;
                                       <http://schema.org/rangeIncludes> <http://www.w3.org/ns/sosa/Actuation> ,
                                                                         <http://www.w3.org/ns/sosa/Observation> ,
                                                                         <http://www.w3.org/ns/sosa/Sampling> ;
                                       rdfs:comment "Relation linking a Result to the Observation or Actuation or act of Sampling that created or caused it."@en ;
                                       rdfs:isDefinedBy <http://www.w3.org/ns/sosa/> ;
                                       rdfs:label "is result of"@en ;
                                       <http://www.w3.org/2004/02/skos/core#definition> "Relation linking a Result to the Observation or Actuation or act of Sampling that created or caused it."@en .


###  http://www.w3.org/ns/sosa/madeBySensor
<http://www.w3.org/ns/sosa/madeBySensor> rdf:type owl:ObjectProperty ;
                                         owl:inverseOf <http://www.w3.org/ns/sosa/madeObservation> ;
                                         rdfs:domain <http://www.w3.org/ns/sosa/Observation> ;
                                         rdfs:range <http://www.w3.org/ns/sosa/Sensor> ;
                                         <http://schema.org/domainIncludes> <http://www.w3.org/ns/sosa/Observation> ;
                                         <http://schema.org/rangeIncludes> <http://www.w3.org/ns/sosa/Sensor> ;
                                         rdfs:comment "Relation between an Observation and the Sensor which made the Observation."@en ;
                                         rdfs:isDefinedBy <http://www.w3.org/ns/sosa/> ;
                                         rdfs:label "made by sensor"@en ;
                                         <http://www.w3.org/2004/02/skos/core#definition> "Relation between an Observation and the Sensor which made the Observation."@en .


###  http://www.w3.org/ns/sosa/madeObservation
<http://www.w3.org/ns/sosa/madeObservation> rdf:type owl:ObjectProperty ;
                                            rdfs:domain <http://www.w3.org/ns/sosa/Sensor> ;
                                            rdfs:range <http://www.w3.org/ns/sosa/Observation> ;
                                            <http://schema.org/domainIncludes> <http://www.w3.org/ns/sosa/Sensor> ;
                                            <http://schema.org/rangeIncludes> <http://www.w3.org/ns/sosa/Observation> ;
                                            rdfs:comment "Relation between a Sensor and an Observation made by the Sensor."@en ;
                                            rdfs:isDefinedBy <http://www.w3.org/ns/sosa/> ;
                                            rdfs:label "made observation"@en ;
                                            <http://www.w3.org/2004/02/skos/core#definition> "Relation between a Sensor and an Observation made by the Sensor."@en .


###  http://www.w3.org/ns/sosa/observedProperty
<http://www.w3.org/ns/sosa/observedProperty> rdf:type owl:ObjectProperty ;
                                             rdfs:domain <http://www.w3.org/ns/sosa/Observation> ;
                                             rdfs:range <http://www.w3.org/ns/sosa/ObservableProperty> ;
                                             <http://schema.org/domainIncludes> <http://www.w3.org/ns/sosa/Observation> ;
                                             <http://schema.org/rangeIncludes> <http://www.w3.org/ns/sosa/ObservableProperty> ;
                                             rdfs:comment "Relation linking an Observation to the property that was observed. The ObservableProperty should be a property of the FeatureOfInterest (linked by hasFeatureOfInterest) of this Observation."@en ;
                                             rdfs:isDefinedBy <http://www.w3.org/ns/sosa/> ;
                                             rdfs:label "observed property"@en ;
                                             <http://www.w3.org/2004/02/skos/core#definition> "Relation linking an Observation to the property that was observed. The ObservableProperty should be a property of the FeatureOfInterest (linked by hasFeatureOfInterest) of this Observation."@en .


###  http://www.w3.org/ns/sosa/observes
<http://www.w3.org/ns/sosa/observes> rdf:type owl:ObjectProperty ;
                                     rdfs:subPropertyOf owl:topObjectProperty ;
                                     rdfs:domain <http://www.w3.org/ns/sosa/Sensor> ;
                                     rdfs:range <http://www.w3.org/ns/sosa/ObservableProperty> ;
                                     <http://schema.org/domainIncludes> <http://www.w3.org/ns/sosa/Sensor> ;
                                     <http://schema.org/rangeIncludes> <http://www.w3.org/ns/sosa/ObservableProperty> ;
                                     rdfs:comment "Relation between a Sensor and an ObservableProperty that it is capable of sensing."@en ;
                                     rdfs:isDefinedBy <http://www.w3.org/ns/sosa/> ;
                                     rdfs:label "observes"@en ;
                                     <http://www.w3.org/2004/02/skos/core#definition> "Relation between a Sensor and an ObservableProperty that it is capable of sensing."@en .


###  http://www.w3.org/ns/ssn/hasProperty
<http://www.w3.org/ns/ssn/hasProperty> rdf:type owl:ObjectProperty ;
                                       owl:inverseOf <http://www.w3.org/ns/ssn/isPropertyOf> ;
                                       rdfs:domain <http://www.w3.org/ns/sosa/FeatureOfInterest> ;
                                       rdfs:range <http://www.w3.org/ns/ssn/Property> ;
                                       rdfs:comment "Relation between an entity and a Property of that entity."@en ;
                                       rdfs:isDefinedBy <http://www.w3.org/ns/ssn/> ;
                                       rdfs:label "has property"@en ;
                                       <http://www.w3.org/2004/02/skos/core#definition> "Relation between an entity and a Property of that entity."@en .


###  http://www.w3.org/ns/ssn/isPropertyOf
<http://www.w3.org/ns/ssn/isPropertyOf> rdf:type owl:ObjectProperty ;
                                        rdfs:domain <http://www.w3.org/ns/ssn/Property> ;
                                        rdfs:range <http://www.w3.org/ns/sosa/FeatureOfInterest> ;
                                        rdfs:comment "Relation between a Property and the entity it belongs to."@en ;
                                        rdfs:isDefinedBy <http://www.w3.org/ns/ssn/> ;
                                        rdfs:label "is property of"@en ;
                                        <http://www.w3.org/2004/02/skos/core#definition> "Relation between a Property and the entity it belongs to."@en .


#################################################################
#    Data properties
#################################################################

###  http://www.w3.org/ns/sosa/hasSimpleResult
<http://www.w3.org/ns/sosa/hasSimpleResult> rdf:type owl:DatatypeProperty ;
                                            rdfs:domain <http://www.w3.org/ns/sosa/Observation> ;
                                            rdfs:range rdfs:Literal ;
                                            <http://schema.org/domainIncludes> <http://www.w3.org/ns/sosa/Actuation> ,
                                                                               <http://www.w3.org/ns/sosa/Observation> ,
                                                                               <http://www.w3.org/ns/sosa/Sampling> ;
                                            rdfs:comment "The simple value of an Observation or Actuation or act of Sampling."@en ;
                                            rdfs:isDefinedBy <http://www.w3.org/ns/sosa/> ;
                                            rdfs:label "has simple result"@en ;
                                            <http://www.w3.org/2004/02/skos/core#definition> "The simple value of an Observation or Actuation or act of Sampling."@en ;
                                            <http://www.w3.org/2004/02/skos/core#example> "For instance, the values 23 or true."@en .


###  http://www.w3.org/ns/sosa/resultTime
<http://www.w3.org/ns/sosa/resultTime> rdf:type owl:DatatypeProperty ;
                                       rdfs:domain <http://www.w3.org/ns/sosa/Observation> ;
                                       rdfs:range xsd:dateTime ;
                                       <http://schema.org/domainIncludes> <http://www.w3.org/ns/sosa/Actuation> ,
                                                                          <http://www.w3.org/ns/sosa/Observation> ,
                                                                          <http://www.w3.org/ns/sosa/Sampling> ;
                                       rdfs:comment "The result time is the instant of time when the Observation, Actuation or Sampling activity was completed."@en ;
                                       rdfs:isDefinedBy <http://www.w3.org/ns/sosa/> ;
                                       rdfs:label "result time"@en ;
                                       <http://www.w3.org/2004/02/skos/core#definition> "The result time is the instant of time when the Observation, Actuation or Sampling activity was completed."@en .


#################################################################
#    Classes
#################################################################

###  http://w3.id.org/def/BiomassOntology#AdditivesContent
:AdditivesContent rdf:type owl:Class ;
                  rdfs:subClassOf <http://www.w3.org/ns/sosa/ObservableProperty> ;
                  rdfs:comment "% in mass of additives"@en ;
                  rdfs:label "Additives Content"@en .


###  http://w3.id.org/def/BiomassOntology#Ash
:Ash rdf:type owl:Class ;
     rdfs:subClassOf <http://www.w3.org/ns/sosa/ObservableProperty> ;
     rdfs:comment "% in mass of ashes"@en ;
     rdfs:label "Ash"@en .


###  http://w3.id.org/def/BiomassOntology#AshMeltingBehaviour
:AshMeltingBehaviour rdf:type owl:Class ;
                     rdfs:subClassOf <http://www.w3.org/ns/sosa/ObservableProperty> ;
                     rdfs:comment "Deformation temperature (DT), hemisphere temperature (HT) and flow temperature (FT)"@en ;
                     rdfs:label "Ash Melting Behaviour"@en .


###  http://w3.id.org/def/BiomassOntology#Bale
:Bale rdf:type owl:Class ;
      owl:equivalentClass [ rdf:type owl:Restriction ;
                            owl:onProperty <http://www.w3.org/ns/sosa/isFeatureOfInterestOf> ;
                            owl:someValuesFrom [ rdf:type owl:Restriction ;
                                                 owl:onProperty <http://www.w3.org/ns/sosa/hasResult> ;
                                                 owl:allValuesFrom :BaleResult
                                               ]
                          ] ,
                          [ rdf:type owl:Restriction ;
                            owl:onProperty <http://www.w3.org/ns/ssn/hasProperty> ;
                            owl:allValuesFrom :BaleProperty
                          ] ;
      rdfs:subClassOf :Biofuel ,
                      <http://www.w3.org/ns/sosa/FeatureOfInterest> ;
      owl:disjointWith :Bark ,
                       :Briquette ,
                       :Charcoal ,
                       :EnergyGrain ,
                       :FruitSeeds ,
                       :LogFirewood ,
                       :OliveResidues ,
                       :Pellet ,
                       :Sawdust ,
                       :Shavings ,
                       :WoodChipsHogFuel ;
      rdfs:comment "Compacted and tightly bound bundle of material, typically agricultural products such as hay, straw, or cotton. It is formed by compressing the material and securing it with binding materials, such as twine or wire, to hold it in a dense, rectangular or cylindrical shape."@en ;
      rdfs:label "Bale"@en .


###  http://w3.id.org/def/BiomassOntology#BaleProperty
:BaleProperty rdf:type owl:Class ;
              owl:equivalentClass [ rdf:type owl:Restriction ;
                                    owl:onProperty <http://www.w3.org/ns/sosa/isObservedBy> ;
                                    owl:someValuesFrom [ rdf:type owl:Restriction ;
                                                         owl:onProperty <http://www.w3.org/ns/sosa/madeObservation> ;
                                                         owl:someValuesFrom [ rdf:type owl:Restriction ;
                                                                              owl:onProperty <http://www.w3.org/ns/sosa/hasResult> ;
                                                                              owl:allValuesFrom :BaleResult
                                                                            ]
                                                       ]
                                  ] ;
              rdfs:subClassOf <http://www.w3.org/ns/sosa/ObservableProperty> ;
              rdfs:comment "Properties of Bales"@en ;
              rdfs:label "Bale Property"@en .


###  http://w3.id.org/def/BiomassOntology#BaleResult
:BaleResult rdf:type owl:Class ;
            rdfs:subClassOf <http://www.w3.org/ns/sosa/Result> ;
            rdfs:comment "Result of an observation made on Bales"@en ;
            rdfs:label "Bale Result"@en .


###  http://w3.id.org/def/BiomassOntology#Bark
:Bark rdf:type owl:Class ;
      owl:equivalentClass [ rdf:type owl:Restriction ;
                            owl:onProperty <http://www.w3.org/ns/sosa/isFeatureOfInterestOf> ;
                            owl:someValuesFrom [ rdf:type owl:Restriction ;
                                                 owl:onProperty <http://www.w3.org/ns/sosa/hasResult> ;
                                                 owl:allValuesFrom :BarkResult
                                               ]
                          ] ,
                          [ rdf:type owl:Restriction ;
                            owl:onProperty <http://www.w3.org/ns/ssn/hasProperty> ;
                            owl:allValuesFrom :BarkProperty
                          ] ;
      rdfs:subClassOf :Biofuel ,
                      <http://www.w3.org/ns/sosa/FeatureOfInterest> ;
      owl:disjointWith :Briquette ,
                       :Charcoal ,
                       :EnergyGrain ,
                       :FruitSeeds ,
                       :LogFirewood ,
                       :OliveResidues ,
                       :Pellet ,
                       :Sawdust ,
                       :Shavings ,
                       :WoodChipsHogFuel ;
      rdfs:comment "Outer protective layer of a tree trunk and branches."@en ;
      rdfs:label "Bark"@en .


###  http://w3.id.org/def/BiomassOntology#BarkProperty
:BarkProperty rdf:type owl:Class ;
              owl:equivalentClass [ rdf:type owl:Restriction ;
                                    owl:onProperty <http://www.w3.org/ns/sosa/isObservedBy> ;
                                    owl:someValuesFrom [ rdf:type owl:Restriction ;
                                                         owl:onProperty <http://www.w3.org/ns/sosa/madeObservation> ;
                                                         owl:someValuesFrom [ rdf:type owl:Restriction ;
                                                                              owl:onProperty <http://www.w3.org/ns/sosa/hasResult> ;
                                                                              owl:allValuesFrom :BarkResult
                                                                            ]
                                                       ]
                                  ] ;
              rdfs:subClassOf <http://www.w3.org/ns/sosa/ObservableProperty> ;
              rdfs:comment "Properties of Bark"@en ;
              rdfs:label "Bark Property"@en .


###  http://w3.id.org/def/BiomassOntology#BarkResult
:BarkResult rdf:type owl:Class ;
            rdfs:subClassOf <http://www.w3.org/ns/sosa/Result> ;
            rdfs:comment "Result of an observation made on Bark"@en ;
            rdfs:label "Bark Result"@en .


###  http://w3.id.org/def/BiomassOntology#Biofuel
:Biofuel rdf:type owl:Class ;
         owl:equivalentClass [ rdf:type owl:Restriction ;
                               owl:onProperty :fromBiomass ;
                               owl:someValuesFrom [ owl:intersectionOf ( <http://www.w3.org/2004/02/skos/core#Concept>
                                                                         [ rdf:type owl:Restriction ;
                                                                           owl:onProperty <http://www.w3.org/2004/02/skos/core#inScheme> ;
                                                                           owl:hasValue :BiomassScheme
                                                                         ]
                                                                       ) ;
                                                    rdf:type owl:Class
                                                  ]
                             ] ;
         rdfs:comment "Type of fuel that is derived from renewable biological resources, such as plant matter or animal waste."@en ;
         rdfs:label "Biofuel"@en .


###  http://w3.id.org/def/BiomassOntology#Briquette
:Briquette rdf:type owl:Class ;
           owl:equivalentClass [ rdf:type owl:Restriction ;
                                 owl:onProperty <http://www.w3.org/ns/sosa/isFeatureOfInterestOf> ;
                                 owl:someValuesFrom [ rdf:type owl:Restriction ;
                                                      owl:onProperty <http://www.w3.org/ns/sosa/hasResult> ;
                                                      owl:allValuesFrom :BriquetteResult
                                                    ]
                               ] ,
                               [ rdf:type owl:Restriction ;
                                 owl:onProperty <http://www.w3.org/ns/ssn/hasProperty> ;
                                 owl:allValuesFrom :BriquetteProperty
                               ] ;
           rdfs:subClassOf :Biofuel ,
                           <http://www.w3.org/ns/sosa/FeatureOfInterest> ;
           owl:disjointWith :Charcoal ,
                            :EnergyGrain ,
                            :FruitSeeds ,
                            :LogFirewood ,
                            :OliveResidues ,
                            :Pellet ,
                            :Sawdust ,
                            :Shavings ,
                            :WoodChipsHogFuel ;
           rdfs:comment "Compacted block of combustible material typically used as a fuel source. It is formed by compressing biomass or other organic materials under high pressure without the use of binders or adhesives. The process of creating briquettes involves reducing the moisture content and compacting the material to form a dense and uniform block."@en ;
           rdfs:label "Briquette"@en .


###  http://w3.id.org/def/BiomassOntology#BriquetteProperty
:BriquetteProperty rdf:type owl:Class ;
                   owl:equivalentClass [ rdf:type owl:Restriction ;
                                         owl:onProperty <http://www.w3.org/ns/sosa/isObservedBy> ;
                                         owl:someValuesFrom [ rdf:type owl:Restriction ;
                                                              owl:onProperty <http://www.w3.org/ns/sosa/madeObservation> ;
                                                              owl:someValuesFrom [ rdf:type owl:Restriction ;
                                                                                   owl:onProperty <http://www.w3.org/ns/sosa/hasResult> ;
                                                                                   owl:allValuesFrom :BriquetteResult
                                                                                 ]
                                                            ]
                                       ] ;
                   rdfs:subClassOf <http://www.w3.org/ns/sosa/ObservableProperty> ;
                   rdfs:comment "Properties of Briquettes"@en ;
                   rdfs:label "Briquette Property"@en .


###  http://w3.id.org/def/BiomassOntology#BriquetteResult
:BriquetteResult rdf:type owl:Class ;
                 rdfs:subClassOf <http://www.w3.org/ns/sosa/Result> ;
                 rdfs:comment "Result of an observation made on Briquettes"@en ;
                 rdfs:label "Briquette Result"@en .


###  http://w3.id.org/def/BiomassOntology#BulkDensity
:BulkDensity rdf:type owl:Class ;
             rdfs:subClassOf :Density ;
             rdfs:comment "g/cm3 or kg/m3 of a material loosely packed or in a bulk state"@en ;
             rdfs:label "Bulk Density"@en .


###  http://w3.id.org/def/BiomassOntology#CalorificValue
:CalorificValue rdf:type owl:Class ;
                rdfs:subClassOf <http://www.w3.org/ns/sosa/ObservableProperty> ;
                rdfs:comment "MJ/kg or kWh/kg of energy content of a fuel"@en ;
                rdfs:label "Net Calorific Value"@en .


###  http://w3.id.org/def/BiomassOntology#Charcoal
:Charcoal rdf:type owl:Class ;
          owl:equivalentClass [ rdf:type owl:Restriction ;
                                owl:onProperty <http://www.w3.org/ns/sosa/isFeatureOfInterestOf> ;
                                owl:someValuesFrom [ rdf:type owl:Restriction ;
                                                     owl:onProperty <http://www.w3.org/ns/sosa/hasResult> ;
                                                     owl:allValuesFrom :CharcoalResult
                                                   ]
                              ] ,
                              [ rdf:type owl:Restriction ;
                                owl:onProperty <http://www.w3.org/ns/ssn/hasProperty> ;
                                owl:allValuesFrom :CharcoalProperty
                              ] ;
          rdfs:subClassOf :Biofuel ,
                          <http://www.w3.org/ns/sosa/FeatureOfInterest> ;
          owl:disjointWith :EnergyGrain ,
                           :FruitSeeds ,
                           :LogFirewood ,
                           :OliveResidues ,
                           :Pellet ,
                           :Sawdust ,
                           :Shavings ,
                           :WoodChipsHogFuel ;
          rdfs:comment "Black, porous, and lightweight carbon-rich material obtained by heating organic matter, such as wood, in the absence of oxygen."@en ;
          rdfs:label "Charcoal"@en .


###  http://w3.id.org/def/BiomassOntology#CharcoalProperty
:CharcoalProperty rdf:type owl:Class ;
                  owl:equivalentClass [ rdf:type owl:Restriction ;
                                        owl:onProperty <http://www.w3.org/ns/sosa/isObservedBy> ;
                                        owl:someValuesFrom [ rdf:type owl:Restriction ;
                                                             owl:onProperty <http://www.w3.org/ns/sosa/madeObservation> ;
                                                             owl:someValuesFrom [ rdf:type owl:Restriction ;
                                                                                  owl:onProperty <http://www.w3.org/ns/sosa/hasResult> ;
                                                                                  owl:allValuesFrom :CharcoalResult
                                                                                ]
                                                           ]
                                      ] ;
                  rdfs:subClassOf <http://www.w3.org/ns/sosa/ObservableProperty> ;
                  rdfs:comment "Properties of Charcoal"@en ;
                  rdfs:label "Charcoal Property"@en .


###  http://w3.id.org/def/BiomassOntology#CharcoalResult
:CharcoalResult rdf:type owl:Class ;
                rdfs:subClassOf <http://www.w3.org/ns/sosa/Result> ;
                rdfs:comment "Result of an observation made on Charcoal"@en ;
                rdfs:label "Charcoal Result"@en .


###  http://w3.id.org/def/BiomassOntology#Chlorine
:Chlorine rdf:type owl:Class ;
          rdfs:subClassOf <http://www.w3.org/ns/sosa/ObservableProperty> ;
          rdfs:comment "% in mass of chlorine"@en ;
          rdfs:label "Chlorine"@en .


###  http://w3.id.org/def/BiomassOntology#Density
:Density rdf:type owl:Class ;
         rdfs:subClassOf <http://www.w3.org/ns/sosa/ObservableProperty> ;
         rdfs:comment "g/cm3 or kg/m3 of a material"@en ;
         rdfs:label "Density"@en .


###  http://w3.id.org/def/BiomassOntology#Diameter
:Diameter rdf:type owl:Class ;
          rdfs:subClassOf :Dimensions ;
          rdfs:comment "m, cm or mm in diameter (D)"@en ;
          rdfs:label "Diameter"@en .


###  http://w3.id.org/def/BiomassOntology#Dimensions
:Dimensions rdf:type owl:Class ;
            rdfs:subClassOf <http://www.w3.org/ns/sosa/ObservableProperty> ;
            rdfs:comment "m, cm or mm size"@en ;
            rdfs:label "Dimensions"@en .


###  http://w3.id.org/def/BiomassOntology#EnergyGrain
:EnergyGrain rdf:type owl:Class ;
             owl:equivalentClass [ rdf:type owl:Restriction ;
                                   owl:onProperty <http://www.w3.org/ns/sosa/isFeatureOfInterestOf> ;
                                   owl:someValuesFrom [ rdf:type owl:Restriction ;
                                                        owl:onProperty <http://www.w3.org/ns/sosa/hasResult> ;
                                                        owl:allValuesFrom :EnergyGrainResult
                                                      ]
                                 ] ,
                                 [ rdf:type owl:Restriction ;
                                   owl:onProperty <http://www.w3.org/ns/ssn/hasProperty> ;
                                   owl:allValuesFrom :EnergyGrainProperty
                                 ] ;
             rdfs:subClassOf :Biofuel ,
                             <http://www.w3.org/ns/sosa/FeatureOfInterest> ;
             owl:disjointWith :FruitSeeds ,
                              :LogFirewood ,
                              :OliveResidues ,
                              :Pellet ,
                              :Sawdust ,
                              :Shavings ,
                              :WoodChipsHogFuel ;
             rdfs:comment "Specific types of crops or grains that are cultivated and used for the production of biofuels."@en ;
             rdfs:label "Energy Grain"@en .


###  http://w3.id.org/def/BiomassOntology#EnergyGrainProperty
:EnergyGrainProperty rdf:type owl:Class ;
                     owl:equivalentClass [ rdf:type owl:Restriction ;
                                           owl:onProperty <http://www.w3.org/ns/sosa/isObservedBy> ;
                                           owl:someValuesFrom [ rdf:type owl:Restriction ;
                                                                owl:onProperty <http://www.w3.org/ns/sosa/madeObservation> ;
                                                                owl:someValuesFrom [ rdf:type owl:Restriction ;
                                                                                     owl:onProperty <http://www.w3.org/ns/sosa/hasResult> ;
                                                                                     owl:allValuesFrom :EnergyGrainResult
                                                                                   ]
                                                              ]
                                         ] ;
                     rdfs:subClassOf <http://www.w3.org/ns/sosa/ObservableProperty> ;
                     rdfs:comment "Properties of Energy Grain"@en ;
                     rdfs:label "Energy Grain Property"@en .


###  http://w3.id.org/def/BiomassOntology#EnergyGrainResult
:EnergyGrainResult rdf:type owl:Class ;
                   rdfs:subClassOf <http://www.w3.org/ns/sosa/Result> ;
                   rdfs:comment "Result of an observation made on Energy Grain"@en ;
                   rdfs:label "Energy Grain Result"@en .


###  http://w3.id.org/def/BiomassOntology#FixedCarbon
:FixedCarbon rdf:type owl:Class ;
             rdfs:subClassOf <http://www.w3.org/ns/sosa/ObservableProperty> ;
             rdfs:comment "% in mass of fixed carbon"@en ;
             rdfs:label "Fixed Carbon"@en .


###  http://w3.id.org/def/BiomassOntology#FruitSeeds
:FruitSeeds rdf:type owl:Class ;
            owl:equivalentClass [ rdf:type owl:Restriction ;
                                  owl:onProperty <http://www.w3.org/ns/sosa/isFeatureOfInterestOf> ;
                                  owl:someValuesFrom [ rdf:type owl:Restriction ;
                                                       owl:onProperty <http://www.w3.org/ns/sosa/hasResult> ;
                                                       owl:allValuesFrom :FruitSeedsResult
                                                     ]
                                ] ,
                                [ rdf:type owl:Restriction ;
                                  owl:onProperty <http://www.w3.org/ns/ssn/hasProperty> ;
                                  owl:allValuesFrom :FruitSeedsProperty
                                ] ;
            rdfs:subClassOf :Biofuel ,
                            <http://www.w3.org/ns/sosa/FeatureOfInterest> ;
            owl:disjointWith :LogFirewood ,
                             :OliveResidues ,
                             :Pellet ,
                             :Sawdust ,
                             :Shavings ,
                             :WoodChipsHogFuel ;
            rdfs:comment "Seeds or kernels found within certain fruits that contain high levels of oil or fats."@en ;
            rdfs:label "Fruit Seeds"@en .


###  http://w3.id.org/def/BiomassOntology#FruitSeedsProperty
:FruitSeedsProperty rdf:type owl:Class ;
                    owl:equivalentClass [ rdf:type owl:Restriction ;
                                          owl:onProperty <http://www.w3.org/ns/sosa/isObservedBy> ;
                                          owl:someValuesFrom [ rdf:type owl:Restriction ;
                                                               owl:onProperty <http://www.w3.org/ns/sosa/madeObservation> ;
                                                               owl:someValuesFrom [ rdf:type owl:Restriction ;
                                                                                    owl:onProperty <http://www.w3.org/ns/sosa/hasResult> ;
                                                                                    owl:allValuesFrom :FruitSeedsResult
                                                                                  ]
                                                             ]
                                        ] ;
                    rdfs:subClassOf <http://www.w3.org/ns/sosa/ObservableProperty> ;
                    rdfs:comment "Properties of Fruit Seeds"@en ;
                    rdfs:label "Fruit Seeds Property"@en .


###  http://w3.id.org/def/BiomassOntology#FruitSeedsResult
:FruitSeedsResult rdf:type owl:Class ;
                  rdfs:subClassOf <http://www.w3.org/ns/sosa/Result> ;
                  rdfs:comment "Result of an observation made on Fruit Seeds"@en ;
                  rdfs:label "Fruit Seeds Result"@en .


###  http://w3.id.org/def/BiomassOntology#Height
:Height rdf:type owl:Class ;
        rdfs:subClassOf :Dimensions ;
        rdfs:comment "m, cm or mm high (L3)"@en ;
        rdfs:label "Height"@en .


###  http://w3.id.org/def/BiomassOntology#Length
:Length rdf:type owl:Class ;
        rdfs:subClassOf :Dimensions ;
        rdfs:comment "m, cm or mm long (L or L1)"@en ;
        rdfs:label "Length"@en .


###  http://w3.id.org/def/BiomassOntology#LogFirewood
:LogFirewood rdf:type owl:Class ;
             owl:equivalentClass [ rdf:type owl:Restriction ;
                                   owl:onProperty <http://www.w3.org/ns/sosa/isFeatureOfInterestOf> ;
                                   owl:someValuesFrom [ rdf:type owl:Restriction ;
                                                        owl:onProperty <http://www.w3.org/ns/sosa/hasResult> ;
                                                        owl:allValuesFrom :LogFirewoodResult
                                                      ]
                                 ] ,
                                 [ rdf:type owl:Restriction ;
                                   owl:onProperty <http://www.w3.org/ns/ssn/hasProperty> ;
                                   owl:allValuesFrom :LogFirewoodProperty
                                 ] ;
             rdfs:subClassOf :Biofuel ,
                             <http://www.w3.org/ns/sosa/FeatureOfInterest> ;
             owl:disjointWith :OliveResidues ,
                              :Pellet ,
                              :Sawdust ,
                              :Shavings ,
                              :WoodChipsHogFuel ;
             rdfs:comment """Log wood refers to large pieces of wood that are typically obtained from trees and are in their natural form, i.e., they have not been processed or cut into smaller pieces.
Firewood refers to wood that has been cut and prepared specifically for use as fuel in fires."""@en ;
             rdfs:label "Log Wood/Firewood"@en .


###  http://w3.id.org/def/BiomassOntology#LogFirewoodProperty
:LogFirewoodProperty rdf:type owl:Class ;
                     owl:equivalentClass [ rdf:type owl:Restriction ;
                                           owl:onProperty <http://www.w3.org/ns/sosa/isObservedBy> ;
                                           owl:someValuesFrom [ rdf:type owl:Restriction ;
                                                                owl:onProperty <http://www.w3.org/ns/sosa/madeObservation> ;
                                                                owl:someValuesFrom [ rdf:type owl:Restriction ;
                                                                                     owl:onProperty <http://www.w3.org/ns/sosa/hasResult> ;
                                                                                     owl:allValuesFrom :LogFirewoodResult
                                                                                   ]
                                                              ]
                                         ] ;
                     rdfs:subClassOf <http://www.w3.org/ns/sosa/ObservableProperty> ;
                     rdfs:comment "Properties of Log Wood and Firewood"@en ;
                     rdfs:label "Log Wood/Firewood Property"@en .


###  http://w3.id.org/def/BiomassOntology#LogFirewoodResult
:LogFirewoodResult rdf:type owl:Class ;
                   rdfs:subClassOf <http://www.w3.org/ns/sosa/Result> ;
                   rdfs:comment "Result of an observation made on Log Wood or Firewood"@en ;
                   rdfs:label "Log Wood/Firewood Result"@en .


###  http://w3.id.org/def/BiomassOntology#MechanicalDurability
:MechanicalDurability rdf:type owl:Class ;
                      rdfs:subClassOf <http://www.w3.org/ns/sosa/ObservableProperty> ;
                      rdfs:comment "% in mass of biofuel after testing"@en ;
                      rdfs:label "Mechanical Durability"@en .


###  http://w3.id.org/def/BiomassOntology#Moisture
:Moisture rdf:type owl:Class ;
          rdfs:subClassOf <http://www.w3.org/ns/sosa/ObservableProperty> ;
          rdfs:comment "% in mass of moisture"@en ;
          rdfs:label "Moisture"@en .


###  http://w3.id.org/def/BiomassOntology#Nitrogen
:Nitrogen rdf:type owl:Class ;
          rdfs:subClassOf <http://www.w3.org/ns/sosa/ObservableProperty> ;
          rdfs:comment "% in mass of nitrogen"@en ;
          rdfs:label "Nitrogen"@en .


###  http://w3.id.org/def/BiomassOntology#OliveResidues
:OliveResidues rdf:type owl:Class ;
               owl:equivalentClass [ rdf:type owl:Restriction ;
                                     owl:onProperty <http://www.w3.org/ns/sosa/isFeatureOfInterestOf> ;
                                     owl:someValuesFrom [ rdf:type owl:Restriction ;
                                                          owl:onProperty <http://www.w3.org/ns/sosa/hasResult> ;
                                                          owl:allValuesFrom :OliveResiduesResult
                                                        ]
                                   ] ,
                                   [ rdf:type owl:Restriction ;
                                     owl:onProperty <http://www.w3.org/ns/ssn/hasProperty> ;
                                     owl:allValuesFrom :OliveResiduesProperty
                                   ] ;
               rdfs:subClassOf :Biofuel ,
                               <http://www.w3.org/ns/sosa/FeatureOfInterest> ;
               owl:disjointWith :Pellet ,
                                :Sawdust ,
                                :Shavings ,
                                :WoodChipsHogFuel ;
               rdfs:comment "Byproducts and waste materials generated during the production of olive oil. These residues can include olive pomace, olive pits or stones, and olive mill wastewater (OMW)."@en ;
               rdfs:label "Olive Residues"@en .


###  http://w3.id.org/def/BiomassOntology#OliveResiduesProperty
:OliveResiduesProperty rdf:type owl:Class ;
                       owl:equivalentClass [ rdf:type owl:Restriction ;
                                             owl:onProperty <http://www.w3.org/ns/sosa/isObservedBy> ;
                                             owl:someValuesFrom [ rdf:type owl:Restriction ;
                                                                  owl:onProperty <http://www.w3.org/ns/sosa/madeObservation> ;
                                                                  owl:someValuesFrom [ rdf:type owl:Restriction ;
                                                                                       owl:onProperty <http://www.w3.org/ns/sosa/hasResult> ;
                                                                                       owl:allValuesFrom :OliveResiduesResult
                                                                                     ]
                                                                ]
                                           ] ;
                       rdfs:subClassOf <http://www.w3.org/ns/sosa/ObservableProperty> ;
                       rdfs:comment "Properties of Olive Residues"@en ;
                       rdfs:label "Olive Residues Property"@en .


###  http://w3.id.org/def/BiomassOntology#OliveResiduesResult
:OliveResiduesResult rdf:type owl:Class ;
                     rdfs:subClassOf <http://www.w3.org/ns/sosa/Result> ;
                     rdfs:comment "Result of an observation made on Olive Residues"@en ;
                     rdfs:label "Olive Residues Result"@en .


###  http://w3.id.org/def/BiomassOntology#Pellet
:Pellet rdf:type owl:Class ;
        owl:equivalentClass [ rdf:type owl:Restriction ;
                              owl:onProperty <http://www.w3.org/ns/sosa/isFeatureOfInterestOf> ;
                              owl:someValuesFrom [ rdf:type owl:Restriction ;
                                                   owl:onProperty <http://www.w3.org/ns/sosa/hasResult> ;
                                                   owl:allValuesFrom :PelletResult
                                                 ]
                            ] ,
                            [ rdf:type owl:Restriction ;
                              owl:onProperty <http://www.w3.org/ns/ssn/hasProperty> ;
                              owl:allValuesFrom :PelletProperty
                            ] ;
        rdfs:subClassOf :Biofuel ,
                        <http://www.w3.org/ns/sosa/FeatureOfInterest> ;
        owl:disjointWith :Sawdust ,
                         :Shavings ,
                         :WoodChipsHogFuel ;
        rdfs:comment "Small, cylindrical, and compacted form of biomass fuel. Pellets are commonly produced from various biomass materials, such as wood, agricultural residues, or energy crops."@en ;
        rdfs:label "Pellet"@en .


###  http://w3.id.org/def/BiomassOntology#PelletProperty
:PelletProperty rdf:type owl:Class ;
                owl:equivalentClass [ rdf:type owl:Restriction ;
                                      owl:onProperty <http://www.w3.org/ns/sosa/isObservedBy> ;
                                      owl:someValuesFrom [ rdf:type owl:Restriction ;
                                                           owl:onProperty <http://www.w3.org/ns/sosa/madeObservation> ;
                                                           owl:someValuesFrom [ rdf:type owl:Restriction ;
                                                                                owl:onProperty <http://www.w3.org/ns/sosa/hasResult> ;
                                                                                owl:allValuesFrom :PelletResult
                                                                              ]
                                                         ]
                                    ] ;
                rdfs:subClassOf <http://www.w3.org/ns/sosa/ObservableProperty> ;
                rdfs:comment "Properties of Pellets"@en ;
                rdfs:label "Pellet Property"@en .


###  http://w3.id.org/def/BiomassOntology#PelletResult
:PelletResult rdf:type owl:Class ;
              rdfs:subClassOf <http://www.w3.org/ns/sosa/Result> ;
              rdfs:comment "Result of an observation made on Pellets"@en ;
              rdfs:label "Pellet Result"@en .


###  http://w3.id.org/def/BiomassOntology#Sawdust
:Sawdust rdf:type owl:Class ;
         owl:equivalentClass [ rdf:type owl:Restriction ;
                               owl:onProperty <http://www.w3.org/ns/sosa/isFeatureOfInterestOf> ;
                               owl:someValuesFrom [ rdf:type owl:Restriction ;
                                                    owl:onProperty <http://www.w3.org/ns/sosa/hasResult> ;
                                                    owl:allValuesFrom :SawdustResult
                                                  ]
                             ] ,
                             [ rdf:type owl:Restriction ;
                               owl:onProperty <http://www.w3.org/ns/ssn/hasProperty> ;
                               owl:allValuesFrom :SawdustProperty
                             ] ;
         rdfs:subClassOf :Biofuel ,
                         <http://www.w3.org/ns/sosa/FeatureOfInterest> ;
         owl:disjointWith :Shavings ,
                          :WoodChipsHogFuel ;
         rdfs:comment "Powdery residue or small wood particles that are produced during the process of sawing or cutting wood."@en ;
         rdfs:label "Sawdust"@en .


###  http://w3.id.org/def/BiomassOntology#SawdustProperty
:SawdustProperty rdf:type owl:Class ;
                 owl:equivalentClass [ rdf:type owl:Restriction ;
                                       owl:onProperty <http://www.w3.org/ns/sosa/isObservedBy> ;
                                       owl:someValuesFrom [ rdf:type owl:Restriction ;
                                                            owl:onProperty <http://www.w3.org/ns/sosa/madeObservation> ;
                                                            owl:someValuesFrom [ rdf:type owl:Restriction ;
                                                                                 owl:onProperty <http://www.w3.org/ns/sosa/hasResult> ;
                                                                                 owl:allValuesFrom :SawdustResult
                                                                               ]
                                                          ]
                                     ] ;
                 rdfs:subClassOf <http://www.w3.org/ns/sosa/ObservableProperty> ;
                 rdfs:comment "Properties of Sawdust"@en ;
                 rdfs:label "Sawdust Property"@en .


###  http://w3.id.org/def/BiomassOntology#SawdustResult
:SawdustResult rdf:type owl:Class ;
               rdfs:subClassOf <http://www.w3.org/ns/sosa/Result> ;
               rdfs:comment "Result of an observation made on Sawdust"@en ;
               rdfs:label "Sawdust Result"@en .


###  http://w3.id.org/def/BiomassOntology#Shavings
:Shavings rdf:type owl:Class ;
          owl:equivalentClass [ rdf:type owl:Restriction ;
                                owl:onProperty <http://www.w3.org/ns/sosa/isFeatureOfInterestOf> ;
                                owl:someValuesFrom [ rdf:type owl:Restriction ;
                                                     owl:onProperty <http://www.w3.org/ns/sosa/hasResult> ;
                                                     owl:allValuesFrom :ShavingsResult
                                                   ]
                              ] ,
                              [ rdf:type owl:Restriction ;
                                owl:onProperty <http://www.w3.org/ns/ssn/hasProperty> ;
                                owl:allValuesFrom :ShavingsProperty
                              ] ;
          rdfs:subClassOf :Biofuel ,
                          <http://www.w3.org/ns/sosa/FeatureOfInterest> ;
          owl:disjointWith :WoodChipsHogFuel ;
          rdfs:comment "Small, thin, and elongated pieces of wood that are produced as byproducts of woodworking processes. Wood shavings are often generated during activities such as planing, shaping, or shaving wood."@en ;
          rdfs:label "Shavings"@en .


###  http://w3.id.org/def/BiomassOntology#ShavingsProperty
:ShavingsProperty rdf:type owl:Class ;
                  owl:equivalentClass [ rdf:type owl:Restriction ;
                                        owl:onProperty <http://www.w3.org/ns/sosa/isObservedBy> ;
                                        owl:someValuesFrom [ rdf:type owl:Restriction ;
                                                             owl:onProperty <http://www.w3.org/ns/sosa/madeObservation> ;
                                                             owl:someValuesFrom [ rdf:type owl:Restriction ;
                                                                                  owl:onProperty <http://www.w3.org/ns/sosa/hasResult> ;
                                                                                  owl:allValuesFrom :ShavingsResult
                                                                                ]
                                                           ]
                                      ] ;
                  rdfs:subClassOf <http://www.w3.org/ns/sosa/ObservableProperty> ;
                  rdfs:comment "Properties of Shavings"@en ;
                  rdfs:label "Shavings Property"@en .


###  http://w3.id.org/def/BiomassOntology#ShavingsResult
:ShavingsResult rdf:type owl:Class ;
                rdfs:subClassOf <http://www.w3.org/ns/sosa/Result> ;
                rdfs:comment "Result of an observation made on Shavings"@en ;
                rdfs:label "Shavings Result"@en .


###  http://w3.id.org/def/BiomassOntology#Sulfur
:Sulfur rdf:type owl:Class ;
        rdfs:subClassOf <http://www.w3.org/ns/sosa/ObservableProperty> ;
        rdfs:comment "% in mass of sulfur"@en ;
        rdfs:label "Sulfur"@en .


###  http://w3.id.org/def/BiomassOntology#Width
:Width rdf:type owl:Class ;
       rdfs:subClassOf :Dimensions ;
       rdfs:comment "m, cm or mm wide (L2)"@en ;
       rdfs:label "Width"@en .


###  http://w3.id.org/def/BiomassOntology#WoodChipsHogFuel
:WoodChipsHogFuel rdf:type owl:Class ;
                  owl:equivalentClass [ rdf:type owl:Restriction ;
                                        owl:onProperty <http://www.w3.org/ns/sosa/isFeatureOfInterestOf> ;
                                        owl:someValuesFrom [ rdf:type owl:Restriction ;
                                                             owl:onProperty <http://www.w3.org/ns/sosa/hasResult> ;
                                                             owl:allValuesFrom :WoodChipsHogFuelResult
                                                           ]
                                      ] ,
                                      [ rdf:type owl:Restriction ;
                                        owl:onProperty <http://www.w3.org/ns/ssn/hasProperty> ;
                                        owl:allValuesFrom :WoodChipsHogFuelProperty
                                      ] ;
                  rdfs:subClassOf :Biofuel ,
                                  <http://www.w3.org/ns/sosa/FeatureOfInterest> ;
                  rdfs:comment """Wood chips are small pieces or chunks of wood that are produced by chipping or shredding logs, branches, or other wood materials. They are typically larger in size compared to sawdust or shavings and can vary in shape and texture depending on the chipping process and equipment used.
Hog fuel refers to a type of coarse wood fuel that is commonly used in industrial processes. Hog fuel is typically a mixture of wood chips, bark, sawdust, and other wood residues. It is often derived from the byproducts of timber harvesting and processing."""@en ;
                  rdfs:label "Wood Chips/Hog Fuel"@en .


###  http://w3.id.org/def/BiomassOntology#WoodChipsHogFuelProperty
:WoodChipsHogFuelProperty rdf:type owl:Class ;
                          owl:equivalentClass [ rdf:type owl:Restriction ;
                                                owl:onProperty <http://www.w3.org/ns/sosa/isObservedBy> ;
                                                owl:someValuesFrom [ rdf:type owl:Restriction ;
                                                                     owl:onProperty <http://www.w3.org/ns/sosa/madeObservation> ;
                                                                     owl:someValuesFrom [ rdf:type owl:Restriction ;
                                                                                          owl:onProperty <http://www.w3.org/ns/sosa/hasResult> ;
                                                                                          owl:allValuesFrom :WoodChipsHogFuelResult
                                                                                        ]
                                                                   ]
                                              ] ;
                          rdfs:subClassOf <http://www.w3.org/ns/sosa/ObservableProperty> ;
                          rdfs:comment "Properties of Wood Chips and Hog Fuel"@en ;
                          rdfs:label "Wood Chips/Hog Fuel Property"@en .


###  http://w3.id.org/def/BiomassOntology#WoodChipsHogFuelResult
:WoodChipsHogFuelResult rdf:type owl:Class ;
                        rdfs:subClassOf <http://www.w3.org/ns/sosa/Result> ;
                        rdfs:comment "Result of an observation made on Wood Chips or Hog fuel"@en ;
                        rdfs:label "Wood Chips/Hog Fuel Result"@en .


###  http://www.w3.org/2004/02/skos/core#Concept
<http://www.w3.org/2004/02/skos/core#Concept> rdf:type owl:Class ;
                                              owl:disjointWith <http://www.w3.org/2004/02/skos/core#ConceptScheme> ;
                                              rdfs:isDefinedBy <http://www.w3.org/2004/02/skos/core> ;
                                              rdfs:label "Concept"@en ;
                                              <http://www.w3.org/2004/02/skos/core#definition> "An idea or notion; a unit of thought."@en .


###  http://www.w3.org/2004/02/skos/core#ConceptScheme
<http://www.w3.org/2004/02/skos/core#ConceptScheme> rdf:type owl:Class ;
                                                    rdfs:isDefinedBy <http://www.w3.org/2004/02/skos/core> ;
                                                    rdfs:label "Concept Scheme"@en ;
                                                    <http://www.w3.org/2004/02/skos/core#definition> "A set of concepts, optionally including statements about semantic relationships between those concepts."@en ;
                                                    <http://www.w3.org/2004/02/skos/core#example> "Thesauri, classification schemes, subject heading lists, taxonomies, 'folksonomies', and other types of controlled vocabulary are all examples of concept schemes. Concept schemes are also embedded in glossaries and terminologies."@en ;
                                                    <http://www.w3.org/2004/02/skos/core#scopeNote> "A concept scheme may be defined to include concepts from different sources."@en .


###  http://www.w3.org/ns/sosa/FeatureOfInterest
<http://www.w3.org/ns/sosa/FeatureOfInterest> rdf:type owl:Class ;
                                              rdfs:subClassOf [ rdf:type owl:Restriction ;
                                                                owl:onProperty <http://www.w3.org/ns/ssn/hasProperty> ;
                                                                owl:allValuesFrom <http://www.w3.org/ns/ssn/Property>
                                                              ] ,
                                                              [ rdf:type owl:Restriction ;
                                                                owl:onProperty <http://www.w3.org/ns/ssn/hasProperty> ;
                                                                owl:minCardinality "1"^^xsd:nonNegativeInteger
                                                              ] ;
                                              rdfs:comment "The thing whose property is being estimated or calculated in the course of an Observation to arrive at a Result or whose property is being manipulated by an Actuator, or which is being sampled or transformed in an act of Sampling."@en ;
                                              rdfs:isDefinedBy <http://www.w3.org/ns/sosa/> ;
                                              rdfs:label "Feature Of Interest"@en ;
                                              <http://www.w3.org/2004/02/skos/core#definition> "The thing whose property is being estimated or calculated in the course of an Observation to arrive at a Result or whose property is being manipulated by an Actuator, or which is being sampled or transformed in an act of Sampling."@en ;
                                              <http://www.w3.org/2004/02/skos/core#example> "When measuring the height of a tree, the height is the observed ObservableProperty, 20m may be the Result of the Observation, and the tree is the FeatureOfInterest. A window is a FeatureOfInterest for an automatic window control Actuator."@en .


###  http://www.w3.org/ns/sosa/ObservableProperty
<http://www.w3.org/ns/sosa/ObservableProperty> rdf:type owl:Class ;
                                               rdfs:subClassOf <http://www.w3.org/ns/ssn/Property> ,
                                                               [ rdf:type owl:Restriction ;
                                                                 owl:onProperty <http://www.w3.org/ns/sosa/isObservedBy> ;
                                                                 owl:allValuesFrom <http://www.w3.org/ns/sosa/Sensor>
                                                               ] ,
                                                               [ rdf:type owl:Restriction ;
                                                                 owl:onProperty [ owl:inverseOf <http://www.w3.org/ns/sosa/observedProperty>
                                                                                ] ;
                                                                 owl:allValuesFrom <http://www.w3.org/ns/sosa/Observation>
                                                               ] ;
                                               rdfs:comment "An observable quality (property, characteristic) of a FeatureOfInterest."@en ;
                                               rdfs:isDefinedBy <http://www.w3.org/ns/sosa/> ;
                                               rdfs:label "Observable Property"@en ;
                                               <http://www.w3.org/2004/02/skos/core#definition> "An observable quality (property, characteristic) of a FeatureOfInterest."@en ;
                                               <http://www.w3.org/2004/02/skos/core#example> "The height of a tree, the depth of a water body, or the temperature of a surface are examples of observable properties, while the value of a classic car is not (directly) observable but asserted."@en .


###  http://www.w3.org/ns/sosa/Observation
<http://www.w3.org/ns/sosa/Observation> rdf:type owl:Class ;
                                        rdfs:subClassOf [ rdf:type owl:Restriction ;
                                                          owl:onProperty <http://www.w3.org/ns/sosa/hasFeatureOfInterest> ;
                                                          owl:allValuesFrom <http://www.w3.org/ns/sosa/FeatureOfInterest>
                                                        ] ,
                                                        [ rdf:type owl:Restriction ;
                                                          owl:onProperty <http://www.w3.org/ns/sosa/hasResult> ;
                                                          owl:allValuesFrom <http://www.w3.org/ns/sosa/Result>
                                                        ] ,
                                                        [ rdf:type owl:Restriction ;
                                                          owl:onProperty <http://www.w3.org/ns/sosa/madeBySensor> ;
                                                          owl:allValuesFrom <http://www.w3.org/ns/sosa/Sensor>
                                                        ] ,
                                                        [ rdf:type owl:Restriction ;
                                                          owl:onProperty <http://www.w3.org/ns/sosa/observedProperty> ;
                                                          owl:allValuesFrom <http://www.w3.org/ns/sosa/ObservableProperty>
                                                        ] ,
                                                        [ rdf:type owl:Restriction ;
                                                          owl:onProperty <http://www.w3.org/ns/sosa/hasResult> ;
                                                          owl:minCardinality "1"^^xsd:nonNegativeInteger
                                                        ] ,
                                                        [ rdf:type owl:Restriction ;
                                                          owl:onProperty <http://www.w3.org/ns/sosa/hasFeatureOfInterest> ;
                                                          owl:cardinality "1"^^xsd:nonNegativeInteger
                                                        ] ,
                                                        [ rdf:type owl:Restriction ;
                                                          owl:onProperty <http://www.w3.org/ns/sosa/madeBySensor> ;
                                                          owl:cardinality "1"^^xsd:nonNegativeInteger
                                                        ] ,
                                                        [ rdf:type owl:Restriction ;
                                                          owl:onProperty <http://www.w3.org/ns/sosa/observedProperty> ;
                                                          owl:cardinality "1"^^xsd:nonNegativeInteger
                                                        ] ,
                                                        [ rdf:type owl:Restriction ;
                                                          owl:onProperty <http://www.w3.org/ns/sosa/resultTime> ;
                                                          owl:cardinality "1"^^xsd:nonNegativeInteger
                                                        ] ;
                                        rdfs:comment "Act of carrying out an (Observation) Procedure to estimate or calculate a value of a property of a FeatureOfInterest. Links to a Sensor to describe what made the Observation and how; links to an ObservableProperty to describe what the result is an estimate of, and to a FeatureOfInterest to detail what that property was associated with."@en ;
                                        rdfs:isDefinedBy <http://www.w3.org/ns/sosa/> ;
                                        rdfs:label "Observation"@en ;
                                        <http://www.w3.org/2004/02/skos/core#definition> "Act of carrying out an (Observation) Procedure to estimate or calculate a value of a property of a FeatureOfInterest. Links to a Sensor to describe what made the Observation and how; links to an ObservableProperty to describe what the result is an estimate of, and to a FeatureOfInterest to detail what that property was associated with."@en ;
                                        <http://www.w3.org/2004/02/skos/core#example> "The activity of estimating the intensity of an Earthquake using the Mercalli intensity scale is an Observation as is measuring the moment magnitude, i.e., the energy released by said earthquake."@en .


###  http://www.w3.org/ns/sosa/Result
<http://www.w3.org/ns/sosa/Result> rdf:type owl:Class ;
                                   rdfs:subClassOf [ rdf:type owl:Restriction ;
                                                     owl:onProperty <http://www.w3.org/ns/sosa/isResultOf> ;
                                                     owl:minCardinality "1"^^xsd:nonNegativeInteger
                                                   ] ;
                                   rdfs:comment "The Result of an Observation, Actuation, or act of Sampling. To store an observation's simple result value one can use the hasSimpleResult property."@en ;
                                   rdfs:isDefinedBy <http://www.w3.org/ns/sosa/> ;
                                   rdfs:label "Result"@en ;
                                   <http://www.w3.org/2004/02/skos/core#definition> "The Result of an Observation, Actuation, or act of Sampling. To store an observation's simple result value one can use the hasSimpleResult property."@en ;
                                   <http://www.w3.org/2004/02/skos/core#example> "The value 20 as the height of a certain tree together with the unit, e.g., Meter."@en .


###  http://www.w3.org/ns/sosa/Sensor
<http://www.w3.org/ns/sosa/Sensor> rdf:type owl:Class ;
                                   rdfs:subClassOf [ rdf:type owl:Restriction ;
                                                     owl:onProperty <http://www.w3.org/ns/sosa/madeObservation> ;
                                                     owl:allValuesFrom <http://www.w3.org/ns/sosa/Observation>
                                                   ] ,
                                                   [ rdf:type owl:Restriction ;
                                                     owl:onProperty <http://www.w3.org/ns/sosa/observes> ;
                                                     owl:allValuesFrom <http://www.w3.org/ns/sosa/ObservableProperty>
                                                   ] ;
                                   rdfs:comment "Device, agent (including humans), or software (simulation) involved in, or implementing, a Procedure. Sensors respond to a stimulus, e.g., a change in the environment, or input data composed from the results of prior Observations, and generate a Result. Sensors can be hosted by Platforms."@en ;
                                   rdfs:isDefinedBy <http://www.w3.org/ns/sosa/> ;
                                   rdfs:label "Sensor"@en ;
                                   <http://www.w3.org/2004/02/skos/core#definition> "Device, agent (including humans), or software (simulation) involved in, or implementing, a Procedure. Sensors respond to a stimulus, e.g., a change in the environment, or input data composed from the results of prior Observations, and generate a Result. Sensors can be hosted by Platforms."@en ;
                                   <http://www.w3.org/2004/02/skos/core#example> "Accelerometers, gyroscopes, barometers, magnetometers, and so forth are Sensors that are typically mounted on a modern smart phone (which acts as Platform). Other examples of sensors include the human eyes."@en .


###  http://www.w3.org/ns/ssn/Property
<http://www.w3.org/ns/ssn/Property> rdf:type owl:Class ;
                                    rdfs:subClassOf [ rdf:type owl:Restriction ;
                                                      owl:onProperty <http://www.w3.org/ns/ssn/isPropertyOf> ;
                                                      owl:allValuesFrom <http://www.w3.org/ns/sosa/FeatureOfInterest>
                                                    ] ;
                                    rdfs:comment "A quality of an entity. An aspect of an entity that is intrinsic to and cannot exist without the entity."@en ;
                                    rdfs:isDefinedBy <http://www.w3.org/ns/ssn/> ;
                                    rdfs:label "Property"@en ;
                                    <http://www.w3.org/2004/02/skos/core#definition> "A quality of an entity. An aspect of an entity that is intrinsic to and cannot exist without the entity."@en .


#################################################################
#    Individuals
#################################################################

###  http://w3.id.org/def/BiomassOntology#A0.5Briquette
:A0.5Briquette rdf:type owl:NamedIndividual ,
                        :BriquetteResult ;
               rdfs:comment "≤ 0,5 % in mass of ash in briquettes as received"@en ;
               rdfs:label "A0.5 Briquette"@en .


###  http://w3.id.org/def/BiomassOntology#A0.5Pellet
:A0.5Pellet rdf:type owl:NamedIndividual ,
                     :PelletResult ;
            rdfs:comment "≤ 0,5 % in mass of ash of dry basis in pellets"@en ;
            rdfs:label "A0.5 Pellet"@en .


###  http://w3.id.org/def/BiomassOntology#A0.5Sawdust
:A0.5Sawdust rdf:type owl:NamedIndividual ,
                      :SawdustResult ;
             rdfs:comment "≤ 0,5 % in mass of ash in sawdust of dry basis"@en ;
             rdfs:label "A0.5 Sawdust"@en .


###  http://w3.id.org/def/BiomassOntology#A0.5Shavings
:A0.5Shavings rdf:type owl:NamedIndividual ,
                       :ShavingsResult ;
              rdfs:comment "≤ 0,5 % in mass of ash of dry basis in shavings"@en ;
              rdfs:label "A0.5 Shavings"@en .


###  http://w3.id.org/def/BiomassOntology#A0.5WoodChipsHogFuel
:A0.5WoodChipsHogFuel rdf:type owl:NamedIndividual ,
                               :WoodChipsHogFuelResult ;
                      rdfs:comment "≤ 0,5 % in mass of ash in wood chips/hog fuel of dry basis"@en ;
                      rdfs:label "A0.5 Wood Chips/Hog Fuel"@en .


###  http://w3.id.org/def/BiomassOntology#A0.7Briquette
:A0.7Briquette rdf:type owl:NamedIndividual ,
                        :BriquetteResult ;
               rdfs:comment "≤ 0,7 % in mass of ash in briquettes as received"@en ;
               rdfs:label "A0.7 Briquette"@en .


###  http://w3.id.org/def/BiomassOntology#A0.7Pellet
:A0.7Pellet rdf:type owl:NamedIndividual ,
                     :PelletResult ;
            rdfs:comment "≤ 0,7 % in mass of ash of dry basis in pellets"@en ;
            rdfs:label "A0.7 Pellet"@en .


###  http://w3.id.org/def/BiomassOntology#A0.7Sawdust
:A0.7Sawdust rdf:type owl:NamedIndividual ,
                      :SawdustResult ;
             rdfs:comment "≤ 0,7 % in mass of ash in sawdust of dry basis"@en ;
             rdfs:label "A0.7 Sawdust"@en .


###  http://w3.id.org/def/BiomassOntology#A0.7Shavings
:A0.7Shavings rdf:type owl:NamedIndividual ,
                       :ShavingsResult ;
              rdfs:comment "≤ 0,7 % in mass of ash of dry basis in shavings"@en ;
              rdfs:label "A0.7 Shavings"@en .


###  http://w3.id.org/def/BiomassOntology#A0.7WoodChipsHogFuel
:A0.7WoodChipsHogFuel rdf:type owl:NamedIndividual ,
                               :WoodChipsHogFuelResult ;
                      rdfs:comment "≤ 0,7 % in mass of ash in wood chips/hog fuel of dry basis"@en ;
                      rdfs:label "A0.7 Wood Chips/Hog Fuel"@en .


###  http://w3.id.org/def/BiomassOntology#A1.2Pellet
:A1.2Pellet rdf:type owl:NamedIndividual ,
                     :PelletResult ;
            rdfs:comment "≤ 1,2 % in mass of ash of dry basis in pellets"@en ;
            rdfs:label "A1.2 Pellet"@en .


###  http://w3.id.org/def/BiomassOntology#A1.5Bark
:A1.5Bark rdf:type owl:NamedIndividual ,
                   :BarkResult ;
          rdfs:comment "≤ 1,5 % in mass of ash of dry basis in bark"@en ;
          rdfs:label "A1.5 Bark"@en .


###  http://w3.id.org/def/BiomassOntology#A1.5Briquette
:A1.5Briquette rdf:type owl:NamedIndividual ,
                        :BriquetteResult ;
               rdfs:comment "≤ 1,5 % in mass of ash in briquettes as received"@en ;
               rdfs:label "A1.5 Briquette"@en .


###  http://w3.id.org/def/BiomassOntology#A1.5FruitSeeds
:A1.5FruitSeeds rdf:type owl:NamedIndividual ,
                         :FruitSeedsResult ;
                rdfs:comment "≤ 1,5 % in mass of ash in fruit seeds of dry basis"@en ;
                rdfs:label "A1.5 FruitSeeds"@en .


###  http://w3.id.org/def/BiomassOntology#A1.5OliveResidues
:A1.5OliveResidues rdf:type owl:NamedIndividual ,
                            :OliveResiduesResult ;
                   rdfs:comment "≤ 1,5 % in mass of ash in olive residues of dry basis"@en ;
                   rdfs:label "A1.5 OliveResidues"@en .


###  http://w3.id.org/def/BiomassOntology#A1.5Pellet
:A1.5Pellet rdf:type owl:NamedIndividual ,
                     :PelletResult ;
            rdfs:comment "≤ 1,5 % in mass of ash of dry basis in pellets"@en ;
            rdfs:label "A1.5 Pellet"@en .


###  http://w3.id.org/def/BiomassOntology#A1.5Sawdust
:A1.5Sawdust rdf:type owl:NamedIndividual ,
                      :SawdustResult ;
             rdfs:comment "≤ 1,5 % in mass of ash in sawdust of dry basis"@en ;
             rdfs:label "A1.5 Sawdust"@en .


###  http://w3.id.org/def/BiomassOntology#A1.5Shavings
:A1.5Shavings rdf:type owl:NamedIndividual ,
                       :ShavingsResult ;
              rdfs:comment "≤ 1,5 % in mass of ash of dry basis in shavings"@en ;
              rdfs:label "A1.5 Shavings"@en .


###  http://w3.id.org/def/BiomassOntology#A1.5WoodChipsHogFuel
:A1.5WoodChipsHogFuel rdf:type owl:NamedIndividual ,
                               :WoodChipsHogFuelResult ;
                      rdfs:comment "≤ 1,5 % in mass of ash in wood chips/hog fuel of dry basis"@en ;
                      rdfs:label "A1.5 Wood Chips/Hog Fuel"@en .


###  http://w3.id.org/def/BiomassOntology#A10Bale
:A10Bale rdf:type owl:NamedIndividual ,
                  :BaleResult ;
         rdfs:comment "≤ 10 % in mass of ash of dry basis in bale"@en ;
         rdfs:label "A10.0 Bale"@en .


###  http://w3.id.org/def/BiomassOntology#A10Bark
:A10Bark rdf:type owl:NamedIndividual ,
                  :BarkResult ;
         rdfs:comment "≤ 10,0 % in mass of ash of dry basis in bark"@en ;
         rdfs:label "A10.0 Bark"@en .


###  http://w3.id.org/def/BiomassOntology#A10Briquette
:A10Briquette rdf:type owl:NamedIndividual ,
                       :BriquetteResult ;
              rdfs:comment "≤ 10,0 % in mass of ash in briquettes as received"@en ;
              rdfs:label "A10.0 Briquette"@en .


###  http://w3.id.org/def/BiomassOntology#A10FruitSeeds
:A10FruitSeeds rdf:type owl:NamedIndividual ,
                        :FruitSeedsResult ;
               rdfs:comment "≤ 10,0 % in mass of ash in fruit seeds of dry basis"@en ;
               rdfs:label "A10.0 FruitSeeds"@en .


###  http://w3.id.org/def/BiomassOntology#A10OliveResidues
:A10OliveResidues rdf:type owl:NamedIndividual ,
                           :OliveResiduesResult ;
                  rdfs:comment "≤ 10,0 % in mass of ash in olive residues of dry basis"@en ;
                  rdfs:label "A10.0 OliveResidues"@en .


###  http://w3.id.org/def/BiomassOntology#A10Pellet
:A10Pellet rdf:type owl:NamedIndividual ,
                    :PelletResult ;
           rdfs:comment "≤ 10,0 % in mass of ash of dry basis in pellets"@en ;
           rdfs:label "A10.0 Pellet"@en .


###  http://w3.id.org/def/BiomassOntology#A10Sawdust
:A10Sawdust rdf:type owl:NamedIndividual ,
                     :SawdustResult ;
            rdfs:comment "≤ 10,0 % in mass of ash in sawdust of dry basis"@en ;
            rdfs:label "A10.0 Sawdust"@en .


###  http://w3.id.org/def/BiomassOntology#A10Shavings
:A10Shavings rdf:type owl:NamedIndividual ,
                      :ShavingsResult ;
             rdfs:comment "≤ 10,0 % in mass of ash of dry basis in shavings"@en ;
             rdfs:label "A10.0 Shavings"@en .


###  http://w3.id.org/def/BiomassOntology#A10WoodChipsHogFuel
:A10WoodChipsHogFuel rdf:type owl:NamedIndividual ,
                              :WoodChipsHogFuelResult ;
                     rdfs:comment "≤ 10,0 % in mass of ash in wood chips/hog fuel of dry basis"@en ;
                     rdfs:label "A10.0 Wood Chips/Hog Fuel"@en .


###  http://w3.id.org/def/BiomassOntology#A1Bark
:A1Bark rdf:type owl:NamedIndividual ,
                 :BarkResult ;
        rdfs:comment "≤ 1,0 % in mass of ash of dry basis in bark"@en ;
        rdfs:label "A1.0 Bark"@en .


###  http://w3.id.org/def/BiomassOntology#A1Briquette
:A1Briquette rdf:type owl:NamedIndividual ,
                      :BriquetteResult ;
             rdfs:comment "≤ 1,0 % in mass of ash in briquettes as received"@en ;
             rdfs:label "A1.0 Briquette"@en .


###  http://w3.id.org/def/BiomassOntology#A1Pellet
:A1Pellet rdf:type owl:NamedIndividual ,
                   :PelletResult ;
          rdfs:comment "≤ 1,0 % in mass of ash of dry basis in pellets"@en ;
          rdfs:label "A1.0 Pellet"@en .


###  http://w3.id.org/def/BiomassOntology#A1Sawdust
:A1Sawdust rdf:type owl:NamedIndividual ,
                    :SawdustResult ;
           rdfs:comment "≤ 1,0 % in mass of ash in sawdust of dry basis"@en ;
           rdfs:label "A1.0 Sawdust"@en .


###  http://w3.id.org/def/BiomassOntology#A1Shavings
:A1Shavings rdf:type owl:NamedIndividual ,
                     :ShavingsResult ;
            rdfs:comment "≤ 1,0 % in mass of ash of dry basis in shavings"@en ;
            rdfs:label "A1.0 Shavings"@en .


###  http://w3.id.org/def/BiomassOntology#A1WoodChipsHogFuel
:A1WoodChipsHogFuel rdf:type owl:NamedIndividual ,
                             :WoodChipsHogFuelResult ;
                    rdfs:comment "≤ 1,0 % in mass of ash in wood chips/hog fuel of dry basis"@en ;
                    rdfs:label "A1.0 Wood Chips/Hog Fuel"@en .


###  http://w3.id.org/def/BiomassOntology#A2Bark
:A2Bark rdf:type owl:NamedIndividual ,
                 :BarkResult ;
        rdfs:comment "≤ 2,0 % in mass of ash of dry basis in bark"@en ;
        rdfs:label "A2.0 Bark"@en .


###  http://w3.id.org/def/BiomassOntology#A2Briquette
:A2Briquette rdf:type owl:NamedIndividual ,
                      :BriquetteResult ;
             rdfs:comment "≤ 2,0 % in mass of ash in briquettes as received"@en ;
             rdfs:label "A2.0 Briquette"@en .


###  http://w3.id.org/def/BiomassOntology#A2EnergyGrain
:A2EnergyGrain rdf:type owl:NamedIndividual ,
                        :EnergyGrainResult ;
               rdfs:comment "≤ 2,0 % in mass of ash in energy grain of dry basis"@en ;
               rdfs:label "A2.0 EnergyGrain"@en .


###  http://w3.id.org/def/BiomassOntology#A2FruitSeeds
:A2FruitSeeds rdf:type owl:NamedIndividual ,
                       :FruitSeedsResult ;
              rdfs:comment "≤ 2,0 % in mass of ash in fruit seeds of dry basis"@en ;
              rdfs:label "A2.0 FruitSeeds"@en .


###  http://w3.id.org/def/BiomassOntology#A2OliveResidues
:A2OliveResidues rdf:type owl:NamedIndividual ,
                          :OliveResiduesResult ;
                 rdfs:comment "≤ 2,0 % in mass of ash in olive residues of dry basis"@en ;
                 rdfs:label "A2.0 OliveResidues"@en .


###  http://w3.id.org/def/BiomassOntology#A2Pellet
:A2Pellet rdf:type owl:NamedIndividual ,
                   :PelletResult ;
          rdfs:comment "≤ 2,0 % in mass of ash of dry basis in pellets"@en ;
          rdfs:label "A2.0 Pellet"@en .


###  http://w3.id.org/def/BiomassOntology#A2Sawdust
:A2Sawdust rdf:type owl:NamedIndividual ,
                    :SawdustResult ;
           rdfs:comment "≤ 2,0 % in mass of ash in sawdust of dry basis"@en ;
           rdfs:label "A2.0 Sawdust"@en .


###  http://w3.id.org/def/BiomassOntology#A2Shavings
:A2Shavings rdf:type owl:NamedIndividual ,
                     :ShavingsResult ;
            rdfs:comment "≤ 2,0 % in mass of ash of dry basis in shavings"@en ;
            rdfs:label "A2.0 Shavings"@en .


###  http://w3.id.org/def/BiomassOntology#A2WoodChipsHogFuel
:A2WoodChipsHogFuel rdf:type owl:NamedIndividual ,
                             :WoodChipsHogFuelResult ;
                    rdfs:comment "≤ 2,0 % in mass of ash in wood chips/hog fuel of dry basis"@en ;
                    rdfs:label "A2.0 Wood Chips/Hog Fuel"@en .


###  http://w3.id.org/def/BiomassOntology#A3Bale
:A3Bale rdf:type owl:NamedIndividual ,
                 :BaleResult ;
        rdfs:comment "≤ 3 % in mass of ash of dry basis in bale"@en ;
        rdfs:label "A3.0 Bale"@en .


###  http://w3.id.org/def/BiomassOntology#A3Bark
:A3Bark rdf:type owl:NamedIndividual ,
                 :BarkResult ;
        rdfs:comment "≤ 3,0 % in mass of ash of dry basis in bark"@en ;
        rdfs:label "A3.0 Bark"@en .


###  http://w3.id.org/def/BiomassOntology#A3Briquette
:A3Briquette rdf:type owl:NamedIndividual ,
                      :BriquetteResult ;
             rdfs:comment "≤ 3,0 % in mass of ash in briquettes as received"@en ;
             rdfs:label "A3.0 Briquette"@en .


###  http://w3.id.org/def/BiomassOntology#A3EnergyGrain
:A3EnergyGrain rdf:type owl:NamedIndividual ,
                        :EnergyGrainResult ;
               rdfs:comment "≤ 3,0 % in mass of ash in energy grain of dry basis"@en ;
               rdfs:label "A3.0 EnergyGrain"@en .


###  http://w3.id.org/def/BiomassOntology#A3FruitSeeds
:A3FruitSeeds rdf:type owl:NamedIndividual ,
                       :FruitSeedsResult ;
              rdfs:comment "≤ 3,0 % in mass of ash in fruit seeds of dry basis"@en ;
              rdfs:label "A3.0 FruitSeeds"@en .


###  http://w3.id.org/def/BiomassOntology#A3OliveResidues
:A3OliveResidues rdf:type owl:NamedIndividual ,
                          :OliveResiduesResult ;
                 rdfs:comment "≤ 3,0 % in mass of ash in olive residues of dry basis"@en ;
                 rdfs:label "A3.0 OliveResidues"@en .


###  http://w3.id.org/def/BiomassOntology#A3Pellet
:A3Pellet rdf:type owl:NamedIndividual ,
                   :PelletResult ;
          rdfs:comment "≤ 3,0 % in mass of ash of dry basis in pellets"@en ;
          rdfs:label "A3.0 Pellet"@en .


###  http://w3.id.org/def/BiomassOntology#A3Sawdust
:A3Sawdust rdf:type owl:NamedIndividual ,
                    :SawdustResult ;
           rdfs:comment "≤ 3,0 % in mass of ash in sawdust of dry basis"@en ;
           rdfs:label "A3.0 Sawdust"@en .


###  http://w3.id.org/def/BiomassOntology#A3Shavings
:A3Shavings rdf:type owl:NamedIndividual ,
                     :ShavingsResult ;
            rdfs:comment "≤ 3,0 % in mass of ash of dry basis in shavings"@en ;
            rdfs:label "A3.0 Shavings"@en .


###  http://w3.id.org/def/BiomassOntology#A3WoodChipsHogFuel
:A3WoodChipsHogFuel rdf:type owl:NamedIndividual ,
                             :WoodChipsHogFuelResult ;
                    rdfs:comment "≤ 3,0 % in mass of ash in wood chips/hog fuel of dry basis"@en ;
                    rdfs:label "A3.0 Wood Chips/Hog Fuel"@en .


###  http://w3.id.org/def/BiomassOntology#A4Bale
:A4Bale rdf:type owl:NamedIndividual ,
                 :BaleResult ;
        rdfs:comment "≤ 4 % in mass of ash of dry basis in bale"@en ;
        rdfs:label "A4.0 Bale"@en .


###  http://w3.id.org/def/BiomassOntology#A4Pellet
:A4Pellet rdf:type owl:NamedIndividual ,
                   :PelletResult ;
          rdfs:comment "≤ 4,0 % in mass of ash of dry basis in pellets"@en ;
          rdfs:label "A4.0 Pellet"@en .


###  http://w3.id.org/def/BiomassOntology#A5Bale
:A5Bale rdf:type owl:NamedIndividual ,
                 :BaleResult ;
        rdfs:comment "≤ 5 % in mass of ash of dry basis in bale"@en ;
        rdfs:label "A5.0 Bale"@en .


###  http://w3.id.org/def/BiomassOntology#A5Bark
:A5Bark rdf:type owl:NamedIndividual ,
                 :BarkResult ;
        rdfs:comment "≤ 5,0 % in mass of ash of dry basis in bark"@en ;
        rdfs:label "A5.0 Bark"@en .


###  http://w3.id.org/def/BiomassOntology#A5Briquette
:A5Briquette rdf:type owl:NamedIndividual ,
                      :BriquetteResult ;
             rdfs:comment "≤ 5,0 % in mass of ash in briquettes as received"@en ;
             rdfs:label "A5.0 Briquette"@en .


###  http://w3.id.org/def/BiomassOntology#A5Charcoal
:A5Charcoal rdf:type owl:NamedIndividual ,
                     :CharcoalResult ;
            rdfs:comment "≤ 5,0 % in mass of ash in charcoal of dry basis"@en ;
            rdfs:label "A5.0 Charcoal"@en .


###  http://w3.id.org/def/BiomassOntology#A5EnergyGrain
:A5EnergyGrain rdf:type owl:NamedIndividual ,
                        :EnergyGrainResult ;
               rdfs:comment "≤ 5,0 % in mass of ash in energy grain of dry basis"@en ;
               rdfs:label "A5.0 EnergyGrain"@en .


###  http://w3.id.org/def/BiomassOntology#A5FruitSeeds
:A5FruitSeeds rdf:type owl:NamedIndividual ,
                       :FruitSeedsResult ;
              rdfs:comment "≤ 5,0 % in mass of ash in fruit seeds of dry basis"@en ;
              rdfs:label "A5.0 FruitSeeds"@en .


###  http://w3.id.org/def/BiomassOntology#A5OliveResidues
:A5OliveResidues rdf:type owl:NamedIndividual ,
                          :OliveResiduesResult ;
                 rdfs:comment "≤ 5,0 % in mass of ash in olive residues of dry basis"@en ;
                 rdfs:label "A5.0 OliveResidues"@en .


###  http://w3.id.org/def/BiomassOntology#A5Pellet
:A5Pellet rdf:type owl:NamedIndividual ,
                   :PelletResult ;
          rdfs:comment "≤ 5,0 % in mass of ash of dry basis in pellets"@en ;
          rdfs:label "A5.0 Pellet"@en .


###  http://w3.id.org/def/BiomassOntology#A5Sawdust
:A5Sawdust rdf:type owl:NamedIndividual ,
                    :SawdustResult ;
           rdfs:comment "≤ 5,0 % in mass of ash in sawdust of dry basis"@en ;
           rdfs:label "A5.0 Sawdust"@en .


###  http://w3.id.org/def/BiomassOntology#A5Shavings
:A5Shavings rdf:type owl:NamedIndividual ,
                     :ShavingsResult ;
            rdfs:comment "≤ 5,0 % in mass of ash of dry basis in shavings"@en ;
            rdfs:label "A5.0 Shavings"@en .


###  http://w3.id.org/def/BiomassOntology#A5WoodChipsHogFuel
:A5WoodChipsHogFuel rdf:type owl:NamedIndividual ,
                             :WoodChipsHogFuelResult ;
                    rdfs:comment "≤ 5,0 % in mass of ash in wood chips/hog fuel of dry basis"@en ;
                    rdfs:label "A5.0 Wood Chips/Hog Fuel"@en .


###  http://w3.id.org/def/BiomassOntology#A6Bale
:A6Bale rdf:type owl:NamedIndividual ,
                 :BaleResult ;
        rdfs:comment "≤ 6 % in mass of ash of dry basis in bale"@en ;
        rdfs:label "A6.0 Bale"@en .


###  http://w3.id.org/def/BiomassOntology#A6Pellet
:A6Pellet rdf:type owl:NamedIndividual ,
                   :PelletResult ;
          rdfs:comment "≤ 6,0 % in mass of ash of dry basis in pellets"@en ;
          rdfs:label "A6.0 Pellet"@en .


###  http://w3.id.org/def/BiomassOntology#A7Bale
:A7Bale rdf:type owl:NamedIndividual ,
                 :BaleResult ;
        rdfs:comment "≤ 7 % in mass of ash of dry basis in bale"@en ;
        rdfs:label "A7.0 Bale"@en .


###  http://w3.id.org/def/BiomassOntology#A7Bark
:A7Bark rdf:type owl:NamedIndividual ,
                 :BarkResult ;
        rdfs:comment "≤ 7,0 % in mass of ash of dry basis in bark"@en ;
        rdfs:label "A7.0 Bark"@en .


###  http://w3.id.org/def/BiomassOntology#A7Briquette
:A7Briquette rdf:type owl:NamedIndividual ,
                      :BriquetteResult ;
             rdfs:comment "≤ 7,0 % in mass of ash in briquettes as received"@en ;
             rdfs:label "A7.0 Briquette"@en .


###  http://w3.id.org/def/BiomassOntology#A7FruitSeeds
:A7FruitSeeds rdf:type owl:NamedIndividual ,
                       :FruitSeedsResult ;
              rdfs:comment "≤ 7,0 % in mass of ash in fruit seeds of dry basis"@en ;
              rdfs:label "A7.0 FruitSeeds"@en .


###  http://w3.id.org/def/BiomassOntology#A7OliveResidues
:A7OliveResidues rdf:type owl:NamedIndividual ,
                          :OliveResiduesResult ;
                 rdfs:comment "≤ 7,0 % in mass of ash in olive residues of dry basis"@en ;
                 rdfs:label "A7.0 OliveResidues"@en .


###  http://w3.id.org/def/BiomassOntology#A7Pellet
:A7Pellet rdf:type owl:NamedIndividual ,
                   :PelletResult ;
          rdfs:comment "≤ 7,0 % in mass of ash of dry basis in pellets"@en ;
          rdfs:label "A7.0 Pellet"@en .


###  http://w3.id.org/def/BiomassOntology#A7Sawdust
:A7Sawdust rdf:type owl:NamedIndividual ,
                    :SawdustResult ;
           rdfs:comment "≤ 7,0 % in mass of ash in sawdust of dry basis"@en ;
           rdfs:label "A7.0 Sawdust"@en .


###  http://w3.id.org/def/BiomassOntology#A7Shavings
:A7Shavings rdf:type owl:NamedIndividual ,
                     :ShavingsResult ;
            rdfs:comment "≤ 7,0 % in mass of ash of dry basis in shavings"@en ;
            rdfs:label "A7.0 Shavings"@en .


###  http://w3.id.org/def/BiomassOntology#A7WoodChipsHogFuel
:A7WoodChipsHogFuel rdf:type owl:NamedIndividual ,
                             :WoodChipsHogFuelResult ;
                    rdfs:comment "≤ 7,0 % in mass of ash in wood chips/hog fuel of dry basis"@en ;
                    rdfs:label "A7.0 Wood Chips/Hog Fuel"@en .


###  http://w3.id.org/def/BiomassOntology#A8Bale
:A8Bale rdf:type owl:NamedIndividual ,
                 :BaleResult ;
        rdfs:comment "≤ 8 % in mass of ash of dry basis in bale"@en ;
        rdfs:label "A8.0 Bale"@en .


###  http://w3.id.org/def/BiomassOntology#A8Charcoal
:A8Charcoal rdf:type owl:NamedIndividual ,
                     :CharcoalResult ;
            rdfs:comment "≤ 8,0 % in mass of ash in charcoal of dry basis"@en ;
            rdfs:label "A8.0 Charcoal"@en .


###  http://w3.id.org/def/BiomassOntology#A8Pellet
:A8Pellet rdf:type owl:NamedIndividual ,
                   :PelletResult ;
          rdfs:comment "≤ 8,0 % in mass of ash of dry basis in pellets"@en ;
          rdfs:label "A8.0 Pellet"@en .


###  http://w3.id.org/def/BiomassOntology#BD100Bale
:BD100Bale rdf:type owl:NamedIndividual ,
                    :BaleResult ;
           rdfs:comment "≥ 100 kg/m3 bulk density of bale as received"@en ;
           rdfs:label "BD100 Bale"@en .


###  http://w3.id.org/def/BiomassOntology#BD100Sawdust
:BD100Sawdust rdf:type owl:NamedIndividual ,
                       :SawdustResult ;
              rdfs:comment "≥ 100 kg/m3 bulk density of sawdust as received"@en ;
              rdfs:label "BD100 Sawdust"@en .


###  http://w3.id.org/def/BiomassOntology#BD100Shavings
:BD100Shavings rdf:type owl:NamedIndividual ,
                        :ShavingsResult ;
               rdfs:comment "≥ 100 kg/m3 bulk density of shavings as received"@en ;
               rdfs:label "BD100 Shavings"@en .


###  http://w3.id.org/def/BiomassOntology#BD100WoodChipsHogFuel
:BD100WoodChipsHogFuel rdf:type owl:NamedIndividual ,
                                :WoodChipsHogFuelResult ;
                       rdfs:comment "≥ 100 kg/ m3 bulk density of wood chips/ hog fuel as received"@en ;
                       rdfs:label "BD100 Wood Chips/Hog Fuel"@en .


###  http://w3.id.org/def/BiomassOntology#BD120Bale
:BD120Bale rdf:type owl:NamedIndividual ,
                    :BaleResult ;
           rdfs:comment "≥ 120 kg/m3 bulk density of bale as received"@en ;
           rdfs:label "BD120 Bale"@en .


###  http://w3.id.org/def/BiomassOntology#BD130Charcoal
:BD130Charcoal rdf:type owl:NamedIndividual ,
                        :CharcoalResult ;
               rdfs:comment "≥ 130 kg/m3 bulk density of charcoal as received"@en ;
               rdfs:label "BD130 Charcoal"@en .


###  http://w3.id.org/def/BiomassOntology#BD150Charcoal
:BD150Charcoal rdf:type owl:NamedIndividual ,
                        :CharcoalResult ;
               rdfs:comment "≥ 150 kg/m3 bulk density of charcoal as received"@en ;
               rdfs:label "BD150 Charcoal"@en .


###  http://w3.id.org/def/BiomassOntology#BD150Sawdust
:BD150Sawdust rdf:type owl:NamedIndividual ,
                       :SawdustResult ;
              rdfs:comment "≥ 150 kg/m3 bulk density of sawdust as received"@en ;
              rdfs:label "BD150 Sawdust"@en .


###  http://w3.id.org/def/BiomassOntology#BD150Shavings
:BD150Shavings rdf:type owl:NamedIndividual ,
                        :ShavingsResult ;
               rdfs:comment "≥ 150 kg/m3 bulk density of shavings as received"@en ;
               rdfs:label "BD150 Shavings"@en .


###  http://w3.id.org/def/BiomassOntology#BD150WoodChipsHogFuel
:BD150WoodChipsHogFuel rdf:type owl:NamedIndividual ,
                                :WoodChipsHogFuelResult ;
                       rdfs:comment "≥ 150 kg/ m3 bulk density of wood chips/ hog fuel as received"@en ;
                       rdfs:label "BD150 Wood Chips/Hog Fuel"@en .


###  http://w3.id.org/def/BiomassOntology#BD160Bale
:BD160Bale rdf:type owl:NamedIndividual ,
                    :BaleResult ;
           rdfs:comment "≥ 160 kg/m3 bulk density of bale as received"@en ;
           rdfs:label "BD160 Bale"@en .


###  http://w3.id.org/def/BiomassOntology#BD180Bale
:BD180Bale rdf:type owl:NamedIndividual ,
                    :BaleResult ;
           rdfs:comment "≥ 180 kg/m3 bulk density of bale as received"@en ;
           rdfs:label "BD180 Bale"@en .


###  http://w3.id.org/def/BiomassOntology#BD200Sawdust
:BD200Sawdust rdf:type owl:NamedIndividual ,
                       :SawdustResult ;
              rdfs:comment "≥ 200 kg/m3 bulk density of sawdust as received"@en ;
              rdfs:label "BD200 Sawdust"@en .


###  http://w3.id.org/def/BiomassOntology#BD200Shavings
:BD200Shavings rdf:type owl:NamedIndividual ,
                        :ShavingsResult ;
               rdfs:comment "≥ 200 kg/m3 bulk density of shavings as received"@en ;
               rdfs:label "BD200 Shavings"@en .


###  http://w3.id.org/def/BiomassOntology#BD200WoodChipsHogFuel
:BD200WoodChipsHogFuel rdf:type owl:NamedIndividual ,
                                :WoodChipsHogFuelResult ;
                       rdfs:comment "≥ 200 kg/ m3 bulk density of wood chips/ hog fuel as received"@en ;
                       rdfs:label "BD200 Wood Chips/Hog Fuel"@en .


###  http://w3.id.org/def/BiomassOntology#BD220Bale
:BD220Bale rdf:type owl:NamedIndividual ,
                    :BaleResult ;
           rdfs:comment "≥ 220 kg/m3 bulk density of bale as received"@en ;
           rdfs:label "BD220 Bale"@en .


###  http://w3.id.org/def/BiomassOntology#BD250Bark
:BD250Bark rdf:type owl:NamedIndividual ,
                    :BarkResult ;
           rdfs:comment "≥ 250 kg/m3 bulk density of bark as received"@en ;
           rdfs:label "BD250 Bark"@en .


###  http://w3.id.org/def/BiomassOntology#BD250Sawdust
:BD250Sawdust rdf:type owl:NamedIndividual ,
                       :SawdustResult ;
              rdfs:comment "≥ 250 kg/m3 bulk density of sawdust as received"@en ;
              rdfs:label "BD250 Sawdust"@en .


###  http://w3.id.org/def/BiomassOntology#BD250Shavings
:BD250Shavings rdf:type owl:NamedIndividual ,
                        :ShavingsResult ;
               rdfs:comment "≥ 250 kg/m3 bulk density of shavings as received"@en ;
               rdfs:label "BD250 Shavings"@en .


###  http://w3.id.org/def/BiomassOntology#BD250WoodChipsHogFuel
:BD250WoodChipsHogFuel rdf:type owl:NamedIndividual ,
                                :WoodChipsHogFuelResult ;
                       rdfs:comment "≥ 250 kg/ m3 bulk density of wood chips/ hog fuel as received"@en ;
                       rdfs:label "BD250 Wood Chips/Hog Fuel"@en .


###  http://w3.id.org/def/BiomassOntology#BD300Bark
:BD300Bark rdf:type owl:NamedIndividual ,
                    :BarkResult ;
           rdfs:comment "≥ 300 kg/m3 bulk density of bark as received"@en ;
           rdfs:label "BD300 Bark"@en .


###  http://w3.id.org/def/BiomassOntology#BD300Sawdust
:BD300Sawdust rdf:type owl:NamedIndividual ,
                       :SawdustResult ;
              rdfs:comment "≥ 300 kg/m3 bulk density of sawdust as received"@en ;
              rdfs:label "BD300 Sawdust"@en .


###  http://w3.id.org/def/BiomassOntology#BD300Shavings
:BD300Shavings rdf:type owl:NamedIndividual ,
                        :ShavingsResult ;
               rdfs:comment "≥ 300 kg/m3 bulk density of shavings as received"@en ;
               rdfs:label "BD300 Shavings"@en .


###  http://w3.id.org/def/BiomassOntology#BD300WoodChipsHogFuel
:BD300WoodChipsHogFuel rdf:type owl:NamedIndividual ,
                                :WoodChipsHogFuelResult ;
                       rdfs:comment "≥ 300 kg/ m3 bulk density of wood chips/ hog fuel as received"@en ;
                       rdfs:label "BD300 Wood Chips/Hog Fuel"@en .


###  http://w3.id.org/def/BiomassOntology#BD350Bark
:BD350Bark rdf:type owl:NamedIndividual ,
                    :BarkResult ;
           rdfs:comment "≥ 350 kg/m3 bulk density of bark as received"@en ;
           rdfs:label "BD350 Bark"@en .


###  http://w3.id.org/def/BiomassOntology#BD350EnergyGrain
:BD350EnergyGrain rdf:type owl:NamedIndividual ,
                           :EnergyGrainResult ;
                  rdfs:comment "≥ 350 kg/m3 bulk density of energy grain as received"@en ;
                  rdfs:label "BD350 EnergyGrain"@en .


###  http://w3.id.org/def/BiomassOntology#BD350Sawdust
:BD350Sawdust rdf:type owl:NamedIndividual ,
                       :SawdustResult ;
              rdfs:comment "≥ 350 kg/m3 bulk density of sawdust as received"@en ;
              rdfs:label "BD350 Sawdust"@en .


###  http://w3.id.org/def/BiomassOntology#BD350WoodChipsHogFuel
:BD350WoodChipsHogFuel rdf:type owl:NamedIndividual ,
                                :WoodChipsHogFuelResult ;
                       rdfs:comment "≥ 350 kg/ m3 bulk density of wood chips/ hog fuel as received"@en ;
                       rdfs:label "BD350 Wood Chips/Hog Fuel"@en .


###  http://w3.id.org/def/BiomassOntology#BD400Bark
:BD400Bark rdf:type owl:NamedIndividual ,
                    :BarkResult ;
           rdfs:comment "≥ 400 kg/m3 bulk density of bark as received"@en ;
           rdfs:label "BD400 Bark"@en .


###  http://w3.id.org/def/BiomassOntology#BD400WoodChipsHogFuel
:BD400WoodChipsHogFuel rdf:type owl:NamedIndividual ,
                                :WoodChipsHogFuelResult ;
                       rdfs:comment "≥ 400 kg/ m3 bulk density of wood chips/ hog fuel as received"@en ;
                       rdfs:label "BD400 Wood Chips/Hog Fuel"@en .


###  http://w3.id.org/def/BiomassOntology#BD450Bark
:BD450Bark rdf:type owl:NamedIndividual ,
                    :BarkResult ;
           rdfs:comment "≥ 450 kg/m3 bulk density of bark as received"@en ;
           rdfs:label "BD450 Bark"@en .


###  http://w3.id.org/def/BiomassOntology#BD450EnergyGrain
:BD450EnergyGrain rdf:type owl:NamedIndividual ,
                           :EnergyGrainResult ;
                  rdfs:comment "≥ 450 kg/m3 bulk density of energy grain as received"@en ;
                  rdfs:label "BD450 EnergyGrain"@en .


###  http://w3.id.org/def/BiomassOntology#BD500Pellet
:BD500Pellet rdf:type owl:NamedIndividual ,
                      :PelletResult ;
             rdfs:comment "≥ 500 kg/m3, pellet bulk density as received"@en ;
             rdfs:label "BD500 Pellet"@en .


###  http://w3.id.org/def/BiomassOntology#BD550EnergyGrain
:BD550EnergyGrain rdf:type owl:NamedIndividual ,
                           :EnergyGrainResult ;
                  rdfs:comment "≥ 550 kg/m3 bulk density of energy grain as received"@en ;
                  rdfs:label "BD550 EnergyGrain"@en .


###  http://w3.id.org/def/BiomassOntology#BD550Pellet
:BD550Pellet rdf:type owl:NamedIndividual ,
                      :PelletResult ;
             rdfs:comment "≥ 550 kg/m3, pellet bulk density as received"@en ;
             rdfs:label "BD550 Pellet"@en .


###  http://w3.id.org/def/BiomassOntology#BD580Pellet
:BD580Pellet rdf:type owl:NamedIndividual ,
                      :PelletResult ;
             rdfs:comment "≥ 580 kg/m3, pellet bulk density as received"@en ;
             rdfs:label "BD580 Pellet"@en .


###  http://w3.id.org/def/BiomassOntology#BD600EnergyGrain
:BD600EnergyGrain rdf:type owl:NamedIndividual ,
                           :EnergyGrainResult ;
                  rdfs:comment "≥ 600 kg/m3 bulk density of energy grain as received"@en ;
                  rdfs:label "BD600 EnergyGrain"@en .


###  http://w3.id.org/def/BiomassOntology#BD600Pellet
:BD600Pellet rdf:type owl:NamedIndividual ,
                      :PelletResult ;
             rdfs:comment "≥ 600 kg/m3, pellet bulk density as received"@en ;
             rdfs:label "BD600 Pellet"@en .


###  http://w3.id.org/def/BiomassOntology#BD625Pellet
:BD625Pellet rdf:type owl:NamedIndividual ,
                      :PelletResult ;
             rdfs:comment "≥ 625 kg/m3, pellet bulk density as received"@en ;
             rdfs:label "BD625 Pellet"@en .


###  http://w3.id.org/def/BiomassOntology#BD650Pellet
:BD650Pellet rdf:type owl:NamedIndividual ,
                      :PelletResult ;
             rdfs:comment "≥ 650 kg/m3, pellet bulk density as received"@en ;
             rdfs:label "BD650 Pellet"@en .


###  http://w3.id.org/def/BiomassOntology#BD700Pellet
:BD700Pellet rdf:type owl:NamedIndividual ,
                      :PelletResult ;
             rdfs:comment "≥ 700 kg/m3, pellet bulk density as received"@en ;
             rdfs:label "BD700 Pellet"@en .


###  http://w3.id.org/def/BiomassOntology#BD750Pellet
:BD750Pellet rdf:type owl:NamedIndividual ,
                      :PelletResult ;
             rdfs:comment "≥ 750 kg/m3, pellet bulk density as received"@en ;
             rdfs:label "BD750 Pellet"@en .


###  http://w3.id.org/def/BiomassOntology#BD80Bale
:BD80Bale rdf:type owl:NamedIndividual ,
                   :BaleResult ;
          rdfs:comment "≥ 80 kg/m3 bulk density of bale as received"@en ;
          rdfs:label "BD80 Bale"@en .


###  http://w3.id.org/def/BiomassOntology#BaleA
:BaleA rdf:type owl:NamedIndividual ,
                :Ash ,
                :BaleProperty ;
       rdfs:comment "% in mass of ash of dry basis in bale"@en ;
       rdfs:label "Ash of bale"@en .


###  http://w3.id.org/def/BiomassOntology#BaleAshMB
:BaleAshMB rdf:type owl:NamedIndividual ,
                    :AshMeltingBehaviour ,
                    :BaleProperty ;
           rdfs:comment "Deformation Temperatue, Hemisphere Temperature and Flow Temperature of bale should be stated"@en ;
           rdfs:label "Ash melting behaviour of bale"@en .


###  http://w3.id.org/def/BiomassOntology#BaleBD
:BaleBD rdf:type owl:NamedIndividual ,
                 :BaleProperty ,
                 :BulkDensity ;
        rdfs:comment "kg/m3 of bale as received"@en ;
        rdfs:label "Bulk density of bale"@en .


###  http://w3.id.org/def/BiomassOntology#BaleBinding
:BaleBinding rdf:type owl:NamedIndividual ,
                      :BaleProperty ;
             rdfs:comment "Tying material of bale is recommended to be specified (net, twine, wire or string)."@en ;
             rdfs:label "Type of binding of bale"@en .


###  http://w3.id.org/def/BiomassOntology#BaleBiomassSp
:BaleBiomassSp rdf:type owl:NamedIndividual ,
                        :BaleProperty ;
               rdfs:comment "To be stated (Examples: wheat straw (triticum), spring harvested reed canary grass (Phalaris arundinacea L.) or Miscanthus (Miscanthus Giganteus))"@en ;
               rdfs:label "Species of biomass of bale"@en .


###  http://w3.id.org/def/BiomassOntology#BaleCl
:BaleCl rdf:type owl:NamedIndividual ,
                 :BaleProperty ,
                 :Chlorine ;
        rdfs:comment "% in mass of chlorine of dry basis in bale"@en ;
        rdfs:label "Chlorine of bale"@en .


###  http://w3.id.org/def/BiomassOntology#BaleDimensions
:BaleDimensions rdf:type owl:NamedIndividual ,
                         :BaleProperty ,
                         :Diameter ,
                         :Height ,
                         :Length ,
                         :Width ;
                rdfs:comment "Diameter (D) and length (L) in round bales and length (L1), width (L2) and haight (L3) in square bales"@en ;
                rdfs:label "Dimensions of bale"@en .


###  http://w3.id.org/def/BiomassOntology#BaleM
:BaleM rdf:type owl:NamedIndividual ,
                :BaleProperty ,
                :Moisture ;
       rdfs:comment "% in mass of moisture in bale as received"@en ;
       rdfs:label "Moisture of bale"@en .


###  http://w3.id.org/def/BiomassOntology#BaleN
:BaleN rdf:type owl:NamedIndividual ,
                :BaleProperty ,
                :Nitrogen ;
       rdfs:comment "% in mass of nitrogen of dry basis in bale"@en ;
       rdfs:label "Nitrogen of bale"@en .


###  http://w3.id.org/def/BiomassOntology#BaleProdMethod
:BaleProdMethod rdf:type owl:NamedIndividual ,
                         :BaleProperty ;
                rdfs:comment "It is recommended to declare production methods that influence the size of the straw particles in the bale. For instance, whether the crop has been threshed by rotation or oscillation and whether the straw has been chopped. Harvested as a whole plant for Reed canary grass and Miscanthus."@en ;
                rdfs:label "Production method of bale"@en .


###  http://w3.id.org/def/BiomassOntology#BaleQ
:BaleQ rdf:type owl:NamedIndividual ,
                :BaleProperty ,
                :CalorificValue ;
       rdfs:comment "MJ/kg or kWh/kg of bale as received"@en ;
       rdfs:label "Net calorific value of bale"@en .


###  http://w3.id.org/def/BiomassOntology#BaleTradedForm
:BaleTradedForm rdf:type owl:NamedIndividual ,
                         :BaleProperty ;
                rdfs:comment "To be stated if bale is traded as round or square bales"@en ;
                rdfs:label "Traded form of bale"@en .


###  http://w3.id.org/def/BiomassOntology#BarkA
:BarkA rdf:type owl:NamedIndividual ,
                :Ash ,
                :BarkProperty ;
       rdfs:comment "% in mass of ash of dry basis in bark"@en ;
       rdfs:label "Ash of bark"@en .


###  http://w3.id.org/def/BiomassOntology#BarkAshMB
:BarkAshMB rdf:type owl:NamedIndividual ,
                    :AshMeltingBehaviour ,
                    :BarkProperty ;
           rdfs:comment "Deformation Temperatue, Hemisphere Temperature and Flow Temperature of bark should be stated"@en ;
           rdfs:label "Ash melting behaviour of bark"@en .


###  http://w3.id.org/def/BiomassOntology#BarkBD
:BarkBD rdf:type owl:NamedIndividual ,
                 :BarkProperty ,
                 :BulkDensity ;
        rdfs:comment "kg/m3 as received of bark"@en ;
        rdfs:label "Bulk density of bark"@en .


###  http://w3.id.org/def/BiomassOntology#BarkCl
:BarkCl rdf:type owl:NamedIndividual ,
                 :BarkProperty ,
                 :Chlorine ;
        rdfs:comment "% in mass of chlorine of dry basis in bark"@en ;
        rdfs:label "Chlorine of bark"@en .


###  http://w3.id.org/def/BiomassOntology#BarkDimensions
:BarkDimensions rdf:type owl:NamedIndividual ,
                         :BarkProperty ,
                         :Length ;
                rdfs:comment "Length (mm) of particles in bark"@en ;
                rdfs:label "Dimensions of bark"@en .


###  http://w3.id.org/def/BiomassOntology#BarkM
:BarkM rdf:type owl:NamedIndividual ,
                :BarkProperty ,
                :Moisture ;
       rdfs:comment "% in mass of moisture in bark as received"@en ;
       rdfs:label "Moisture of bark"@en .


###  http://w3.id.org/def/BiomassOntology#BarkN
:BarkN rdf:type owl:NamedIndividual ,
                :BarkProperty ,
                :Nitrogen ;
       rdfs:comment "% in mass of nitrogen of dry basis in bark"@en ;
       rdfs:label "Nitrogen of bark"@en .


###  http://w3.id.org/def/BiomassOntology#BarkQ
:BarkQ rdf:type owl:NamedIndividual ,
                :BarkProperty ,
                :CalorificValue ;
       rdfs:comment "MJ/kg or kWh/kg of bark as received"@en ;
       rdfs:label "Net calorific value of bark"@en .


###  http://w3.id.org/def/BiomassOntology#BarkShredding
:BarkShredding rdf:type owl:NamedIndividual ,
                        :BarkProperty ;
               rdfs:comment "To be stated if bark is shredded or not into pieces"@en ;
               rdfs:label "Shredding of bark"@en .


###  http://w3.id.org/def/BiomassOntology#BiomassScheme
:BiomassScheme rdf:type owl:NamedIndividual ,
                        <http://www.w3.org/2004/02/skos/core#ConceptScheme> ;
               <http://www.w3.org/2004/02/skos/core#definition> "SKOS Concept scheme for biomass origin classification."@en ;
               <http://www.w3.org/2004/02/skos/core#prefLabel> "Biomass  Scheme"@en .


###  http://w3.id.org/def/BiomassOntology#BriquetteA
:BriquetteA rdf:type owl:NamedIndividual ,
                     :Ash ,
                     :BriquetteProperty ;
            rdfs:comment "% in mass of ash in briquettes as received"@en ;
            rdfs:label "Ash of briquette"@en .


###  http://w3.id.org/def/BiomassOntology#BriquetteAdditives
:BriquetteAdditives rdf:type owl:NamedIndividual ,
                             :AdditivesContent ,
                             :BriquetteProperty ;
                    rdfs:comment "% in mass of additives of pressing mass. Type and content of pressing aids, slagging inhibitors or any other additives have to be stated"@en ;
                    rdfs:label "Additives of briquette"@en .


###  http://w3.id.org/def/BiomassOntology#BriquetteAshMB
:BriquetteAshMB rdf:type owl:NamedIndividual ,
                         :AshMeltingBehaviour ,
                         :BriquetteProperty ;
                rdfs:comment "Deformation Temperatue, Hemisphere Temperature and Flow Temperature of briquette should be stated"@en ;
                rdfs:label "Ash melting behaviour of briquette"@en .


###  http://w3.id.org/def/BiomassOntology#BriquetteC
:BriquetteC rdf:type owl:NamedIndividual ,
                     :BriquetteProperty ,
                     :FixedCarbon ;
            rdfs:comment "% in mass of fixed carbon in briquettes of dry basis"@en ;
            rdfs:label "Fixed carbon of briquette"@en .


###  http://w3.id.org/def/BiomassOntology#BriquetteCl
:BriquetteCl rdf:type owl:NamedIndividual ,
                      :BriquetteProperty ,
                      :Chlorine ;
             rdfs:comment "% in mass of chlorine in briquettes of dry basis"@en ;
             rdfs:label "Chlorine of briquette"@en .


###  http://w3.id.org/def/BiomassOntology#BriquetteDE
:BriquetteDE rdf:type owl:NamedIndividual ,
                      :BriquetteProperty ,
                      :Density ;
             rdfs:comment "g/cm3 of a briquette as received"@en ;
             rdfs:label "Particle density of briquette"@en .


###  http://w3.id.org/def/BiomassOntology#BriquetteDU
:BriquetteDU rdf:type owl:NamedIndividual ,
                      :BriquetteProperty ,
                      :MechanicalDurability ;
             rdfs:comment "% in mass of briquette after testing"@en ;
             rdfs:label "Mechanical durability of briquette"@en .


###  http://w3.id.org/def/BiomassOntology#BriquetteDimensions
:BriquetteDimensions rdf:type owl:NamedIndividual ,
                              :BriquetteProperty ,
                              :Diameter ,
                              :Height ,
                              :Length ,
                              :Width ;
                     rdfs:comment "Diameter (D), Length (L1), Width (L2) and Height (L3) mm. Shape should be stated"@en ;
                     rdfs:label "Dimensions of briquette"@en .


###  http://w3.id.org/def/BiomassOntology#BriquetteM
:BriquetteM rdf:type owl:NamedIndividual ,
                     :BriquetteProperty ,
                     :Moisture ;
            rdfs:comment "% in mass of moisture in briquettes as received"@en ;
            rdfs:label "Moisture of briquette"@en .


###  http://w3.id.org/def/BiomassOntology#BriquetteN
:BriquetteN rdf:type owl:NamedIndividual ,
                     :BriquetteProperty ,
                     :Nitrogen ;
            rdfs:comment "% in mass of nitrogen in briquettes of dry basis"@en ;
            rdfs:label "Nitrogen of briquette"@en .


###  http://w3.id.org/def/BiomassOntology#BriquetteQ
:BriquetteQ rdf:type owl:NamedIndividual ,
                     :BriquetteProperty ,
                     :CalorificValue ;
            rdfs:comment "MJ/kg or kWh/kg of briquette as received"@en ;
            rdfs:label "Net calorific value of briquette"@en .


###  http://w3.id.org/def/BiomassOntology#BriquetteS
:BriquetteS rdf:type owl:NamedIndividual ,
                     :BriquetteProperty ,
                     :Sulfur ;
            rdfs:comment "% in mass of sulfur in briquettes of dry basis"@en ;
            rdfs:label "Sulfur of briquette"@en .


###  http://w3.id.org/def/BiomassOntology#BriquetteVM
:BriquetteVM rdf:type owl:NamedIndividual ,
                      :BriquetteProperty ;
             rdfs:comment "% in mass of volatile matter in briquettes of dry basis"@en ;
             rdfs:label "Volatile matter of briquette"@en .


###  http://w3.id.org/def/BiomassOntology#C60Charcoal
:C60Charcoal rdf:type owl:NamedIndividual ,
                      :CharcoalResult ;
             rdfs:comment "≥ 60 % in massof fixed carbon in charcoal of dry basis"@en ;
             rdfs:label "C60 Charcoal"@en .


###  http://w3.id.org/def/BiomassOntology#C75Charcoal
:C75Charcoal rdf:type owl:NamedIndividual ,
                      :CharcoalResult ;
             rdfs:comment "≥ 75 % in massof fixed carbon in charcoal of dry basis"@en ;
             rdfs:label "C75 Charcoal"@en .


###  http://w3.id.org/def/BiomassOntology#CharcoalA
:CharcoalA rdf:type owl:NamedIndividual ,
                    :Ash ,
                    :CharcoalProperty ;
           rdfs:comment "% in mass of ash in charcoal of dry basis"@en ;
           rdfs:label "Ash of charcoal"@en .


###  http://w3.id.org/def/BiomassOntology#CharcoalBD
:CharcoalBD rdf:type owl:NamedIndividual ,
                     :BulkDensity ,
                     :CharcoalProperty ;
            rdfs:comment "kg/m3 of charcoal as received"@en ;
            rdfs:label "Bulk density of charcoal"@en .


###  http://w3.id.org/def/BiomassOntology#CharcoalC
:CharcoalC rdf:type owl:NamedIndividual ,
                    :CharcoalProperty ,
                    :FixedCarbon ;
           rdfs:comment "% in massof fixed carbon in charcoal of dry basis"@en ;
           rdfs:label "Fixed carbon of charcoal"@en .


###  http://w3.id.org/def/BiomassOntology#CharcoalDimensions
:CharcoalDimensions rdf:type owl:NamedIndividual ,
                             :CharcoalProperty ,
                             :Length ;
                    rdfs:comment "Length (mm) of particles of charcoal"@en ;
                    rdfs:label "Dimensions of charcoal"@en .


###  http://w3.id.org/def/BiomassOntology#CharcoalM
:CharcoalM rdf:type owl:NamedIndividual ,
                    :CharcoalProperty ,
                    :Moisture ;
           rdfs:comment "% in mass of moisture in charcoal as received"@en ;
           rdfs:label "Moisture of charcoal"@en .


###  http://w3.id.org/def/BiomassOntology#CharcoalQ
:CharcoalQ rdf:type owl:NamedIndividual ,
                    :CalorificValue ,
                    :CharcoalProperty ;
           rdfs:comment "MJ/kg or kWh/kg of charcoal as received"@en ;
           rdfs:label "Net calorific value of charcoal"@en .


###  http://w3.id.org/def/BiomassOntology#CharcoalVM
:CharcoalVM rdf:type owl:NamedIndividual ,
                     :CharcoalProperty ;
            rdfs:comment "% in mass of volatile matter in charcoal"@en ;
            rdfs:label "Volatile matter of charcoal"@en .


###  http://w3.id.org/def/BiomassOntology#Cl0.01Bale
:Cl0.01Bale rdf:type owl:NamedIndividual ,
                     :BaleResult ;
            rdfs:comment "≤ 0,01 % in mass of chlorine of dry basis in bale"@en ;
            rdfs:label "Cl0.01 Bale"@en .


###  http://w3.id.org/def/BiomassOntology#Cl0.01Briquette
:Cl0.01Briquette rdf:type owl:NamedIndividual ,
                          :BriquetteResult ;
                 rdfs:comment "≤ 0,01 % in mass of chlorine in briquettes of dry basis"@en ;
                 rdfs:label "Cl0.01 Briquette"@en .


###  http://w3.id.org/def/BiomassOntology#Cl0.01Pellet
:Cl0.01Pellet rdf:type owl:NamedIndividual ,
                       :PelletResult ;
              rdfs:comment "≤ 0,01 % in mass of chlorine in pellets of dry basis"@en ;
              rdfs:label "Cl0.01 Pellet"@en .


###  http://w3.id.org/def/BiomassOntology#Cl0.01Sawdust
:Cl0.01Sawdust rdf:type owl:NamedIndividual ,
                        :SawdustResult ;
               rdfs:comment "≤ 0,01 % in mass of chlorine of dry basis in sawdust"@en ;
               rdfs:label "Cl0.01 Sawdust"@en .


###  http://w3.id.org/def/BiomassOntology#Cl0.01Shavings
:Cl0.01Shavings rdf:type owl:NamedIndividual ,
                         :ShavingsResult ;
                rdfs:comment "≤ 0,01 % in mass of chlorine in shavings of dry basis"@en ;
                rdfs:label "Cl0.01 Shavings"@en .


###  http://w3.id.org/def/BiomassOntology#Cl0.02Bale
:Cl0.02Bale rdf:type owl:NamedIndividual ,
                     :BaleResult ;
            rdfs:comment "≤ 0,02 % in mass of chlorine of dry basis in bale"@en ;
            rdfs:label "Cl0.02 Bale"@en .


###  http://w3.id.org/def/BiomassOntology#Cl0.02Bark
:Cl0.02Bark rdf:type owl:NamedIndividual ,
                     :BarkResult ;
            rdfs:comment "≤ 0,02 % in mass of chlorine of dry basis in bark"@en ;
            rdfs:label "Cl0.02 Bark"@en .


###  http://w3.id.org/def/BiomassOntology#Cl0.02Briquette
:Cl0.02Briquette rdf:type owl:NamedIndividual ,
                          :BriquetteResult ;
                 rdfs:comment "≤ 0,02 % in mass of chlorine in briquettes of dry basis"@en ;
                 rdfs:label "Cl0.02 Briquette"@en .


###  http://w3.id.org/def/BiomassOntology#Cl0.02Pellet
:Cl0.02Pellet rdf:type owl:NamedIndividual ,
                       :PelletResult ;
              rdfs:comment "≤ 0,02 % in mass of chlorine in pellets of dry basis"@en ;
              rdfs:label "Cl0.02 Pellet"@en .


###  http://w3.id.org/def/BiomassOntology#Cl0.02Sawdust
:Cl0.02Sawdust rdf:type owl:NamedIndividual ,
                        :SawdustResult ;
               rdfs:comment "≤ 0,02 % in mass of chlorine of dry basis in sawdust"@en ;
               rdfs:label "Cl0.02 Sawdust"@en .


###  http://w3.id.org/def/BiomassOntology#Cl0.02Shavings
:Cl0.02Shavings rdf:type owl:NamedIndividual ,
                         :ShavingsResult ;
                rdfs:comment "≤ 0,02 % in mass of chlorine in shavings of dry basis"@en ;
                rdfs:label "Cl0.02 Shavings"@en .


###  http://w3.id.org/def/BiomassOntology#Cl0.02WoodChipsHogFuel
:Cl0.02WoodChipsHogFuel rdf:type owl:NamedIndividual ,
                                 :WoodChipsHogFuelResult ;
                        rdfs:comment "≤ 0,02 % in mass of chlorine in wood chips/hog fuel of dry basis"@en ;
                        rdfs:label "Cl0.02 Wood Chips/Hog Fuel"@en .


###  http://w3.id.org/def/BiomassOntology#Cl0.03Bale
:Cl0.03Bale rdf:type owl:NamedIndividual ,
                     :BaleResult ;
            rdfs:comment "≤ 0,03 % in mass of chlorine of dry basis in bale"@en ;
            rdfs:label "Cl0.03 Bale"@en .


###  http://w3.id.org/def/BiomassOntology#Cl0.03Bark
:Cl0.03Bark rdf:type owl:NamedIndividual ,
                     :BarkResult ;
            rdfs:comment "≤ 0,03 % in mass of chlorine of dry basis in bark"@en ;
            rdfs:label "Cl0.03 Bark"@en .


###  http://w3.id.org/def/BiomassOntology#Cl0.03Briquette
:Cl0.03Briquette rdf:type owl:NamedIndividual ,
                          :BriquetteResult ;
                 rdfs:comment "≤ 0,03 % in mass of chlorine in briquettes of dry basis"@en ;
                 rdfs:label "Cl0.03 Briquette"@en .


###  http://w3.id.org/def/BiomassOntology#Cl0.03Pellet
:Cl0.03Pellet rdf:type owl:NamedIndividual ,
                       :PelletResult ;
              rdfs:comment "≤ 0,03 % in mass of chlorine in pellets of dry basis"@en ;
              rdfs:label "Cl0.03 Pellet"@en .


###  http://w3.id.org/def/BiomassOntology#Cl0.03Sawdust
:Cl0.03Sawdust rdf:type owl:NamedIndividual ,
                        :SawdustResult ;
               rdfs:comment "≤ 0,03 % in mass of chlorine of dry basis in sawdust"@en ;
               rdfs:label "Cl0.03 Sawdust"@en .


###  http://w3.id.org/def/BiomassOntology#Cl0.03Shavings
:Cl0.03Shavings rdf:type owl:NamedIndividual ,
                         :ShavingsResult ;
                rdfs:comment "≤ 0,03 % in mass of chlorine in shavings of dry basis"@en ;
                rdfs:label "Cl0.03 Shavings"@en .


###  http://w3.id.org/def/BiomassOntology#Cl0.03WoodChipsHogFuel
:Cl0.03WoodChipsHogFuel rdf:type owl:NamedIndividual ,
                                 :WoodChipsHogFuelResult ;
                        rdfs:comment "≤ 0,03 % in mass of chlorine in wood chips/hog fuel of dry basis"@en ;
                        rdfs:label "Cl0.03 Wood Chips/Hog Fuel"@en .


###  http://w3.id.org/def/BiomassOntology#Cl0.05Briquette
:Cl0.05Briquette rdf:type owl:NamedIndividual ,
                          :BriquetteResult ;
                 rdfs:comment "≤ 0,05 % in mass of chlorine in briquettes of dry basis"@en ;
                 rdfs:label "Cl0.05 Briquette"@en .


###  http://w3.id.org/def/BiomassOntology#Cl0.05EnergyGrain
:Cl0.05EnergyGrain rdf:type owl:NamedIndividual ,
                            :EnergyGrainResult ;
                   rdfs:comment "≤ 0,05 % in mass of chlorine in energy grain of dry basis"@en ;
                   rdfs:label "Cl0.05 EnergyGrain"@en .


###  http://w3.id.org/def/BiomassOntology#Cl0.05Pellet
:Cl0.05Pellet rdf:type owl:NamedIndividual ,
                       :PelletResult ;
              rdfs:comment "≤ 0,05 % in mass of chlorine in pellets of dry basis"@en ;
              rdfs:label "Cl0.05 Pellet"@en .


###  http://w3.id.org/def/BiomassOntology#Cl0.05WoodChipsHogFuel
:Cl0.05WoodChipsHogFuel rdf:type owl:NamedIndividual ,
                                 :WoodChipsHogFuelResult ;
                        rdfs:comment "≤ 0,05 % in mass of chlorine in wood chips/hog fuel of dry basis"@en ;
                        rdfs:label "Cl0.05 Wood Chips/Hog Fuel"@en .


###  http://w3.id.org/def/BiomassOntology#Cl0.07Bale
:Cl0.07Bale rdf:type owl:NamedIndividual ,
                     :BaleResult ;
            rdfs:comment "≤ 0,07 % in mass of chlorine of dry basis in bale"@en ;
            rdfs:label "Cl0.07 Bale"@en .


###  http://w3.id.org/def/BiomassOntology#Cl0.07Bark
:Cl0.07Bark rdf:type owl:NamedIndividual ,
                     :BarkResult ;
            rdfs:comment "≤ 0,07 % in mass of chlorine of dry basis in bark"@en ;
            rdfs:label "Cl0.07 Bark"@en .


###  http://w3.id.org/def/BiomassOntology#Cl0.07Briquette
:Cl0.07Briquette rdf:type owl:NamedIndividual ,
                          :BriquetteResult ;
                 rdfs:comment "≤ 0,07 % in mass of chlorine in briquettes of dry basis"@en ;
                 rdfs:label "Cl0.07 Briquette"@en .


###  http://w3.id.org/def/BiomassOntology#Cl0.07Pellet
:Cl0.07Pellet rdf:type owl:NamedIndividual ,
                       :PelletResult ;
              rdfs:comment "≤ 0,07 % in mass of chlorine in pellets of dry basis"@en ;
              rdfs:label "Cl0.07 Pellet"@en .


###  http://w3.id.org/def/BiomassOntology#Cl0.07Sawdust
:Cl0.07Sawdust rdf:type owl:NamedIndividual ,
                        :SawdustResult ;
               rdfs:comment "≤ 0,07 % in mass of chlorine of dry basis in sawdust"@en ;
               rdfs:label "Cl0.07 Sawdust"@en .


###  http://w3.id.org/def/BiomassOntology#Cl0.07Shavings
:Cl0.07Shavings rdf:type owl:NamedIndividual ,
                         :ShavingsResult ;
                rdfs:comment "≤ 0,07 % in mass of chlorine in shavings of dry basis"@en ;
                rdfs:label "Cl0.07 Shavings"@en .


###  http://w3.id.org/def/BiomassOntology#Cl0.07WoodChipsHogFuel
:Cl0.07WoodChipsHogFuel rdf:type owl:NamedIndividual ,
                                 :WoodChipsHogFuelResult ;
                        rdfs:comment "≤ 0,07 % in mass of chlorine in wood chips/hog fuel of dry basis"@en ;
                        rdfs:label "Cl0.07 Wood Chips/Hog Fuel"@en .


###  http://w3.id.org/def/BiomassOntology#Cl0.15EnergyGrain
:Cl0.15EnergyGrain rdf:type owl:NamedIndividual ,
                            :EnergyGrainResult ;
                   rdfs:comment "≤ 0,15 % in mass of chlorine in energy grain of dry basis"@en ;
                   rdfs:label "Cl0.15 EnergyGrain"@en .


###  http://w3.id.org/def/BiomassOntology#Cl0.15FruitSeeds
:Cl0.15FruitSeeds rdf:type owl:NamedIndividual ,
                           :FruitSeedsResult ;
                  rdfs:comment "≤ 0,15 % in mass of chlorine in fruit seeds of dry basis"@en ;
                  rdfs:label "Cl0.15 FruitSeeds"@en .


###  http://w3.id.org/def/BiomassOntology#Cl0.15OliveResidues
:Cl0.15OliveResidues rdf:type owl:NamedIndividual ,
                              :OliveResiduesResult ;
                     rdfs:comment "≤ 0,15 % in mass of chlorine in olive residues of dry basis"@en ;
                     rdfs:label "Cl0.15 OliveResidues"@en .


###  http://w3.id.org/def/BiomassOntology#Cl0.1Bale
:Cl0.1Bale rdf:type owl:NamedIndividual ,
                    :BaleResult ;
           rdfs:comment "≤ 0,10 % in mass of chlorine of dry basis in bale"@en ;
           rdfs:label "Cl0.10 Bale"@en .


###  http://w3.id.org/def/BiomassOntology#Cl0.1Bark
:Cl0.1Bark rdf:type owl:NamedIndividual ,
                    :BarkResult ;
           rdfs:comment "≤ 0,10 % in mass of chlorine of dry basis in bark"@en ;
           rdfs:label "Cl0.10 Bark"@en .


###  http://w3.id.org/def/BiomassOntology#Cl0.1Briquette
:Cl0.1Briquette rdf:type owl:NamedIndividual ,
                         :BriquetteResult ;
                rdfs:comment "≤ 0,10 % in mass of chlorine in briquettes of dry basis"@en ;
                rdfs:label "Cl0.10 Briquette"@en .


###  http://w3.id.org/def/BiomassOntology#Cl0.1EnergyGrain
:Cl0.1EnergyGrain rdf:type owl:NamedIndividual ,
                           :EnergyGrainResult ;
                  rdfs:comment "≤ 0,10 % in mass of chlorine in energy grain of dry basis"@en ;
                  rdfs:label "Cl0.10 EnergyGrain"@en .


###  http://w3.id.org/def/BiomassOntology#Cl0.1FruitSeeds
:Cl0.1FruitSeeds rdf:type owl:NamedIndividual ,
                          :FruitSeedsResult ;
                 rdfs:comment "≤ 0,10 % in mass of chlorine in fruit seeds of dry basis"@en ;
                 rdfs:label "Cl0.10 FruitSeeds"@en .


###  http://w3.id.org/def/BiomassOntology#Cl0.1OliveResidues
:Cl0.1OliveResidues rdf:type owl:NamedIndividual ,
                             :OliveResiduesResult ;
                    rdfs:comment "≤ 0,10 % in mass of chlorine in olive residues of dry basis"@en ;
                    rdfs:label "Cl0.10 OliveResidues"@en .


###  http://w3.id.org/def/BiomassOntology#Cl0.1Pellet
:Cl0.1Pellet rdf:type owl:NamedIndividual ,
                      :PelletResult ;
             rdfs:comment "≤ 0,10 % in mass of chlorine in pellets of dry basis"@en ;
             rdfs:label "Cl0.10 Pellet"@en .


###  http://w3.id.org/def/BiomassOntology#Cl0.1Sawdust
:Cl0.1Sawdust rdf:type owl:NamedIndividual ,
                       :SawdustResult ;
              rdfs:comment "≤ 0,10 % in mass of chlorine of dry basis in sawdust"@en ;
              rdfs:label "Cl0.10 Sawdust"@en .


###  http://w3.id.org/def/BiomassOntology#Cl0.1Shavings
:Cl0.1Shavings rdf:type owl:NamedIndividual ,
                        :ShavingsResult ;
               rdfs:comment "≤ 0,10 % in mass of chlorine in shavings of dry basis"@en ;
               rdfs:label "Cl0.10 Shavings"@en .


###  http://w3.id.org/def/BiomassOntology#Cl0.1WoodChipsHogFuel
:Cl0.1WoodChipsHogFuel rdf:type owl:NamedIndividual ,
                                :WoodChipsHogFuelResult ;
                       rdfs:comment "≤ 0,10 % in mass of chlorine in wood chips/hog fuel of dry basis"@en ;
                       rdfs:label "Cl0.10 Wood Chips/Hog Fuel"@en .


###  http://w3.id.org/def/BiomassOntology#Cl0.2Briquette
:Cl0.2Briquette rdf:type owl:NamedIndividual ,
                         :BriquetteResult ;
                rdfs:comment "≤ 0,20 % in mass of chlorine in briquettes of dry basis"@en ;
                rdfs:label "Cl0.20 Briquette"@en .


###  http://w3.id.org/def/BiomassOntology#Cl0.2Pellet
:Cl0.2Pellet rdf:type owl:NamedIndividual ,
                      :PelletResult ;
             rdfs:comment "≤ 0,20 % in mass of chlorine in pellets of dry basis"@en ;
             rdfs:label "Cl0.20 Pellet"@en .


###  http://w3.id.org/def/BiomassOntology#Cl0.3Briquette
:Cl0.3Briquette rdf:type owl:NamedIndividual ,
                         :BriquetteResult ;
                rdfs:comment "≤ 0,30 % in mass of chlorine in briquettes of dry basis"@en ;
                rdfs:label "Cl0.30 Briquette"@en .


###  http://w3.id.org/def/BiomassOntology#Cl0.3Pellet
:Cl0.3Pellet rdf:type owl:NamedIndividual ,
                      :PelletResult ;
             rdfs:comment "≤ 0,30 % in mass of chlorine in pellets of dry basis"@en ;
             rdfs:label "Cl0.30 Pellet"@en .


###  http://w3.id.org/def/BiomassOntology#D03FruitSeeds
:D03FruitSeeds rdf:type owl:NamedIndividual ,
                        :FruitSeedsResult ;
               rdfs:comment "1 mm ≤ D < 3,15 mm diameter of fruit seeds, (5 % in mass may have diameter over the class)"@en ;
               rdfs:label "D03 FruitSeeds"@en .


###  http://w3.id.org/def/BiomassOntology#D03OliveResidues
:D03OliveResidues rdf:type owl:NamedIndividual ,
                           :OliveResiduesResult ;
                  rdfs:comment "1 mm ≤ D < 3,15 mm diameter of olive residues"@en ;
                  rdfs:label "D03 OliveResidues"@en .


###  http://w3.id.org/def/BiomassOntology#D05EnergyGrain
:D05EnergyGrain rdf:type owl:NamedIndividual ,
                         :EnergyGrainResult ;
                rdfs:comment "1 mm ≤ D < 5 mm diameter of energy grain, (5 % in mass may have diameter over the class)"@en ;
                rdfs:label "D05 EnergyGrain"@en .


###  http://w3.id.org/def/BiomassOntology#D05FruitSeeds
:D05FruitSeeds rdf:type owl:NamedIndividual ,
                        :FruitSeedsResult ;
               rdfs:comment "1 mm ≤ D < 5 mm diameter of fruit seeds, (5 % in mass may have diameter over the class)"@en ;
               rdfs:label "D05 FruitSeeds"@en .


###  http://w3.id.org/def/BiomassOntology#D05OliveResidues
:D05OliveResidues rdf:type owl:NamedIndividual ,
                           :OliveResiduesResult ;
                  rdfs:comment "1 mm ≤ D < 5 mm diameter of olive residues"@en ;
                  rdfs:label "D05 OliveResidues"@en .


###  http://w3.id.org/def/BiomassOntology#D06Pellet
:D06Pellet rdf:type owl:NamedIndividual ,
                    :PelletResult ;
           rdfs:comment "Dimensions of pellet 6 mm ± 1,0 mm D and 3,15 mm ≤ L ≤ 40 mm"@en ;
           rdfs:label "D06 Pellet"@en .


###  http://w3.id.org/def/BiomassOntology#D08Pellet
:D08Pellet rdf:type owl:NamedIndividual ,
                    :PelletResult ;
           rdfs:comment "Dimensions of pellet 8 mm ± 1,0 mm D and 3,15 mm ≤ L ≤ 40 mm"@en ;
           rdfs:label "D08 Pellet"@en .


###  http://w3.id.org/def/BiomassOntology#D10EnergyGrain
:D10EnergyGrain rdf:type owl:NamedIndividual ,
                         :EnergyGrainResult ;
                rdfs:comment "5 mm ≤ D < 10 mm diameter of energy grain, (5 % in mass may have diameter over the class)"@en ;
                rdfs:label "D10 EnergyGrain"@en .


###  http://w3.id.org/def/BiomassOntology#D10FruitSeeds
:D10FruitSeeds rdf:type owl:NamedIndividual ,
                        :FruitSeedsResult ;
               rdfs:comment "1 mm ≤ D < 10 mm diameter of fruit seeds, (5 % in mass may have diameter over the class)"@en ;
               rdfs:label "D10 FruitSeeds"@en .


###  http://w3.id.org/def/BiomassOntology#D10LogFirewood
:D10LogFirewood rdf:type owl:NamedIndividual ,
                         :LogFirewoodResult ;
                rdfs:comment "Diameter of a single piece of log wood/firewood. Main fraction, (minimum 70 % of mass), 5 ≤ D < 10cm; Coarse fraction, < 15% of mass; Maximum diameter, 15cm; Small firewood, 15% of mass"@en ;
                rdfs:label "D10 Log wood/Firewood"@en .


###  http://w3.id.org/def/BiomassOntology#D10OliveResidues
:D10OliveResidues rdf:type owl:NamedIndividual ,
                           :OliveResiduesResult ;
                  rdfs:comment "1 mm ≤ D < 10 mm diameter of olive residues"@en ;
                  rdfs:label "D10 OliveResidues"@en .


###  http://w3.id.org/def/BiomassOntology#D10Pellet
:D10Pellet rdf:type owl:NamedIndividual ,
                    :PelletResult ;
           rdfs:comment "Dimensions of pellet 10 mm ± 1,0 mm D and 3,15 mm ≤ L ≤ 40 mm"@en ;
           rdfs:label "D10 Pellet"@en .


###  http://w3.id.org/def/BiomassOntology#D12Pellet
:D12Pellet rdf:type owl:NamedIndividual ,
                    :PelletResult ;
           rdfs:comment "Dimensions of pellet 12 mm ± 1,0 mm D and 3,15 mm ≤ L ≤ 50 mm"@en ;
           rdfs:label "D12 Pellet"@en .


###  http://w3.id.org/def/BiomassOntology#D15LogFirewood
:D15LogFirewood rdf:type owl:NamedIndividual ,
                         :LogFirewoodResult ;
                rdfs:comment "Diameter of a single piece of log wood/firewood. Main fraction, (minimum 70 % of mass), 10 ≤ D < 15cm; Coarse fraction, < 15% of mass; Maximum diameter, 20cm; Small firewood, 10% of mass"@en ;
                rdfs:label "D15 Log wood/Firewood"@en .


###  http://w3.id.org/def/BiomassOntology#D1Bale
:D1Bale rdf:type owl:NamedIndividual ,
                 :BaleResult ;
        rdfs:comment "Round bale; Diameter (D) 1,2 m – 1,5 m; Length (L1) 1,2 m"@en ;
        rdfs:label "D1 Bale"@en .


###  http://w3.id.org/def/BiomassOntology#D20LogFirewood
:D20LogFirewood rdf:type owl:NamedIndividual ,
                         :LogFirewoodResult ;
                rdfs:comment "Diameter of a single piece of log wood/firewood. Main fraction, (minimum 70 % of mass), 15 ≤ D < 20cm; Coarse fraction, < 15% of mass; Maximum diameter, 25cm; Small firewood, 10% of mass"@en ;
                rdfs:label "D20 Log wood/Firewood"@en .


###  http://w3.id.org/def/BiomassOntology#D25LogFirewood
:D25LogFirewood rdf:type owl:NamedIndividual ,
                         :LogFirewoodResult ;
                rdfs:comment "Diameter of a single piece of log wood/firewood. Main fraction, (minimum 70 % of mass), 20 ≤ D < 25cm; Coarse fraction, < 15% of mass; Maximum diameter, 30cm; Small firewood, 10% of mass"@en ;
                rdfs:label "D25 Log wood/Firewood"@en .


###  http://w3.id.org/def/BiomassOntology#D25Pellet
:D25Pellet rdf:type owl:NamedIndividual ,
                    :PelletResult ;
           rdfs:comment "Dimensions of pellet 25 mm ± 1,0 mm D and 10 mm ≤ L ≤ 50 mm"@en ;
           rdfs:label "D25 Pellet"@en .


###  http://w3.id.org/def/BiomassOntology#D2Bale
:D2Bale rdf:type owl:NamedIndividual ,
                 :BaleResult ;
        rdfs:comment "Round bale; Diameter (D) 1,6 m – 1,8 m; Length (L1) 1,5 m"@en ;
        rdfs:label "D2 Bale"@en .


###  http://w3.id.org/def/BiomassOntology#D2LogFirewood
:D2LogFirewood rdf:type owl:NamedIndividual ,
                        :LogFirewoodResult ;
               rdfs:comment "Diameter of a single piece of log wood/firewood. Main fraction, (minimum 70 % of mass), < 2cm; Coarse fraction, < 15% of mass; Maximum diameter, 3cm"@en ;
               rdfs:label "D2 Log wood/Firewood"@en .


###  http://w3.id.org/def/BiomassOntology#D5LogFirewood
:D5LogFirewood rdf:type owl:NamedIndividual ,
                        :LogFirewoodResult ;
               rdfs:comment "Diameter of a single piece of log wood/firewood. Main fraction, (minimum 70 % of mass), 2 ≤ D < 5cm; Coarse fraction, < 15% of mass; Maximum diameter, 8cm"@en ;
               rdfs:label "D5 Log wood/Firewood"@en .


###  http://w3.id.org/def/BiomassOntology#DE0.6Briquette
:DE0.6Briquette rdf:type owl:NamedIndividual ,
                         :BriquetteResult ;
                rdfs:comment "≥ 0,6 g/cm3 briquette density as received"@en ;
                rdfs:label "DE0.6 Briquette"@en .


###  http://w3.id.org/def/BiomassOntology#DE0.8Briquette
:DE0.8Briquette rdf:type owl:NamedIndividual ,
                         :BriquetteResult ;
                rdfs:comment "≥ 0,8 g/cm3 briquette density as received"@en ;
                rdfs:label "DE0.8 Briquette"@en .


###  http://w3.id.org/def/BiomassOntology#DE0.9Briquette
:DE0.9Briquette rdf:type owl:NamedIndividual ,
                         :BriquetteResult ;
                rdfs:comment "≥ 0,9 g/cm3 briquette density as received"@en ;
                rdfs:label "DE0.9 Briquette"@en .


###  http://w3.id.org/def/BiomassOntology#DE1.1Briquette
:DE1.1Briquette rdf:type owl:NamedIndividual ,
                         :BriquetteResult ;
                rdfs:comment "≥ 1,1 g/cm3 briquette density as received"@en ;
                rdfs:label "DE1.1 Briquette"@en .


###  http://w3.id.org/def/BiomassOntology#DE1Briquette
:DE1Briquette rdf:type owl:NamedIndividual ,
                       :BriquetteResult ;
              rdfs:comment "≥ 1,0 g/cm3 briquette density as received"@en ;
              rdfs:label "DE1.0 Briquette"@en .


###  http://w3.id.org/def/BiomassOntology#DU90-Briquette
:DU90-Briquette rdf:type owl:NamedIndividual ,
                         :BriquetteResult ;
                rdfs:comment "< 90,0 % in mass of biofuel after testing mechanical durability"@en ;
                rdfs:label "DU90.0- Briquette"@en .


###  http://w3.id.org/def/BiomassOntology#DU90Briquette
:DU90Briquette rdf:type owl:NamedIndividual ,
                        :BriquetteResult ;
               rdfs:comment "≥ 90,0 % in mass of biofuel after testing mechanical durability"@en ;
               rdfs:label "DU90.0 Briquette"@en .


###  http://w3.id.org/def/BiomassOntology#DU95-Pellet
:DU95-Pellet rdf:type owl:NamedIndividual ,
                      :PelletResult ;
             rdfs:comment "< 95,0% in mass of pellets after testing mehanical durability"@en ;
             rdfs:label "DU95.0- Pellet"@en .


###  http://w3.id.org/def/BiomassOntology#DU95Briquette
:DU95Briquette rdf:type owl:NamedIndividual ,
                        :BriquetteResult ;
               rdfs:comment "≥ 95,0 % in mass of biofuel after testing mechanical durability"@en ;
               rdfs:label "DU95.0 Briquette"@en .


###  http://w3.id.org/def/BiomassOntology#DU95Pellet
:DU95Pellet rdf:type owl:NamedIndividual ,
                     :PelletResult ;
            rdfs:comment "≥ 95,0% in mass of pellets after testing mehanical durability"@en ;
            rdfs:label "DU95.0 Pellet"@en .


###  http://w3.id.org/def/BiomassOntology#DU96.5Pellet
:DU96.5Pellet rdf:type owl:NamedIndividual ,
                       :PelletResult ;
              rdfs:comment "≥ 96,5% in mass of pellets after testing mehanical durability"@en ;
              rdfs:label "DU96.5 Pellet"@en .


###  http://w3.id.org/def/BiomassOntology#DU96Pellet
:DU96Pellet rdf:type owl:NamedIndividual ,
                     :PelletResult ;
            rdfs:comment "≥ 96,0% in mass of pellets after testing mehanical durability"@en ;
            rdfs:label "DU96.0 Pellet"@en .


###  http://w3.id.org/def/BiomassOntology#DU97.5Pellet
:DU97.5Pellet rdf:type owl:NamedIndividual ,
                       :PelletResult ;
              rdfs:comment "≥ 97,5% in mass of pellets after testing mehanical durability"@en ;
              rdfs:label "DU97.5 Pellet"@en .


###  http://w3.id.org/def/BiomassOntology#DU98Pellet
:DU98Pellet rdf:type owl:NamedIndividual ,
                     :PelletResult ;
            rdfs:comment "≥ 98,0% in mass of pellets after testing mehanical durability"@en ;
            rdfs:label "DU98.0 Pellet"@en .


###  http://w3.id.org/def/BiomassOntology#EnergyGrainA
:EnergyGrainA rdf:type owl:NamedIndividual ,
                       :Ash ,
                       :EnergyGrainProperty ;
              rdfs:comment "% in mass of ash in energy grain of dry basis"@en ;
              rdfs:label "Ash of energy grain"@en .


###  http://w3.id.org/def/BiomassOntology#EnergyGrainAshMB
:EnergyGrainAshMB rdf:type owl:NamedIndividual ,
                           :AshMeltingBehaviour ,
                           :EnergyGrainProperty ;
                  rdfs:comment "Deformation Temperatue, Hemisphere Temperature and Flow Temperature of energy grain should be stated"@en ;
                  rdfs:label "Ash melting behaviour of energy grain"@en .


###  http://w3.id.org/def/BiomassOntology#EnergyGrainBD
:EnergyGrainBD rdf:type owl:NamedIndividual ,
                        :BulkDensity ,
                        :EnergyGrainProperty ;
               rdfs:comment "kg/m3 of energy grain as received"@en ;
               rdfs:label "Bulk density of energy grain"@en .


###  http://w3.id.org/def/BiomassOntology#EnergyGrainCl
:EnergyGrainCl rdf:type owl:NamedIndividual ,
                        :Chlorine ,
                        :EnergyGrainProperty ;
               rdfs:comment "% in mass of chlorine in energy grain of dry basis"@en ;
               rdfs:label "Chlorine of energy grain"@en .


###  http://w3.id.org/def/BiomassOntology#EnergyGrainDimensions
:EnergyGrainDimensions rdf:type owl:NamedIndividual ,
                                :Diameter ,
                                :EnergyGrainProperty ;
                       rdfs:comment "Diameter (D) of energy grain, (5 % in mass may have diameter over the class)"@en ;
                       rdfs:label "Dimensions of energy grain"@en .


###  http://w3.id.org/def/BiomassOntology#EnergyGrainF
:EnergyGrainF rdf:type owl:NamedIndividual ,
                       :EnergyGrainProperty ;
              rdfs:comment "% in mass, fines < 3,15 mm for D 10"@en ;
              rdfs:label "Amount of fines of energy grain"@en .


###  http://w3.id.org/def/BiomassOntology#EnergyGrainFs
:EnergyGrainFs rdf:type owl:NamedIndividual ,
                        :EnergyGrainProperty ;
               rdfs:comment "% in mass,small fines (Fs)< 1 mm for D 05"@en ;
               rdfs:label "Amount of small fines of energy grain"@en .


###  http://w3.id.org/def/BiomassOntology#EnergyGrainM
:EnergyGrainM rdf:type owl:NamedIndividual ,
                       :EnergyGrainProperty ,
                       :Moisture ;
              rdfs:comment "% in mass of moisture in energy grain as received"@en ;
              rdfs:label "Moisture of energy grain"@en .


###  http://w3.id.org/def/BiomassOntology#EnergyGrainN
:EnergyGrainN rdf:type owl:NamedIndividual ,
                       :EnergyGrainProperty ,
                       :Nitrogen ;
              rdfs:comment "% in mass of nitrogen in energy grain of dry basis"@en ;
              rdfs:label "Nitrogen of energy grain"@en .


###  http://w3.id.org/def/BiomassOntology#EnergyGrainQ
:EnergyGrainQ rdf:type owl:NamedIndividual ,
                       :CalorificValue ,
                       :EnergyGrainProperty ;
              rdfs:comment "MJ/kg or kWh/kg of energy grain as received"@en ;
              rdfs:label "Net calorific value of energy grain"@en .


###  http://w3.id.org/def/BiomassOntology#EnergyGrainS
:EnergyGrainS rdf:type owl:NamedIndividual ,
                       :EnergyGrainProperty ,
                       :Sulfur ;
              rdfs:comment "% in mass of sulfur in energy grain of dry basis"@en ;
              rdfs:label "Sulfur of energy grain"@en .


###  http://w3.id.org/def/BiomassOntology#F02WoodChipsHogFuel
:F02WoodChipsHogFuel rdf:type owl:NamedIndividual ,
                              :WoodChipsHogFuelResult ;
                     rdfs:comment "≤ 2 % in mass of fines, < 3,15 mm particles"@en ;
                     rdfs:label "F02 Wood Chips/Hog Fuel"@en .


###  http://w3.id.org/def/BiomassOntology#F05WoodChipsHogFuel
:F05WoodChipsHogFuel rdf:type owl:NamedIndividual ,
                              :WoodChipsHogFuelResult ;
                     rdfs:comment "≤ 5 % in mass of fines, < 3,15 mm particles"@en ;
                     rdfs:label "F05 Wood Chips/Hog Fuel"@en .


###  http://w3.id.org/def/BiomassOntology#F10WoodChipsHogFuel
:F10WoodChipsHogFuel rdf:type owl:NamedIndividual ,
                              :WoodChipsHogFuelResult ;
                     rdfs:comment "≤ 10 % in mass of fines, < 3,15 mm particles"@en ;
                     rdfs:label "F10 Wood Chips/Hog Fuel"@en .


###  http://w3.id.org/def/BiomassOntology#F15WoodChipsHogFuel
:F15WoodChipsHogFuel rdf:type owl:NamedIndividual ,
                              :WoodChipsHogFuelResult ;
                     rdfs:comment "≤ 15 % in mass of fines, < 3,15 mm particles"@en ;
                     rdfs:label "F15 Wood Chips/Hog Fuel"@en .


###  http://w3.id.org/def/BiomassOntology#F1EnergyGrain
:F1EnergyGrain rdf:type owl:NamedIndividual ,
                        :EnergyGrainResult ;
               rdfs:comment "≤ 1,0 % in mass of  fines in energy grain,  fines < 3,15 mm for D 10"@en ;
               rdfs:label "F1.0 EnergyGrain"@en .


###  http://w3.id.org/def/BiomassOntology#F1OliveResidues
:F1OliveResidues rdf:type owl:NamedIndividual ,
                          :OliveResiduesResult ;
                 rdfs:comment "≤ 1,0 % in mass of  fines in olive residues, fines < 3,15 mm for D 10 and D10+"@en ;
                 rdfs:label "F1.0 OliveResidues"@en .


###  http://w3.id.org/def/BiomassOntology#F1Pellet
:F1Pellet rdf:type owl:NamedIndividual ,
                   :PelletResult ;
          rdfs:comment "≤ 1,0 % in mass of fines, particles < 3,15 mm. after production when loaded or packed"@en ;
          rdfs:label "F1.0 Pellet"@en .


###  http://w3.id.org/def/BiomassOntology#F20WoodChipsHogFuel
:F20WoodChipsHogFuel rdf:type owl:NamedIndividual ,
                              :WoodChipsHogFuelResult ;
                     rdfs:comment "≤ 20 % in mass of fines, < 3,15 mm particles"@en ;
                     rdfs:label "F20 Wood Chips/Hog Fuel"@en .


###  http://w3.id.org/def/BiomassOntology#F25WoodChipsHogFuel
:F25WoodChipsHogFuel rdf:type owl:NamedIndividual ,
                              :WoodChipsHogFuelResult ;
                     rdfs:comment "≤ 25 % in mass of fines, < 3,15 mm particles"@en ;
                     rdfs:label "F25 Wood Chips/Hog Fuel"@en .


###  http://w3.id.org/def/BiomassOntology#F2Pellet
:F2Pellet rdf:type owl:NamedIndividual ,
                   :PelletResult ;
          rdfs:comment "≤ 2,0 % in mass of fines, particles < 3,15 mm. after production when loaded or packed"@en ;
          rdfs:label "F2.0 Pellet"@en .


###  http://w3.id.org/def/BiomassOntology#F30WoodChipsHogFuel
:F30WoodChipsHogFuel rdf:type owl:NamedIndividual ,
                              :WoodChipsHogFuelResult ;
                     rdfs:comment "≤ 30 % in mass of fines, < 3,15 mm particles"@en ;
                     rdfs:label "F30 Wood Chips/Hog Fuel"@en .


###  http://w3.id.org/def/BiomassOntology#F3Pellet
:F3Pellet rdf:type owl:NamedIndividual ,
                   :PelletResult ;
          rdfs:comment "≤ 3,0 % in mass of fines, particles < 3,15 mm. after production when loaded or packed"@en ;
          rdfs:label "F3.0 Pellet"@en .


###  http://w3.id.org/def/BiomassOntology#F4Pellet
:F4Pellet rdf:type owl:NamedIndividual ,
                   :PelletResult ;
          rdfs:comment "≤ 4,0 % in mass of fines, particles < 3,15 mm. after production when loaded or packed"@en ;
          rdfs:label "F4.0 Pellet"@en .


###  http://w3.id.org/def/BiomassOntology#F5Pellet
:F5Pellet rdf:type owl:NamedIndividual ,
                   :PelletResult ;
          rdfs:comment "≤ 5,0 % in mass of fines, particles < 3,15 mm. after production when loaded or packed"@en ;
          rdfs:label "F5.0 Pellet"@en .


###  http://w3.id.org/def/BiomassOntology#F6Pellet
:F6Pellet rdf:type owl:NamedIndividual ,
                   :PelletResult ;
          rdfs:comment "≤ 6,0 % in mass of fines, particles < 3,15 mm. after production when loaded or packed"@en ;
          rdfs:label "F6.0 Pellet"@en .


###  http://w3.id.org/def/BiomassOntology#FruitSeedsA
:FruitSeedsA rdf:type owl:NamedIndividual ,
                      :Ash ,
                      :FruitSeedsProperty ;
             rdfs:comment "% in mass of ash in fruit seeds of dry basis"@en ;
             rdfs:label "Ash of fruit seeds"@en .


###  http://w3.id.org/def/BiomassOntology#FruitSeedsAdditives
:FruitSeedsAdditives rdf:type owl:NamedIndividual ,
                              :AdditivesContent ,
                              :FruitSeedsProperty ;
                     rdfs:comment "% in mass of fruit seeds. Type and content of additives have to be stated"@en ;
                     rdfs:label "Additives of fruit seeds"@en .


###  http://w3.id.org/def/BiomassOntology#FruitSeedsAshMB
:FruitSeedsAshMB rdf:type owl:NamedIndividual ,
                          :AshMeltingBehaviour ,
                          :FruitSeedsProperty ;
                 rdfs:comment "Deformation Temperatue, Hemisphere Temperature and Flow Temperature of fruit seeds should be stated"@en ;
                 rdfs:label "Ash melting behaviour of fruit seeds"@en .


###  http://w3.id.org/def/BiomassOntology#FruitSeedsBD
:FruitSeedsBD rdf:type owl:NamedIndividual ,
                       :BulkDensity ,
                       :FruitSeedsProperty ;
              rdfs:comment "kg/m3 of fruit seeds as received. Recommended to be stated if traded on a volume basis"@en ;
              rdfs:label "Bulk density of fruit seeds"@en .


###  http://w3.id.org/def/BiomassOntology#FruitSeedsCl
:FruitSeedsCl rdf:type owl:NamedIndividual ,
                       :Chlorine ,
                       :FruitSeedsProperty ;
              rdfs:comment "% in mass of chlorine in fruit seeds of dry basis"@en ;
              rdfs:label "Chlorine of fruit seeds"@en .


###  http://w3.id.org/def/BiomassOntology#FruitSeedsDimensions
:FruitSeedsDimensions rdf:type owl:NamedIndividual ,
                               :Diameter ,
                               :FruitSeedsProperty ;
                      rdfs:comment "Diameter (D) of fruit seeds, (5 % in mass may have diameter over the class)"@en ;
                      rdfs:label "Dimensions of fruit seeds"@en .


###  http://w3.id.org/def/BiomassOntology#FruitSeedsFs
:FruitSeedsFs rdf:type owl:NamedIndividual ,
                       :FruitSeedsProperty ;
              rdfs:comment "% in mass, small fines < 1 mm"@en ;
              rdfs:label "Amount of small fines of fruit seeds"@en .


###  http://w3.id.org/def/BiomassOntology#FruitSeedsM
:FruitSeedsM rdf:type owl:NamedIndividual ,
                      :FruitSeedsProperty ,
                      :Moisture ;
             rdfs:comment "% in mass of moisture in fruit seeds as received"@en ;
             rdfs:label "Moisture of fruit seeds"@en .


###  http://w3.id.org/def/BiomassOntology#FruitSeedsN
:FruitSeedsN rdf:type owl:NamedIndividual ,
                      :FruitSeedsProperty ,
                      :Nitrogen ;
             rdfs:comment "% in mass of nitrogen in fruit seeds of dry basis"@en ;
             rdfs:label "Nitrogen of fruit seeds"@en .


###  http://w3.id.org/def/BiomassOntology#FruitSeedsQ
:FruitSeedsQ rdf:type owl:NamedIndividual ,
                      :CalorificValue ,
                      :FruitSeedsProperty ;
             rdfs:comment "MJ/kg or kWh/kg of fruit seeds as received"@en ;
             rdfs:label "Net calorific value of fruit seeds"@en .


###  http://w3.id.org/def/BiomassOntology#FruitSeedsS
:FruitSeedsS rdf:type owl:NamedIndividual ,
                      :FruitSeedsProperty ,
                      :Sulfur ;
             rdfs:comment "% in mass of sulfur in fruit seeds of dry basis"@en ;
             rdfs:label "Sulfur of fruit seeds"@en .


###  http://w3.id.org/def/BiomassOntology#Fs1EnergyGrain
:Fs1EnergyGrain rdf:type owl:NamedIndividual ,
                         :EnergyGrainResult ;
                rdfs:comment "≤ 1,0 % in mass of small fines in energy grain, small fines (Fs)< 1 mm for D 05"@en ;
                rdfs:label "Fs1.0 EnergyGrain"@en .


###  http://w3.id.org/def/BiomassOntology#Fs1FruitSeeds
:Fs1FruitSeeds rdf:type owl:NamedIndividual ,
                        :FruitSeedsResult ;
               rdfs:comment "≤ 1,0 % in mass of small fines in fruit seeds, small fines < 1 mm"@en ;
               rdfs:label "Fs1.0 FruitSeeds"@en .


###  http://w3.id.org/def/BiomassOntology#Fs1OliveResidues
:Fs1OliveResidues rdf:type owl:NamedIndividual ,
                           :OliveResiduesResult ;
                  rdfs:comment "≤ 1,0 % in mass of small fines in olive residues, small fines < 1 mm for for D 03 and D 05"@en ;
                  rdfs:label "Fs1.0 OliveResidues"@en .


###  http://w3.id.org/def/BiomassOntology#L100LogFirewood
:L100LogFirewood rdf:type owl:NamedIndividual ,
                          :LogFirewoodResult ;
                 rdfs:comment "100 cm ± 5 cm maximum length of a single piece of log wood/ firewood"@en ;
                 rdfs:label "L100 Log wood/Firewood"@en .


###  http://w3.id.org/def/BiomassOntology#L20-LogFirewood
:L20-LogFirewood rdf:type owl:NamedIndividual ,
                          :LogFirewoodResult ;
                 rdfs:comment "< 20 cm maximum length of a single piece of log wood/ firewood"@en ;
                 rdfs:label "L20- Log wood/Firewood"@en .


###  http://w3.id.org/def/BiomassOntology#L20LogFirewood
:L20LogFirewood rdf:type owl:NamedIndividual ,
                         :LogFirewoodResult ;
                rdfs:comment "20 cm ± 2 cm maximum length of a single piece of log wood/ firewood"@en ;
                rdfs:label "L20 Log wood/Firewood"@en .


###  http://w3.id.org/def/BiomassOntology#L25LogFirewood
:L25LogFirewood rdf:type owl:NamedIndividual ,
                         :LogFirewoodResult ;
                rdfs:comment "25 cm ± 2 cm maximum length of a single piece of log wood/ firewood"@en ;
                rdfs:label "L25 Log wood/Firewood"@en .


###  http://w3.id.org/def/BiomassOntology#L30LogFirewood
:L30LogFirewood rdf:type owl:NamedIndividual ,
                         :LogFirewoodResult ;
                rdfs:comment "30 cm ± 2 cm maximum length of a single piece of log wood/ firewood"@en ;
                rdfs:label "L30 Log wood/Firewood"@en .


###  http://w3.id.org/def/BiomassOntology#L33LogFirewood
:L33LogFirewood rdf:type owl:NamedIndividual ,
                         :LogFirewoodResult ;
                rdfs:comment "33 cm ± 2 cm maximum length of a single piece of log wood/ firewood"@en ;
                rdfs:label "L33 Log wood/Firewood"@en .


###  http://w3.id.org/def/BiomassOntology#L40LogFirewood
:L40LogFirewood rdf:type owl:NamedIndividual ,
                         :LogFirewoodResult ;
                rdfs:comment "40 cm ± 2 cm maximum length of a single piece of log wood/ firewood"@en ;
                rdfs:label "L40 Log wood/Firewood"@en .


###  http://w3.id.org/def/BiomassOntology#L50LogFirewood
:L50LogFirewood rdf:type owl:NamedIndividual ,
                         :LogFirewoodResult ;
                rdfs:comment "50 cm ± 4 cm maximum length of a single piece of log wood/ firewood"@en ;
                rdfs:label "L50 Log wood/Firewood"@en .


###  http://w3.id.org/def/BiomassOntology#LogFirewoodCutOffSurface
:LogFirewoodCutOffSurface rdf:type owl:NamedIndividual ,
                                   :LogFirewoodProperty ;
                          rdfs:comment "To be stated if the cut-off surface of log wood is even and smooth d or ends of log wood is uneven"@en ;
                          rdfs:label "Cut-off surface of log wood/ firewood"@en .


###  http://w3.id.org/def/BiomassOntology#LogFirewoodD
:LogFirewoodD rdf:type owl:NamedIndividual ,
                       :LogFirewoodProperty ;
              rdfs:comment "Diameter of a single piece of log wood/ firewood (cm)"@en ;
              rdfs:label "Diameter of log wood/ firewood"@en .


###  http://w3.id.org/def/BiomassOntology#LogFirewoodDecayMould
:LogFirewoodDecayMould rdf:type owl:NamedIndividual ,
                                :LogFirewoodProperty ;
                       rdfs:comment "No visible decay or mould < 5% of pieces. If significant amount (more than 10% of pieces) of decay or mould exists it should be stated."@en ;
                       rdfs:label "Decay and mould of log wood/ firewood"@en .


###  http://w3.id.org/def/BiomassOntology#LogFirewoodDrying
:LogFirewoodDrying rdf:type owl:NamedIndividual ,
                            :LogFirewoodProperty ;
                   rdfs:comment "To be stated, if firewood is dried by natural seasoning by ambient air or artificially by hot air."@en ;
                   rdfs:label "Drying of log wood/ firewood"@en .


###  http://w3.id.org/def/BiomassOntology#LogFirewoodL
:LogFirewoodL rdf:type owl:NamedIndividual ,
                       :Length ,
                       :LogFirewoodProperty ;
              rdfs:comment "Maximum length of a single piece of log wood/ firewood (cm)"@en ;
              rdfs:label "Length of log wood/ firewood"@en .


###  http://w3.id.org/def/BiomassOntology#LogFirewoodM
:LogFirewoodM rdf:type owl:NamedIndividual ,
                       :LogFirewoodProperty ,
                       :Moisture ;
              rdfs:comment "% in mass of moisture as received on wet basis of log wood/ firewood"@en ;
              rdfs:label "Moisture of log wood/ firewood"@en .


###  http://w3.id.org/def/BiomassOntology#LogFirewoodQ
:LogFirewoodQ rdf:type owl:NamedIndividual ,
                       :CalorificValue ,
                       :LogFirewoodProperty ;
              rdfs:comment "MJ/kg or kWh/kg of log wood/ firewood as received"@en ;
              rdfs:label "Net calorific value of log wood/ firewood"@en .


###  http://w3.id.org/def/BiomassOntology#LogFirewoodSplitVolume
:LogFirewoodSplitVolume rdf:type owl:NamedIndividual ,
                                 :LogFirewoodProperty ;
                        rdfs:comment "No split (= mainly round wood) or ≥ 50% or ≥ 90% split volume of log wood/ firewood"@en ;
                        rdfs:label "Proportion of split volume of log wood/ firewood"@en .


###  http://w3.id.org/def/BiomassOntology#LogFirewoodVolumeWeight
:LogFirewoodVolumeWeight rdf:type owl:NamedIndividual ,
                                  :LogFirewoodProperty ;
                         rdfs:comment "To be stated which unit is used when retailed (m3 stacked or m3 loose, kg) and/or packaged log woods weight."@en ;
                         rdfs:label "Volume stacked or loose or weight as received of log wood/ firewood"@en .


###  http://w3.id.org/def/BiomassOntology#M05Pellet
:M05Pellet rdf:type owl:NamedIndividual ,
                    :PelletResult ;
           rdfs:comment "≤ 5 % in mass of moisture in pellets as received"@en ;
           rdfs:label "M05 Pellet"@en .


###  http://w3.id.org/def/BiomassOntology#M08Pellet
:M08Pellet rdf:type owl:NamedIndividual ,
                    :PelletResult ;
           rdfs:comment "≤ 8 % in mass of moisture in pellets as received"@en ;
           rdfs:label "M08 Pellet"@en .


###  http://w3.id.org/def/BiomassOntology#M10Bale
:M10Bale rdf:type owl:NamedIndividual ,
                  :BaleResult ;
         rdfs:comment "≤ 10 % in mass of moisture in bale as received"@en ;
         rdfs:label "M10 Bale"@en .


###  http://w3.id.org/def/BiomassOntology#M10Briquette
:M10Briquette rdf:type owl:NamedIndividual ,
                       :BriquetteResult ;
              rdfs:comment "≤ 10 % in mass of moisture in briquettes as received"@en ;
              rdfs:label "M10 Briquette"@en .


###  http://w3.id.org/def/BiomassOntology#M10Charcoal
:M10Charcoal rdf:type owl:NamedIndividual ,
                      :CharcoalResult ;
             rdfs:comment "≤ 10 % in mass of moisture in charcoal as received"@en ;
             rdfs:label "M10 Charcoal"@en .


###  http://w3.id.org/def/BiomassOntology#M10EnergyGrain
:M10EnergyGrain rdf:type owl:NamedIndividual ,
                         :EnergyGrainResult ;
                rdfs:comment "≤ 10 % in mass of moisture in energy grain as received"@en ;
                rdfs:label "M10 EnergyGrain"@en .


###  http://w3.id.org/def/BiomassOntology#M10FruitSeeds
:M10FruitSeeds rdf:type owl:NamedIndividual ,
                        :FruitSeedsResult ;
               rdfs:comment "≤ 10 % in mass of moisture in fruit seeds as received"@en ;
               rdfs:label "M10 FruitSeeds"@en .


###  http://w3.id.org/def/BiomassOntology#M10LogFirewood
:M10LogFirewood rdf:type owl:NamedIndividual ,
                         :LogFirewoodResult ;
                rdfs:comment "≤ 10% in mass of moisture as received on wet basis of log wood/ firewood"@en ;
                rdfs:label "M10 Log wood/Firewood"@en .


###  http://w3.id.org/def/BiomassOntology#M10OliveResidues
:M10OliveResidues rdf:type owl:NamedIndividual ,
                           :OliveResiduesResult ;
                  rdfs:comment "≤ 10 % in mass of moisture in olive residues as received"@en ;
                  rdfs:label "M10 OliveResidues"@en .


###  http://w3.id.org/def/BiomassOntology#M10Pellet
:M10Pellet rdf:type owl:NamedIndividual ,
                    :PelletResult ;
           rdfs:comment "≤ 10 % in mass of moisture in pellets as received"@en ;
           rdfs:label "M10 Pellet"@en .


###  http://w3.id.org/def/BiomassOntology#M10Sawdust
:M10Sawdust rdf:type owl:NamedIndividual ,
                     :SawdustResult ;
            rdfs:comment "≤ 10 % in mass of moisture in sawdust as received"@en ;
            rdfs:label "M10 Sawdust"@en .


###  http://w3.id.org/def/BiomassOntology#M10Shavings
:M10Shavings rdf:type owl:NamedIndividual ,
                      :ShavingsResult ;
             rdfs:comment "≤ 10 % in mass of moisture in shavings as received"@en ;
             rdfs:label "M10 Shavings"@en .


###  http://w3.id.org/def/BiomassOntology#M10WoodChipsHogFuel
:M10WoodChipsHogFuel rdf:type owl:NamedIndividual ,
                              :WoodChipsHogFuelResult ;
                     rdfs:comment "≤ 10 % in mass of moisture in wood chips/hog fuel as received"@en ;
                     rdfs:label "M10 Wood Chips/Hog Fuel"@en .


###  http://w3.id.org/def/BiomassOntology#M12Briquette
:M12Briquette rdf:type owl:NamedIndividual ,
                       :BriquetteResult ;
              rdfs:comment "≤ 12 % in mass of moisture in briquettes as received"@en ;
              rdfs:label "M12 Briquette"@en .


###  http://w3.id.org/def/BiomassOntology#M12Pellet
:M12Pellet rdf:type owl:NamedIndividual ,
                    :PelletResult ;
           rdfs:comment "≤ 12 % in mass of moisture in pellets as received"@en ;
           rdfs:label "M12 Pellet"@en .


###  http://w3.id.org/def/BiomassOntology#M15Bale
:M15Bale rdf:type owl:NamedIndividual ,
                  :BaleResult ;
         rdfs:comment "≤ 15 % in mass of moisture in bale as received"@en ;
         rdfs:label "M15 Bale"@en .


###  http://w3.id.org/def/BiomassOntology#M15Briquette
:M15Briquette rdf:type owl:NamedIndividual ,
                       :BriquetteResult ;
              rdfs:comment "≤ 15 % in mass of moisture in briquettes as received"@en ;
              rdfs:label "M15 Briquette"@en .


###  http://w3.id.org/def/BiomassOntology#M15EnergyGrain
:M15EnergyGrain rdf:type owl:NamedIndividual ,
                         :EnergyGrainResult ;
                rdfs:comment "≤ 15 % in mass of moisture in energy grain as received"@en ;
                rdfs:label "M15 EnergyGrain"@en .


###  http://w3.id.org/def/BiomassOntology#M15FruitSeeds
:M15FruitSeeds rdf:type owl:NamedIndividual ,
                        :FruitSeedsResult ;
               rdfs:comment "≤ 15 % in mass of moisture in fruit seeds as received"@en ;
               rdfs:label "M15 FruitSeeds"@en .


###  http://w3.id.org/def/BiomassOntology#M15LogFirewood
:M15LogFirewood rdf:type owl:NamedIndividual ,
                         :LogFirewoodResult ;
                rdfs:comment "≤ 15% in mass of moisture as received on wet basis of log wood/ firewood"@en ;
                rdfs:label "M15 Log wood/Firewood"@en .


###  http://w3.id.org/def/BiomassOntology#M15OliveResidues
:M15OliveResidues rdf:type owl:NamedIndividual ,
                           :OliveResiduesResult ;
                  rdfs:comment "≤ 15 % in mass of moisture in olive residues as received"@en ;
                  rdfs:label "M15 OliveResidues"@en .


###  http://w3.id.org/def/BiomassOntology#M15Pellet
:M15Pellet rdf:type owl:NamedIndividual ,
                    :PelletResult ;
           rdfs:comment "≤ 15 % in mass of moisture in pellets as received"@en ;
           rdfs:label "M15 Pellet"@en .


###  http://w3.id.org/def/BiomassOntology#M15Sawdust
:M15Sawdust rdf:type owl:NamedIndividual ,
                     :SawdustResult ;
            rdfs:comment "≤ 15 % in mass of moisture in sawdust as received"@en ;
            rdfs:label "M15 Sawdust"@en .


###  http://w3.id.org/def/BiomassOntology#M15Shavings
:M15Shavings rdf:type owl:NamedIndividual ,
                      :ShavingsResult ;
             rdfs:comment "≤ 15 % in mass of moisture in shavings as received"@en ;
             rdfs:label "M15 Shavings"@en .


###  http://w3.id.org/def/BiomassOntology#M15WoodChipsHogFuel
:M15WoodChipsHogFuel rdf:type owl:NamedIndividual ,
                              :WoodChipsHogFuelResult ;
                     rdfs:comment "≤ 15 % in mass of moisture in wood chips/hog fuel as received"@en ;
                     rdfs:label "M15 Wood Chips/Hog Fuel"@en .


###  http://w3.id.org/def/BiomassOntology#M20Bale
:M20Bale rdf:type owl:NamedIndividual ,
                  :BaleResult ;
         rdfs:comment "≤ 20 % in mass of moisture in bale as received"@en ;
         rdfs:label "M20 Bale"@en .


###  http://w3.id.org/def/BiomassOntology#M20Bark
:M20Bark rdf:type owl:NamedIndividual ,
                  :BarkResult ;
         rdfs:comment "≤ 20 % in mass of moisture in bark as received"@en ;
         rdfs:label "M20 Bark"@en .


###  http://w3.id.org/def/BiomassOntology#M20LogFirewood
:M20LogFirewood rdf:type owl:NamedIndividual ,
                         :LogFirewoodResult ;
                rdfs:comment "≤ 20% in mass of moisture as received on wet basis of log wood/ firewood"@en ;
                rdfs:label "M20 Log wood/Firewood"@en .


###  http://w3.id.org/def/BiomassOntology#M20Sawdust
:M20Sawdust rdf:type owl:NamedIndividual ,
                     :SawdustResult ;
            rdfs:comment "≤ 20 % in mass of moisture in sawdust as received"@en ;
            rdfs:label "M20 Sawdust"@en .


###  http://w3.id.org/def/BiomassOntology#M20Shavings
:M20Shavings rdf:type owl:NamedIndividual ,
                      :ShavingsResult ;
             rdfs:comment "≤ 20 % in mass of moisture in shavings as received"@en ;
             rdfs:label "M20 Shavings"@en .


###  http://w3.id.org/def/BiomassOntology#M20WoodChipsHogFuel
:M20WoodChipsHogFuel rdf:type owl:NamedIndividual ,
                              :WoodChipsHogFuelResult ;
                     rdfs:comment "≤ 20 % in mass of moisture in wood chips/hog fuel as received"@en ;
                     rdfs:label "M20 Wood Chips/Hog Fuel"@en .


###  http://w3.id.org/def/BiomassOntology#M25Bale
:M25Bale rdf:type owl:NamedIndividual ,
                  :BaleResult ;
         rdfs:comment "≤ 25 % in mass of moisture in bale as received"@en ;
         rdfs:label "M25 Bale"@en .


###  http://w3.id.org/def/BiomassOntology#M25Bark
:M25Bark rdf:type owl:NamedIndividual ,
                  :BarkResult ;
         rdfs:comment "≤ 25 % in mass of moisture in bark as received"@en ;
         rdfs:label "M25 Bark"@en .


###  http://w3.id.org/def/BiomassOntology#M25LogFirewood
:M25LogFirewood rdf:type owl:NamedIndividual ,
                         :LogFirewoodResult ;
                rdfs:comment "≤ 25% in mass of moisture as received on wet basis of log wood/ firewood"@en ;
                rdfs:label "M25 Log wood/Firewood"@en .


###  http://w3.id.org/def/BiomassOntology#M25Sawdust
:M25Sawdust rdf:type owl:NamedIndividual ,
                     :SawdustResult ;
            rdfs:comment "≤ 25 % in mass of moisture in sawdust as received"@en ;
            rdfs:label "M25 Sawdust"@en .


###  http://w3.id.org/def/BiomassOntology#M25WoodChipsHogFuel
:M25WoodChipsHogFuel rdf:type owl:NamedIndividual ,
                              :WoodChipsHogFuelResult ;
                     rdfs:comment "≤ 25 % in mass of moisture in wood chips/hog fuel as received"@en ;
                     rdfs:label "M25 Wood Chips/Hog Fuel"@en .


###  http://w3.id.org/def/BiomassOntology#M30Bale
:M30Bale rdf:type owl:NamedIndividual ,
                  :BaleResult ;
         rdfs:comment "≤ 30 % in mass of moisture in bale as received"@en ;
         rdfs:label "M30 Bale"@en .


###  http://w3.id.org/def/BiomassOntology#M30Bark
:M30Bark rdf:type owl:NamedIndividual ,
                  :BarkResult ;
         rdfs:comment "≤ 30 % in mass of moisture in bark as received"@en ;
         rdfs:label "M30 Bark"@en .


###  http://w3.id.org/def/BiomassOntology#M30LogFirewood
:M30LogFirewood rdf:type owl:NamedIndividual ,
                         :LogFirewoodResult ;
                rdfs:comment "≤ 30% in mass of moisture as received on wet basis of log wood/ firewood"@en ;
                rdfs:label "M30 Log wood/Firewood"@en .


###  http://w3.id.org/def/BiomassOntology#M30Sawdust
:M30Sawdust rdf:type owl:NamedIndividual ,
                     :SawdustResult ;
            rdfs:comment "≤ 30 % in mass of moisture in sawdust as received"@en ;
            rdfs:label "M30 Sawdust"@en .


###  http://w3.id.org/def/BiomassOntology#M30Shavings
:M30Shavings rdf:type owl:NamedIndividual ,
                      :ShavingsResult ;
             rdfs:comment "≤ 30 % in mass of moisture in shavings as received"@en ;
             rdfs:label "M30 Shavings"@en .


###  http://w3.id.org/def/BiomassOntology#M30WoodChipsHogFuel
:M30WoodChipsHogFuel rdf:type owl:NamedIndividual ,
                              :WoodChipsHogFuelResult ;
                     rdfs:comment "≤ 30 % in mass of moisture in wood chips/hog fuel as received"@en ;
                     rdfs:label "M30 Wood Chips/Hog Fuel"@en .


###  http://w3.id.org/def/BiomassOntology#M35Bark
:M35Bark rdf:type owl:NamedIndividual ,
                  :BarkResult ;
         rdfs:comment "≤ 35 % in mass of moisture in bark as received"@en ;
         rdfs:label "M35 Bark"@en .


###  http://w3.id.org/def/BiomassOntology#M35LogFirewood
:M35LogFirewood rdf:type owl:NamedIndividual ,
                         :LogFirewoodResult ;
                rdfs:comment "≤ 35% in mass of moisture as received on wet basis of log wood/ firewood"@en ;
                rdfs:label "M35 Log wood/Firewood"@en .


###  http://w3.id.org/def/BiomassOntology#M35Sawdust
:M35Sawdust rdf:type owl:NamedIndividual ,
                     :SawdustResult ;
            rdfs:comment "≤ 35 % in mass of moisture in sawdust as received"@en ;
            rdfs:label "M35 Sawdust"@en .


###  http://w3.id.org/def/BiomassOntology#M35WoodChipsHogFuel
:M35WoodChipsHogFuel rdf:type owl:NamedIndividual ,
                              :WoodChipsHogFuelResult ;
                     rdfs:comment "≤ 35 % in mass of moisture in wood chips/hog fuel as received"@en ;
                     rdfs:label "M35 Wood Chips/Hog Fuel"@en .


###  http://w3.id.org/def/BiomassOntology#M40Bark
:M40Bark rdf:type owl:NamedIndividual ,
                  :BarkResult ;
         rdfs:comment "≤ 40 % in mass of moisture in bark as received"@en ;
         rdfs:label "M40 Bark"@en .


###  http://w3.id.org/def/BiomassOntology#M40LogFirewood
:M40LogFirewood rdf:type owl:NamedIndividual ,
                         :LogFirewoodResult ;
                rdfs:comment "≤ 40% in mass of moisture as received on wet basis of log wood/ firewood"@en ;
                rdfs:label "M40 Log wood/Firewood"@en .


###  http://w3.id.org/def/BiomassOntology#M40WoodChipsHogFuel
:M40WoodChipsHogFuel rdf:type owl:NamedIndividual ,
                              :WoodChipsHogFuelResult ;
                     rdfs:comment "≤ 40 % in mass of moisture in wood chips/hog fuel as received"@en ;
                     rdfs:label "M40 Wood Chips/Hog Fuel"@en .


###  http://w3.id.org/def/BiomassOntology#M45Bark
:M45Bark rdf:type owl:NamedIndividual ,
                  :BarkResult ;
         rdfs:comment "≤ 45 % in mass of moisture in bark as received"@en ;
         rdfs:label "M45 Bark"@en .


###  http://w3.id.org/def/BiomassOntology#M45LogFirewood
:M45LogFirewood rdf:type owl:NamedIndividual ,
                         :LogFirewoodResult ;
                rdfs:comment "≤ 45% in mass of moisture as received on wet basis of log wood/ firewood"@en ;
                rdfs:label "M45 Log wood/Firewood"@en .


###  http://w3.id.org/def/BiomassOntology#M45Sawdust
:M45Sawdust rdf:type owl:NamedIndividual ,
                     :SawdustResult ;
            rdfs:comment "≤ 45 % in mass of moisture in sawdust as received"@en ;
            rdfs:label "M45 Sawdust"@en .


###  http://w3.id.org/def/BiomassOntology#M45WoodChipsHogFuel
:M45WoodChipsHogFuel rdf:type owl:NamedIndividual ,
                              :WoodChipsHogFuelResult ;
                     rdfs:comment "≤ 45 % in mass of moisture in wood chips/hog fuel as received"@en ;
                     rdfs:label "M45 Wood Chips/Hog Fuel"@en .


###  http://w3.id.org/def/BiomassOntology#M50Bark
:M50Bark rdf:type owl:NamedIndividual ,
                  :BarkResult ;
         rdfs:comment "≤ 50 % in mass of moisture in bark as received"@en ;
         rdfs:label "M50 Bark"@en .


###  http://w3.id.org/def/BiomassOntology#M50Sawdust
:M50Sawdust rdf:type owl:NamedIndividual ,
                     :SawdustResult ;
            rdfs:comment "≤ 50 % in mass of moisture in sawdust as received"@en ;
            rdfs:label "M50 Sawdust"@en .


###  http://w3.id.org/def/BiomassOntology#M50WoodChipsHogFuel
:M50WoodChipsHogFuel rdf:type owl:NamedIndividual ,
                              :WoodChipsHogFuelResult ;
                     rdfs:comment "≤ 50 % in mass of moisture in wood chips/hog fuel as received"@en ;
                     rdfs:label "M50 Wood Chips/Hog Fuel"@en .


###  http://w3.id.org/def/BiomassOntology#M55Bark
:M55Bark rdf:type owl:NamedIndividual ,
                  :BarkResult ;
         rdfs:comment "≤ 55 % in mass of moisture in bark as received"@en ;
         rdfs:label "M55 Bark"@en .


###  http://w3.id.org/def/BiomassOntology#M55LogFirewood
:M55LogFirewood rdf:type owl:NamedIndividual ,
                         :LogFirewoodResult ;
                rdfs:comment "≤ 55% in mass of moisture as received on wet basis of log wood/ firewood"@en ;
                rdfs:label "M55 Log wood/Firewood"@en .


###  http://w3.id.org/def/BiomassOntology#M55Sawdust
:M55Sawdust rdf:type owl:NamedIndividual ,
                     :SawdustResult ;
            rdfs:comment "≤ 55 % in mass of moisture in sawdust as received"@en ;
            rdfs:label "M55 Sawdust"@en .


###  http://w3.id.org/def/BiomassOntology#M55WoodChipsHogFuel
:M55WoodChipsHogFuel rdf:type owl:NamedIndividual ,
                              :WoodChipsHogFuelResult ;
                     rdfs:comment "≤ 55 % in mass of moisture in wood chips/hog fuel as received"@en ;
                     rdfs:label "M55 Wood Chips/Hog Fuel"@en .


###  http://w3.id.org/def/BiomassOntology#M60Bark
:M60Bark rdf:type owl:NamedIndividual ,
                  :BarkResult ;
         rdfs:comment "≤ 60 % in mass of moisture in bark as received"@en ;
         rdfs:label "M60 Bark"@en .


###  http://w3.id.org/def/BiomassOntology#M60Sawdust
:M60Sawdust rdf:type owl:NamedIndividual ,
                     :SawdustResult ;
            rdfs:comment "≤ 60 % in mass of moisture in sawdust as received"@en ;
            rdfs:label "M60 Sawdust"@en .


###  http://w3.id.org/def/BiomassOntology#M65Bark
:M65Bark rdf:type owl:NamedIndividual ,
                  :BarkResult ;
         rdfs:comment "≤ 65 % in mass of moisture in bark as received"@en ;
         rdfs:label "M65 Bark"@en .


###  http://w3.id.org/def/BiomassOntology#M65Sawdust
:M65Sawdust rdf:type owl:NamedIndividual ,
                     :SawdustResult ;
            rdfs:comment "≤ 65 % in mass of moisture in sawdust as received"@en ;
            rdfs:label "M65 Sawdust"@en .


###  http://w3.id.org/def/BiomassOntology#M8Charcoal
:M8Charcoal rdf:type owl:NamedIndividual ,
                     :CharcoalResult ;
            rdfs:comment "≤ 8 % in mass of moisture in charcoal as received"@en ;
            rdfs:label "M8 Charcoal"@en .


###  http://w3.id.org/def/BiomassOntology#N0.2Briquette
:N0.2Briquette rdf:type owl:NamedIndividual ,
                        :BriquetteResult ;
               rdfs:comment "≤ 0,2 % in mass of nitrogen in briquettes of dry basis"@en ;
               rdfs:label "N0.2 Briquette"@en .


###  http://w3.id.org/def/BiomassOntology#N0.2Pellet
:N0.2Pellet rdf:type owl:NamedIndividual ,
                     :PelletResult ;
            rdfs:comment "≤ 0,2 % in mass of nitrogen in pellets of dry basis"@en ;
            rdfs:label "N0.2 Pellet"@en .


###  http://w3.id.org/def/BiomassOntology#N0.2Sawdust
:N0.2Sawdust rdf:type owl:NamedIndividual ,
                      :SawdustResult ;
             rdfs:comment "≤ 0,2 % in mass of nitrogen of dry basis in sawdust"@en ;
             rdfs:label "N0.2 Sawdust"@en .


###  http://w3.id.org/def/BiomassOntology#N0.2Shavings
:N0.2Shavings rdf:type owl:NamedIndividual ,
                       :ShavingsResult ;
              rdfs:comment "≤ 0,2 % in mass of nitrogen in shavings of dry basis"@en ;
              rdfs:label "N0.2 Shavings"@en .


###  http://w3.id.org/def/BiomassOntology#N0.2WoodChipsHogFuel
:N0.2WoodChipsHogFuel rdf:type owl:NamedIndividual ,
                               :WoodChipsHogFuelResult ;
                      rdfs:comment "≤ 0,2 % in mass of nitrogen in wood chips/hog fuel of dry basis"@en ;
                      rdfs:label "N0.2 Wood Chips/Hog Fuel"@en .


###  http://w3.id.org/def/BiomassOntology#N0.3Briquette
:N0.3Briquette rdf:type owl:NamedIndividual ,
                        :BriquetteResult ;
               rdfs:comment "≤ 0,3 % in mass of nitrogen in briquettes of dry basis"@en ;
               rdfs:label "N0.3 Briquette"@en .


###  http://w3.id.org/def/BiomassOntology#N0.3Pellet
:N0.3Pellet rdf:type owl:NamedIndividual ,
                     :PelletResult ;
            rdfs:comment "≤ 0,3 % in mass of nitrogen in pellets of dry basis"@en ;
            rdfs:label "N0.3 Pellet"@en .


###  http://w3.id.org/def/BiomassOntology#N0.3Sawdust
:N0.3Sawdust rdf:type owl:NamedIndividual ,
                      :SawdustResult ;
             rdfs:comment "≤ 0,3 % in mass of nitrogen of dry basis in sawdust"@en ;
             rdfs:label "N0.3 Sawdust"@en .


###  http://w3.id.org/def/BiomassOntology#N0.3Shavings
:N0.3Shavings rdf:type owl:NamedIndividual ,
                       :ShavingsResult ;
              rdfs:comment "≤ 0,3 % in mass of nitrogen in shavings of dry basis"@en ;
              rdfs:label "N0.3 Shavings"@en .


###  http://w3.id.org/def/BiomassOntology#N0.3WoodChipsHogFuel
:N0.3WoodChipsHogFuel rdf:type owl:NamedIndividual ,
                               :WoodChipsHogFuelResult ;
                      rdfs:comment "≤ 0,3 % in mass of nitrogen in wood chips/hog fuel of dry basis"@en ;
                      rdfs:label "N0.3 Wood Chips/Hog Fuel"@en .


###  http://w3.id.org/def/BiomassOntology#N0.5Bale
:N0.5Bale rdf:type owl:NamedIndividual ,
                   :BaleResult ;
          rdfs:comment "≤ 0,5 % in mass of nitrogen of dry basis in bale"@en ;
          rdfs:label "N0.5 Bale"@en .


###  http://w3.id.org/def/BiomassOntology#N0.5Bark
:N0.5Bark rdf:type owl:NamedIndividual ,
                   :BarkResult ;
          rdfs:comment "≤ 0,5 % in mass of nitrogen of dry basis in bark"@en ;
          rdfs:label "N0.5 Bark"@en .


###  http://w3.id.org/def/BiomassOntology#N0.5Briquette
:N0.5Briquette rdf:type owl:NamedIndividual ,
                        :BriquetteResult ;
               rdfs:comment "≤ 0,5 % in mass of nitrogen in briquettes of dry basis"@en ;
               rdfs:label "N0.5 Briquette"@en .


###  http://w3.id.org/def/BiomassOntology#N0.5Pellet
:N0.5Pellet rdf:type owl:NamedIndividual ,
                     :PelletResult ;
            rdfs:comment "≤ 0,5 % in mass of nitrogen in pellets of dry basis"@en ;
            rdfs:label "N0.5 Pellet"@en .


###  http://w3.id.org/def/BiomassOntology#N0.5Sawdust
:N0.5Sawdust rdf:type owl:NamedIndividual ,
                      :SawdustResult ;
             rdfs:comment "≤ 0,5 % in mass of nitrogen of dry basis in sawdust"@en ;
             rdfs:label "N0.5 Sawdust"@en .


###  http://w3.id.org/def/BiomassOntology#N0.5Shavings
:N0.5Shavings rdf:type owl:NamedIndividual ,
                       :ShavingsResult ;
              rdfs:comment "≤ 0,5 % in mass of nitrogen in shavings of dry basis"@en ;
              rdfs:label "N0.5 Shavings"@en .


###  http://w3.id.org/def/BiomassOntology#N0.5WoodChipsHogFuel
:N0.5WoodChipsHogFuel rdf:type owl:NamedIndividual ,
                               :WoodChipsHogFuelResult ;
                      rdfs:comment "≤ 0,5 % in mass of nitrogen in wood chips/hog fuel of dry basis"@en ;
                      rdfs:label "N0.5 Wood Chips/Hog Fuel"@en .


###  http://w3.id.org/def/BiomassOntology#N0.6Pellet
:N0.6Pellet rdf:type owl:NamedIndividual ,
                     :PelletResult ;
            rdfs:comment "≤ 0,6 % in mass of nitrogen in pellets of dry basis"@en ;
            rdfs:label "N0.6 Pellet"@en .


###  http://w3.id.org/def/BiomassOntology#N0.7Briquette
:N0.7Briquette rdf:type owl:NamedIndividual ,
                        :BriquetteResult ;
               rdfs:comment "≤ 0,7 % in mass of nitrogen in briquettes of dry basis"@en ;
               rdfs:label "N0.7 Briquette"@en .


###  http://w3.id.org/def/BiomassOntology#N0.7Pellet
:N0.7Pellet rdf:type owl:NamedIndividual ,
                     :PelletResult ;
            rdfs:comment "≤ 0,7 % in mass of nitrogen in pellets of dry basis"@en ;
            rdfs:label "N0.7 Pellet"@en .


###  http://w3.id.org/def/BiomassOntology#N1.5Briquette
:N1.5Briquette rdf:type owl:NamedIndividual ,
                        :BriquetteResult ;
               rdfs:comment "≤ 1,5 % in mass of nitrogen in briquettes of dry basis"@en ;
               rdfs:label "N1.5 Briquette"@en .


###  http://w3.id.org/def/BiomassOntology#N1.5FruitSeeds
:N1.5FruitSeeds rdf:type owl:NamedIndividual ,
                         :FruitSeedsResult ;
                rdfs:comment "≤ 1,5 % in mass of nitrogen in fruit seeds of dry basis"@en ;
                rdfs:label "N1.5 FruitSeeds"@en .


###  http://w3.id.org/def/BiomassOntology#N1.5OliveResidues
:N1.5OliveResidues rdf:type owl:NamedIndividual ,
                            :OliveResiduesResult ;
                   rdfs:comment "≤ 1,5 % in mass of nitrogen in olive residues of dry basis"@en ;
                   rdfs:label "N1.5 OliveResidues"@en .


###  http://w3.id.org/def/BiomassOntology#N1.5Pellet
:N1.5Pellet rdf:type owl:NamedIndividual ,
                     :PelletResult ;
            rdfs:comment "≤ 1,5 % in mass of nitrogen in pellets of dry basis"@en ;
            rdfs:label "N1.5 Pellet"@en .


###  http://w3.id.org/def/BiomassOntology#N1.5WoodChipsHogFuel
:N1.5WoodChipsHogFuel rdf:type owl:NamedIndividual ,
                               :WoodChipsHogFuelResult ;
                      rdfs:comment "≤ 1,5 % in mass of nitrogen in wood chips/hog fuel of dry basis"@en ;
                      rdfs:label "N1.5 Wood Chips/Hog Fuel"@en .


###  http://w3.id.org/def/BiomassOntology#N1Bale
:N1Bale rdf:type owl:NamedIndividual ,
                 :BaleResult ;
        rdfs:comment "≤ 1,0 % in mass of nitrogen of dry basis in bale"@en ;
        rdfs:label "N1.0 Bale"@en .


###  http://w3.id.org/def/BiomassOntology#N1Bark
:N1Bark rdf:type owl:NamedIndividual ,
                 :BarkResult ;
        rdfs:comment "≤ 1,0 % in mass of nitrogen of dry basis in bark"@en ;
        rdfs:label "N1.0 Bark"@en .


###  http://w3.id.org/def/BiomassOntology#N1Briquette
:N1Briquette rdf:type owl:NamedIndividual ,
                      :BriquetteResult ;
             rdfs:comment "≤ 1,0 % in mass of nitrogen in briquettes of dry basis"@en ;
             rdfs:label "N1.0 Briquette"@en .


###  http://w3.id.org/def/BiomassOntology#N1FruitSeeds
:N1FruitSeeds rdf:type owl:NamedIndividual ,
                       :FruitSeedsResult ;
              rdfs:comment "≤ 1,0 % in mass of nitrogen in fruit seeds of dry basis"@en ;
              rdfs:label "N1.0 FruitSeeds"@en .


###  http://w3.id.org/def/BiomassOntology#N1OliveResidues
:N1OliveResidues rdf:type owl:NamedIndividual ,
                          :OliveResiduesResult ;
                 rdfs:comment "≤ 1,0 % in mass of nitrogen in olive residues of dry basis"@en ;
                 rdfs:label "N1.0 OliveResidues"@en .


###  http://w3.id.org/def/BiomassOntology#N1Pellet
:N1Pellet rdf:type owl:NamedIndividual ,
                   :PelletResult ;
          rdfs:comment "≤ 1,0 % in mass of nitrogen in pellets of dry basis"@en ;
          rdfs:label "N1.0 Pellet"@en .


###  http://w3.id.org/def/BiomassOntology#N1Sawdust
:N1Sawdust rdf:type owl:NamedIndividual ,
                    :SawdustResult ;
           rdfs:comment "≤ 1,0 % in mass of nitrogen of dry basis in sawdust"@en ;
           rdfs:label "N1.0 Sawdust"@en .


###  http://w3.id.org/def/BiomassOntology#N1Shavings
:N1Shavings rdf:type owl:NamedIndividual ,
                     :ShavingsResult ;
            rdfs:comment "≤ 1,0 % in mass of nitrogen in shavings of dry basis"@en ;
            rdfs:label "N1.0 Shavings"@en .


###  http://w3.id.org/def/BiomassOntology#N1WoodChipsHogFuel
:N1WoodChipsHogFuel rdf:type owl:NamedIndividual ,
                             :WoodChipsHogFuelResult ;
                    rdfs:comment "≤ 1,0 % in mass of nitrogen in wood chips/hog fuel of dry basis"@en ;
                    rdfs:label "N1.0 Wood Chips/Hog Fuel"@en .


###  http://w3.id.org/def/BiomassOntology#N2Bale
:N2Bale rdf:type owl:NamedIndividual ,
                 :BaleResult ;
        rdfs:comment "≤ 2,0 % in mass of nitrogen of dry basis in bale"@en ;
        rdfs:label "N2.0 Bale"@en .


###  http://w3.id.org/def/BiomassOntology#N2Bark
:N2Bark rdf:type owl:NamedIndividual ,
                 :BarkResult ;
        rdfs:comment "≤ 2,0 % in mass of nitrogen of dry basis in bark"@en ;
        rdfs:label "N2.0 Bark"@en .


###  http://w3.id.org/def/BiomassOntology#N2Briquette
:N2Briquette rdf:type owl:NamedIndividual ,
                      :BriquetteResult ;
             rdfs:comment "≤ 2,0 % in mass of nitrogen in briquettes of dry basis"@en ;
             rdfs:label "N2.0 Briquette"@en .


###  http://w3.id.org/def/BiomassOntology#N2EnergyGrain
:N2EnergyGrain rdf:type owl:NamedIndividual ,
                        :EnergyGrainResult ;
               rdfs:comment "≤ 2,0 % in mass of nitrogen in energy grain of dry basis"@en ;
               rdfs:label "N2.0 EnergyGrain"@en .


###  http://w3.id.org/def/BiomassOntology#N2FruitSeeds
:N2FruitSeeds rdf:type owl:NamedIndividual ,
                       :FruitSeedsResult ;
              rdfs:comment "≤ 2,0 % in mass of nitrogen in fruit seeds of dry basis"@en ;
              rdfs:label "N2.0 FruitSeeds"@en .


###  http://w3.id.org/def/BiomassOntology#N2OliveResidues
:N2OliveResidues rdf:type owl:NamedIndividual ,
                          :OliveResiduesResult ;
                 rdfs:comment "≤ 2,0 % in mass of nitrogen in olive residues of dry basis"@en ;
                 rdfs:label "N2.0 OliveResidues"@en .


###  http://w3.id.org/def/BiomassOntology#N2Pellet
:N2Pellet rdf:type owl:NamedIndividual ,
                   :PelletResult ;
          rdfs:comment "≤ 2,0 % in mass of nitrogen in pellets of dry basis"@en ;
          rdfs:label "N2.0 Pellet"@en .


###  http://w3.id.org/def/BiomassOntology#N2Sawdust
:N2Sawdust rdf:type owl:NamedIndividual ,
                    :SawdustResult ;
           rdfs:comment "≤ 2,0 % in mass of nitrogen of dry basis in sawdust"@en ;
           rdfs:label "N2.0 Sawdust"@en .


###  http://w3.id.org/def/BiomassOntology#N2Shavings
:N2Shavings rdf:type owl:NamedIndividual ,
                     :ShavingsResult ;
            rdfs:comment "≤ 2,0 % in mass of nitrogen in shavings of dry basis"@en ;
            rdfs:label "N2.0 Shavings"@en .


###  http://w3.id.org/def/BiomassOntology#N2WoodChipsHogFuel
:N2WoodChipsHogFuel rdf:type owl:NamedIndividual ,
                             :WoodChipsHogFuelResult ;
                    rdfs:comment "≤ 2,0 % in mass of nitrogen in wood chips/hog fuel of dry basis"@en ;
                    rdfs:label "N2.0 Wood Chips/Hog Fuel"@en .


###  http://w3.id.org/def/BiomassOntology#N3Bark
:N3Bark rdf:type owl:NamedIndividual ,
                 :BarkResult ;
        rdfs:comment "≤ 3,0 % in mass of nitrogen of dry basis in bark"@en ;
        rdfs:label "N3.0 Bark"@en .


###  http://w3.id.org/def/BiomassOntology#N3Briquette
:N3Briquette rdf:type owl:NamedIndividual ,
                      :BriquetteResult ;
             rdfs:comment "≤ 3,0 % in mass of nitrogen in briquettes of dry basis"@en ;
             rdfs:label "N3.0 Briquette"@en .


###  http://w3.id.org/def/BiomassOntology#N3FruitSeeds
:N3FruitSeeds rdf:type owl:NamedIndividual ,
                       :FruitSeedsResult ;
              rdfs:comment "≤ 3,0 % in mass of nitrogen in fruit seeds of dry basis"@en ;
              rdfs:label "N3.0 FruitSeeds"@en .


###  http://w3.id.org/def/BiomassOntology#N3OliveResidues
:N3OliveResidues rdf:type owl:NamedIndividual ,
                          :OliveResiduesResult ;
                 rdfs:comment "≤ 3,0 % in mass of nitrogen in olive residues of dry basis"@en ;
                 rdfs:label "N3.0 OliveResidues"@en .


###  http://w3.id.org/def/BiomassOntology#N3Pellet
:N3Pellet rdf:type owl:NamedIndividual ,
                   :PelletResult ;
          rdfs:comment "≤ 3,0 % in mass of nitrogen in pellets of dry basis"@en ;
          rdfs:label "N3.0 Pellet"@en .


###  http://w3.id.org/def/BiomassOntology#N3Sawdust
:N3Sawdust rdf:type owl:NamedIndividual ,
                    :SawdustResult ;
           rdfs:comment "≤ 3,0 % in mass of nitrogen of dry basis in sawdust"@en ;
           rdfs:label "N3.0 Sawdust"@en .


###  http://w3.id.org/def/BiomassOntology#N3Shavings
:N3Shavings rdf:type owl:NamedIndividual ,
                     :ShavingsResult ;
            rdfs:comment "≤ 3,0 % in mass of nitrogen in shavings of dry basis"@en ;
            rdfs:label "N3.0 Shavings"@en .


###  http://w3.id.org/def/BiomassOntology#N3WoodChipsHogFuel
:N3WoodChipsHogFuel rdf:type owl:NamedIndividual ,
                             :WoodChipsHogFuelResult ;
                    rdfs:comment "≤ 3,0 % in mass of nitrogen in wood chips/hog fuel of dry basis"@en ;
                    rdfs:label "N3.0 Wood Chips/Hog Fuel"@en .


###  http://w3.id.org/def/BiomassOntology#OliveResiduesA
:OliveResiduesA rdf:type owl:NamedIndividual ,
                         :Ash ,
                         :OliveResiduesProperty ;
                rdfs:comment "% in mass of ash in olive residues of dry basis"@en ;
                rdfs:label "Ash of olive residues"@en .


###  http://w3.id.org/def/BiomassOntology#OliveResiduesAdditives
:OliveResiduesAdditives rdf:type owl:NamedIndividual ,
                                 :AdditivesContent ,
                                 :OliveResiduesProperty ;
                        rdfs:comment "% in mass of olive residues. Type and content of additives have to be stated"@en ;
                        rdfs:label "Additives of olive residues"@en .


###  http://w3.id.org/def/BiomassOntology#OliveResiduesAshMB
:OliveResiduesAshMB rdf:type owl:NamedIndividual ,
                             :AshMeltingBehaviour ,
                             :OliveResiduesProperty ;
                    rdfs:comment "Deformation Temperatue, Hemisphere Temperature and Flow Temperature of olive residues should be stated"@en ;
                    rdfs:label "Ash melting behaviour of olive residues"@en .


###  http://w3.id.org/def/BiomassOntology#OliveResiduesBD
:OliveResiduesBD rdf:type owl:NamedIndividual ,
                          :BulkDensity ,
                          :OliveResiduesProperty ;
                 rdfs:comment "kg/m3 of olive residues as received. Recommended to be stated if traded on a volume basis"@en ;
                 rdfs:label "Bulk density of olive residues"@en .


###  http://w3.id.org/def/BiomassOntology#OliveResiduesCl
:OliveResiduesCl rdf:type owl:NamedIndividual ,
                          :Chlorine ,
                          :OliveResiduesProperty ;
                 rdfs:comment "% in mass of chlorine in olive residues of dry basis"@en ;
                 rdfs:label "Chlorine of olive residues"@en .


###  http://w3.id.org/def/BiomassOntology#OliveResiduesDimensions
:OliveResiduesDimensions rdf:type owl:NamedIndividual ,
                                  :Diameter ,
                                  :OliveResiduesProperty ;
                         rdfs:comment "Diameter (D) of olive residues"@en ;
                         rdfs:label "Dimensions of olive residues"@en .


###  http://w3.id.org/def/BiomassOntology#OliveResiduesF
:OliveResiduesF rdf:type owl:NamedIndividual ,
                         :OliveResiduesProperty ;
                rdfs:comment "% in mass, fines < 3,15 mm for D 10 and D10+"@en ;
                rdfs:label "Amount of fines of olive residues"@en .


###  http://w3.id.org/def/BiomassOntology#OliveResiduesFs
:OliveResiduesFs rdf:type owl:NamedIndividual ,
                          :OliveResiduesProperty ;
                 rdfs:comment "% in mass, small fines < 1 mm for for D 03 and D 05"@en ;
                 rdfs:label "Amount of small fines of olive residues"@en .


###  http://w3.id.org/def/BiomassOntology#OliveResiduesM
:OliveResiduesM rdf:type owl:NamedIndividual ,
                         :Moisture ,
                         :OliveResiduesProperty ;
                rdfs:comment "% in mass of moisture in olive residues as received"@en ;
                rdfs:label "Moisture of olive residues"@en .


###  http://w3.id.org/def/BiomassOntology#OliveResiduesN
:OliveResiduesN rdf:type owl:NamedIndividual ,
                         :Nitrogen ,
                         :OliveResiduesProperty ;
                rdfs:comment "% in mass of nitrogen in olive residues of dry basis"@en ;
                rdfs:label "Nitrogen of olive residues"@en .


###  http://w3.id.org/def/BiomassOntology#OliveResiduesQ
:OliveResiduesQ rdf:type owl:NamedIndividual ,
                         :CalorificValue ,
                         :OliveResiduesProperty ;
                rdfs:comment "MJ/kg or kWh/kg of olive residues as received"@en ;
                rdfs:label "Net calorific value of olive residues"@en .


###  http://w3.id.org/def/BiomassOntology#OliveResiduesS
:OliveResiduesS rdf:type owl:NamedIndividual ,
                         :OliveResiduesProperty ,
                         :Sulfur ;
                rdfs:comment "% in mass of sulfur in olive residues of dry basis"@en ;
                rdfs:label "Sulfur of olive residues"@en .


###  http://w3.id.org/def/BiomassOntology#P100Bark
:P100Bark rdf:type owl:NamedIndividual ,
                   :BarkResult ;
          rdfs:comment "Length of bark. Minimum 95 % in mass of particles below the particle class in length, < 100 mm; Max. length of a particle, 250 mm"@en ;
          rdfs:label "P100 Bark"@en .


###  http://w3.id.org/def/BiomassOntology#P16Bark
:P16Bark rdf:type owl:NamedIndividual ,
                  :BarkResult ;
         rdfs:comment "Length of bark. Minimum 95 % in mass of particles below the particle class in length, < 16 mm; Max. length of a particle, 45 mm"@en ;
         rdfs:label "P16 Bark"@en .


###  http://w3.id.org/def/BiomassOntology#P16WoodChipsHogFuel
:P16WoodChipsHogFuel rdf:type owl:NamedIndividual ,
                              :WoodChipsHogFuelResult ;
                     rdfs:comment "Dimensions of wood chips or hog fuel. Main fraction (minimum 60 % in mass), 3,15 mm ≤ m < 16 mm; Coarse fraction, % in mass(sieve aperture size or length of particle, mm) ≤ 6 %, ≥ 31,5 mm"@en ;
                     rdfs:label "P16 Wood Chip/Hog Fuel"@en .


###  http://w3.id.org/def/BiomassOntology#P16sWoodChipsHogFuel
:P16sWoodChipsHogFuel rdf:type owl:NamedIndividual ,
                               :WoodChipsHogFuelResult ;
                      rdfs:comment "Dimensions of wood chips or hog fuel. Main fraction (minimum 60 % in mass), 3,15 mm ≤ m < 16 mm; Coarse fraction, % in mass(sieve aperture size or length  of particle, mm) ≤ 6 %, ≥ 31,5 mm; Fines fraction (F) (< 3,15 mm), % in mass ≤ 15 %; Maximum length (L) of particles, mm 45 mm"@en ;
                      rdfs:label "P16s Wood Chip/Hog Fuel"@en .


###  http://w3.id.org/def/BiomassOntology#P1Bale
:P1Bale rdf:type owl:NamedIndividual ,
                 :BaleResult ;
        rdfs:comment "Square bale; Length (L 1) ≤ 0,5 m; Width (L 2) ≤ 0,4 m; Height (L 3) ≤ 0,35 m"@en ;
        rdfs:label "P1 Bale"@en .


###  http://w3.id.org/def/BiomassOntology#P200Bark
:P200Bark rdf:type owl:NamedIndividual ,
                   :BarkResult ;
          rdfs:comment "Length of bark. Minimum 95 % in mass of particles below the particle class in length, < 200 mm; Max. length of a particle, 350 mm"@en ;
          rdfs:label "P200 Bark"@en .


###  http://w3.id.org/def/BiomassOntology#P2Bale
:P2Bale rdf:type owl:NamedIndividual ,
                 :BaleResult ;
        rdfs:comment "Square bale; Length (L 1) 1,5 m – 2,8 m; Width (L 2) ≤ 1,2 m; Height (L 3) ≤ 0,9 m"@en ;
        rdfs:label "P2 Bale"@en .


###  http://w3.id.org/def/BiomassOntology#P300Bark
:P300Bark rdf:type owl:NamedIndividual ,
                   :BarkResult ;
          rdfs:comment "Length of bark. Minimum 95 % in mass of particles below the particle class in length, < 300 mm; Max. length of a particle, 500 mm"@en ;
          rdfs:label "P300 Bark"@en .


###  http://w3.id.org/def/BiomassOntology#P31Bark
:P31Bark rdf:type owl:NamedIndividual ,
                  :BarkResult ;
         rdfs:comment "Length of bark. Minimum 95 % in mass of particles below the particle class in length, < 31,5 mm; Max. length of a particle, 63 mm"@en ;
         rdfs:label "P31 Bark"@en .


###  http://w3.id.org/def/BiomassOntology#P31WoodChipsHogFuel
:P31WoodChipsHogFuel rdf:type owl:NamedIndividual ,
                              :WoodChipsHogFuelResult ;
                     rdfs:comment "Dimensions of wood chips or hog fuel. Main fraction (minimum 60 % in mass), 3,15 mm ≤ m < 31,5 mm; Coarse fraction, % in mass(sieve aperture size or length of particle, mm) ≤ 6 %, ≥ 45 mm"@en ;
                     rdfs:label "P31 Wood Chip/Hog Fuel"@en .


###  http://w3.id.org/def/BiomassOntology#P31sWoodChipsHogFuel
:P31sWoodChipsHogFuel rdf:type owl:NamedIndividual ,
                               :WoodChipsHogFuelResult ;
                      rdfs:comment "Dimensions of wood chips or hog fuel. Main fraction (minimum 60 % in mass), 3,15 mm ≤ m < 31,5 mm; Coarse fraction, % in mass(sieve aperture size or length of particle, mm) ≤ 6 %, ≥ 45 mm; Fines fraction (F) (< 3,15 mm), % in mass ≤ 10 %; Maximum length (L) of particles, mm 120 m"@en ;
                      rdfs:label "P31s Wood Chip/Hog Fuel"@en .


###  http://w3.id.org/def/BiomassOntology#P3Bale
:P3Bale rdf:type owl:NamedIndividual ,
                 :BaleResult ;
        rdfs:comment "Square bale; Length (L 1) 1,0 m – 3,0 m; Width (L 2) ≤ 1,2 m; Height (L 3) ≤ 1,3 m"@en ;
        rdfs:label "P3 Bale"@en .


###  http://w3.id.org/def/BiomassOntology#P45Bark
:P45Bark rdf:type owl:NamedIndividual ,
                  :BarkResult ;
         rdfs:comment "Length of bark. Minimum 95 % in mass of particles below the particle class in length, < 45 mm; Max. length of a particle, 100 mm"@en ;
         rdfs:label "P45 Bark"@en .


###  http://w3.id.org/def/BiomassOntology#P45WoodChipsHogFuel
:P45WoodChipsHogFuel rdf:type owl:NamedIndividual ,
                              :WoodChipsHogFuelResult ;
                     rdfs:comment "Dimensions of wood chips or hog fuel. Main fraction (minimum 60 % in mass), 3,15 mm ≤ m < 45 mm; Coarse fraction, % in mass(sieve aperture size or length of particle, mm) ≤ 10 % , ≥ 63 mm"@en ;
                     rdfs:label "P45 Wood Chip/Hog Fuel"@en .


###  http://w3.id.org/def/BiomassOntology#P45sWoodChipsHogFuel
:P45sWoodChipsHogFuel rdf:type owl:NamedIndividual ,
                               :WoodChipsHogFuelResult ;
                      rdfs:comment "Dimensions of wood chips or hog fuel. Main fraction (minimum 60 % in mass), 3,15 mm ≤ m < 45 mm; Coarse fraction, % in mass(sieve aperture size or length of particle, mm) ≤ 10 % , ≥ 63 mm; Fines fraction (F) (< 3,15 mm), % in mass ≤ 10 %; Maximum length (L) of particles, mm 200 mm"@en ;
                      rdfs:label "P45s Wood Chip/Hog Fuel"@en .


###  http://w3.id.org/def/BiomassOntology#P63Bark
:P63Bark rdf:type owl:NamedIndividual ,
                  :BarkResult ;
         rdfs:comment "Length of bark. Minimum 95 % in mass of particles below the particle class in length, < 63 mm; Max. length of a particle, 150 mm"@en ;
         rdfs:label "P63 Bark"@en .


###  http://w3.id.org/def/BiomassOntology#P63WoodChipsHogFuel
:P63WoodChipsHogFuel rdf:type owl:NamedIndividual ,
                              :WoodChipsHogFuelResult ;
                     rdfs:comment "Dimensions of wood chips or hog fuel. Main fraction (minimum 60 % in mass), 3,15 mm ≤ m < 63 mm; Coarse fraction, % in mass(sieve aperture size or length of particle, mm) ≤ 10 %, ≥ 100 mm"@en ;
                     rdfs:label "P63 Wood Chip/Hog Fuel"@en .


###  http://w3.id.org/def/BiomassOntology#P80Charcoal
:P80Charcoal rdf:type owl:NamedIndividual ,
                      :CharcoalResult ;
             rdfs:comment "Dimensions of charcoal. Main fraction (minimum 80 % in mass), 20 mm ≤ P ≤ 80 mm; Small particle fraction, (< 10 mm), ≤ 7 % in mass; Coarse fraction, (% in mass), max. length of particle, mm: ≤ 10 % , 80 mm to 100 mm, all < 150 mm"@en ;
             rdfs:label "P80 Charcoal"@en .


###  http://w3.id.org/def/BiomassOntology#PL10WoodChipsHogFuel
:PL10WoodChipsHogFuel rdf:type owl:NamedIndividual ,
                               :WoodChipsHogFuelResult ;
                      rdfs:comment "Dimensions of wood chips or hog fuel. Mass of long particles (100 mm ≤ m ≤ maximum length of particle), 0 % ≤ m ≤ 10 % in mass"@en ;
                      rdfs:label "PL10 Wood Chip/Hog Fuel"@en .


###  http://w3.id.org/def/BiomassOntology#PL20WoodChipsHogFuel
:PL20WoodChipsHogFuel rdf:type owl:NamedIndividual ,
                               :WoodChipsHogFuelResult ;
                      rdfs:comment "Dimensions of wood chips or hog fuel. Mass of long particles (100 mm ≤ m ≤ maximum length of particle), 10 %< m ≤ 20 % in mass"@en ;
                      rdfs:label "PL20 Wood Chip/Hog Fuel"@en .


###  http://w3.id.org/def/BiomassOntology#PL30WoodChipsHogFuel
:PL30WoodChipsHogFuel rdf:type owl:NamedIndividual ,
                               :WoodChipsHogFuelResult ;
                      rdfs:comment "Dimensions of wood chips or hog fuel. Mass of long particles (100 mm ≤ m ≤ maximum length of particle), 20 %< m ≤ 30 % in mass"@en ;
                      rdfs:label "PL30 Wood Chip/Hog Fuel"@en .


###  http://w3.id.org/def/BiomassOntology#PelletA
:PelletA rdf:type owl:NamedIndividual ,
                  :Ash ,
                  :PelletProperty ;
         rdfs:comment "% in mass of ash of dry basis in pellets"@en ;
         rdfs:label "Ash of pellet"@en .


###  http://w3.id.org/def/BiomassOntology#PelletAdditives
:PelletAdditives rdf:type owl:NamedIndividual ,
                          :AdditivesContent ,
                          :PelletProperty ;
                 rdfs:comment "% in mass of additives of pressing mass. Type and content of pressing aids, slagging inhibitors or any other additives have to be stated"@en ;
                 rdfs:label "Additives of pellet"@en .


###  http://w3.id.org/def/BiomassOntology#PelletAshMB
:PelletAshMB rdf:type owl:NamedIndividual ,
                      :AshMeltingBehaviour ,
                      :PelletProperty ;
             rdfs:comment "Deformation Temperatue, Hemisphere Temperature and Flow Temperature of pellet should be stated"@en ;
             rdfs:label "Ash melting behaviour of pellet"@en .


###  http://w3.id.org/def/BiomassOntology#PelletBD
:PelletBD rdf:type owl:NamedIndividual ,
                   :BulkDensity ,
                   :PelletProperty ;
          rdfs:comment "kg/ m3 of pellet as received"@en ;
          rdfs:label "Bulk density of pellet"@en .


###  http://w3.id.org/def/BiomassOntology#PelletC
:PelletC rdf:type owl:NamedIndividual ,
                  :FixedCarbon ,
                  :PelletProperty ;
         rdfs:comment "% in mass of fixed carbon in pellets of dry basis"@en ;
         rdfs:label "Fixed carbon of pellet"@en .


###  http://w3.id.org/def/BiomassOntology#PelletCl
:PelletCl rdf:type owl:NamedIndividual ,
                   :Chlorine ,
                   :PelletProperty ;
          rdfs:comment "% in mass of chlorine in pellets of dry basis"@en ;
          rdfs:label "Chlorine of pellet"@en .


###  http://w3.id.org/def/BiomassOntology#PelletDU
:PelletDU rdf:type owl:NamedIndividual ,
                   :MechanicalDurability ,
                   :PelletProperty ;
          rdfs:comment "% in mass of pellets after testing"@en ;
          rdfs:label "Mechanical durability of pellet"@en .


###  http://w3.id.org/def/BiomassOntology#PelletDimensions
:PelletDimensions rdf:type owl:NamedIndividual ,
                           :Diameter ,
                           :Length ,
                           :PelletProperty ;
                  rdfs:comment "Diameter (D) and Length (L) mm"@en ;
                  rdfs:label "Dimensions of pellet"@en .


###  http://w3.id.org/def/BiomassOntology#PelletF
:PelletF rdf:type owl:NamedIndividual ,
                  :PelletProperty ;
         rdfs:comment "% in mass of particles < 3,15 mm. after production when loaded or packed"@en ;
         rdfs:label "Amount of fines of pellet"@en .


###  http://w3.id.org/def/BiomassOntology#PelletM
:PelletM rdf:type owl:NamedIndividual ,
                  :Moisture ,
                  :PelletProperty ;
         rdfs:comment "% in mass of moisture in pellets as received"@en ;
         rdfs:label "Moisture of pellet"@en .


###  http://w3.id.org/def/BiomassOntology#PelletN
:PelletN rdf:type owl:NamedIndividual ,
                  :Nitrogen ,
                  :PelletProperty ;
         rdfs:comment "% in mass of nitrogen in pellets of dry basis"@en ;
         rdfs:label "Nitrogen of pellet"@en .


###  http://w3.id.org/def/BiomassOntology#PelletParticleSize
:PelletParticleSize rdf:type owl:NamedIndividual ,
                             :PelletProperty ;
                    rdfs:comment "% in mass of dry basis for pellets for industrial use"@en ;
                    rdfs:label "Particle size distribution of disintegrated pellets"@en .


###  http://w3.id.org/def/BiomassOntology#PelletQ
:PelletQ rdf:type owl:NamedIndividual ,
                  :CalorificValue ,
                  :PelletProperty ;
         rdfs:comment "MJ/kg or kWh/kg of pellet as received"@en ;
         rdfs:label "Net calorific value of pellet"@en .


###  http://w3.id.org/def/BiomassOntology#PelletS
:PelletS rdf:type owl:NamedIndividual ,
                  :PelletProperty ,
                  :Sulfur ;
         rdfs:comment "% in mass of sulfur in pellets of dry basis"@en ;
         rdfs:label "Sulfur of pellet"@en .


###  http://w3.id.org/def/BiomassOntology#PelletVM
:PelletVM rdf:type owl:NamedIndividual ,
                   :PelletProperty ;
          rdfs:comment "% in mass of volatile matter in pellets of dry basis"@en ;
          rdfs:label "Volatile matter of pellet"@en .


###  http://w3.id.org/def/BiomassOntology#S0.02Briquette
:S0.02Briquette rdf:type owl:NamedIndividual ,
                         :BriquetteResult ;
                rdfs:comment "≤ 0,02 % in mass of sulfur in briquettes of dry basis"@en ;
                rdfs:label "S0.02 Briquette"@en .


###  http://w3.id.org/def/BiomassOntology#S0.02Pellet
:S0.02Pellet rdf:type owl:NamedIndividual ,
                      :PelletResult ;
             rdfs:comment "≤ 0,02 % in mass of sulfur in pellets of dry basis"@en ;
             rdfs:label "S0.02 Pellet"@en .


###  http://w3.id.org/def/BiomassOntology#S0.02WoodChipsHogFuel
:S0.02WoodChipsHogFuel rdf:type owl:NamedIndividual ,
                                :WoodChipsHogFuelResult ;
                       rdfs:comment "≤ 0,02 % in mass of sulfur in wood chips/hog fuel of dry basis"@en ;
                       rdfs:label "S0.02 Wood Chips/Hog Fuel"@en .


###  http://w3.id.org/def/BiomassOntology#S0.03Briquette
:S0.03Briquette rdf:type owl:NamedIndividual ,
                         :BriquetteResult ;
                rdfs:comment "≤ 0,03 % in mass of sulfur in briquettes of dry basis"@en ;
                rdfs:label "S0.03 Briquette"@en .


###  http://w3.id.org/def/BiomassOntology#S0.03Pellet
:S0.03Pellet rdf:type owl:NamedIndividual ,
                      :PelletResult ;
             rdfs:comment "≤ 0,03 % in mass of sulfur in pellets of dry basis"@en ;
             rdfs:label "S0.03 Pellet"@en .


###  http://w3.id.org/def/BiomassOntology#S0.03WoodChipsHogFuel
:S0.03WoodChipsHogFuel rdf:type owl:NamedIndividual ,
                                :WoodChipsHogFuelResult ;
                       rdfs:comment "≤ 0,03 % in mass of sulfur in wood chips/hog fuel of dry basis"@en ;
                       rdfs:label "S0.03 Wood Chips/Hog Fuel"@en .


###  http://w3.id.org/def/BiomassOntology#S0.04Briquette
:S0.04Briquette rdf:type owl:NamedIndividual ,
                         :BriquetteResult ;
                rdfs:comment "≤ 0,04 % in mass of sulfur in briquettes of dry basis"@en ;
                rdfs:label "S0.04 Briquette"@en .


###  http://w3.id.org/def/BiomassOntology#S0.04Pellet
:S0.04Pellet rdf:type owl:NamedIndividual ,
                      :PelletResult ;
             rdfs:comment "≤ 0,04 % in mass of sulfur in pellets of dry basis"@en ;
             rdfs:label "S0.04 Pellet"@en .


###  http://w3.id.org/def/BiomassOntology#S0.04WoodChipsHogFuel
:S0.04WoodChipsHogFuel rdf:type owl:NamedIndividual ,
                                :WoodChipsHogFuelResult ;
                       rdfs:comment "≤ 0,04 % in mass of sulfur in wood chips/hog fuel of dry basis"@en ;
                       rdfs:label "S0.04 Wood Chips/Hog Fuel"@en .


###  http://w3.id.org/def/BiomassOntology#S0.05Briquette
:S0.05Briquette rdf:type owl:NamedIndividual ,
                         :BriquetteResult ;
                rdfs:comment "≤ 0,05 % in mass of sulfur in briquettes of dry basis"@en ;
                rdfs:label "S0.05 Briquette"@en .


###  http://w3.id.org/def/BiomassOntology#S0.05Pellet
:S0.05Pellet rdf:type owl:NamedIndividual ,
                      :PelletResult ;
             rdfs:comment "≤ 0,05 % in mass of sulfur in pellets of dry basis"@en ;
             rdfs:label "S0.05 Pellet"@en .


###  http://w3.id.org/def/BiomassOntology#S0.05WoodChipsHogFuel
:S0.05WoodChipsHogFuel rdf:type owl:NamedIndividual ,
                                :WoodChipsHogFuelResult ;
                       rdfs:comment "≤ 0,05 % in mass of sulfur in wood chips/hog fuel of dry basis"@en ;
                       rdfs:label "S0.05 Wood Chips/Hog Fuel"@en .


###  http://w3.id.org/def/BiomassOntology#S0.08Briquette
:S0.08Briquette rdf:type owl:NamedIndividual ,
                         :BriquetteResult ;
                rdfs:comment "≤ 0,08 % in mass of sulfur in briquettes of dry basis"@en ;
                rdfs:label "S0.08 Briquette"@en .


###  http://w3.id.org/def/BiomassOntology#S0.08Pellet
:S0.08Pellet rdf:type owl:NamedIndividual ,
                      :PelletResult ;
             rdfs:comment "≤ 0,08 % in mass of sulfur in pellets of dry basis"@en ;
             rdfs:label "S0.08 Pellet"@en .


###  http://w3.id.org/def/BiomassOntology#S0.08WoodChipsHogFuel
:S0.08WoodChipsHogFuel rdf:type owl:NamedIndividual ,
                                :WoodChipsHogFuelResult ;
                       rdfs:comment "≤ 0,08 % in mass of sulfur in wood chips/hog fuel of dry basis"@en ;
                       rdfs:label "S0.08 Wood Chips/Hog Fuel"@en .


###  http://w3.id.org/def/BiomassOntology#S0.15FruitSeeds
:S0.15FruitSeeds rdf:type owl:NamedIndividual ,
                          :FruitSeedsResult ;
                 rdfs:comment "≤ 0,15 % in mass of sulfur in fruit seeds of dry basis"@en ;
                 rdfs:label "S0.15 FruitSeeds"@en .


###  http://w3.id.org/def/BiomassOntology#S0.15OliveResidues
:S0.15OliveResidues rdf:type owl:NamedIndividual ,
                             :OliveResiduesResult ;
                    rdfs:comment "≤ 0,15 % in mass of sulfur in olive residues of dry basis"@en ;
                    rdfs:label "S0.15 OliveResidues"@en .


###  http://w3.id.org/def/BiomassOntology#S0.1Briquette
:S0.1Briquette rdf:type owl:NamedIndividual ,
                        :BriquetteResult ;
               rdfs:comment "≤ 0,10 % in mass of sulfur in briquettes of dry basis"@en ;
               rdfs:label "S0.10 Briquette"@en .


###  http://w3.id.org/def/BiomassOntology#S0.1Pellet
:S0.1Pellet rdf:type owl:NamedIndividual ,
                     :PelletResult ;
            rdfs:comment "≤ 0,10 % in mass of sulfur in pellets of dry basis"@en ;
            rdfs:label "S0.10 Pellet"@en .


###  http://w3.id.org/def/BiomassOntology#S0.1WoodChipsHogFuel
:S0.1WoodChipsHogFuel rdf:type owl:NamedIndividual ,
                               :WoodChipsHogFuelResult ;
                      rdfs:comment "≤ 0,10 % in mass of sulfur in wood chips/hog fuel of dry basis"@en ;
                      rdfs:label "S0.10 Wood Chips/Hog Fuel"@en .


###  http://w3.id.org/def/BiomassOntology#S0.2Briquette
:S0.2Briquette rdf:type owl:NamedIndividual ,
                        :BriquetteResult ;
               rdfs:comment "≤ 0,20 % in mass of sulfur in briquettes of dry basis"@en ;
               rdfs:label "S0.20 Briquette"@en .


###  http://w3.id.org/def/BiomassOntology#S0.2EnergyGrain
:S0.2EnergyGrain rdf:type owl:NamedIndividual ,
                          :EnergyGrainResult ;
                 rdfs:comment "≤ 0,20 % in mass of sulfur in energy grain of dry basis"@en ;
                 rdfs:label "S0.2 EnergyGrain"@en .


###  http://w3.id.org/def/BiomassOntology#S0.2FruitSeeds
:S0.2FruitSeeds rdf:type owl:NamedIndividual ,
                         :FruitSeedsResult ;
                rdfs:comment "≤ 0,20 % in mass of sulfur in fruit seeds of dry basis"@en ;
                rdfs:label "S0.20 FruitSeeds"@en .


###  http://w3.id.org/def/BiomassOntology#S0.2OliveResidues
:S0.2OliveResidues rdf:type owl:NamedIndividual ,
                            :OliveResiduesResult ;
                   rdfs:comment "≤ 0,20 % in mass of sulfur in olive residues of dry basis"@en ;
                   rdfs:label "S0.20 OliveResidues"@en .


###  http://w3.id.org/def/BiomassOntology#S0.2Pellet
:S0.2Pellet rdf:type owl:NamedIndividual ,
                     :PelletResult ;
            rdfs:comment "≤ 0,20 % in mass of sulfur in pellets of dry basis"@en ;
            rdfs:label "S0.20 Pellet"@en .


###  http://w3.id.org/def/BiomassOntology#S0.3Briquette
:S0.3Briquette rdf:type owl:NamedIndividual ,
                        :BriquetteResult ;
               rdfs:comment "≤ 0,30 % in mass of sulfur in briquettes of dry basis"@en ;
               rdfs:label "S0.30 Briquette"@en .


###  http://w3.id.org/def/BiomassOntology#S0.3Pellet
:S0.3Pellet rdf:type owl:NamedIndividual ,
                     :PelletResult ;
            rdfs:comment "≤ 0,30 % in mass of sulfur in pellets of dry basis"@en ;
            rdfs:label "S0.30 Pellet"@en .


###  http://w3.id.org/def/BiomassOntology#SawdustA
:SawdustA rdf:type owl:NamedIndividual ,
                   :Ash ,
                   :SawdustProperty ;
          rdfs:comment "% in mass of ash of dry basis in sawdust"@en ;
          rdfs:label "Ash of sawdust"@en .


###  http://w3.id.org/def/BiomassOntology#SawdustAshMB
:SawdustAshMB rdf:type owl:NamedIndividual ,
                       :AshMeltingBehaviour ,
                       :SawdustProperty ;
              rdfs:comment "Deformation Temperatue, Hemisphere Temperature and Flow Temperature of sawdust should be stated"@en ;
              rdfs:label "Ash melting behaviour of sawdust"@en .


###  http://w3.id.org/def/BiomassOntology#SawdustBD
:SawdustBD rdf:type owl:NamedIndividual ,
                    :BulkDensity ,
                    :SawdustProperty ;
           rdfs:comment "kg/ m3 of sawdust as received"@en ;
           rdfs:label "Bulk density of sawdust"@en .


###  http://w3.id.org/def/BiomassOntology#SawdustCl
:SawdustCl rdf:type owl:NamedIndividual ,
                    :Chlorine ,
                    :SawdustProperty ;
           rdfs:comment "% in mass of chlorine of dry basis in sawdust"@en ;
           rdfs:label "Chlorine of sawdust"@en .


###  http://w3.id.org/def/BiomassOntology#SawdustM
:SawdustM rdf:type owl:NamedIndividual ,
                   :Moisture ,
                   :SawdustProperty ;
          rdfs:comment "% in mass of moisture in sawdust as received"@en ;
          rdfs:label "Moisture of sawdust"@en .


###  http://w3.id.org/def/BiomassOntology#SawdustN
:SawdustN rdf:type owl:NamedIndividual ,
                   :Nitrogen ,
                   :SawdustProperty ;
          rdfs:comment "% in mass of nitrogen of dry basis in sawdust"@en ;
          rdfs:label "Nitrogen of sawdust"@en .


###  http://w3.id.org/def/BiomassOntology#SawdustQ
:SawdustQ rdf:type owl:NamedIndividual ,
                   :CalorificValue ,
                   :SawdustProperty ;
          rdfs:comment "MJ/kg or kWh/kg of sawdust as received"@en ;
          rdfs:label "Net calorific value of sawdust"@en .


###  http://w3.id.org/def/BiomassOntology#SawdustSieving
:SawdustSieving rdf:type owl:NamedIndividual ,
                         :SawdustProperty ;
                rdfs:comment "Sieving and the screen size of the sieve should be stated"@en ;
                rdfs:label "Sieving of sawdust"@en .


###  http://w3.id.org/def/BiomassOntology#ShavingsA
:ShavingsA rdf:type owl:NamedIndividual ,
                    :Ash ,
                    :ShavingsProperty ;
           rdfs:comment "% in mass of ash of dry basis in shavings"@en ;
           rdfs:label "Ash of shavings"@en .


###  http://w3.id.org/def/BiomassOntology#ShavingsAshMB
:ShavingsAshMB rdf:type owl:NamedIndividual ,
                        :AshMeltingBehaviour ,
                        :ShavingsProperty ;
               rdfs:comment "Deformation Temperatue, Hemisphere Temperature and Flow Temperature of shavings should be stated"@en ;
               rdfs:label "Ash melting behaviour of shavings"@en .


###  http://w3.id.org/def/BiomassOntology#ShavingsBD
:ShavingsBD rdf:type owl:NamedIndividual ,
                     :BulkDensity ,
                     :ShavingsProperty ;
            rdfs:comment "kg/m3 as received of shavings"@en ;
            rdfs:label "Bulk density of shavings"@en .


###  http://w3.id.org/def/BiomassOntology#ShavingsCl
:ShavingsCl rdf:type owl:NamedIndividual ,
                     :Chlorine ,
                     :ShavingsProperty ;
            rdfs:comment "% in mass of chlorine in shavings of dry basis"@en ;
            rdfs:label "Chlorine of shavings"@en .


###  http://w3.id.org/def/BiomassOntology#ShavingsM
:ShavingsM rdf:type owl:NamedIndividual ,
                    :Moisture ,
                    :ShavingsProperty ;
           rdfs:comment "% in mass of moisture in shavings as received"@en ;
           rdfs:label "Moisture of shavings"@en .


###  http://w3.id.org/def/BiomassOntology#ShavingsN
:ShavingsN rdf:type owl:NamedIndividual ,
                    :Nitrogen ,
                    :ShavingsProperty ;
           rdfs:comment "% in mass of nitrogen in shavings of dry basis"@en ;
           rdfs:label "Nitrogen of shavings"@en .


###  http://w3.id.org/def/BiomassOntology#ShavingsQ
:ShavingsQ rdf:type owl:NamedIndividual ,
                    :CalorificValue ,
                    :ShavingsProperty ;
           rdfs:comment "MJ/kg or kWh/kg of shavings as received"@en ;
           rdfs:label "Net calorific value of shavings"@en .


###  http://w3.id.org/def/BiomassOntology#ShavingsSieving
:ShavingsSieving rdf:type owl:NamedIndividual ,
                          :ShavingsProperty ;
                 rdfs:comment "Sieving and the screen size of the sieve should be stated"@en ;
                 rdfs:label "Sieving of shavings"@en .


###  http://w3.id.org/def/BiomassOntology#WoodChipsHogFuelA
:WoodChipsHogFuelA rdf:type owl:NamedIndividual ,
                            :Ash ,
                            :WoodChipsHogFuelProperty ;
                   rdfs:comment "% in mass of ash of dry basis"@en ;
                   rdfs:label "Ash of wood chips/ hog fuel"@en .


###  http://w3.id.org/def/BiomassOntology#WoodChipsHogFuelAshMB
:WoodChipsHogFuelAshMB rdf:type owl:NamedIndividual ,
                                :AshMeltingBehaviour ,
                                :WoodChipsHogFuelProperty ;
                       rdfs:comment "Deformation Temperatue, Hemisphere Temperature and Flow Temperature of wood chip/ hog fuel should be stated"@en ;
                       rdfs:label "Ash melting behaviour of wood chips/ hog fuel"@en .


###  http://w3.id.org/def/BiomassOntology#WoodChipsHogFuelBD
:WoodChipsHogFuelBD rdf:type owl:NamedIndividual ,
                             :BulkDensity ,
                             :WoodChipsHogFuelProperty ;
                    rdfs:comment "kg/ m3  of wood chips/ hog fuel as received"@en ;
                    rdfs:label "Bulk density of wood chips/ hog fuel"@en .


###  http://w3.id.org/def/BiomassOntology#WoodChipsHogFuelCl
:WoodChipsHogFuelCl rdf:type owl:NamedIndividual ,
                             :Chlorine ,
                             :WoodChipsHogFuelProperty ;
                    rdfs:comment "% in mass of chlorine of dry basis"@en ;
                    rdfs:label "Chlorine of wood chips/ hog fuel"@en .


###  http://w3.id.org/def/BiomassOntology#WoodChipsHogFuelDimensions
:WoodChipsHogFuelDimensions rdf:type owl:NamedIndividual ,
                                     :Length ,
                                     :WoodChipsHogFuelProperty ;
                            rdfs:comment "Length (mm) of the different fractions"@en ;
                            rdfs:label "Dimensions of wood chips/ hog fuel"@en .


###  http://w3.id.org/def/BiomassOntology#WoodChipsHogFuelF
:WoodChipsHogFuelF rdf:type owl:NamedIndividual ,
                            :WoodChipsHogFuelProperty ;
                   rdfs:comment "< 3,15 mm particles,  % in mass of fines"@en ;
                   rdfs:label "Fines fraction of wood chips/ hog fuel"@en .


###  http://w3.id.org/def/BiomassOntology#WoodChipsHogFuelM
:WoodChipsHogFuelM rdf:type owl:NamedIndividual ,
                            :Moisture ,
                            :WoodChipsHogFuelProperty ;
                   rdfs:comment "% in mass of moisture as received"@en ;
                   rdfs:label "Miosture of wood chips/ hog fuel"@en .


###  http://w3.id.org/def/BiomassOntology#WoodChipsHogFuelN
:WoodChipsHogFuelN rdf:type owl:NamedIndividual ,
                            :Nitrogen ,
                            :WoodChipsHogFuelProperty ;
                   rdfs:comment "% in mass of nitrogen of dry basis"@en ;
                   rdfs:label "Nitrogen of wood chips/ hog fuel"@en .


###  http://w3.id.org/def/BiomassOntology#WoodChipsHogFuelQ
:WoodChipsHogFuelQ rdf:type owl:NamedIndividual ,
                            :CalorificValue ,
                            :WoodChipsHogFuelProperty ;
                   rdfs:comment "MJ/kg or kWh/kg of wood chips/ hog fuel as received"@en ;
                   rdfs:label "Net calorific value of wood chips/ hog fuel"@en .


###  http://w3.id.org/def/BiomassOntology#WoodChipsHogFuelS
:WoodChipsHogFuelS rdf:type owl:NamedIndividual ,
                            :Sulfur ,
                            :WoodChipsHogFuelProperty ;
                   rdfs:comment "% in mass of sulfur of dry basis"@en ;
                   rdfs:label "Sulfur of wood chips/ hog fuel"@en .


###  http://w3.id.org/def/BiomassOntology#pellet_01
:pellet_01 rdf:type owl:NamedIndividual ,
                    :Pellet ;
           rdfs:comment "Pellet from company A" ;
           rdfs:label "Pellet 01" .


###  http://w3.id.org/def/BiomassOntology#pellet_02
:pellet_02 rdf:type owl:NamedIndividual ,
                    :Pellet ;
           rdfs:comment "Pellet from company B" ;
           rdfs:label "Pellet 02" .


###  http://w3.id.org/def/BiomassOntology#1-WoodyBiomass
<http://w3.id.org/def/BiomassOntology#1-WoodyBiomass> rdf:type owl:NamedIndividual ,
                                                               <http://www.w3.org/2004/02/skos/core#Concept> ;
                                                      <http://www.w3.org/2004/02/skos/core#topConceptOf> :BiomassScheme ;
                                                      <http://www.w3.org/2004/02/skos/core#definition> "Biomass from trees, bushes and shrubs."@en ;
                                                      <http://www.w3.org/2004/02/skos/core#prefLabel> "1. Woody biomass"@en .


###  http://w3.id.org/def/BiomassOntology#1-1-ForestPlantation
<http://w3.id.org/def/BiomassOntology#1-1-ForestPlantation> rdf:type owl:NamedIndividual ,
                                                                     <http://www.w3.org/2004/02/skos/core#Concept> ;
                                                            <http://www.w3.org/2004/02/skos/core#broader> <http://w3.id.org/def/BiomassOntology#1-WoodyBiomass> ;
                                                            <http://www.w3.org/2004/02/skos/core#inScheme> :BiomassScheme ;
                                                            <http://www.w3.org/2004/02/skos/core#definition> "Forest, plantation and other virgin wood in this group may only have been subjected to size reduction, debarking, drying or wetting. Forest, plantation and other virgin wood includes wood from forests, parks, gardens, plantations, roadside maintenance and from short rotation forests and coppice."@en ;
                                                            <http://www.w3.org/2004/02/skos/core#prefLabel> "1.1. Forest, plantation and other virgin wood"@en .


###  http://w3.id.org/def/BiomassOntology#1-1-1-WholeTrees
<http://w3.id.org/def/BiomassOntology#1-1-1-WholeTrees> rdf:type owl:NamedIndividual ,
                                                                 <http://www.w3.org/2004/02/skos/core#Concept> ;
                                                        <http://www.w3.org/2004/02/skos/core#broader> <http://w3.id.org/def/BiomassOntology#1-1-ForestPlantation> ;
                                                        <http://www.w3.org/2004/02/skos/core#inScheme> :BiomassScheme ;
                                                        <http://www.w3.org/2004/02/skos/core#definition> "Woody biomass consisting of whole trees without roots."@en ;
                                                        <http://www.w3.org/2004/02/skos/core#prefLabel> "1.1.1. Whole trees"@en .


###  http://w3.id.org/def/BiomassOntology#1-1-1-1-BroadLeaf
<http://w3.id.org/def/BiomassOntology#1-1-1-1-BroadLeaf> rdf:type owl:NamedIndividual ,
                                                                  <http://www.w3.org/2004/02/skos/core#Concept> ;
                                                         <http://www.w3.org/2004/02/skos/core#broader> <http://w3.id.org/def/BiomassOntology#1-1-1-WholeTrees> ;
                                                         <http://www.w3.org/2004/02/skos/core#inScheme> :BiomassScheme ;
                                                         <http://www.w3.org/2004/02/skos/core#definition> "Woody biomass consisting of whole broad-leaf trees."@en ;
                                                         <http://www.w3.org/2004/02/skos/core#prefLabel> "1.1.1.1. Broad-leaf"@en .


###  http://w3.id.org/def/BiomassOntology#1-1-1-2-Coniferous
<http://w3.id.org/def/BiomassOntology#1-1-1-2-Coniferous> rdf:type owl:NamedIndividual ,
                                                                   <http://www.w3.org/2004/02/skos/core#Concept> ;
                                                          <http://www.w3.org/2004/02/skos/core#broader> <http://w3.id.org/def/BiomassOntology#1-1-1-WholeTrees> ;
                                                          <http://www.w3.org/2004/02/skos/core#inScheme> :BiomassScheme ;
                                                          <http://www.w3.org/2004/02/skos/core#definition> "Woody biomass consisting of whole coniferous trees."@en ;
                                                          <http://www.w3.org/2004/02/skos/core#prefLabel> "1.1.1.2. Coniferous"@en .


###  http://w3.id.org/def/BiomassOntology#1-1-1-3-ShortRotationCoppice
<http://w3.id.org/def/BiomassOntology#1-1-1-3-ShortRotationCoppice> rdf:type owl:NamedIndividual ,
                                                                             <http://www.w3.org/2004/02/skos/core#Concept> ;
                                                                    <http://www.w3.org/2004/02/skos/core#broader> <http://w3.id.org/def/BiomassOntology#1-1-1-WholeTrees> ;
                                                                    <http://www.w3.org/2004/02/skos/core#inScheme> :BiomassScheme ;
                                                                    <http://www.w3.org/2004/02/skos/core#definition> "Woody biomass consisting of short rotation coppice whole trees."@en ;
                                                                    <http://www.w3.org/2004/02/skos/core#prefLabel> "1.1.1.3. Short rotation coppice"@en .


###  http://w3.id.org/def/BiomassOntology#1-1-1-4-Bushes
<http://w3.id.org/def/BiomassOntology#1-1-1-4-Bushes> rdf:type owl:NamedIndividual ,
                                                               <http://www.w3.org/2004/02/skos/core#Concept> ;
                                                      <http://www.w3.org/2004/02/skos/core#broader> <http://w3.id.org/def/BiomassOntology#1-1-1-WholeTrees> ;
                                                      <http://www.w3.org/2004/02/skos/core#inScheme> :BiomassScheme ;
                                                      <http://www.w3.org/2004/02/skos/core#definition> "Woody biomass consisting of whole bushes."@en ;
                                                      <http://www.w3.org/2004/02/skos/core#prefLabel> "1.1.1.4. Bushes"@en .


###  http://w3.id.org/def/BiomassOntology#1-1-1-5-BlendsMixtures
<http://w3.id.org/def/BiomassOntology#1-1-1-5-BlendsMixtures> rdf:type owl:NamedIndividual ,
                                                                       <http://www.w3.org/2004/02/skos/core#Concept> ;
                                                              <http://www.w3.org/2004/02/skos/core#broader> <http://w3.id.org/def/BiomassOntology#1-1-1-WholeTrees> ;
                                                              <http://www.w3.org/2004/02/skos/core#inScheme> :BiomassScheme ;
                                                              <http://www.w3.org/2004/02/skos/core#definition> "This refers to blends and mixtures of whole trees in the groups 1.1.1.1. to 1.1.1.4. The mixing can be either intentional (blends) or unintentional (mixtures)."@en ;
                                                              <http://www.w3.org/2004/02/skos/core#prefLabel> "1.1.1..5. Blends and mixtures"@en .


###  http://w3.id.org/def/BiomassOntology#1-1-2-WholeTreesRoots
<http://w3.id.org/def/BiomassOntology#1-1-2-WholeTreesRoots> rdf:type owl:NamedIndividual ,
                                                                      <http://www.w3.org/2004/02/skos/core#Concept> ;
                                                             <http://www.w3.org/2004/02/skos/core#broader> <http://w3.id.org/def/BiomassOntology#1-1-ForestPlantation> ;
                                                             <http://www.w3.org/2004/02/skos/core#inScheme> :BiomassScheme ;
                                                             <http://www.w3.org/2004/02/skos/core#definition> "Woody biomass consisting of whole trees with roots."@en ;
                                                             <http://www.w3.org/2004/02/skos/core#prefLabel> "1.1.2. Whole trees with roots"@en .


###  http://w3.id.org/def/BiomassOntology#1-1-2-1-BroadLeaf
<http://w3.id.org/def/BiomassOntology#1-1-2-1-BroadLeaf> rdf:type owl:NamedIndividual ,
                                                                  <http://www.w3.org/2004/02/skos/core#Concept> ;
                                                         <http://www.w3.org/2004/02/skos/core#broader> <http://w3.id.org/def/BiomassOntology#1-1-2-WholeTreesRoots> ;
                                                         <http://www.w3.org/2004/02/skos/core#inScheme> :BiomassScheme ;
                                                         <http://www.w3.org/2004/02/skos/core#definition> "Woody biomass consisting of whole broad-leaf trees with roots."@en ;
                                                         <http://www.w3.org/2004/02/skos/core#prefLabel> "1.1.2.1. Broad-leaf"@en .


###  http://w3.id.org/def/BiomassOntology#1-1-2-2-Coniferous
<http://w3.id.org/def/BiomassOntology#1-1-2-2-Coniferous> rdf:type owl:NamedIndividual ,
                                                                   <http://www.w3.org/2004/02/skos/core#Concept> ;
                                                          <http://www.w3.org/2004/02/skos/core#broader> <http://w3.id.org/def/BiomassOntology#1-1-2-WholeTreesRoots> ;
                                                          <http://www.w3.org/2004/02/skos/core#inScheme> :BiomassScheme ;
                                                          <http://www.w3.org/2004/02/skos/core#definition> "Woody biomass consisting of whole coniferous trees with roots."@en ;
                                                          <http://www.w3.org/2004/02/skos/core#prefLabel> "1.1.2.2. Coniferous"@en .


###  http://w3.id.org/def/BiomassOntology#1-1-2-3-ShortRotationCoppice
<http://w3.id.org/def/BiomassOntology#1-1-2-3-ShortRotationCoppice> rdf:type owl:NamedIndividual ,
                                                                             <http://www.w3.org/2004/02/skos/core#Concept> ;
                                                                    <http://www.w3.org/2004/02/skos/core#broader> <http://w3.id.org/def/BiomassOntology#1-1-2-WholeTreesRoots> ;
                                                                    <http://www.w3.org/2004/02/skos/core#inScheme> :BiomassScheme ;
                                                                    <http://www.w3.org/2004/02/skos/core#definition> "Woody biomass consisting of short rotation coppice whole trees with roots."@en ;
                                                                    <http://www.w3.org/2004/02/skos/core#prefLabel> "1.1.2.3. Short rotation coppice"@en .


###  http://w3.id.org/def/BiomassOntology#1-1-2-4-Bushes
<http://w3.id.org/def/BiomassOntology#1-1-2-4-Bushes> rdf:type owl:NamedIndividual ,
                                                               <http://www.w3.org/2004/02/skos/core#Concept> ;
                                                      <http://www.w3.org/2004/02/skos/core#broader> <http://w3.id.org/def/BiomassOntology#1-1-2-WholeTreesRoots> ;
                                                      <http://www.w3.org/2004/02/skos/core#inScheme> :BiomassScheme ;
                                                      <http://www.w3.org/2004/02/skos/core#definition> "Woody biomass consisting of whole bushes with roots."@en ;
                                                      <http://www.w3.org/2004/02/skos/core#prefLabel> "1.1.2.4. Bushes"@en .


###  http://w3.id.org/def/BiomassOntology#1-1-2-5-BlendsMixtures
<http://w3.id.org/def/BiomassOntology#1-1-2-5-BlendsMixtures> rdf:type owl:NamedIndividual ,
                                                                       <http://www.w3.org/2004/02/skos/core#Concept> ;
                                                              <http://www.w3.org/2004/02/skos/core#broader> <http://w3.id.org/def/BiomassOntology#1-1-2-WholeTreesRoots> ;
                                                              <http://www.w3.org/2004/02/skos/core#inScheme> :BiomassScheme ;
                                                              <http://www.w3.org/2004/02/skos/core#definition> "This refers to blends and mixtures of whole trees with roots in the groups 1.1.2.1. to 1.1.2.4. The mixing can be either intentional (blends) or unintentional (mixtures)."@en ;
                                                              <http://www.w3.org/2004/02/skos/core#prefLabel> "1.1.2.5. Blends and mixtures"@en .


###  http://w3.id.org/def/BiomassOntology#1-1-3-Stemwood
<http://w3.id.org/def/BiomassOntology#1-1-3-Stemwood> rdf:type owl:NamedIndividual ,
                                                               <http://www.w3.org/2004/02/skos/core#Concept> ;
                                                      <http://www.w3.org/2004/02/skos/core#broader> <http://w3.id.org/def/BiomassOntology#1-1-ForestPlantation> ;
                                                      <http://www.w3.org/2004/02/skos/core#inScheme> :BiomassScheme ;
                                                      <http://www.w3.org/2004/02/skos/core#definition> "Woody biomass consisting of stemwood."@en ;
                                                      <http://www.w3.org/2004/02/skos/core#prefLabel> "1.1.3. Stemwood"@en .


###  http://w3.id.org/def/BiomassOntology#1-1-3-1-BroadLeafBark
<http://w3.id.org/def/BiomassOntology#1-1-3-1-BroadLeafBark> rdf:type owl:NamedIndividual ,
                                                                      <http://www.w3.org/2004/02/skos/core#Concept> ;
                                                             <http://www.w3.org/2004/02/skos/core#broader> <http://w3.id.org/def/BiomassOntology#1-1-3-Stemwood> ;
                                                             <http://www.w3.org/2004/02/skos/core#inScheme> :BiomassScheme ;
                                                             <http://www.w3.org/2004/02/skos/core#definition> "Woody biomass consisting of broad-leaf trees' stemwood with bark."@en ;
                                                             <http://www.w3.org/2004/02/skos/core#prefLabel> "1.1.3.1. Broad-leaf with bark"@en .


###  http://w3.id.org/def/BiomassOntology#1-1-3-2-ConiferousBark
<http://w3.id.org/def/BiomassOntology#1-1-3-2-ConiferousBark> rdf:type owl:NamedIndividual ,
                                                                       <http://www.w3.org/2004/02/skos/core#Concept> ;
                                                              <http://www.w3.org/2004/02/skos/core#broader> <http://w3.id.org/def/BiomassOntology#1-1-3-Stemwood> ;
                                                              <http://www.w3.org/2004/02/skos/core#inScheme> :BiomassScheme ;
                                                              <http://www.w3.org/2004/02/skos/core#definition> "Woody biomass consisting of coniferous trees' stemwood with bark."@en ;
                                                              <http://www.w3.org/2004/02/skos/core#prefLabel> "1.1.3.2. Coniferous with bark"@en .


###  http://w3.id.org/def/BiomassOntology#1-1-3-3-BroadLeaf
<http://w3.id.org/def/BiomassOntology#1-1-3-3-BroadLeaf> rdf:type owl:NamedIndividual ,
                                                                  <http://www.w3.org/2004/02/skos/core#Concept> ;
                                                         <http://www.w3.org/2004/02/skos/core#broader> <http://w3.id.org/def/BiomassOntology#1-1-3-Stemwood> ;
                                                         <http://www.w3.org/2004/02/skos/core#inScheme> :BiomassScheme ;
                                                         <http://www.w3.org/2004/02/skos/core#definition> "Woody biomass consisting of broad-leaf trees' stemwood without bark."@en ;
                                                         <http://www.w3.org/2004/02/skos/core#prefLabel> "1.1.3.3. Broad-leaf without bark"@en .


###  http://w3.id.org/def/BiomassOntology#1-1-3-4-Coniferous
<http://w3.id.org/def/BiomassOntology#1-1-3-4-Coniferous> rdf:type owl:NamedIndividual ,
                                                                   <http://www.w3.org/2004/02/skos/core#Concept> ;
                                                          <http://www.w3.org/2004/02/skos/core#broader> <http://w3.id.org/def/BiomassOntology#1-1-3-Stemwood> ;
                                                          <http://www.w3.org/2004/02/skos/core#inScheme> :BiomassScheme ;
                                                          <http://www.w3.org/2004/02/skos/core#definition> "Woody biomass consisting of coniferous trees' stemwood without bark."@en ;
                                                          <http://www.w3.org/2004/02/skos/core#prefLabel> "1.1.3.4. Coniferous without bark"@en .


###  http://w3.id.org/def/BiomassOntology#1-1-3-5-BlendsMixtures
<http://w3.id.org/def/BiomassOntology#1-1-3-5-BlendsMixtures> rdf:type owl:NamedIndividual ,
                                                                       <http://www.w3.org/2004/02/skos/core#Concept> ;
                                                              <http://www.w3.org/2004/02/skos/core#broader> <http://w3.id.org/def/BiomassOntology#1-1-3-Stemwood> ;
                                                              <http://www.w3.org/2004/02/skos/core#inScheme> :BiomassScheme ;
                                                              <http://www.w3.org/2004/02/skos/core#definition> "This refers to blends and mixtures of stemwood in the groups 1.1.3.1. to 1.1.3.4. The mixing can be either intentional (blends) or unintentional (mixtures)."@en ;
                                                              <http://www.w3.org/2004/02/skos/core#prefLabel> "1.1.3.5. Blends and mixtures"@en .


###  http://w3.id.org/def/BiomassOntology#1-1-4-LoggingResidues
<http://w3.id.org/def/BiomassOntology#1-1-4-LoggingResidues> rdf:type owl:NamedIndividual ,
                                                                      <http://www.w3.org/2004/02/skos/core#Concept> ;
                                                             <http://www.w3.org/2004/02/skos/core#broader> <http://w3.id.org/def/BiomassOntology#1-1-ForestPlantation> ;
                                                             <http://www.w3.org/2004/02/skos/core#inScheme> :BiomassScheme ;
                                                             <http://www.w3.org/2004/02/skos/core#definition> "Woody biomass consisting of logging residues."@en ;
                                                             <http://www.w3.org/2004/02/skos/core#prefLabel> "1.1.4. Logging residues"@en .


###  http://w3.id.org/def/BiomassOntology#1-1-4-1-FreshBroadLeaf
<http://w3.id.org/def/BiomassOntology#1-1-4-1-FreshBroadLeaf> rdf:type owl:NamedIndividual ,
                                                                       <http://www.w3.org/2004/02/skos/core#Concept> ;
                                                              <http://www.w3.org/2004/02/skos/core#broader> <http://w3.id.org/def/BiomassOntology#1-1-4-LoggingResidues> ;
                                                              <http://www.w3.org/2004/02/skos/core#inScheme> :BiomassScheme ;
                                                              <http://www.w3.org/2004/02/skos/core#definition> "Woody biomass consisting of fresh broad-leaf trees' logging residues, including leaves."@en ;
                                                              <http://www.w3.org/2004/02/skos/core#prefLabel> "1.1.4.1. Fresh/green, broad-leaf (including leaves)"@en .


###  http://w3.id.org/def/BiomassOntology#1-1-4-2-FreshConiferous
<http://w3.id.org/def/BiomassOntology#1-1-4-2-FreshConiferous> rdf:type owl:NamedIndividual ,
                                                                        <http://www.w3.org/2004/02/skos/core#Concept> ;
                                                               <http://www.w3.org/2004/02/skos/core#broader> <http://w3.id.org/def/BiomassOntology#1-1-4-LoggingResidues> ;
                                                               <http://www.w3.org/2004/02/skos/core#inScheme> :BiomassScheme ;
                                                               <http://www.w3.org/2004/02/skos/core#definition> "Woody biomass consisting of fresh coniferous trees' logging residues, including needles."@en ;
                                                               <http://www.w3.org/2004/02/skos/core#prefLabel> "1.1.4.2. Fresh/green, coniferous (including needles)"@en .


###  http://w3.id.org/def/BiomassOntology#1-1-4-3-StoredBroadLeaf
<http://w3.id.org/def/BiomassOntology#1-1-4-3-StoredBroadLeaf> rdf:type owl:NamedIndividual ,
                                                                        <http://www.w3.org/2004/02/skos/core#Concept> ;
                                                               <http://www.w3.org/2004/02/skos/core#broader> <http://w3.id.org/def/BiomassOntology#1-1-4-LoggingResidues> ;
                                                               <http://www.w3.org/2004/02/skos/core#inScheme> :BiomassScheme ;
                                                               <http://www.w3.org/2004/02/skos/core#definition> "Woody biomass consisting of stored broad-leaf trees' logging residues."@en ;
                                                               <http://www.w3.org/2004/02/skos/core#prefLabel> "1.1.4.3. Stored, broad-leaf"@en .


###  http://w3.id.org/def/BiomassOntology#1-1-4-4-StoredConiferous
<http://w3.id.org/def/BiomassOntology#1-1-4-4-StoredConiferous> rdf:type owl:NamedIndividual ,
                                                                         <http://www.w3.org/2004/02/skos/core#Concept> ;
                                                                <http://www.w3.org/2004/02/skos/core#broader> <http://w3.id.org/def/BiomassOntology#1-1-4-LoggingResidues> ;
                                                                <http://www.w3.org/2004/02/skos/core#inScheme> :BiomassScheme ;
                                                                <http://www.w3.org/2004/02/skos/core#definition> "Woody biomass consisting of stored coniferous trees' logging residues."@en ;
                                                                <http://www.w3.org/2004/02/skos/core#prefLabel> "1.1.4.4. Stored, coniferous"@en .


###  http://w3.id.org/def/BiomassOntology#1-1-4-5-BlendsMixtures
<http://w3.id.org/def/BiomassOntology#1-1-4-5-BlendsMixtures> rdf:type owl:NamedIndividual ,
                                                                       <http://www.w3.org/2004/02/skos/core#Concept> ;
                                                              <http://www.w3.org/2004/02/skos/core#broader> <http://w3.id.org/def/BiomassOntology#1-1-4-LoggingResidues> ;
                                                              <http://www.w3.org/2004/02/skos/core#inScheme> :BiomassScheme ;
                                                              <http://www.w3.org/2004/02/skos/core#definition> "This refers to blends and mixtures of logging residues in the groups 1.1.4.1. to 1.1.4.4. The mixing can be either intentional (blends) or unintentional (mixtures)."@en ;
                                                              <http://www.w3.org/2004/02/skos/core#prefLabel> "1.1.4.5. Blends and mixtures"@en .


###  http://w3.id.org/def/BiomassOntology#1-1-5-StumpsRoots
<http://w3.id.org/def/BiomassOntology#1-1-5-StumpsRoots> rdf:type owl:NamedIndividual ,
                                                                  <http://www.w3.org/2004/02/skos/core#Concept> ;
                                                         <http://www.w3.org/2004/02/skos/core#broader> <http://w3.id.org/def/BiomassOntology#1-1-ForestPlantation> ;
                                                         <http://www.w3.org/2004/02/skos/core#inScheme> :BiomassScheme ;
                                                         <http://www.w3.org/2004/02/skos/core#definition> "Woody biomass consisting of stumps and/or roots."@en ;
                                                         <http://www.w3.org/2004/02/skos/core#prefLabel> "1.1..5. Stumps/roots"@en .


###  http://w3.id.org/def/BiomassOntology#1-1-5-1-BroadLeaf
<http://w3.id.org/def/BiomassOntology#1-1-5-1-BroadLeaf> rdf:type owl:NamedIndividual ,
                                                                  <http://www.w3.org/2004/02/skos/core#Concept> ;
                                                         <http://www.w3.org/2004/02/skos/core#broader> <http://w3.id.org/def/BiomassOntology#1-1-5-StumpsRoots> ;
                                                         <http://www.w3.org/2004/02/skos/core#inScheme> :BiomassScheme ;
                                                         <http://www.w3.org/2004/02/skos/core#definition> "Woody biomass consisting of broad-leaf trees' stumps and/or roots."@en ;
                                                         <http://www.w3.org/2004/02/skos/core#prefLabel> "1.1.5.1. Broad-leaf"@en .


###  http://w3.id.org/def/BiomassOntology#1-1-5-2-Coniferous
<http://w3.id.org/def/BiomassOntology#1-1-5-2-Coniferous> rdf:type owl:NamedIndividual ,
                                                                   <http://www.w3.org/2004/02/skos/core#Concept> ;
                                                          <http://www.w3.org/2004/02/skos/core#broader> <http://w3.id.org/def/BiomassOntology#1-1-5-StumpsRoots> ;
                                                          <http://www.w3.org/2004/02/skos/core#inScheme> :BiomassScheme ;
                                                          <http://www.w3.org/2004/02/skos/core#definition> "Woody biomass consisting of coniferous trees' stumps and/or roots."@en ;
                                                          <http://www.w3.org/2004/02/skos/core#prefLabel> "1.1.5.2. Coniferous"@en .


###  http://w3.id.org/def/BiomassOntology#1-1-5-3-ShortRotationCoppice
<http://w3.id.org/def/BiomassOntology#1-1-5-3-ShortRotationCoppice> rdf:type owl:NamedIndividual ,
                                                                             <http://www.w3.org/2004/02/skos/core#Concept> ;
                                                                    <http://www.w3.org/2004/02/skos/core#broader> <http://w3.id.org/def/BiomassOntology#1-1-5-StumpsRoots> ;
                                                                    <http://www.w3.org/2004/02/skos/core#inScheme> :BiomassScheme ;
                                                                    <http://www.w3.org/2004/02/skos/core#definition> "Woody biomass consisting of short rotation coppice trees' stumps and/or roots."@en ;
                                                                    <http://www.w3.org/2004/02/skos/core#prefLabel> "1.1.5.3.Short rotation coppice"@en .


###  http://w3.id.org/def/BiomassOntology#1-1-5-4-Bushes
<http://w3.id.org/def/BiomassOntology#1-1-5-4-Bushes> rdf:type owl:NamedIndividual ,
                                                               <http://www.w3.org/2004/02/skos/core#Concept> ;
                                                      <http://www.w3.org/2004/02/skos/core#broader> <http://w3.id.org/def/BiomassOntology#1-1-5-StumpsRoots> ;
                                                      <http://www.w3.org/2004/02/skos/core#inScheme> :BiomassScheme ;
                                                      <http://www.w3.org/2004/02/skos/core#definition> "Woody biomass consisting of bushes' stumps and/or roots."@en ;
                                                      <http://www.w3.org/2004/02/skos/core#prefLabel> "1.1.5.4. Bushes"@en .


###  http://w3.id.org/def/BiomassOntology#1-1-5-5-BlendsMixtures
<http://w3.id.org/def/BiomassOntology#1-1-5-5-BlendsMixtures> rdf:type owl:NamedIndividual ,
                                                                       <http://www.w3.org/2004/02/skos/core#Concept> ;
                                                              <http://www.w3.org/2004/02/skos/core#broader> <http://w3.id.org/def/BiomassOntology#1-1-5-StumpsRoots> ;
                                                              <http://www.w3.org/2004/02/skos/core#inScheme> :BiomassScheme ;
                                                              <http://www.w3.org/2004/02/skos/core#definition> "This refers to blends and mixtures of stumps and/or roots in the groups 1.1.5.1. to 1.1.5.4. The mixing can be either intentional (blends) or unintentional (mixtures)."@en ;
                                                              <http://www.w3.org/2004/02/skos/core#prefLabel> "1.1.5.5. Blends and mixtures"@en .


###  http://w3.id.org/def/BiomassOntology#1-1-6-Bark
<http://w3.id.org/def/BiomassOntology#1-1-6-Bark> rdf:type owl:NamedIndividual ,
                                                           <http://www.w3.org/2004/02/skos/core#Concept> ;
                                                  <http://www.w3.org/2004/02/skos/core#broader> <http://w3.id.org/def/BiomassOntology#1-1-ForestPlantation> ;
                                                  <http://www.w3.org/2004/02/skos/core#inScheme> :BiomassScheme ;
                                                  <http://www.w3.org/2004/02/skos/core#definition> "Woody biomass consisting of bark from forestry operations."@en ;
                                                  <http://www.w3.org/2004/02/skos/core#prefLabel> "1.1.6. Bark (from forestry operations)"@en .


###  http://w3.id.org/def/BiomassOntology#1-1-7-SegregatedWood
<http://w3.id.org/def/BiomassOntology#1-1-7-SegregatedWood> rdf:type owl:NamedIndividual ,
                                                                     <http://www.w3.org/2004/02/skos/core#Concept> ;
                                                            <http://www.w3.org/2004/02/skos/core#broader> <http://w3.id.org/def/BiomassOntology#1-1-ForestPlantation> ;
                                                            <http://www.w3.org/2004/02/skos/core#inScheme> :BiomassScheme ;
                                                            <http://www.w3.org/2004/02/skos/core#definition> "Woody biomass consisting of segregated wood from gardens, parks, roadside maintenance, vineyards, fruit orchards and/or driftwood from freshwater."@en ;
                                                            <http://www.w3.org/2004/02/skos/core#prefLabel> "1.1.7. Segregated wood from gardens, parks, roadside maintenance, vineyards, fruit orchards and driftwood from freshwater"@en .


###  http://w3.id.org/def/BiomassOntology#1-1-8-BlendsMixtures
<http://w3.id.org/def/BiomassOntology#1-1-8-BlendsMixtures> rdf:type owl:NamedIndividual ,
                                                                     <http://www.w3.org/2004/02/skos/core#Concept> ;
                                                            <http://www.w3.org/2004/02/skos/core#broader> <http://w3.id.org/def/BiomassOntology#1-1-ForestPlantation> ;
                                                            <http://www.w3.org/2004/02/skos/core#inScheme> :BiomassScheme ;
                                                            <http://www.w3.org/2004/02/skos/core#definition> "This refers to blends and mixtures of woody biomass in the groups 1.1.1 to 1.1.7. The mixing can be either intentional (blends) or unintentional (mixtures)."@en ;
                                                            <http://www.w3.org/2004/02/skos/core#prefLabel> "1.1.8. Blends and mixtures"@en .


###  http://w3.id.org/def/BiomassOntology#1-2-WoodByProducts
<http://w3.id.org/def/BiomassOntology#1-2-WoodByProducts> rdf:type owl:NamedIndividual ,
                                                                   <http://www.w3.org/2004/02/skos/core#Concept> ;
                                                          <http://www.w3.org/2004/02/skos/core#broader> <http://w3.id.org/def/BiomassOntology#1-WoodyBiomass> ;
                                                          <http://www.w3.org/2004/02/skos/core#inScheme> :BiomassScheme ;
                                                          <http://www.w3.org/2004/02/skos/core#definition> "Wood by-products and wood residues from industrial production are classified in this group. These biofuels can be chemically untreated (for example residues from debarking, sawing or size reduction, shaping, pressing) or chemically treated wood residues from wood processing and the production of panels and furniture (glued, painted, coated, lacquered or otherwise treated wood), as long as they do not contain heavy metals or halogenated organic compounds as a result of treatment with wood preservatives or coating."@en ;
                                                          <http://www.w3.org/2004/02/skos/core#prefLabel> "1.2. By-products and residues from wood processing industry"@en .


###  http://w3.id.org/def/BiomassOntology#1-2-1-ChemicallyUntreatedWood
<http://w3.id.org/def/BiomassOntology#1-2-1-ChemicallyUntreatedWood> rdf:type owl:NamedIndividual ,
                                                                              <http://www.w3.org/2004/02/skos/core#Concept> ;
                                                                     <http://www.w3.org/2004/02/skos/core#broader> <http://w3.id.org/def/BiomassOntology#1-2-WoodByProducts> ;
                                                                     <http://www.w3.org/2004/02/skos/core#inScheme> :BiomassScheme ;
                                                                     <http://www.w3.org/2004/02/skos/core#prefLabel> "1.2.1. Chemically untreated wood by-products and residues"@en ,
                                                                                                                     "Woody biomass consisting of chemically untreated wood by-products and residues."@en .


###  http://w3.id.org/def/BiomassOntology#1-2-1-1-BroadLeafBark
<http://w3.id.org/def/BiomassOntology#1-2-1-1-BroadLeafBark> rdf:type owl:NamedIndividual ,
                                                                      <http://www.w3.org/2004/02/skos/core#Concept> ;
                                                             <http://www.w3.org/2004/02/skos/core#broader> <http://w3.id.org/def/BiomassOntology#1-2-1-ChemicallyUntreatedWood> ;
                                                             <http://www.w3.org/2004/02/skos/core#inScheme> :BiomassScheme ;
                                                             <http://www.w3.org/2004/02/skos/core#definition> "Woody biomass consisting of chemically untreated broad-leaf trees' by-products and residues with bark."@en ;
                                                             <http://www.w3.org/2004/02/skos/core#prefLabel> "1.2.1.1. Broad-leaf with bark"@en .


###  http://w3.id.org/def/BiomassOntology#1-2-1-2-ConiferousBark
<http://w3.id.org/def/BiomassOntology#1-2-1-2-ConiferousBark> rdf:type owl:NamedIndividual ,
                                                                       <http://www.w3.org/2004/02/skos/core#Concept> ;
                                                              <http://www.w3.org/2004/02/skos/core#broader> <http://w3.id.org/def/BiomassOntology#1-2-1-ChemicallyUntreatedWood> ;
                                                              <http://www.w3.org/2004/02/skos/core#inScheme> :BiomassScheme ;
                                                              <http://www.w3.org/2004/02/skos/core#definition> "Woody biomass consisting of chemically untreated coniferous trees' by-products and residues with bark."@en ;
                                                              <http://www.w3.org/2004/02/skos/core#prefLabel> "1.2.1.2. Coniferous with bark"@en .


###  http://w3.id.org/def/BiomassOntology#1-2-1-3-BroadLeaf
<http://w3.id.org/def/BiomassOntology#1-2-1-3-BroadLeaf> rdf:type owl:NamedIndividual ,
                                                                  <http://www.w3.org/2004/02/skos/core#Concept> ;
                                                         <http://www.w3.org/2004/02/skos/core#broader> <http://w3.id.org/def/BiomassOntology#1-2-1-ChemicallyUntreatedWood> ;
                                                         <http://www.w3.org/2004/02/skos/core#inScheme> :BiomassScheme ;
                                                         <http://www.w3.org/2004/02/skos/core#definition> "Woody biomass consisting of chemically untreated broad-leaf trees' by-products and residues without bark."@en ;
                                                         <http://www.w3.org/2004/02/skos/core#prefLabel> "1.2.1.3. Broad-leaf without bark"@en .


###  http://w3.id.org/def/BiomassOntology#1-2-1-4-Coniferous
<http://w3.id.org/def/BiomassOntology#1-2-1-4-Coniferous> rdf:type owl:NamedIndividual ,
                                                                   <http://www.w3.org/2004/02/skos/core#Concept> ;
                                                          <http://www.w3.org/2004/02/skos/core#broader> <http://w3.id.org/def/BiomassOntology#1-2-1-ChemicallyUntreatedWood> ;
                                                          <http://www.w3.org/2004/02/skos/core#inScheme> :BiomassScheme ;
                                                          <http://www.w3.org/2004/02/skos/core#definition> "Woody biomass consisting of chemically untreated coniferous trees' by-products and residues without bark."@en ;
                                                          <http://www.w3.org/2004/02/skos/core#prefLabel> "1.2.1.4. Coniferous without bark"@en .


###  http://w3.id.org/def/BiomassOntology#1-2-1-5-Bark
<http://w3.id.org/def/BiomassOntology#1-2-1-5-Bark> rdf:type owl:NamedIndividual ,
                                                             <http://www.w3.org/2004/02/skos/core#Concept> ;
                                                    <http://www.w3.org/2004/02/skos/core#broader> <http://w3.id.org/def/BiomassOntology#1-2-1-ChemicallyUntreatedWood> ;
                                                    <http://www.w3.org/2004/02/skos/core#inScheme> :BiomassScheme ;
                                                    <http://www.w3.org/2004/02/skos/core#definition> "Woody biomass consisting of chemically untreated bark by-products and residues from industry operations."@en ;
                                                    <http://www.w3.org/2004/02/skos/core#prefLabel> "1.2.1.5. Bark (from industry operations)"@en .


###  http://w3.id.org/def/BiomassOntology#1-2-2-ChemicallyTreatedWood
<http://w3.id.org/def/BiomassOntology#1-2-2-ChemicallyTreatedWood> rdf:type owl:NamedIndividual ,
                                                                            <http://www.w3.org/2004/02/skos/core#Concept> ;
                                                                   <http://www.w3.org/2004/02/skos/core#broader> <http://w3.id.org/def/BiomassOntology#1-2-WoodByProducts> ;
                                                                   <http://www.w3.org/2004/02/skos/core#inScheme> :BiomassScheme ;
                                                                   <http://www.w3.org/2004/02/skos/core#definition> "Woody biomass consisting of chemically treated wood by-products and residues."@en ;
                                                                   <http://www.w3.org/2004/02/skos/core#prefLabel> "1.2.2. Chemically treated wood by-products, residues, fibres and wood constituents"@en .


###  http://w3.id.org/def/BiomassOntology#1-2-2-1-WithoutBark
<http://w3.id.org/def/BiomassOntology#1-2-2-1-WithoutBark> rdf:type owl:NamedIndividual ,
                                                                    <http://www.w3.org/2004/02/skos/core#Concept> ;
                                                           <http://www.w3.org/2004/02/skos/core#broader> <http://w3.id.org/def/BiomassOntology#1-2-2-ChemicallyTreatedWood> ;
                                                           <http://www.w3.org/2004/02/skos/core#inScheme> :BiomassScheme ;
                                                           <http://www.w3.org/2004/02/skos/core#definition> "Woody biomass consisting of chemically treated wood by-products and residues without bark."@en ;
                                                           <http://www.w3.org/2004/02/skos/core#prefLabel> "1.2.2.1. Without bark"@en .


###  http://w3.id.org/def/BiomassOntology#1-2-2-2-WithBark
<http://w3.id.org/def/BiomassOntology#1-2-2-2-WithBark> rdf:type owl:NamedIndividual ,
                                                                 <http://www.w3.org/2004/02/skos/core#Concept> ;
                                                        <http://www.w3.org/2004/02/skos/core#broader> <http://w3.id.org/def/BiomassOntology#1-2-2-ChemicallyTreatedWood> ;
                                                        <http://www.w3.org/2004/02/skos/core#inScheme> :BiomassScheme ;
                                                        <http://www.w3.org/2004/02/skos/core#definition> "Woody biomass consisting of chemically treated wood by-products and residues with bark."@en ;
                                                        <http://www.w3.org/2004/02/skos/core#prefLabel> "1.2.2.2. With bark"@en .


###  http://w3.id.org/def/BiomassOntology#1-2-2-3-Bark
<http://w3.id.org/def/BiomassOntology#1-2-2-3-Bark> rdf:type owl:NamedIndividual ,
                                                             <http://www.w3.org/2004/02/skos/core#Concept> ;
                                                    <http://www.w3.org/2004/02/skos/core#broader> <http://w3.id.org/def/BiomassOntology#1-2-2-ChemicallyTreatedWood> ;
                                                    <http://www.w3.org/2004/02/skos/core#inScheme> :BiomassScheme ;
                                                    <http://www.w3.org/2004/02/skos/core#definition> "Woody biomass consisting of chemically treated bark by-products and residues from industry operations."@en ;
                                                    <http://www.w3.org/2004/02/skos/core#prefLabel> "1.2.2.3. Bark (from industry operations)"@en .


###  http://w3.id.org/def/BiomassOntology#1-2-2-4-Fibres
<http://w3.id.org/def/BiomassOntology#1-2-2-4-Fibres> rdf:type owl:NamedIndividual ,
                                                               <http://www.w3.org/2004/02/skos/core#Concept> ;
                                                      <http://www.w3.org/2004/02/skos/core#broader> <http://w3.id.org/def/BiomassOntology#1-2-2-ChemicallyTreatedWood> ;
                                                      <http://www.w3.org/2004/02/skos/core#inScheme> :BiomassScheme ;
                                                      <http://www.w3.org/2004/02/skos/core#definition> "Woody biomass consisting of chemically treated fibres and wood constituents by-products and residues."@en ;
                                                      <http://www.w3.org/2004/02/skos/core#prefLabel> "1.2.2.4. Fibres and wood constituents"@en .


###  http://w3.id.org/def/BiomassOntology#1-2-3-BlendsMixtures
<http://w3.id.org/def/BiomassOntology#1-2-3-BlendsMixtures> rdf:type owl:NamedIndividual ,
                                                                     <http://www.w3.org/2004/02/skos/core#Concept> ;
                                                            <http://www.w3.org/2004/02/skos/core#broader> <http://w3.id.org/def/BiomassOntology#1-2-WoodByProducts> ;
                                                            <http://www.w3.org/2004/02/skos/core#inScheme> :BiomassScheme ;
                                                            <http://www.w3.org/2004/02/skos/core#definition> "This refers to blends and mixtures of wood by-products and residues in the groups 1.2.1 to 1.2.2. The mixing can be either intentional (blends) or unintentional (mixtures)."@en ;
                                                            <http://www.w3.org/2004/02/skos/core#prefLabel> "1.2.3. Blends and mixtures"@en .


###  http://w3.id.org/def/BiomassOntology#1-3-UsedWood
<http://w3.id.org/def/BiomassOntology#1-3-UsedWood> rdf:type owl:NamedIndividual ,
                                                             <http://www.w3.org/2004/02/skos/core#Concept> ;
                                                    <http://www.w3.org/2004/02/skos/core#broader> <http://w3.id.org/def/BiomassOntology#1-WoodyBiomass> ;
                                                    <http://www.w3.org/2004/02/skos/core#inScheme> :BiomassScheme ;
                                                    <http://www.w3.org/2004/02/skos/core#definition> "This group includes post-consumer/post society wood waste; natural or merely mechanically processed wood, contaminated only to an insignificant extent during use by substances that are not normally found in wood in its natural state (for example pallets, transport cases, boxes, wood packages, cable reels, construction wood). With respect to treatment the same criteria apply as with respect to “wood processing industry by-products and residues”, i.e. the used wood shall not contain heavy metals more than in virgin wood, or halogenated organic compounds as a result of treatment with wood preservatives or coating."@en ;
                                                    <http://www.w3.org/2004/02/skos/core#prefLabel> "1.3. Used wood"@en .


###  http://w3.id.org/def/BiomassOntology#1-3-1-ChemicallyUntreated
<http://w3.id.org/def/BiomassOntology#1-3-1-ChemicallyUntreated> rdf:type owl:NamedIndividual ,
                                                                          <http://www.w3.org/2004/02/skos/core#Concept> ;
                                                                 <http://www.w3.org/2004/02/skos/core#broader> <http://w3.id.org/def/BiomassOntology#1-3-UsedWood> ;
                                                                 <http://www.w3.org/2004/02/skos/core#inScheme> :BiomassScheme ;
                                                                 <http://www.w3.org/2004/02/skos/core#definition> "Woody biomass consisting of chemically untreated used wood."@en ;
                                                                 <http://www.w3.org/2004/02/skos/core#prefLabel> "1.3.1. Chemically untreated used wood"@en .


###  http://w3.id.org/def/BiomassOntology#1-3-1-1-WithoutBark
<http://w3.id.org/def/BiomassOntology#1-3-1-1-WithoutBark> rdf:type owl:NamedIndividual ,
                                                                    <http://www.w3.org/2004/02/skos/core#Concept> ;
                                                           <http://www.w3.org/2004/02/skos/core#broader> <http://w3.id.org/def/BiomassOntology#1-3-1-ChemicallyUntreated> ;
                                                           <http://www.w3.org/2004/02/skos/core#inScheme> :BiomassScheme ;
                                                           <http://www.w3.org/2004/02/skos/core#definition> "Woody biomass consisting of chemically untreated used wood without bark."@en ;
                                                           <http://www.w3.org/2004/02/skos/core#prefLabel> "1.3.1.1. Without bark"@en .


###  http://w3.id.org/def/BiomassOntology#1-3-1-2-WithBark
<http://w3.id.org/def/BiomassOntology#1-3-1-2-WithBark> rdf:type owl:NamedIndividual ,
                                                                 <http://www.w3.org/2004/02/skos/core#Concept> ;
                                                        <http://www.w3.org/2004/02/skos/core#broader> <http://w3.id.org/def/BiomassOntology#1-3-1-ChemicallyUntreated> ;
                                                        <http://www.w3.org/2004/02/skos/core#inScheme> :BiomassScheme ;
                                                        <http://www.w3.org/2004/02/skos/core#definition> "Woody biomass consisting of chemically untreated used wood with bark."@en ;
                                                        <http://www.w3.org/2004/02/skos/core#prefLabel> "1.3.1.2. With bark"@en .


###  http://w3.id.org/def/BiomassOntology#1-3-1-3-Bark
<http://w3.id.org/def/BiomassOntology#1-3-1-3-Bark> rdf:type owl:NamedIndividual ,
                                                             <http://www.w3.org/2004/02/skos/core#Concept> ;
                                                    <http://www.w3.org/2004/02/skos/core#broader> <http://w3.id.org/def/BiomassOntology#1-3-1-ChemicallyUntreated> ;
                                                    <http://www.w3.org/2004/02/skos/core#inScheme> :BiomassScheme ;
                                                    <http://www.w3.org/2004/02/skos/core#definition> "Woody biomass consisting of chemically untreated used bark."@en ;
                                                    <http://www.w3.org/2004/02/skos/core#prefLabel> "1.3.1.3. Bark"@en .


###  http://w3.id.org/def/BiomassOntology#1-3-2-ChemicallyTreated
<http://w3.id.org/def/BiomassOntology#1-3-2-ChemicallyTreated> rdf:type owl:NamedIndividual ,
                                                                        <http://www.w3.org/2004/02/skos/core#Concept> ;
                                                               <http://www.w3.org/2004/02/skos/core#broader> <http://w3.id.org/def/BiomassOntology#1-3-UsedWood> ;
                                                               <http://www.w3.org/2004/02/skos/core#inScheme> :BiomassScheme ;
                                                               <http://www.w3.org/2004/02/skos/core#definition> "Woody biomass consisting of chemically treated used wood."@en ;
                                                               <http://www.w3.org/2004/02/skos/core#prefLabel> "1.3.2. Chemically treated used wood"@en .


###  http://w3.id.org/def/BiomassOntology#1-3-2-1-WithoutBark
<http://w3.id.org/def/BiomassOntology#1-3-2-1-WithoutBark> rdf:type owl:NamedIndividual ,
                                                                    <http://www.w3.org/2004/02/skos/core#Concept> ;
                                                           <http://www.w3.org/2004/02/skos/core#broader> <http://w3.id.org/def/BiomassOntology#1-3-2-ChemicallyTreated> ;
                                                           <http://www.w3.org/2004/02/skos/core#inScheme> :BiomassScheme ;
                                                           <http://www.w3.org/2004/02/skos/core#definition> "Woody biomass consisting of chemically treated used wood without bark."@en ;
                                                           <http://www.w3.org/2004/02/skos/core#prefLabel> "1.3.2.1. Without bark"@en .


###  http://w3.id.org/def/BiomassOntology#1-3-2-2-WithBark
<http://w3.id.org/def/BiomassOntology#1-3-2-2-WithBark> rdf:type owl:NamedIndividual ,
                                                                 <http://www.w3.org/2004/02/skos/core#Concept> ;
                                                        <http://www.w3.org/2004/02/skos/core#broader> <http://w3.id.org/def/BiomassOntology#1-3-2-ChemicallyTreated> ;
                                                        <http://www.w3.org/2004/02/skos/core#inScheme> :BiomassScheme ;
                                                        <http://www.w3.org/2004/02/skos/core#definition> "Woody biomass consisting of chemically treated used wood with bark."@en ;
                                                        <http://www.w3.org/2004/02/skos/core#prefLabel> "1.3.2.2. With bark"@en .


###  http://w3.id.org/def/BiomassOntology#1-3-2-3-Bark
<http://w3.id.org/def/BiomassOntology#1-3-2-3-Bark> rdf:type owl:NamedIndividual ,
                                                             <http://www.w3.org/2004/02/skos/core#Concept> ;
                                                    <http://www.w3.org/2004/02/skos/core#broader> <http://w3.id.org/def/BiomassOntology#1-3-2-ChemicallyTreated> ;
                                                    <http://www.w3.org/2004/02/skos/core#inScheme> :BiomassScheme ;
                                                    <http://www.w3.org/2004/02/skos/core#definition> "Woody biomass consisting of chemically treated used bark."@en ;
                                                    <http://www.w3.org/2004/02/skos/core#prefLabel> "1.3.2.3. Bark"@en .


###  http://w3.id.org/def/BiomassOntology#1-3-3-BlendsMixtures
<http://w3.id.org/def/BiomassOntology#1-3-3-BlendsMixtures> rdf:type owl:NamedIndividual ,
                                                                     <http://www.w3.org/2004/02/skos/core#Concept> ;
                                                            <http://www.w3.org/2004/02/skos/core#broader> <http://w3.id.org/def/BiomassOntology#1-3-UsedWood> ;
                                                            <http://www.w3.org/2004/02/skos/core#inScheme> :BiomassScheme ;
                                                            <http://www.w3.org/2004/02/skos/core#definition> "This refers to blends and mixtures of used wood in the groups 1.3.1 to 1.3.2. The mixing can be either intentional (blends) or unintentional (mixtures)."@en ;
                                                            <http://www.w3.org/2004/02/skos/core#prefLabel> "1.3.3. Blends and mixtures"@en .


###  http://w3.id.org/def/BiomassOntology#1-4-BlendsMixtures
<http://w3.id.org/def/BiomassOntology#1-4-BlendsMixtures> rdf:type owl:NamedIndividual ,
                                                                   <http://www.w3.org/2004/02/skos/core#Concept> ;
                                                          <http://www.w3.org/2004/02/skos/core#broader> <http://w3.id.org/def/BiomassOntology#1-WoodyBiomass> ;
                                                          <http://www.w3.org/2004/02/skos/core#inScheme> :BiomassScheme ;
                                                          <http://www.w3.org/2004/02/skos/core#definition> "This refers to blends and mixtures of woody biomass in the groups 1.1 to 1.3. The mixing can be either intentional (blends) or unintentional (mixtures)."@en ;
                                                          <http://www.w3.org/2004/02/skos/core#prefLabel> "1.4. Blends and mixtures"@en .


###  http://w3.id.org/def/BiomassOntology#2-HerbaceousBiomass
<http://w3.id.org/def/BiomassOntology#2-HerbaceousBiomass> rdf:type owl:NamedIndividual ,
                                                                    <http://www.w3.org/2004/02/skos/core#Concept> ;
                                                           <http://www.w3.org/2004/02/skos/core#topConceptOf> :BiomassScheme ;
                                                           <http://www.w3.org/2004/02/skos/core#definition> "Biomass from plants that have a non-woody stem and which die back at the end of the growing season. It includes grains and their by-products such as cereals."@en ;
                                                           <http://www.w3.org/2004/02/skos/core#prefLabel> "2. Herbaceous biomass"@en .


###  http://w3.id.org/def/BiomassOntology#2-1-AgricultureHorticulture
<http://w3.id.org/def/BiomassOntology#2-1-AgricultureHorticulture> rdf:type owl:NamedIndividual ,
                                                                            <http://www.w3.org/2004/02/skos/core#Concept> ;
                                                                   <http://www.w3.org/2004/02/skos/core#broader> <http://w3.id.org/def/BiomassOntology#2-HerbaceousBiomass> ;
                                                                   <http://www.w3.org/2004/02/skos/core#inScheme> :BiomassScheme ;
                                                                   <http://www.w3.org/2004/02/skos/core#definition> "Material, which comes directly from the field, perhaps after a storage period, and may only have been subject to size reduction and drying is included here. It covers herbaceous material from agricultural and horticultural fields and from gardens and parks."@en ;
                                                                   <http://www.w3.org/2004/02/skos/core#prefLabel> "2.1. Herbaceous biomass from agriculture and horticulture"@en .


###  http://w3.id.org/def/BiomassOntology#2-1-1-CerealCrops
<http://w3.id.org/def/BiomassOntology#2-1-1-CerealCrops> rdf:type owl:NamedIndividual ,
                                                                  <http://www.w3.org/2004/02/skos/core#Concept> ;
                                                         <http://www.w3.org/2004/02/skos/core#broader> <http://w3.id.org/def/BiomassOntology#2-1-AgricultureHorticulture> ;
                                                         <http://www.w3.org/2004/02/skos/core#inScheme> :BiomassScheme ;
                                                         <http://www.w3.org/2004/02/skos/core#definition> "Herbaceous biomass consisting of cereal crops."@en ;
                                                         <http://www.w3.org/2004/02/skos/core#prefLabel> "2.1.1. Cereal crops"@en .


###  http://w3.id.org/def/BiomassOntology#2-1-1-1-WholePlant
<http://w3.id.org/def/BiomassOntology#2-1-1-1-WholePlant> rdf:type owl:NamedIndividual ,
                                                                   <http://www.w3.org/2004/02/skos/core#Concept> ;
                                                          <http://www.w3.org/2004/02/skos/core#broader> <http://w3.id.org/def/BiomassOntology#2-1-1-CerealCrops> ;
                                                          <http://www.w3.org/2004/02/skos/core#inScheme> :BiomassScheme ;
                                                          <http://www.w3.org/2004/02/skos/core#definition> "Herbaceous biomass consisting of whole plants from cereal crops."@en ;
                                                          <http://www.w3.org/2004/02/skos/core#prefLabel> "2.1.1.1. Whole plant"@en .


###  http://w3.id.org/def/BiomassOntology#2-1-1-2-StrawParts
<http://w3.id.org/def/BiomassOntology#2-1-1-2-StrawParts> rdf:type owl:NamedIndividual ,
                                                                   <http://www.w3.org/2004/02/skos/core#Concept> ;
                                                          <http://www.w3.org/2004/02/skos/core#broader> <http://w3.id.org/def/BiomassOntology#2-1-1-CerealCrops> ;
                                                          <http://www.w3.org/2004/02/skos/core#inScheme> :BiomassScheme ;
                                                          <http://www.w3.org/2004/02/skos/core#definition> "Herbaceous biomass consisting of straw parts from cereal crops."@en ;
                                                          <http://www.w3.org/2004/02/skos/core#prefLabel> "2.1.1.2. Straw parts"@en .


###  http://w3.id.org/def/BiomassOntology#2-1-1-3-GrainsSeeds
<http://w3.id.org/def/BiomassOntology#2-1-1-3-GrainsSeeds> rdf:type owl:NamedIndividual ,
                                                                    <http://www.w3.org/2004/02/skos/core#Concept> ;
                                                           <http://www.w3.org/2004/02/skos/core#broader> <http://w3.id.org/def/BiomassOntology#2-1-1-CerealCrops> ;
                                                           <http://www.w3.org/2004/02/skos/core#inScheme> :BiomassScheme ;
                                                           <http://www.w3.org/2004/02/skos/core#definition> "Herbaceous biomass consisting of grains or seeds from cereal crops."@en ;
                                                           <http://www.w3.org/2004/02/skos/core#prefLabel> "2.1.1.3. Grains or seeds"@en .


###  http://w3.id.org/def/BiomassOntology#2-1-1-4-HusksShells
<http://w3.id.org/def/BiomassOntology#2-1-1-4-HusksShells> rdf:type owl:NamedIndividual ,
                                                                    <http://www.w3.org/2004/02/skos/core#Concept> ;
                                                           <http://www.w3.org/2004/02/skos/core#broader> <http://w3.id.org/def/BiomassOntology#2-1-1-CerealCrops> ;
                                                           <http://www.w3.org/2004/02/skos/core#inScheme> :BiomassScheme ;
                                                           <http://www.w3.org/2004/02/skos/core#definition> "Herbaceous biomass consisting of husks or shells from cereal crops."@en ;
                                                           <http://www.w3.org/2004/02/skos/core#prefLabel> "2.1.1.4. Husks or shells"@en .


###  http://w3.id.org/def/BiomassOntology#2-1-1-5-BlendsMixtures
<http://w3.id.org/def/BiomassOntology#2-1-1-5-BlendsMixtures> rdf:type owl:NamedIndividual ,
                                                                       <http://www.w3.org/2004/02/skos/core#Concept> ;
                                                              <http://www.w3.org/2004/02/skos/core#broader> <http://w3.id.org/def/BiomassOntology#2-1-1-CerealCrops> ;
                                                              <http://www.w3.org/2004/02/skos/core#inScheme> :BiomassScheme ;
                                                              <http://www.w3.org/2004/02/skos/core#definition> "This refers to blends and mixtures of cereal crops in the groups 2.1.1.1. to 2.1.1.4. The mixing can be either intentional (blends) or unintentional (mixtures)."@en ;
                                                              <http://www.w3.org/2004/02/skos/core#prefLabel> "2.1.1.5. Blends and mixtures"@en .


###  http://w3.id.org/def/BiomassOntology#2-1-2-Grasses
<http://w3.id.org/def/BiomassOntology#2-1-2-Grasses> rdf:type owl:NamedIndividual ,
                                                              <http://www.w3.org/2004/02/skos/core#Concept> ;
                                                     <http://www.w3.org/2004/02/skos/core#broader> <http://w3.id.org/def/BiomassOntology#2-1-AgricultureHorticulture> ;
                                                     <http://www.w3.org/2004/02/skos/core#inScheme> :BiomassScheme ;
                                                     <http://www.w3.org/2004/02/skos/core#definition> "Herbaceous biomass consisting of grasses."@en ;
                                                     <http://www.w3.org/2004/02/skos/core#prefLabel> "2.1.2. Grasses"@en .


###  http://w3.id.org/def/BiomassOntology#2-1-2-1-WholePlant
<http://w3.id.org/def/BiomassOntology#2-1-2-1-WholePlant> rdf:type owl:NamedIndividual ,
                                                                   <http://www.w3.org/2004/02/skos/core#Concept> ;
                                                          <http://www.w3.org/2004/02/skos/core#broader> <http://w3.id.org/def/BiomassOntology#2-1-2-Grasses> ;
                                                          <http://www.w3.org/2004/02/skos/core#inScheme> :BiomassScheme ;
                                                          <http://www.w3.org/2004/02/skos/core#definition> "Herbaceous biomass consisting of whole plants from grasses."@en ;
                                                          <http://www.w3.org/2004/02/skos/core#prefLabel> "2.1.2.1. Whole plant"@en .


###  http://w3.id.org/def/BiomassOntology#2-1-2-2-StrawParts
<http://w3.id.org/def/BiomassOntology#2-1-2-2-StrawParts> rdf:type owl:NamedIndividual ,
                                                                   <http://www.w3.org/2004/02/skos/core#Concept> ;
                                                          <http://www.w3.org/2004/02/skos/core#broader> <http://w3.id.org/def/BiomassOntology#2-1-2-Grasses> ;
                                                          <http://www.w3.org/2004/02/skos/core#inScheme> :BiomassScheme ;
                                                          <http://www.w3.org/2004/02/skos/core#definition> "Herbaceous biomass consisting of straw parts from grasses."@en ;
                                                          <http://www.w3.org/2004/02/skos/core#prefLabel> "2.1.2.2. Straw parts"@en .


###  http://w3.id.org/def/BiomassOntology#2-1-2-3-Seeds
<http://w3.id.org/def/BiomassOntology#2-1-2-3-Seeds> rdf:type owl:NamedIndividual ,
                                                              <http://www.w3.org/2004/02/skos/core#Concept> ;
                                                     <http://www.w3.org/2004/02/skos/core#broader> <http://w3.id.org/def/BiomassOntology#2-1-2-Grasses> ;
                                                     <http://www.w3.org/2004/02/skos/core#inScheme> :BiomassScheme ;
                                                     <http://www.w3.org/2004/02/skos/core#definition> "Herbaceous biomass consisting of seeds from grasses."@en ;
                                                     <http://www.w3.org/2004/02/skos/core#prefLabel> "2.1.2.3. Seeds"@en .


###  http://w3.id.org/def/BiomassOntology#2-1-2-4-Shells
<http://w3.id.org/def/BiomassOntology#2-1-2-4-Shells> rdf:type owl:NamedIndividual ,
                                                               <http://www.w3.org/2004/02/skos/core#Concept> ;
                                                      <http://www.w3.org/2004/02/skos/core#broader> <http://w3.id.org/def/BiomassOntology#2-1-2-Grasses> ;
                                                      <http://www.w3.org/2004/02/skos/core#inScheme> :BiomassScheme ;
                                                      <http://www.w3.org/2004/02/skos/core#definition> "Herbaceous biomass consisting of shells from grasses."@en ;
                                                      <http://www.w3.org/2004/02/skos/core#prefLabel> "2.1.2.4. Shells"@en .


###  http://w3.id.org/def/BiomassOntology#2-1-2-5-Bamboo
<http://w3.id.org/def/BiomassOntology#2-1-2-5-Bamboo> rdf:type owl:NamedIndividual ,
                                                               <http://www.w3.org/2004/02/skos/core#Concept> ;
                                                      <http://www.w3.org/2004/02/skos/core#broader> <http://w3.id.org/def/BiomassOntology#2-1-2-Grasses> ;
                                                      <http://www.w3.org/2004/02/skos/core#inScheme> :BiomassScheme ;
                                                      <http://www.w3.org/2004/02/skos/core#definition> "Herbaceous biomass consisting of bamboo grass."@en ;
                                                      <http://www.w3.org/2004/02/skos/core#prefLabel> "2.1.2.5. Bamboo"@en .


###  http://w3.id.org/def/BiomassOntology#2-1-2-6-BlendsMixtures
<http://w3.id.org/def/BiomassOntology#2-1-2-6-BlendsMixtures> rdf:type owl:NamedIndividual ,
                                                                       <http://www.w3.org/2004/02/skos/core#Concept> ;
                                                              <http://www.w3.org/2004/02/skos/core#broader> <http://w3.id.org/def/BiomassOntology#2-1-2-Grasses> ;
                                                              <http://www.w3.org/2004/02/skos/core#inScheme> :BiomassScheme ;
                                                              <http://www.w3.org/2004/02/skos/core#definition> "This refers to blends and mixtures of grasses in the groups 2.1.2.1. to 2.1.2.5. The mixing can be either intentional (blends) or unintentional (mixtures)."@en ;
                                                              <http://www.w3.org/2004/02/skos/core#prefLabel> "2.1.2.6. Blends and mixtures"@en .


###  http://w3.id.org/def/BiomassOntology#2-1-3-OilSeedCrops
<http://w3.id.org/def/BiomassOntology#2-1-3-OilSeedCrops> rdf:type owl:NamedIndividual ,
                                                                   <http://www.w3.org/2004/02/skos/core#Concept> ;
                                                          <http://www.w3.org/2004/02/skos/core#broader> <http://w3.id.org/def/BiomassOntology#2-1-AgricultureHorticulture> ;
                                                          <http://www.w3.org/2004/02/skos/core#inScheme> :BiomassScheme ;
                                                          <http://www.w3.org/2004/02/skos/core#definition> "Herbaceous biomass consisting of oil seed crops."@en ;
                                                          <http://www.w3.org/2004/02/skos/core#prefLabel> "2.1.3. Oil seed crops"@en .


###  http://w3.id.org/def/BiomassOntology#2-1-3-1-WholePlant
<http://w3.id.org/def/BiomassOntology#2-1-3-1-WholePlant> rdf:type owl:NamedIndividual ,
                                                                   <http://www.w3.org/2004/02/skos/core#Concept> ;
                                                          <http://www.w3.org/2004/02/skos/core#broader> <http://w3.id.org/def/BiomassOntology#2-1-3-OilSeedCrops> ;
                                                          <http://www.w3.org/2004/02/skos/core#inScheme> :BiomassScheme ;
                                                          <http://www.w3.org/2004/02/skos/core#definition> "Herbaceous biomass consisting of whole plants from oil seed crops."@en ;
                                                          <http://www.w3.org/2004/02/skos/core#prefLabel> "2.1.3.1. Whole plant"@en .


###  http://w3.id.org/def/BiomassOntology#2-1-3-2-StalkLeaves
<http://w3.id.org/def/BiomassOntology#2-1-3-2-StalkLeaves> rdf:type owl:NamedIndividual ,
                                                                    <http://www.w3.org/2004/02/skos/core#Concept> ;
                                                           <http://www.w3.org/2004/02/skos/core#broader> <http://w3.id.org/def/BiomassOntology#2-1-3-OilSeedCrops> ;
                                                           <http://www.w3.org/2004/02/skos/core#inScheme> :BiomassScheme ;
                                                           <http://www.w3.org/2004/02/skos/core#definition> "Herbaceous biomass consisting of stalk and leaves from oil seed crops."@en ;
                                                           <http://www.w3.org/2004/02/skos/core#prefLabel> "2.1.3.2. Stalks and leaves"@en .


###  http://w3.id.org/def/BiomassOntology#2-1-3-3-Seeds
<http://w3.id.org/def/BiomassOntology#2-1-3-3-Seeds> rdf:type owl:NamedIndividual ,
                                                              <http://www.w3.org/2004/02/skos/core#Concept> ;
                                                     <http://www.w3.org/2004/02/skos/core#broader> <http://w3.id.org/def/BiomassOntology#2-1-3-OilSeedCrops> ;
                                                     <http://www.w3.org/2004/02/skos/core#inScheme> :BiomassScheme ;
                                                     <http://www.w3.org/2004/02/skos/core#definition> "Herbaceous biomass consisting of seeds from oil seed crops."@en ;
                                                     <http://www.w3.org/2004/02/skos/core#prefLabel> "2.1.3.3. Seeds"@en .


###  http://w3.id.org/def/BiomassOntology#2-1-3-4-HusksShells
<http://w3.id.org/def/BiomassOntology#2-1-3-4-HusksShells> rdf:type owl:NamedIndividual ,
                                                                    <http://www.w3.org/2004/02/skos/core#Concept> ;
                                                           <http://www.w3.org/2004/02/skos/core#broader> <http://w3.id.org/def/BiomassOntology#2-1-3-OilSeedCrops> ;
                                                           <http://www.w3.org/2004/02/skos/core#inScheme> :BiomassScheme ;
                                                           <http://www.w3.org/2004/02/skos/core#definition> "Herbaceous biomass consisting of husks or shells from oil seed crops."@en ;
                                                           <http://www.w3.org/2004/02/skos/core#prefLabel> "2.1.3.4. Husks or shells"@en .


###  http://w3.id.org/def/BiomassOntology#2-1-3-5-BlendsMixtures
<http://w3.id.org/def/BiomassOntology#2-1-3-5-BlendsMixtures> rdf:type owl:NamedIndividual ,
                                                                       <http://www.w3.org/2004/02/skos/core#Concept> ;
                                                              <http://www.w3.org/2004/02/skos/core#broader> <http://w3.id.org/def/BiomassOntology#2-1-3-OilSeedCrops> ;
                                                              <http://www.w3.org/2004/02/skos/core#inScheme> :BiomassScheme ;
                                                              <http://www.w3.org/2004/02/skos/core#definition> "This refers to blends and mixtures of oil seed crops in the groups 2.1.3.1. to 2.1.3.4. The mixing can be either intentional (blends) or unintentional (mixtures)."@en .


###  http://w3.id.org/def/BiomassOntology#2-1-4-RootCrops
<http://w3.id.org/def/BiomassOntology#2-1-4-RootCrops> rdf:type owl:NamedIndividual ,
                                                                <http://www.w3.org/2004/02/skos/core#Concept> ;
                                                       <http://www.w3.org/2004/02/skos/core#broader> <http://w3.id.org/def/BiomassOntology#2-1-AgricultureHorticulture> ;
                                                       <http://www.w3.org/2004/02/skos/core#inScheme> :BiomassScheme ;
                                                       <http://www.w3.org/2004/02/skos/core#definition> "Herbaceous biomass consisting of root crops."@en ;
                                                       <http://www.w3.org/2004/02/skos/core#prefLabel> "2.1.4. Root crops"@en .


###  http://w3.id.org/def/BiomassOntology#2-1-4-1-WholePlant
<http://w3.id.org/def/BiomassOntology#2-1-4-1-WholePlant> rdf:type owl:NamedIndividual ,
                                                                   <http://www.w3.org/2004/02/skos/core#Concept> ;
                                                          <http://www.w3.org/2004/02/skos/core#broader> <http://w3.id.org/def/BiomassOntology#2-1-4-RootCrops> ;
                                                          <http://www.w3.org/2004/02/skos/core#inScheme> :BiomassScheme ;
                                                          <http://www.w3.org/2004/02/skos/core#definition> "Herbaceous biomass consisting of whole plants from root crops."@en ;
                                                          <http://www.w3.org/2004/02/skos/core#prefLabel> "2.1.4.1. Whole plant"@en .


###  http://w3.id.org/def/BiomassOntology#2-1-4-2-StalkLeaves
<http://w3.id.org/def/BiomassOntology#2-1-4-2-StalkLeaves> rdf:type owl:NamedIndividual ,
                                                                    <http://www.w3.org/2004/02/skos/core#Concept> ;
                                                           <http://www.w3.org/2004/02/skos/core#broader> <http://w3.id.org/def/BiomassOntology#2-1-4-RootCrops> ;
                                                           <http://www.w3.org/2004/02/skos/core#inScheme> :BiomassScheme ;
                                                           <http://www.w3.org/2004/02/skos/core#definition> "Herbaceous biomass consisting of stalk and leaves from root crops."@en ;
                                                           <http://www.w3.org/2004/02/skos/core#prefLabel> "2.1.4.2. Stalks and leaves"@en .


###  http://w3.id.org/def/BiomassOntology#2-1-4-3-Root
<http://w3.id.org/def/BiomassOntology#2-1-4-3-Root> rdf:type owl:NamedIndividual ,
                                                             <http://www.w3.org/2004/02/skos/core#Concept> ;
                                                    <http://www.w3.org/2004/02/skos/core#broader> <http://w3.id.org/def/BiomassOntology#2-1-4-RootCrops> ;
                                                    <http://www.w3.org/2004/02/skos/core#inScheme> :BiomassScheme ;
                                                    <http://www.w3.org/2004/02/skos/core#definition> "Herbaceous biomass consisting of roots from root crops."@en ;
                                                    <http://www.w3.org/2004/02/skos/core#prefLabel> "2.1.4.3. Root"@en .


###  http://w3.id.org/def/BiomassOntology#2-1-4-4-BlendsMixtures
<http://w3.id.org/def/BiomassOntology#2-1-4-4-BlendsMixtures> rdf:type owl:NamedIndividual ,
                                                                       <http://www.w3.org/2004/02/skos/core#Concept> ;
                                                              <http://www.w3.org/2004/02/skos/core#broader> <http://w3.id.org/def/BiomassOntology#2-1-4-RootCrops> ;
                                                              <http://www.w3.org/2004/02/skos/core#inScheme> :BiomassScheme ;
                                                              <http://www.w3.org/2004/02/skos/core#definition> "This refers to blends and mixtures of root crops in the groups 2.1.4.1. to 2.1.4.3. The mixing can be either intentional (blends) or unintentional (mixtures)."@en ;
                                                              <http://www.w3.org/2004/02/skos/core#prefLabel> "2.1.4.4. Blends and mixtures"@en .


###  http://w3.id.org/def/BiomassOntology#2-1-5-LegumeCrops
<http://w3.id.org/def/BiomassOntology#2-1-5-LegumeCrops> rdf:type owl:NamedIndividual ,
                                                                  <http://www.w3.org/2004/02/skos/core#Concept> ;
                                                         <http://www.w3.org/2004/02/skos/core#broader> <http://w3.id.org/def/BiomassOntology#2-1-AgricultureHorticulture> ;
                                                         <http://www.w3.org/2004/02/skos/core#inScheme> :BiomassScheme ;
                                                         <http://www.w3.org/2004/02/skos/core#definition> "Herbaceous biomass consisting of legume crops."@en ;
                                                         <http://www.w3.org/2004/02/skos/core#prefLabel> "2.1.5. Legume crops"@en .


###  http://w3.id.org/def/BiomassOntology#2-1-5-1-WholePlant
<http://w3.id.org/def/BiomassOntology#2-1-5-1-WholePlant> rdf:type owl:NamedIndividual ,
                                                                   <http://www.w3.org/2004/02/skos/core#Concept> ;
                                                          <http://www.w3.org/2004/02/skos/core#broader> <http://w3.id.org/def/BiomassOntology#2-1-5-LegumeCrops> ;
                                                          <http://www.w3.org/2004/02/skos/core#inScheme> :BiomassScheme ;
                                                          <http://www.w3.org/2004/02/skos/core#definition> "Herbaceous biomass consisting of whole plants from legume crops."@en ;
                                                          <http://www.w3.org/2004/02/skos/core#prefLabel> "2.1.5.1. Whole plant"@en .


###  http://w3.id.org/def/BiomassOntology#2-1-5-2-StalkLeaves
<http://w3.id.org/def/BiomassOntology#2-1-5-2-StalkLeaves> rdf:type owl:NamedIndividual ,
                                                                    <http://www.w3.org/2004/02/skos/core#Concept> ;
                                                           <http://www.w3.org/2004/02/skos/core#broader> <http://w3.id.org/def/BiomassOntology#2-1-5-LegumeCrops> ;
                                                           <http://www.w3.org/2004/02/skos/core#inScheme> :BiomassScheme ;
                                                           <http://www.w3.org/2004/02/skos/core#definition> "Herbaceous biomass consisting of stalk and leaves from legume crops."@en ;
                                                           <http://www.w3.org/2004/02/skos/core#prefLabel> "2.1.5.2. Stalks and leaves"@en .


###  http://w3.id.org/def/BiomassOntology#2-1-5-3-Fruit
<http://w3.id.org/def/BiomassOntology#2-1-5-3-Fruit> rdf:type owl:NamedIndividual ,
                                                              <http://www.w3.org/2004/02/skos/core#Concept> ;
                                                     <http://www.w3.org/2004/02/skos/core#broader> <http://w3.id.org/def/BiomassOntology#2-1-5-LegumeCrops> ;
                                                     <http://www.w3.org/2004/02/skos/core#inScheme> :BiomassScheme ;
                                                     <http://www.w3.org/2004/02/skos/core#definition> "Herbaceous biomass consisting of fruits from legume crops."@en ;
                                                     <http://www.w3.org/2004/02/skos/core#prefLabel> "2.1.5.3. Fruit"@en .


###  http://w3.id.org/def/BiomassOntology#2-1-5-4-Pods
<http://w3.id.org/def/BiomassOntology#2-1-5-4-Pods> rdf:type owl:NamedIndividual ,
                                                             <http://www.w3.org/2004/02/skos/core#Concept> ;
                                                    <http://www.w3.org/2004/02/skos/core#broader> <http://w3.id.org/def/BiomassOntology#2-1-5-LegumeCrops> ;
                                                    <http://www.w3.org/2004/02/skos/core#inScheme> :BiomassScheme ;
                                                    <http://www.w3.org/2004/02/skos/core#definition> "Herbaceous biomass consisting of pods from legume crops."@en ;
                                                    <http://www.w3.org/2004/02/skos/core#prefLabel> "2.1.5.4. Pods"@en .


###  http://w3.id.org/def/BiomassOntology#2-1-5-5-BlendsMixtures
<http://w3.id.org/def/BiomassOntology#2-1-5-5-BlendsMixtures> rdf:type owl:NamedIndividual ,
                                                                       <http://www.w3.org/2004/02/skos/core#Concept> ;
                                                              <http://www.w3.org/2004/02/skos/core#broader> <http://w3.id.org/def/BiomassOntology#2-1-5-LegumeCrops> ;
                                                              <http://www.w3.org/2004/02/skos/core#inScheme> :BiomassScheme ;
                                                              <http://www.w3.org/2004/02/skos/core#definition> "This refers to blends and mixtures of legume crops in the groups 2.1.5.1. to 2.1.5.4. The mixing can be either intentional (blends) or unintentional (mixtures)."@en ;
                                                              <http://www.w3.org/2004/02/skos/core#prefLabel> "2.1.5.5. Blends and mixtures"@en .


###  http://w3.id.org/def/BiomassOntology#2-1-6-Flowers
<http://w3.id.org/def/BiomassOntology#2-1-6-Flowers> rdf:type owl:NamedIndividual ,
                                                              <http://www.w3.org/2004/02/skos/core#Concept> ;
                                                     <http://www.w3.org/2004/02/skos/core#broader> <http://w3.id.org/def/BiomassOntology#2-1-AgricultureHorticulture> ;
                                                     <http://www.w3.org/2004/02/skos/core#inScheme> :BiomassScheme ;
                                                     <http://www.w3.org/2004/02/skos/core#definition> "Herbaceous biomass consisting of flowers."@en ;
                                                     <http://www.w3.org/2004/02/skos/core#prefLabel> "2.1.6. Flowers"@en .


###  http://w3.id.org/def/BiomassOntology#2-1-6-1-WholePlant
<http://w3.id.org/def/BiomassOntology#2-1-6-1-WholePlant> rdf:type owl:NamedIndividual ,
                                                                   <http://www.w3.org/2004/02/skos/core#Concept> ;
                                                          <http://www.w3.org/2004/02/skos/core#broader> <http://w3.id.org/def/BiomassOntology#2-1-6-Flowers> ;
                                                          <http://www.w3.org/2004/02/skos/core#inScheme> :BiomassScheme ;
                                                          <http://www.w3.org/2004/02/skos/core#definition> "Herbaceous biomass consisting of whole plants from flowers."@en ;
                                                          <http://www.w3.org/2004/02/skos/core#prefLabel> "2.1.6.1. Whole plant"@en .


###  http://w3.id.org/def/BiomassOntology#2-1-6-2-StalksLeaves
<http://w3.id.org/def/BiomassOntology#2-1-6-2-StalksLeaves> rdf:type owl:NamedIndividual ,
                                                                     <http://www.w3.org/2004/02/skos/core#Concept> ;
                                                            <http://www.w3.org/2004/02/skos/core#broader> <http://w3.id.org/def/BiomassOntology#2-1-6-Flowers> ;
                                                            <http://www.w3.org/2004/02/skos/core#inScheme> :BiomassScheme ;
                                                            <http://www.w3.org/2004/02/skos/core#definition> "Herbaceous biomass consisting of stalks and leaves from flowers."@en ;
                                                            <http://www.w3.org/2004/02/skos/core#prefLabel> "2.1.6.2. Stalks and leaves"@en .


###  http://w3.id.org/def/BiomassOntology#2-1-6-3-Seeds
<http://w3.id.org/def/BiomassOntology#2-1-6-3-Seeds> rdf:type owl:NamedIndividual ,
                                                              <http://www.w3.org/2004/02/skos/core#Concept> ;
                                                     <http://www.w3.org/2004/02/skos/core#broader> <http://w3.id.org/def/BiomassOntology#2-1-6-Flowers> ;
                                                     <http://www.w3.org/2004/02/skos/core#inScheme> :BiomassScheme ;
                                                     <http://www.w3.org/2004/02/skos/core#definition> "Herbaceous biomass consisting of seeds from flowers."@en ;
                                                     <http://www.w3.org/2004/02/skos/core#prefLabel> "2.1.6.3. Seeds"@en .


###  http://w3.id.org/def/BiomassOntology#2-1-6-4-BlendsMixtures
<http://w3.id.org/def/BiomassOntology#2-1-6-4-BlendsMixtures> rdf:type owl:NamedIndividual ,
                                                                       <http://www.w3.org/2004/02/skos/core#Concept> ;
                                                              <http://www.w3.org/2004/02/skos/core#broader> <http://w3.id.org/def/BiomassOntology#2-1-6-Flowers> ;
                                                              <http://www.w3.org/2004/02/skos/core#inScheme> :BiomassScheme ;
                                                              <http://www.w3.org/2004/02/skos/core#definition> "This refers to blends and mixtures of flowers in the groups 2.1.6.1. to 2.1.6.3. The mixing can be either intentional (blends) or unintentional (mixtures)."@en ;
                                                              <http://www.w3.org/2004/02/skos/core#prefLabel> "2.1.6.4. Blends and mixtures"@en .


###  http://w3.id.org/def/BiomassOntology#2-1-7-SegregatedHerbaceous
<http://w3.id.org/def/BiomassOntology#2-1-7-SegregatedHerbaceous> rdf:type owl:NamedIndividual ,
                                                                           <http://www.w3.org/2004/02/skos/core#Concept> ;
                                                                  <http://www.w3.org/2004/02/skos/core#broader> <http://w3.id.org/def/BiomassOntology#2-1-AgricultureHorticulture> ;
                                                                  <http://www.w3.org/2004/02/skos/core#inScheme> :BiomassScheme ;
                                                                  <http://www.w3.org/2004/02/skos/core#definition> "Herbaceous biomass consisting of segregated herbaceous biomass from gardens, parks, roadside maintenance, vineyards and fruit orchards."@en ;
                                                                  <http://www.w3.org/2004/02/skos/core#prefLabel> "2.1.7. Segregated herbaceous biomass from gardens, parks, roadside maintenance, vineyards and fruit orchards"@en .


###  http://w3.id.org/def/BiomassOntology#2-1-8-BlendsMixtures
<http://w3.id.org/def/BiomassOntology#2-1-8-BlendsMixtures> rdf:type owl:NamedIndividual ,
                                                                     <http://www.w3.org/2004/02/skos/core#Concept> ;
                                                            <http://www.w3.org/2004/02/skos/core#broader> <http://w3.id.org/def/BiomassOntology#2-1-AgricultureHorticulture> ;
                                                            <http://www.w3.org/2004/02/skos/core#inScheme> :BiomassScheme ;
                                                            <http://www.w3.org/2004/02/skos/core#definition> "This refers to blends and mixtures of herbaceous biomass in the groups 2.1.1 to 2.1.7. The mixing can be either intentional (blends) or unintentional (mixtures)."@en ;
                                                            <http://www.w3.org/2004/02/skos/core#prefLabel> "2.1.8. Blends and mixtures"@en .


###  http://w3.id.org/def/BiomassOntology#2-2-HerbaceousByProducts
<http://w3.id.org/def/BiomassOntology#2-2-HerbaceousByProducts> rdf:type owl:NamedIndividual ,
                                                                         <http://www.w3.org/2004/02/skos/core#Concept> ;
                                                                <http://www.w3.org/2004/02/skos/core#broader> <http://w3.id.org/def/BiomassOntology#2-HerbaceousBiomass> ;
                                                                <http://www.w3.org/2004/02/skos/core#inScheme> :BiomassScheme ;
                                                                <http://www.w3.org/2004/02/skos/core#definition> "This refers to any herbaceous biomass material that is left over after industrial handling and treatment. Examples are residues from the production of sugar from sugar beets, barley malt residues from beer production and raw vegetable residues from food processing industry."@en ;
                                                                <http://www.w3.org/2004/02/skos/core#prefLabel> "2.2. By-products and residues from food and herbaceous processing industry"@en .


###  http://w3.id.org/def/BiomassOntology#2-2-1-ChemicallyUntreated
<http://w3.id.org/def/BiomassOntology#2-2-1-ChemicallyUntreated> rdf:type owl:NamedIndividual ,
                                                                          <http://www.w3.org/2004/02/skos/core#Concept> ;
                                                                 <http://www.w3.org/2004/02/skos/core#broader> <http://w3.id.org/def/BiomassOntology#2-2-HerbaceousByProducts> ;
                                                                 <http://www.w3.org/2004/02/skos/core#inScheme> :BiomassScheme ;
                                                                 <http://www.w3.org/2004/02/skos/core#definition> "Herbaceous biomass consisting of chemically untreated by-products and residues from food and herbaceous processing industry."@en ;
                                                                 <http://www.w3.org/2004/02/skos/core#prefLabel> "2.2.1. Chemically untreated herbaceous residues"@en .


###  http://w3.id.org/def/BiomassOntology#2-2-1-1-CerealCropsGrasses
<http://w3.id.org/def/BiomassOntology#2-2-1-1-CerealCropsGrasses> rdf:type owl:NamedIndividual ,
                                                                           <http://www.w3.org/2004/02/skos/core#Concept> ;
                                                                  <http://www.w3.org/2004/02/skos/core#broader> <http://w3.id.org/def/BiomassOntology#2-2-1-ChemicallyUntreated> ;
                                                                  <http://www.w3.org/2004/02/skos/core#inScheme> :BiomassScheme ;
                                                                  <http://www.w3.org/2004/02/skos/core#definition> "Herbaceous biomass consisting of chemically untreated cereal crops and grasses."@en ;
                                                                  <http://www.w3.org/2004/02/skos/core#prefLabel> "2.2.1.1. Cereal crops and grasses"@en .


###  http://w3.id.org/def/BiomassOntology#2-2-1-2-OilSeedCrops
<http://w3.id.org/def/BiomassOntology#2-2-1-2-OilSeedCrops> rdf:type owl:NamedIndividual ,
                                                                     <http://www.w3.org/2004/02/skos/core#Concept> ;
                                                            <http://www.w3.org/2004/02/skos/core#broader> <http://w3.id.org/def/BiomassOntology#2-2-1-ChemicallyUntreated> ;
                                                            <http://www.w3.org/2004/02/skos/core#inScheme> :BiomassScheme ;
                                                            <http://www.w3.org/2004/02/skos/core#definition> "Herbaceous biomass consisting of chemically untreated oil seed crops."@en ;
                                                            <http://www.w3.org/2004/02/skos/core#prefLabel> "2.2.1.2. Oil seed crops"@en .


###  http://w3.id.org/def/BiomassOntology#2-2-1-3-RootCrops
<http://w3.id.org/def/BiomassOntology#2-2-1-3-RootCrops> rdf:type owl:NamedIndividual ,
                                                                  <http://www.w3.org/2004/02/skos/core#Concept> ;
                                                         <http://www.w3.org/2004/02/skos/core#broader> <http://w3.id.org/def/BiomassOntology#2-2-1-ChemicallyUntreated> ;
                                                         <http://www.w3.org/2004/02/skos/core#inScheme> :BiomassScheme ;
                                                         <http://www.w3.org/2004/02/skos/core#definition> "Herbaceous biomass consisting of chemically untreated root crops."@en ;
                                                         <http://www.w3.org/2004/02/skos/core#prefLabel> "2.2.1.3. Root crops"@en .


###  http://w3.id.org/def/BiomassOntology#2-2-1-4-LegumeCrops
<http://w3.id.org/def/BiomassOntology#2-2-1-4-LegumeCrops> rdf:type owl:NamedIndividual ,
                                                                    <http://www.w3.org/2004/02/skos/core#Concept> ;
                                                           <http://www.w3.org/2004/02/skos/core#broader> <http://w3.id.org/def/BiomassOntology#2-2-1-ChemicallyUntreated> ;
                                                           <http://www.w3.org/2004/02/skos/core#inScheme> :BiomassScheme ;
                                                           <http://www.w3.org/2004/02/skos/core#definition> "Herbaceous biomass consisting of chemically untreated legume crops."@en ;
                                                           <http://www.w3.org/2004/02/skos/core#prefLabel> "2.2.1.4. Legume crops"@en .


###  http://w3.id.org/def/BiomassOntology#2-2-1-5-Flowers
<http://w3.id.org/def/BiomassOntology#2-2-1-5-Flowers> rdf:type owl:NamedIndividual ,
                                                                <http://www.w3.org/2004/02/skos/core#Concept> ;
                                                       <http://www.w3.org/2004/02/skos/core#broader> <http://w3.id.org/def/BiomassOntology#2-2-1-ChemicallyUntreated> ;
                                                       <http://www.w3.org/2004/02/skos/core#inScheme> :BiomassScheme ;
                                                       <http://www.w3.org/2004/02/skos/core#definition> "Herbaceous biomass consisting of chemically untreated flowers."@en ;
                                                       <http://www.w3.org/2004/02/skos/core#prefLabel> "2.2.1.5. Flowers"@en .


###  http://w3.id.org/def/BiomassOntology#2-2-1-6-BlendsMixtures
<http://w3.id.org/def/BiomassOntology#2-2-1-6-BlendsMixtures> rdf:type owl:NamedIndividual ,
                                                                       <http://www.w3.org/2004/02/skos/core#Concept> ;
                                                              <http://www.w3.org/2004/02/skos/core#broader> <http://w3.id.org/def/BiomassOntology#2-2-1-ChemicallyUntreated> ;
                                                              <http://www.w3.org/2004/02/skos/core#inScheme> :BiomassScheme ;
                                                              <http://www.w3.org/2004/02/skos/core#definition> "This refers to blends and mixtures of herbaceous biomass in the groups 2.2.1. to 2.2.5. The mixing can be either intentional (blends) or unintentional (mixtures)."@en ;
                                                              <http://www.w3.org/2004/02/skos/core#prefLabel> "2.2.1.6. Blends and mixtures"@en .


###  http://w3.id.org/def/BiomassOntology#2-2-2-ChemicallyTreated
<http://w3.id.org/def/BiomassOntology#2-2-2-ChemicallyTreated> rdf:type owl:NamedIndividual ,
                                                                        <http://www.w3.org/2004/02/skos/core#Concept> ;
                                                               <http://www.w3.org/2004/02/skos/core#broader> <http://w3.id.org/def/BiomassOntology#2-2-HerbaceousByProducts> ;
                                                               <http://www.w3.org/2004/02/skos/core#inScheme> :BiomassScheme ;
                                                               <http://www.w3.org/2004/02/skos/core#definition> "Herbaceous biomass consisting of chemically treated by-products and residues from food and herbaceous processing industry."@en ;
                                                               <http://www.w3.org/2004/02/skos/core#prefLabel> "2.2.2. Chemically treated herbaceous residues"@en .


###  http://w3.id.org/def/BiomassOntology#2-2-2-1-CerealCropsGrasses
<http://w3.id.org/def/BiomassOntology#2-2-2-1-CerealCropsGrasses> rdf:type owl:NamedIndividual ,
                                                                           <http://www.w3.org/2004/02/skos/core#Concept> ;
                                                                  <http://www.w3.org/2004/02/skos/core#broader> <http://w3.id.org/def/BiomassOntology#2-2-2-ChemicallyTreated> ;
                                                                  <http://www.w3.org/2004/02/skos/core#inScheme> :BiomassScheme ;
                                                                  <http://www.w3.org/2004/02/skos/core#definition> "Herbaceous biomass consisting of chemically treated cereal crops and grasses."@en ;
                                                                  <http://www.w3.org/2004/02/skos/core#prefLabel> "2.2.2.1. Cereal crops and grasses"@en .


###  http://w3.id.org/def/BiomassOntology#2-2-2-2-OilSeedCrops
<http://w3.id.org/def/BiomassOntology#2-2-2-2-OilSeedCrops> rdf:type owl:NamedIndividual ,
                                                                     <http://www.w3.org/2004/02/skos/core#Concept> ;
                                                            <http://www.w3.org/2004/02/skos/core#broader> <http://w3.id.org/def/BiomassOntology#2-2-2-ChemicallyTreated> ;
                                                            <http://www.w3.org/2004/02/skos/core#inScheme> :BiomassScheme ;
                                                            <http://www.w3.org/2004/02/skos/core#definition> "Herbaceous biomass consisting of chemically treated oil seed crops."@en ;
                                                            <http://www.w3.org/2004/02/skos/core#prefLabel> "2.2.2.2. Oil seed crops"@en .


###  http://w3.id.org/def/BiomassOntology#2-2-2-3-RootCrops
<http://w3.id.org/def/BiomassOntology#2-2-2-3-RootCrops> rdf:type owl:NamedIndividual ,
                                                                  <http://www.w3.org/2004/02/skos/core#Concept> ;
                                                         <http://www.w3.org/2004/02/skos/core#broader> <http://w3.id.org/def/BiomassOntology#2-2-2-ChemicallyTreated> ;
                                                         <http://www.w3.org/2004/02/skos/core#inScheme> :BiomassScheme ;
                                                         <http://www.w3.org/2004/02/skos/core#definition> "Herbaceous biomass consisting of chemically treated root crops."@en ;
                                                         <http://www.w3.org/2004/02/skos/core#prefLabel> "2.2.2.3. Root crops"@en .


###  http://w3.id.org/def/BiomassOntology#2-2-2-4-Flowers
<http://w3.id.org/def/BiomassOntology#2-2-2-4-Flowers> rdf:type owl:NamedIndividual ,
                                                                <http://www.w3.org/2004/02/skos/core#Concept> ;
                                                       <http://www.w3.org/2004/02/skos/core#broader> <http://w3.id.org/def/BiomassOntology#2-2-2-ChemicallyTreated> ;
                                                       <http://www.w3.org/2004/02/skos/core#inScheme> :BiomassScheme ;
                                                       <http://www.w3.org/2004/02/skos/core#definition> "Herbaceous biomass consisting of chemically treated flowers."@en ;
                                                       <http://www.w3.org/2004/02/skos/core#prefLabel> "2.2.2.5. Flowers"@en .


###  http://w3.id.org/def/BiomassOntology#2-2-2-4-LegumeCrops
<http://w3.id.org/def/BiomassOntology#2-2-2-4-LegumeCrops> rdf:type owl:NamedIndividual ,
                                                                    <http://www.w3.org/2004/02/skos/core#Concept> ;
                                                           <http://www.w3.org/2004/02/skos/core#broader> <http://w3.id.org/def/BiomassOntology#2-2-2-ChemicallyTreated> ;
                                                           <http://www.w3.org/2004/02/skos/core#inScheme> :BiomassScheme ;
                                                           <http://www.w3.org/2004/02/skos/core#definition> "Herbaceous biomass consisting of chemically treated legume crops."@en ;
                                                           <http://www.w3.org/2004/02/skos/core#prefLabel> "2.2.2.4. Legume crops"@en .


###  http://w3.id.org/def/BiomassOntology#2-2-2-6-BlendsMixtures
<http://w3.id.org/def/BiomassOntology#2-2-2-6-BlendsMixtures> rdf:type owl:NamedIndividual ,
                                                                       <http://www.w3.org/2004/02/skos/core#Concept> ;
                                                              <http://www.w3.org/2004/02/skos/core#broader> <http://w3.id.org/def/BiomassOntology#2-2-2-ChemicallyTreated> ;
                                                              <http://www.w3.org/2004/02/skos/core#inScheme> :BiomassScheme ;
                                                              <http://www.w3.org/2004/02/skos/core#definition> "This refers to blends and mixtures of chemmically treated herbaceous by-products and residues in the groups 2.2.2.1. to 2.2.2.5. The mixing can be either intentional (blends) or unintentional (mixtures)."@en ;
                                                              <http://www.w3.org/2004/02/skos/core#prefLabel> "2.2.2.6. Blends and mixtures"@en .


###  http://w3.id.org/def/BiomassOntology#2-2-3-BlendsMixtures
<http://w3.id.org/def/BiomassOntology#2-2-3-BlendsMixtures> rdf:type owl:NamedIndividual ,
                                                                     <http://www.w3.org/2004/02/skos/core#Concept> ;
                                                            <http://www.w3.org/2004/02/skos/core#broader> <http://w3.id.org/def/BiomassOntology#2-2-HerbaceousByProducts> ;
                                                            <http://www.w3.org/2004/02/skos/core#inScheme> :BiomassScheme ;
                                                            <http://www.w3.org/2004/02/skos/core#definition> "This refers to blends and mixtures of herbaceous by-products and residues in the groups 2.2.1 to 2.2.2. The mixing can be either intentional (blends) or unintentional (mixtures)."@en ;
                                                            <http://www.w3.org/2004/02/skos/core#prefLabel> "2.2.3. Blends and mixtures"@en .


###  http://w3.id.org/def/BiomassOntology#2-3-BlendsMixtures
<http://w3.id.org/def/BiomassOntology#2-3-BlendsMixtures> rdf:type owl:NamedIndividual ,
                                                                   <http://www.w3.org/2004/02/skos/core#Concept> ;
                                                          <http://www.w3.org/2004/02/skos/core#broader> <http://w3.id.org/def/BiomassOntology#2-HerbaceousBiomass> ;
                                                          <http://www.w3.org/2004/02/skos/core#inScheme> :BiomassScheme ;
                                                          <http://www.w3.org/2004/02/skos/core#definition> "This refers to blends and mixtures of herbaceous biomass in the groups 2.1 to 2.2. The mixing can be either intentional (blends) or unintentional (mixtures)."@en ;
                                                          <http://www.w3.org/2004/02/skos/core#prefLabel> "2.3. Blends and mixtures"@en .


###  http://w3.id.org/def/BiomassOntology#3-FruitBiomass
<http://w3.id.org/def/BiomassOntology#3-FruitBiomass> rdf:type owl:NamedIndividual ,
                                                               <http://www.w3.org/2004/02/skos/core#Concept> ;
                                                      <http://www.w3.org/2004/02/skos/core#topConceptOf> :BiomassScheme ;
                                                      <http://www.w3.org/2004/02/skos/core#definition> "Biomass from those parts of a plant which are from or hold seeds."@en ;
                                                      <http://www.w3.org/2004/02/skos/core#prefLabel> "3. Fruit biomass"@en .


###  http://w3.id.org/def/BiomassOntology#3-1-OrchardHorticultureFruit
<http://w3.id.org/def/BiomassOntology#3-1-OrchardHorticultureFruit> rdf:type owl:NamedIndividual ,
                                                                             <http://www.w3.org/2004/02/skos/core#Concept> ;
                                                                    <http://www.w3.org/2004/02/skos/core#broader> <http://w3.id.org/def/BiomassOntology#3-FruitBiomass> ;
                                                                    <http://www.w3.org/2004/02/skos/core#inScheme> :BiomassScheme ;
                                                                    <http://www.w3.org/2004/02/skos/core#definition> "Fruit from trees, bushes and fruit from herbs (e.g. tomatoes and grapes) are classified in this group."@en ;
                                                                    <http://www.w3.org/2004/02/skos/core#prefLabel> "3.1. Orchard and horticulture fruit"@en .


###  http://w3.id.org/def/BiomassOntology#3-1-1-Berries
<http://w3.id.org/def/BiomassOntology#3-1-1-Berries> rdf:type owl:NamedIndividual ,
                                                              <http://www.w3.org/2004/02/skos/core#Concept> ;
                                                     <http://www.w3.org/2004/02/skos/core#broader> <http://w3.id.org/def/BiomassOntology#3-1-OrchardHorticultureFruit> ;
                                                     <http://www.w3.org/2004/02/skos/core#inScheme> :BiomassScheme ;
                                                     <http://www.w3.org/2004/02/skos/core#definition> "Fruit biomass consisting of berries from orchards and horticulture."@en ;
                                                     <http://www.w3.org/2004/02/skos/core#prefLabel> "3.1.1. Berries"@en .


###  http://w3.id.org/def/BiomassOntology#3-1-1-1-WholeBerries
<http://w3.id.org/def/BiomassOntology#3-1-1-1-WholeBerries> rdf:type owl:NamedIndividual ,
                                                                     <http://www.w3.org/2004/02/skos/core#Concept> ;
                                                            <http://www.w3.org/2004/02/skos/core#broader> <http://w3.id.org/def/BiomassOntology#3-1-1-Berries> ;
                                                            <http://www.w3.org/2004/02/skos/core#inScheme> :BiomassScheme ;
                                                            <http://www.w3.org/2004/02/skos/core#definition> "Fruit biomass consisting of whole berries from orchards and horticulture."@en ;
                                                            <http://www.w3.org/2004/02/skos/core#prefLabel> "3.1.1.1. Whole berries"@en .


###  http://w3.id.org/def/BiomassOntology#3-1-1-2-Flesh
<http://w3.id.org/def/BiomassOntology#3-1-1-2-Flesh> rdf:type owl:NamedIndividual ,
                                                              <http://www.w3.org/2004/02/skos/core#Concept> ;
                                                     <http://www.w3.org/2004/02/skos/core#broader> <http://w3.id.org/def/BiomassOntology#3-1-1-Berries> ;
                                                     <http://www.w3.org/2004/02/skos/core#inScheme> :BiomassScheme ;
                                                     <http://www.w3.org/2004/02/skos/core#definition> "Fruit biomass consisting of flesh of berries from orchards and horticulture."@en ;
                                                     <http://www.w3.org/2004/02/skos/core#prefLabel> "3.1.1.2. Flesh"@en .


###  http://w3.id.org/def/BiomassOntology#3-1-1-3-Seeds
<http://w3.id.org/def/BiomassOntology#3-1-1-3-Seeds> rdf:type owl:NamedIndividual ,
                                                              <http://www.w3.org/2004/02/skos/core#Concept> ;
                                                     <http://www.w3.org/2004/02/skos/core#broader> <http://w3.id.org/def/BiomassOntology#3-1-1-Berries> ;
                                                     <http://www.w3.org/2004/02/skos/core#inScheme> :BiomassScheme ;
                                                     <http://www.w3.org/2004/02/skos/core#definition> "Fruit biomass consisting of seeds of berries from orchards and horticulture."@en ;
                                                     <http://www.w3.org/2004/02/skos/core#prefLabel> "3.1.1.3. Seeds"@en .


###  http://w3.id.org/def/BiomassOntology#3-1-1-4-BlendsMixtures
<http://w3.id.org/def/BiomassOntology#3-1-1-4-BlendsMixtures> rdf:type owl:NamedIndividual ,
                                                                       <http://www.w3.org/2004/02/skos/core#Concept> ;
                                                              <http://www.w3.org/2004/02/skos/core#broader> <http://w3.id.org/def/BiomassOntology#3-1-1-Berries> ;
                                                              <http://www.w3.org/2004/02/skos/core#inScheme> :BiomassScheme ;
                                                              <http://www.w3.org/2004/02/skos/core#definition> "This refers to blends and mixtures of berries from orchards and horticulture in the groups 3.1.1.1. to 3.1.1.3. The mixing can be either intentional (blends) or unintentional (mixtures)."@en ;
                                                              <http://www.w3.org/2004/02/skos/core#prefLabel> "3.1.1.4. Blends and mixtures"@en .


###  http://w3.id.org/def/BiomassOntology#3-1-2-StoneKernelFruits
<http://w3.id.org/def/BiomassOntology#3-1-2-StoneKernelFruits> rdf:type owl:NamedIndividual ,
                                                                        <http://www.w3.org/2004/02/skos/core#Concept> ;
                                                               <http://www.w3.org/2004/02/skos/core#broader> <http://w3.id.org/def/BiomassOntology#3-1-OrchardHorticultureFruit> ;
                                                               <http://www.w3.org/2004/02/skos/core#inScheme> :BiomassScheme ;
                                                               <http://www.w3.org/2004/02/skos/core#definition> "Fruit biomass consisting of stone/kernel fruits from orchards and horticulture."@en ;
                                                               <http://www.w3.org/2004/02/skos/core#prefLabel> "3.1.2. Stone/kernel fruits"@en .


###  http://w3.id.org/def/BiomassOntology#3-1-2-1-WholeFruit
<http://w3.id.org/def/BiomassOntology#3-1-2-1-WholeFruit> rdf:type owl:NamedIndividual ,
                                                                   <http://www.w3.org/2004/02/skos/core#Concept> ;
                                                          <http://www.w3.org/2004/02/skos/core#broader> <http://w3.id.org/def/BiomassOntology#3-1-2-StoneKernelFruits> ;
                                                          <http://www.w3.org/2004/02/skos/core#inScheme> :BiomassScheme ;
                                                          <http://www.w3.org/2004/02/skos/core#definition> "Fruit biomass consisting of whole stone/kernel fruits from orchards and horticulture."@en ;
                                                          <http://www.w3.org/2004/02/skos/core#prefLabel> "3.1.2.1. Whole fruit"@en .


###  http://w3.id.org/def/BiomassOntology#3-1-2-2-Flesh
<http://w3.id.org/def/BiomassOntology#3-1-2-2-Flesh> rdf:type owl:NamedIndividual ,
                                                              <http://www.w3.org/2004/02/skos/core#Concept> ;
                                                     <http://www.w3.org/2004/02/skos/core#broader> <http://w3.id.org/def/BiomassOntology#3-1-2-StoneKernelFruits> ;
                                                     <http://www.w3.org/2004/02/skos/core#inScheme> :BiomassScheme ;
                                                     <http://www.w3.org/2004/02/skos/core#definition> "Fruit biomass consisting of flesh of stone/kernel fruits from orchards and horticulture."@en ;
                                                     <http://www.w3.org/2004/02/skos/core#prefLabel> "3.1.2.2. Flesh"@en .


###  http://w3.id.org/def/BiomassOntology#3-1-2-3-StoneKernelFibre
<http://w3.id.org/def/BiomassOntology#3-1-2-3-StoneKernelFibre> rdf:type owl:NamedIndividual ,
                                                                         <http://www.w3.org/2004/02/skos/core#Concept> ;
                                                                <http://www.w3.org/2004/02/skos/core#broader> <http://w3.id.org/def/BiomassOntology#3-1-2-StoneKernelFruits> ;
                                                                <http://www.w3.org/2004/02/skos/core#inScheme> :BiomassScheme ;
                                                                <http://www.w3.org/2004/02/skos/core#definition> "Fruit biomass consisting of stones/kernels/fruit fibres of stone/kernel fruits from orchards and horticulture."@en ;
                                                                <http://www.w3.org/2004/02/skos/core#prefLabel> "3.1.2.3. Stone/kernel/fruit fibre"@en .


###  http://w3.id.org/def/BiomassOntology#3-1-2-4-BlendsMixtures
<http://w3.id.org/def/BiomassOntology#3-1-2-4-BlendsMixtures> rdf:type owl:NamedIndividual ,
                                                                       <http://www.w3.org/2004/02/skos/core#Concept> ;
                                                              <http://www.w3.org/2004/02/skos/core#broader> <http://w3.id.org/def/BiomassOntology#3-1-2-StoneKernelFruits> ;
                                                              <http://www.w3.org/2004/02/skos/core#inScheme> :BiomassScheme ;
                                                              <http://www.w3.org/2004/02/skos/core#definition> "This refers to blends and mixtures of stone/kernel fruits from orchards and horticulture in the groups 3.1.2.1. to 3.1.2.3. The mixing can be either intentional (blends) or unintentional (mixtures)."@en ;
                                                              <http://www.w3.org/2004/02/skos/core#prefLabel> "3.1.2.4. Blends and mixtures"@en .


###  http://w3.id.org/def/BiomassOntology#3-1-3-NutsAcorns
<http://w3.id.org/def/BiomassOntology#3-1-3-NutsAcorns> rdf:type owl:NamedIndividual ,
                                                                 <http://www.w3.org/2004/02/skos/core#Concept> ;
                                                        <http://www.w3.org/2004/02/skos/core#broader> <http://w3.id.org/def/BiomassOntology#3-1-OrchardHorticultureFruit> ;
                                                        <http://www.w3.org/2004/02/skos/core#inScheme> :BiomassScheme ;
                                                        <http://www.w3.org/2004/02/skos/core#definition> "Fruit biomass consisting of nuts and acorns from orchards and horticulture."@en ;
                                                        <http://www.w3.org/2004/02/skos/core#prefLabel> "3.1.3. Nuts and acorns"@en .


###  http://w3.id.org/def/BiomassOntology#3-1-3-1-WholeNuts
<http://w3.id.org/def/BiomassOntology#3-1-3-1-WholeNuts> rdf:type owl:NamedIndividual ,
                                                                  <http://www.w3.org/2004/02/skos/core#Concept> ;
                                                         <http://www.w3.org/2004/02/skos/core#broader> <http://w3.id.org/def/BiomassOntology#3-1-3-NutsAcorns> ;
                                                         <http://www.w3.org/2004/02/skos/core#inScheme> :BiomassScheme ;
                                                         <http://www.w3.org/2004/02/skos/core#definition> "Fruit biomass consisting of whole nuts and acorns from orchards and horticulture."@en ;
                                                         <http://www.w3.org/2004/02/skos/core#prefLabel> "3.1.3.1. Whole nuts"@en .


###  http://w3.id.org/def/BiomassOntology#3-1-3-2-ShellsHusks
<http://w3.id.org/def/BiomassOntology#3-1-3-2-ShellsHusks> rdf:type owl:NamedIndividual ,
                                                                    <http://www.w3.org/2004/02/skos/core#Concept> ;
                                                           <http://www.w3.org/2004/02/skos/core#broader> <http://w3.id.org/def/BiomassOntology#3-1-3-NutsAcorns> ;
                                                           <http://www.w3.org/2004/02/skos/core#inScheme> :BiomassScheme ;
                                                           <http://www.w3.org/2004/02/skos/core#definition> "Fruit biomass consisting of shells and husks of nuts and acorns from orchards and horticulture."@en ;
                                                           <http://www.w3.org/2004/02/skos/core#prefLabel> "3.1.3.2. Shells/husks"@en .


###  http://w3.id.org/def/BiomassOntology#3-1-3-3-Kernels
<http://w3.id.org/def/BiomassOntology#3-1-3-3-Kernels> rdf:type owl:NamedIndividual ,
                                                                <http://www.w3.org/2004/02/skos/core#Concept> ;
                                                       <http://www.w3.org/2004/02/skos/core#broader> <http://w3.id.org/def/BiomassOntology#3-1-3-NutsAcorns> ;
                                                       <http://www.w3.org/2004/02/skos/core#inScheme> :BiomassScheme ;
                                                       <http://www.w3.org/2004/02/skos/core#prefLabel> "3.1.3.3. Kernels"@en ,
                                                                                                       "Fruit biomass consisting of kernels of nuts and acorns from orchards and horticulture."@en .


###  http://w3.id.org/def/BiomassOntology#3-1-3-4-BlendsMixtures
<http://w3.id.org/def/BiomassOntology#3-1-3-4-BlendsMixtures> rdf:type owl:NamedIndividual ,
                                                                       <http://www.w3.org/2004/02/skos/core#Concept> ;
                                                              <http://www.w3.org/2004/02/skos/core#broader> <http://w3.id.org/def/BiomassOntology#3-1-3-NutsAcorns> ;
                                                              <http://www.w3.org/2004/02/skos/core#inScheme> :BiomassScheme ;
                                                              <http://www.w3.org/2004/02/skos/core#definition> "This refers to blends and mixtures of nuts and acorns from orchards and horticulture in the groups 3.1.3.1. to 3.1.3.3. The mixing can be either intentional (blends) or unintentional (mixtures)."@en ;
                                                              <http://www.w3.org/2004/02/skos/core#prefLabel> "3.1.3.4. Blends and mixtures"@en .


###  http://w3.id.org/def/BiomassOntology#3-1-4-BlendsMixtures
<http://w3.id.org/def/BiomassOntology#3-1-4-BlendsMixtures> rdf:type owl:NamedIndividual ,
                                                                     <http://www.w3.org/2004/02/skos/core#Concept> ;
                                                            <http://www.w3.org/2004/02/skos/core#broader> <http://w3.id.org/def/BiomassOntology#3-1-OrchardHorticultureFruit> ;
                                                            <http://www.w3.org/2004/02/skos/core#inScheme> :BiomassScheme ;
                                                            <http://www.w3.org/2004/02/skos/core#definition> "This refers to blends and mixtures of orchards and horticulture fruits in the groups 3.1.1 to 3.1.3. The mixing can be either intentional (blends) or unintentional (mixtures)."@en ;
                                                            <http://www.w3.org/2004/02/skos/core#prefLabel> "3.1.4. Blends and mixtures"@en .


###  http://w3.id.org/def/BiomassOntology#3-2-FruitByProducts
<http://w3.id.org/def/BiomassOntology#3-2-FruitByProducts> rdf:type owl:NamedIndividual ,
                                                                    <http://www.w3.org/2004/02/skos/core#Concept> ;
                                                           <http://www.w3.org/2004/02/skos/core#broader> <http://w3.id.org/def/BiomassOntology#3-FruitBiomass> ;
                                                           <http://www.w3.org/2004/02/skos/core#inScheme> :BiomassScheme ;
                                                           <http://www.w3.org/2004/02/skos/core#definition> "This refers to a fruit biomass material that is left over after industrial handling and treatment. Examples are pressing residues from olive oil or apple juice production and processed (e.g. heated, steamed, cooked, etc.) vegetable residues from food processing industry."@en ;
                                                           <http://www.w3.org/2004/02/skos/core#prefLabel> "3.2. By-products and residues from food and fruit processing industry"@en .


###  http://w3.id.org/def/BiomassOntology#3-2-1-ChemicallyUntreated
<http://w3.id.org/def/BiomassOntology#3-2-1-ChemicallyUntreated> rdf:type owl:NamedIndividual ,
                                                                          <http://www.w3.org/2004/02/skos/core#Concept> ;
                                                                 <http://www.w3.org/2004/02/skos/core#broader> <http://w3.id.org/def/BiomassOntology#3-2-FruitByProducts> ;
                                                                 <http://www.w3.org/2004/02/skos/core#inScheme> :BiomassScheme ;
                                                                 <http://www.w3.org/2004/02/skos/core#definition> "Fruit biomass consisting of chemically untreated by-products and residues from food and fruit processing industry."@en ;
                                                                 <http://www.w3.org/2004/02/skos/core#prefLabel> "3.2.1. Chemically untreated fruit residues"@en .


###  http://w3.id.org/def/BiomassOntology#3-2-1-1-Berries
<http://w3.id.org/def/BiomassOntology#3-2-1-1-Berries> rdf:type owl:NamedIndividual ,
                                                                <http://www.w3.org/2004/02/skos/core#Concept> ;
                                                       <http://www.w3.org/2004/02/skos/core#broader> <http://w3.id.org/def/BiomassOntology#3-2-1-ChemicallyUntreated> ;
                                                       <http://www.w3.org/2004/02/skos/core#inScheme> :BiomassScheme ;
                                                       <http://www.w3.org/2004/02/skos/core#definition> "Fruit biomass consisting of chemically untreated berries."@en ;
                                                       <http://www.w3.org/2004/02/skos/core#prefLabel> "3.2.1.1. Berries"@en .


###  http://w3.id.org/def/BiomassOntology#3-2-1-2-StoneKernelFibre
<http://w3.id.org/def/BiomassOntology#3-2-1-2-StoneKernelFibre> rdf:type owl:NamedIndividual ,
                                                                         <http://www.w3.org/2004/02/skos/core#Concept> ;
                                                                <http://www.w3.org/2004/02/skos/core#broader> <http://w3.id.org/def/BiomassOntology#3-2-1-ChemicallyUntreated> ;
                                                                <http://www.w3.org/2004/02/skos/core#inScheme> :BiomassScheme ;
                                                                <http://www.w3.org/2004/02/skos/core#definition> "Fruit biomass consisting of chemically untreated stone/kernel fruits and fruit fibre."@en ;
                                                                <http://www.w3.org/2004/02/skos/core#prefLabel> "3.2.1.2. Stone/kernel fruits/fruit fibre"@en .


###  http://w3.id.org/def/BiomassOntology#3-2-1-3-NutsAcorns
<http://w3.id.org/def/BiomassOntology#3-2-1-3-NutsAcorns> rdf:type owl:NamedIndividual ,
                                                                   <http://www.w3.org/2004/02/skos/core#Concept> ;
                                                          <http://www.w3.org/2004/02/skos/core#broader> <http://w3.id.org/def/BiomassOntology#3-2-1-ChemicallyUntreated> ;
                                                          <http://www.w3.org/2004/02/skos/core#inScheme> :BiomassScheme ;
                                                          <http://www.w3.org/2004/02/skos/core#definition> "Fruit biomass consisting of chemically untreated nuts and acorns."@en ;
                                                          <http://www.w3.org/2004/02/skos/core#prefLabel> "3.2.1.3. Nuts and acorns"@en .


###  http://w3.id.org/def/BiomassOntology#3-2-1-4-CrudeOliveCake
<http://w3.id.org/def/BiomassOntology#3-2-1-4-CrudeOliveCake> rdf:type owl:NamedIndividual ,
                                                                       <http://www.w3.org/2004/02/skos/core#Concept> ;
                                                              <http://www.w3.org/2004/02/skos/core#broader> <http://w3.id.org/def/BiomassOntology#3-2-1-ChemicallyUntreated> ;
                                                              <http://www.w3.org/2004/02/skos/core#inScheme> :BiomassScheme ;
                                                              <http://www.w3.org/2004/02/skos/core#definition> "Fruit biomass consisting of chemically untreated crude olive cake."@en ;
                                                              <http://www.w3.org/2004/02/skos/core#prefLabel> "3.2.1.4. Crude olive cake"@en .


###  http://w3.id.org/def/BiomassOntology#3-2-1-5-BlendsMixtures
<http://w3.id.org/def/BiomassOntology#3-2-1-5-BlendsMixtures> rdf:type owl:NamedIndividual ,
                                                                       <http://www.w3.org/2004/02/skos/core#Concept> ;
                                                              <http://www.w3.org/2004/02/skos/core#broader> <http://w3.id.org/def/BiomassOntology#3-2-1-ChemicallyUntreated> ;
                                                              <http://www.w3.org/2004/02/skos/core#inScheme> :BiomassScheme ;
                                                              <http://www.w3.org/2004/02/skos/core#definition> "This refers to blends and mixtures of chemically untreated fruit residues in the groups 3.2.1.1. to 3.2.1.4. The mixing can be either intentional (blends) or unintentional (mixtures)."@en ;
                                                              <http://www.w3.org/2004/02/skos/core#prefLabel> "3.2.1.5. Blends and mixtures"@en .


###  http://w3.id.org/def/BiomassOntology#3-2-2-ChemicallyTreated
<http://w3.id.org/def/BiomassOntology#3-2-2-ChemicallyTreated> rdf:type owl:NamedIndividual ,
                                                                        <http://www.w3.org/2004/02/skos/core#Concept> ;
                                                               <http://www.w3.org/2004/02/skos/core#broader> <http://w3.id.org/def/BiomassOntology#3-2-FruitByProducts> ;
                                                               <http://www.w3.org/2004/02/skos/core#inScheme> :BiomassScheme ;
                                                               <http://www.w3.org/2004/02/skos/core#definition> "Fruit biomass consisting of chemically treated by-products and residues from food and fruit processing industry."@en ;
                                                               <http://www.w3.org/2004/02/skos/core#prefLabel> "3.2.2. Chemically treated fruit residues"@en .


###  http://w3.id.org/def/BiomassOntology#3-2-2-1-Berries
<http://w3.id.org/def/BiomassOntology#3-2-2-1-Berries> rdf:type owl:NamedIndividual ,
                                                                <http://www.w3.org/2004/02/skos/core#Concept> ;
                                                       <http://www.w3.org/2004/02/skos/core#broader> <http://w3.id.org/def/BiomassOntology#3-2-2-ChemicallyTreated> ;
                                                       <http://www.w3.org/2004/02/skos/core#inScheme> :BiomassScheme ;
                                                       <http://www.w3.org/2004/02/skos/core#definition> "Fruit biomass consisting of chemically treated berries."@en ;
                                                       <http://www.w3.org/2004/02/skos/core#prefLabel> "3.2.2.1. Berries"@en .


###  http://w3.id.org/def/BiomassOntology#3-2-2-2-StoneKernel
<http://w3.id.org/def/BiomassOntology#3-2-2-2-StoneKernel> rdf:type owl:NamedIndividual ,
                                                                    <http://www.w3.org/2004/02/skos/core#Concept> ;
                                                           <http://www.w3.org/2004/02/skos/core#broader> <http://w3.id.org/def/BiomassOntology#3-2-2-ChemicallyTreated> ;
                                                           <http://www.w3.org/2004/02/skos/core#inScheme> :BiomassScheme ;
                                                           <http://www.w3.org/2004/02/skos/core#definition> "Fruit biomass consisting of chemically treated stone/kernel fruits."@en ;
                                                           <http://www.w3.org/2004/02/skos/core#prefLabel> "3.2.2.2. Stone/kernel fruits"@en .


###  http://w3.id.org/def/BiomassOntology#3-2-2-3-NutsAcorns
<http://w3.id.org/def/BiomassOntology#3-2-2-3-NutsAcorns> rdf:type owl:NamedIndividual ,
                                                                   <http://www.w3.org/2004/02/skos/core#Concept> ;
                                                          <http://www.w3.org/2004/02/skos/core#broader> <http://w3.id.org/def/BiomassOntology#3-2-2-ChemicallyTreated> ;
                                                          <http://www.w3.org/2004/02/skos/core#inScheme> :BiomassScheme ;
                                                          <http://www.w3.org/2004/02/skos/core#definition> "Fruit biomass consisting of chemically treated nuts and acorns."@en ;
                                                          <http://www.w3.org/2004/02/skos/core#prefLabel> "3.2.2.3. Nuts and acorns"@en .


###  http://w3.id.org/def/BiomassOntology#3-2-2-4-ExhaustedOliveCake
<http://w3.id.org/def/BiomassOntology#3-2-2-4-ExhaustedOliveCake> rdf:type owl:NamedIndividual ,
                                                                           <http://www.w3.org/2004/02/skos/core#Concept> ;
                                                                  <http://www.w3.org/2004/02/skos/core#broader> <http://w3.id.org/def/BiomassOntology#3-2-2-ChemicallyTreated> ;
                                                                  <http://www.w3.org/2004/02/skos/core#inScheme> :BiomassScheme ;
                                                                  <http://www.w3.org/2004/02/skos/core#definition> "Fruit biomass consisting of chemically treated exhausted olive cake."@en ;
                                                                  <http://www.w3.org/2004/02/skos/core#prefLabel> "3.2.2.4. Exhausted olive cake"@en .


###  http://w3.id.org/def/BiomassOntology#3-2-2-5-BlendsMixtures
<http://w3.id.org/def/BiomassOntology#3-2-2-5-BlendsMixtures> rdf:type owl:NamedIndividual ,
                                                                       <http://www.w3.org/2004/02/skos/core#Concept> ;
                                                              <http://www.w3.org/2004/02/skos/core#broader> <http://w3.id.org/def/BiomassOntology#3-2-2-ChemicallyTreated> ;
                                                              <http://www.w3.org/2004/02/skos/core#inScheme> :BiomassScheme ;
                                                              <http://www.w3.org/2004/02/skos/core#definition> "This refers to blends and mixtures of chemically treated fruit residues in the groups 3.2.2.1. to 3.2.2.4. The mixing can be either intentional (blends) or unintentional (mixtures)."@en ;
                                                              <http://www.w3.org/2004/02/skos/core#prefLabel> "3.2.2.5. Blends and mixtures"@en .


###  http://w3.id.org/def/BiomassOntology#3-2-3-BlendsMixtures
<http://w3.id.org/def/BiomassOntology#3-2-3-BlendsMixtures> rdf:type owl:NamedIndividual ,
                                                                     <http://www.w3.org/2004/02/skos/core#Concept> ;
                                                            <http://www.w3.org/2004/02/skos/core#broader> <http://w3.id.org/def/BiomassOntology#3-2-FruitByProducts> ;
                                                            <http://www.w3.org/2004/02/skos/core#inScheme> :BiomassScheme ;
                                                            <http://www.w3.org/2004/02/skos/core#definition> "This refers to blends and mixtures of fruit by-products and residues in the groups 3.2.1 to 3.2.2. The mixing can be either intentional (blends) or unintentional (mixtures)."@en ;
                                                            <http://www.w3.org/2004/02/skos/core#prefLabel> "3.2.3. Blends and mixtures"@en .


###  http://w3.id.org/def/BiomassOntology#3-3-BlendsMixtures
<http://w3.id.org/def/BiomassOntology#3-3-BlendsMixtures> rdf:type owl:NamedIndividual ,
                                                                   <http://www.w3.org/2004/02/skos/core#Concept> ;
                                                          <http://www.w3.org/2004/02/skos/core#broader> <http://w3.id.org/def/BiomassOntology#3-FruitBiomass> ;
                                                          <http://www.w3.org/2004/02/skos/core#inScheme> :BiomassScheme ;
                                                          <http://www.w3.org/2004/02/skos/core#definition> "This refers to blends and mixtures of fruit biomass in the groups 3.1 to 3.2. The mixing can be either intentional (blends) or unintentional (mixtures)."@en ;
                                                          <http://www.w3.org/2004/02/skos/core#prefLabel> "3.3. Blends and mixtures"@en .


###  http://w3.id.org/def/BiomassOntology#4-AquaticBiomass
<http://w3.id.org/def/BiomassOntology#4-AquaticBiomass> rdf:type owl:NamedIndividual ,
                                                                 <http://www.w3.org/2004/02/skos/core#Concept> ;
                                                        <http://www.w3.org/2004/02/skos/core#topConceptOf> :BiomassScheme ;
                                                        <http://www.w3.org/2004/02/skos/core#definition> "Biomass from so called hydrophytic plants or hydrophytes, which are plants that have adapted to living in or on aquatic environments."@en ;
                                                        <http://www.w3.org/2004/02/skos/core#prefLabel> "4. Aquatic biomass"@en .


###  http://w3.id.org/def/BiomassOntology#4-1-Algae
<http://w3.id.org/def/BiomassOntology#4-1-Algae> rdf:type owl:NamedIndividual ,
                                                          <http://www.w3.org/2004/02/skos/core#Concept> ;
                                                 <http://www.w3.org/2004/02/skos/core#broader> <http://w3.id.org/def/BiomassOntology#4-AquaticBiomass> ;
                                                 <http://www.w3.org/2004/02/skos/core#inScheme> :BiomassScheme ;
                                                 <http://www.w3.org/2004/02/skos/core#definition> "Aquatic biomass consisting of algae."@en ;
                                                 <http://www.w3.org/2004/02/skos/core#prefLabel> "4.1. Algae"@en .


###  http://w3.id.org/def/BiomassOntology#4-1-1-MicroAlgae
<http://w3.id.org/def/BiomassOntology#4-1-1-MicroAlgae> rdf:type owl:NamedIndividual ,
                                                                 <http://www.w3.org/2004/02/skos/core#Concept> ;
                                                        <http://www.w3.org/2004/02/skos/core#broader> <http://w3.id.org/def/BiomassOntology#4-1-Algae> ;
                                                        <http://www.w3.org/2004/02/skos/core#inScheme> :BiomassScheme ;
                                                        <http://www.w3.org/2004/02/skos/core#definition> "Aquatic biomass consisting of micro algae."@en ;
                                                        <http://www.w3.org/2004/02/skos/core#prefLabel> "4.1.1. Micro algae (Latin name to be stated)"@en .


###  http://w3.id.org/def/BiomassOntology#4-1-2-MacroAlgae
<http://w3.id.org/def/BiomassOntology#4-1-2-MacroAlgae> rdf:type owl:NamedIndividual ,
                                                                 <http://www.w3.org/2004/02/skos/core#Concept> ;
                                                        <http://www.w3.org/2004/02/skos/core#broader> <http://w3.id.org/def/BiomassOntology#4-1-Algae> ;
                                                        <http://www.w3.org/2004/02/skos/core#inScheme> :BiomassScheme ;
                                                        <http://www.w3.org/2004/02/skos/core#definition> "Aquatic biomass consisting of macro algae."@en ;
                                                        <http://www.w3.org/2004/02/skos/core#prefLabel> "4.1.2. Macro algae (Latin name to be stated)"@en .


###  http://w3.id.org/def/BiomassOntology#4-1-2-1-GreenSeaWeed
<http://w3.id.org/def/BiomassOntology#4-1-2-1-GreenSeaWeed> rdf:type owl:NamedIndividual ,
                                                                     <http://www.w3.org/2004/02/skos/core#Concept> ;
                                                            <http://www.w3.org/2004/02/skos/core#broader> <http://w3.id.org/def/BiomassOntology#4-1-2-MacroAlgae> ;
                                                            <http://www.w3.org/2004/02/skos/core#inScheme> :BiomassScheme ;
                                                            <http://www.w3.org/2004/02/skos/core#definition> "Aquatic biomass consisting of green sea weed."@en ;
                                                            <http://www.w3.org/2004/02/skos/core#prefLabel> "4.1.2.1. Green sea weed (Latin name to be stated)"@en .


###  http://w3.id.org/def/BiomassOntology#4-1-2-2-BrownSeaWeed
<http://w3.id.org/def/BiomassOntology#4-1-2-2-BrownSeaWeed> rdf:type owl:NamedIndividual ,
                                                                     <http://www.w3.org/2004/02/skos/core#Concept> ;
                                                            <http://www.w3.org/2004/02/skos/core#broader> <http://w3.id.org/def/BiomassOntology#4-1-2-MacroAlgae> ;
                                                            <http://www.w3.org/2004/02/skos/core#inScheme> :BiomassScheme ;
                                                            <http://www.w3.org/2004/02/skos/core#definition> "Aquatic biomass consisting of brown sea weed."@en ;
                                                            <http://www.w3.org/2004/02/skos/core#prefLabel> "4.1.2.2. Brown sea weed (Latin name to be sated)"@en .


###  http://w3.id.org/def/BiomassOntology#4-1-2-3-RedSeaWeed
<http://w3.id.org/def/BiomassOntology#4-1-2-3-RedSeaWeed> rdf:type owl:NamedIndividual ,
                                                                   <http://www.w3.org/2004/02/skos/core#Concept> ;
                                                          <http://www.w3.org/2004/02/skos/core#broader> <http://w3.id.org/def/BiomassOntology#4-1-2-MacroAlgae> ;
                                                          <http://www.w3.org/2004/02/skos/core#inScheme> :BiomassScheme ;
                                                          <http://www.w3.org/2004/02/skos/core#definition> "Aquatic biomass consisting of red sea weed."@en ;
                                                          <http://www.w3.org/2004/02/skos/core#prefLabel> "4.1.2.3. Red sea weed (Latin name to be stated)"@en .


###  http://w3.id.org/def/BiomassOntology#4-1-3-BlendsMixtures
<http://w3.id.org/def/BiomassOntology#4-1-3-BlendsMixtures> rdf:type owl:NamedIndividual ,
                                                                     <http://www.w3.org/2004/02/skos/core#Concept> ;
                                                            <http://www.w3.org/2004/02/skos/core#broader> <http://w3.id.org/def/BiomassOntology#4-1-Algae> ;
                                                            <http://www.w3.org/2004/02/skos/core#inScheme> :BiomassScheme ;
                                                            <http://www.w3.org/2004/02/skos/core#definition> "This refers to blends and mixtures of algae in the groups4.1.1 to 4.1.2. The mixing can be either intentional (blends) or unintentional (mixtures)."@en ;
                                                            <http://www.w3.org/2004/02/skos/core#prefLabel> "4.1.3. Blends and mixtures"@en .


###  http://w3.id.org/def/BiomassOntology#4-2-WaterHyacinth
<http://w3.id.org/def/BiomassOntology#4-2-WaterHyacinth> rdf:type owl:NamedIndividual ,
                                                                  <http://www.w3.org/2004/02/skos/core#Concept> ;
                                                         <http://www.w3.org/2004/02/skos/core#broader> <http://w3.id.org/def/BiomassOntology#4-AquaticBiomass> ;
                                                         <http://www.w3.org/2004/02/skos/core#inScheme> :BiomassScheme ;
                                                         <http://www.w3.org/2004/02/skos/core#definition> "Aquatic biomass consisting of water hyacinth."@en ;
                                                         <http://www.w3.org/2004/02/skos/core#prefLabel> "4.2 Water hyacinth"@en .


###  http://w3.id.org/def/BiomassOntology#4-3-LakeSeaGrass
<http://w3.id.org/def/BiomassOntology#4-3-LakeSeaGrass> rdf:type owl:NamedIndividual ,
                                                                 <http://www.w3.org/2004/02/skos/core#Concept> ;
                                                        <http://www.w3.org/2004/02/skos/core#broader> <http://w3.id.org/def/BiomassOntology#4-AquaticBiomass> ;
                                                        <http://www.w3.org/2004/02/skos/core#inScheme> :BiomassScheme ;
                                                        <http://www.w3.org/2004/02/skos/core#definition> "Aquatic biomass consisting of lake and sea grass."@en ;
                                                        <http://www.w3.org/2004/02/skos/core#prefLabel> "4.3. Lake and sea grass"@en .


###  http://w3.id.org/def/BiomassOntology#4-3-1-LakeGrass
<http://w3.id.org/def/BiomassOntology#4-3-1-LakeGrass> rdf:type owl:NamedIndividual ,
                                                                <http://www.w3.org/2004/02/skos/core#Concept> ;
                                                       <http://www.w3.org/2004/02/skos/core#broader> <http://w3.id.org/def/BiomassOntology#4-3-LakeSeaGrass> ;
                                                       <http://www.w3.org/2004/02/skos/core#inScheme> :BiomassScheme ;
                                                       <http://www.w3.org/2004/02/skos/core#definition> "Aquatic biomass consisting of lake grass."@en ;
                                                       <http://www.w3.org/2004/02/skos/core#prefLabel> "4.3.1. Lake grass (Latin name to be stated)"@en .


###  http://w3.id.org/def/BiomassOntology#4-3-2-SeaGrass
<http://w3.id.org/def/BiomassOntology#4-3-2-SeaGrass> rdf:type owl:NamedIndividual ,
                                                               <http://www.w3.org/2004/02/skos/core#Concept> ;
                                                      <http://www.w3.org/2004/02/skos/core#broader> <http://w3.id.org/def/BiomassOntology#4-3-LakeSeaGrass> ;
                                                      <http://www.w3.org/2004/02/skos/core#inScheme> :BiomassScheme ;
                                                      <http://www.w3.org/2004/02/skos/core#definition> "Aquatic biomass consisting of sea grass."@en ;
                                                      <http://www.w3.org/2004/02/skos/core#prefLabel> "4.3.2. Sea grass (Latin name to be stated)"@en .


###  http://w3.id.org/def/BiomassOntology#4-3-3-BlendsMixtures
<http://w3.id.org/def/BiomassOntology#4-3-3-BlendsMixtures> rdf:type owl:NamedIndividual ,
                                                                     <http://www.w3.org/2004/02/skos/core#Concept> ;
                                                            <http://www.w3.org/2004/02/skos/core#broader> <http://w3.id.org/def/BiomassOntology#4-3-LakeSeaGrass> ;
                                                            <http://www.w3.org/2004/02/skos/core#inScheme> :BiomassScheme ;
                                                            <http://www.w3.org/2004/02/skos/core#definition> "This refers to blends and mixtures of lake and sea grass in the groups 4.3.1 to 4.3.2. The mixing can be either intentional (blends) or unintentional (mixtures)."@en ;
                                                            <http://www.w3.org/2004/02/skos/core#prefLabel> "4.3.3. Blends and mixtures"@en .


###  http://w3.id.org/def/BiomassOntology#4-4-Reeds
<http://w3.id.org/def/BiomassOntology#4-4-Reeds> rdf:type owl:NamedIndividual ,
                                                          <http://www.w3.org/2004/02/skos/core#Concept> ;
                                                 <http://www.w3.org/2004/02/skos/core#broader> <http://w3.id.org/def/BiomassOntology#4-AquaticBiomass> ;
                                                 <http://www.w3.org/2004/02/skos/core#inScheme> :BiomassScheme ;
                                                 <http://www.w3.org/2004/02/skos/core#definition> "Aquatic biomass consisting of reeds."@en ;
                                                 <http://www.w3.org/2004/02/skos/core#prefLabel> "4.4 Reeds"@en .


###  http://w3.id.org/def/BiomassOntology#4-4-1-CommonReed
<http://w3.id.org/def/BiomassOntology#4-4-1-CommonReed> rdf:type owl:NamedIndividual ,
                                                                 <http://www.w3.org/2004/02/skos/core#Concept> ;
                                                        <http://www.w3.org/2004/02/skos/core#broader> <http://w3.id.org/def/BiomassOntology#4-4-Reeds> ;
                                                        <http://www.w3.org/2004/02/skos/core#inScheme> :BiomassScheme ;
                                                        <http://www.w3.org/2004/02/skos/core#definition> "Aquatic biomass consisting of common reed."@en ;
                                                        <http://www.w3.org/2004/02/skos/core#prefLabel> "4.4.1. Common reed"@en .


###  http://w3.id.org/def/BiomassOntology#4-4-2-OtherReed
<http://w3.id.org/def/BiomassOntology#4-4-2-OtherReed> rdf:type owl:NamedIndividual ,
                                                                <http://www.w3.org/2004/02/skos/core#Concept> ;
                                                       <http://www.w3.org/2004/02/skos/core#broader> <http://w3.id.org/def/BiomassOntology#4-4-Reeds> ;
                                                       <http://www.w3.org/2004/02/skos/core#inScheme> :BiomassScheme ;
                                                       <http://www.w3.org/2004/02/skos/core#definition> "Aquatic biomass consisting of other reed rather than common reed."@en ;
                                                       <http://www.w3.org/2004/02/skos/core#prefLabel> "4.4.2. Other reed"@en .


###  http://w3.id.org/def/BiomassOntology#4-4-3-BlendsMixtures
<http://w3.id.org/def/BiomassOntology#4-4-3-BlendsMixtures> rdf:type owl:NamedIndividual ,
                                                                     <http://www.w3.org/2004/02/skos/core#Concept> ;
                                                            <http://www.w3.org/2004/02/skos/core#broader> <http://w3.id.org/def/BiomassOntology#4-4-Reeds> ;
                                                            <http://www.w3.org/2004/02/skos/core#inScheme> :BiomassScheme ;
                                                            <http://www.w3.org/2004/02/skos/core#definition> "This refers to blends and mixtures of reeds in the groups 4.4.1 to 4.4.2. The mixing can be either intentional (blends) or unintentional (mixtures)."@en ;
                                                            <http://www.w3.org/2004/02/skos/core#prefLabel> "4.4.3. Blends and mixtures"@en .


###  http://w3.id.org/def/BiomassOntology#4-5-BlendsMixtures
<http://w3.id.org/def/BiomassOntology#4-5-BlendsMixtures> rdf:type owl:NamedIndividual ,
                                                                   <http://www.w3.org/2004/02/skos/core#Concept> ;
                                                          <http://www.w3.org/2004/02/skos/core#broader> <http://w3.id.org/def/BiomassOntology#4-AquaticBiomass> ;
                                                          <http://www.w3.org/2004/02/skos/core#inScheme> :BiomassScheme ;
                                                          <http://www.w3.org/2004/02/skos/core#definition> "This refers to blends and mixtures of aquatic biomass in the groups 4.1 to 4.4. The mixing can be either intentional (blends) or unintentional (mixtures)."@en ;
                                                          <http://www.w3.org/2004/02/skos/core#prefLabel> "4.5. Blends and mixtures"@en .


###  http://w3.id.org/def/BiomassOntology#5-BlendsMixtures
<http://w3.id.org/def/BiomassOntology#5-BlendsMixtures> rdf:type owl:NamedIndividual ,
                                                                 <http://www.w3.org/2004/02/skos/core#Concept> ;
                                                        <http://www.w3.org/2004/02/skos/core#topConceptOf> :BiomassScheme ;
                                                        <http://www.w3.org/2004/02/skos/core#definition> "Material of various origin within the given box in the classification table and appears on all four classification levels (groups from 1. to 4.)."@en ;
                                                        <http://www.w3.org/2004/02/skos/core#prefLabel> "5. Blends and mixtures"@en .


###  http://w3.id.org/def/BiomassOntology#5-1-Blends
<http://w3.id.org/def/BiomassOntology#5-1-Blends> rdf:type owl:NamedIndividual ,
                                                           <http://www.w3.org/2004/02/skos/core#Concept> ;
                                                  <http://www.w3.org/2004/02/skos/core#broader> <http://w3.id.org/def/BiomassOntology#5-BlendsMixtures> ;
                                                  <http://www.w3.org/2004/02/skos/core#inScheme> :BiomassScheme ;
                                                  <http://www.w3.org/2004/02/skos/core#definition> "Intentionally mixed biofuels."@en ;
                                                  <http://www.w3.org/2004/02/skos/core#prefLabel> "5.1. Blends"@en .


###  http://w3.id.org/def/BiomassOntology#5-2-Mixtures
<http://w3.id.org/def/BiomassOntology#5-2-Mixtures> rdf:type owl:NamedIndividual ,
                                                             <http://www.w3.org/2004/02/skos/core#Concept> ;
                                                    <http://www.w3.org/2004/02/skos/core#broader> <http://w3.id.org/def/BiomassOntology#5-BlendsMixtures> ;
                                                    <http://www.w3.org/2004/02/skos/core#inScheme> :BiomassScheme ;
                                                    <http://www.w3.org/2004/02/skos/core#definition> "Unintentionally mixed biofuels."@en ;
                                                    <http://www.w3.org/2004/02/skos/core#prefLabel> "5.2. Mixtures"@en .


###  http://w3.id.org/def/BiomassOntology#A10+Bale
<http://w3.id.org/def/BiomassOntology#A10+Bale> rdf:type owl:NamedIndividual ,
                                                         :BaleResult ;
                                                rdfs:comment "> 10 % in mass of ash of dry basis in bale"@en ;
                                                rdfs:label "A10.0+ Bale"@en .


###  http://w3.id.org/def/BiomassOntology#A10+Bark
<http://w3.id.org/def/BiomassOntology#A10+Bark> rdf:type owl:NamedIndividual ,
                                                         :BarkResult ;
                                                rdfs:comment "> 10,0 % in mass of ash of dry basis in bark"@en ;
                                                rdfs:label "A10.0+ Bark"@en .


###  http://w3.id.org/def/BiomassOntology#A10+Briquette
<http://w3.id.org/def/BiomassOntology#A10+Briquette> rdf:type owl:NamedIndividual ,
                                                              :BriquetteResult ;
                                                     rdfs:comment "> 10,0 % in mass of ash in briquettes as received"@en ;
                                                     rdfs:label "A10.0+ Briquette"@en .


###  http://w3.id.org/def/BiomassOntology#A10+FruitSeeds
<http://w3.id.org/def/BiomassOntology#A10+FruitSeeds> rdf:type owl:NamedIndividual ,
                                                               :FruitSeedsResult ;
                                                      rdfs:comment "> 10,0 % in mass of ash in fruit seeds of dry basis"@en ;
                                                      rdfs:label "A10.0+ FruitSeeds"@en .


###  http://w3.id.org/def/BiomassOntology#A10+OliveResidues
<http://w3.id.org/def/BiomassOntology#A10+OliveResidues> rdf:type owl:NamedIndividual ,
                                                                  :OliveResiduesResult ;
                                                         rdfs:comment "> 10,0 % in mass of ash in olive residues of dry basis"@en ;
                                                         rdfs:label "A10.0+ OliveResidues"@en .


###  http://w3.id.org/def/BiomassOntology#A10+Pellet
<http://w3.id.org/def/BiomassOntology#A10+Pellet> rdf:type owl:NamedIndividual ,
                                                           :PelletResult ;
                                                  rdfs:comment "> 10,0 % in mass of ash of dry basis in pellets"@en ;
                                                  rdfs:label "A10.0+ Pellet"@en .


###  http://w3.id.org/def/BiomassOntology#A10+Sawdust
<http://w3.id.org/def/BiomassOntology#A10+Sawdust> rdf:type owl:NamedIndividual ,
                                                            :SawdustResult ;
                                                   rdfs:comment "> 10,0 % in mass of ash in sawdust of dry basis"@en ;
                                                   rdfs:label "A10.0+ Sawdust"@en .


###  http://w3.id.org/def/BiomassOntology#A10+Shavings
<http://w3.id.org/def/BiomassOntology#A10+Shavings> rdf:type owl:NamedIndividual ,
                                                             :ShavingsResult ;
                                                    rdfs:comment "> 10,0 % in mass of ash of dry basis in shavings"@en ;
                                                    rdfs:label "A10.0+ Shavings"@en .


###  http://w3.id.org/def/BiomassOntology#A10+WoodChipsHogFuel
<http://w3.id.org/def/BiomassOntology#A10+WoodChipsHogFuel> rdf:type owl:NamedIndividual ,
                                                                     :WoodChipsHogFuelResult ;
                                                            rdfs:comment "> 10,0 % in mass of ash in wood chips/hog fuel of dry basis"@en ;
                                                            rdfs:label "A10.0+ Wood Chips/Hog Fuel"@en .


###  http://w3.id.org/def/BiomassOntology#A5+EnergyGrain
<http://w3.id.org/def/BiomassOntology#A5+EnergyGrain> rdf:type owl:NamedIndividual ,
                                                               :EnergyGrainResult ;
                                                      rdfs:comment "> 5,0 % in mass of ash in energy grain of dry basis"@en ;
                                                      rdfs:label "A5.0+ EnergyGrain"@en .


###  http://w3.id.org/def/BiomassOntology#A8+Charcoal
<http://w3.id.org/def/BiomassOntology#A8+Charcoal> rdf:type owl:NamedIndividual ,
                                                            :CharcoalResult ;
                                                   rdfs:comment "> 8,0 % in mass of ash in charcoal of dry basis"@en ;
                                                   rdfs:label "A8.0+ Charcoal"@en .


###  http://w3.id.org/def/BiomassOntology#BD240+Bale
<http://w3.id.org/def/BiomassOntology#BD240+Bale> rdf:type owl:NamedIndividual ,
                                                           :BaleResult ;
                                                  rdfs:comment "≥ 240 kg/m3 bulk density of bale as received"@en ;
                                                  rdfs:label "BD240+ Bale"@en .


###  http://w3.id.org/def/BiomassOntology#BD350+Shavings
<http://w3.id.org/def/BiomassOntology#BD350+Shavings> rdf:type owl:NamedIndividual ,
                                                               :ShavingsResult ;
                                                      rdfs:comment "> 350 kg/m3 bulk density of shavings as received"@en ;
                                                      rdfs:label "BD350+ Shavings"@en .


###  http://w3.id.org/def/BiomassOntology#BD400+Sawdust
<http://w3.id.org/def/BiomassOntology#BD400+Sawdust> rdf:type owl:NamedIndividual ,
                                                              :SawdustResult ;
                                                     rdfs:comment "> 400 kg/m3 bulk density of sawdust as received"@en ;
                                                     rdfs:label "BD400+ Sawdust"@en .


###  http://w3.id.org/def/BiomassOntology#BD450+WoodChipsHogFuel
<http://w3.id.org/def/BiomassOntology#BD450+WoodChipsHogFuel> rdf:type owl:NamedIndividual ,
                                                                       :WoodChipsHogFuelResult ;
                                                              rdfs:comment "> 450 kg/ m3 bulk density of wood chips/ hog fuel as received"@en ;
                                                              rdfs:label "BD450+ Wood Chips/Hog Fuel"@en .


###  http://w3.id.org/def/BiomassOntology#BD650+EnergyGrain
<http://w3.id.org/def/BiomassOntology#BD650+EnergyGrain> rdf:type owl:NamedIndividual ,
                                                                  :EnergyGrainResult ;
                                                         rdfs:comment "> 650 kg/m3 bulk density of energy grain as received"@en ;
                                                         rdfs:label "BD650+ EnergyGrain"@en .


###  http://w3.id.org/def/BiomassOntology#BD800+Pellet
<http://w3.id.org/def/BiomassOntology#BD800+Pellet> rdf:type owl:NamedIndividual ,
                                                             :PelletResult ;
                                                    rdfs:comment "> 800 kg/m3, pellet bulk density as received"@en ;
                                                    rdfs:label "BD800+ Pellet"@en .


###  http://w3.id.org/def/BiomassOntology#Cl0.1+Bale
<http://w3.id.org/def/BiomassOntology#Cl0.1+Bale> rdf:type owl:NamedIndividual ,
                                                           :BaleResult ;
                                                  rdfs:comment "> 0,10 % in mass of chlorine of dry basis in bale"@en ;
                                                  rdfs:label "Cl0.10+ Bale"@en .


###  http://w3.id.org/def/BiomassOntology#Cl0.1+Bark
<http://w3.id.org/def/BiomassOntology#Cl0.1+Bark> rdf:type owl:NamedIndividual ,
                                                           :BarkResult ;
                                                  rdfs:comment "> 0,10 % in mass of chlorine of dry basis in bark"@en ;
                                                  rdfs:label "Cl0.10+ Bark"@en .


###  http://w3.id.org/def/BiomassOntology#Cl0.1+Sawdust
<http://w3.id.org/def/BiomassOntology#Cl0.1+Sawdust> rdf:type owl:NamedIndividual ,
                                                              :SawdustResult ;
                                                     rdfs:comment "> 0,10 % in mass of chlorine of dry basis in sawdust"@en ;
                                                     rdfs:label "Cl0.10+ Sawdust"@en .


###  http://w3.id.org/def/BiomassOntology#Cl0.1+Shavings
<http://w3.id.org/def/BiomassOntology#Cl0.1+Shavings> rdf:type owl:NamedIndividual ,
                                                               :ShavingsResult ;
                                                      rdfs:comment "> 0,10 % in mass of chlorine in shavings of dry basis"@en ;
                                                      rdfs:label "Cl0.10+ Shavings"@en .


###  http://w3.id.org/def/BiomassOntology#Cl0.1+WoodChipsHogFuel
<http://w3.id.org/def/BiomassOntology#Cl0.1+WoodChipsHogFuel> rdf:type owl:NamedIndividual ,
                                                                       :WoodChipsHogFuelResult ;
                                                              rdfs:comment "> 0,10 % in mass of chlorine in wood chips/hog fuel of dry basis"@en ;
                                                              rdfs:label "Cl0.10+ Wood Chips/Hog Fuel"@en .


###  http://w3.id.org/def/BiomassOntology#Cl0.15+EnergyGrain
<http://w3.id.org/def/BiomassOntology#Cl0.15+EnergyGrain> rdf:type owl:NamedIndividual ,
                                                                   :EnergyGrainResult ;
                                                          rdfs:comment "> 0,15 % in mass of chlorine in energy grain of dry basis"@en ;
                                                          rdfs:label "Cl0.15+ EnergyGrain"@en .


###  http://w3.id.org/def/BiomassOntology#Cl0.15+FruitSeeds
<http://w3.id.org/def/BiomassOntology#Cl0.15+FruitSeeds> rdf:type owl:NamedIndividual ,
                                                                  :FruitSeedsResult ;
                                                         rdfs:comment "> 0,15 % in mass of chlorine in fruit seeds of dry basis"@en ;
                                                         rdfs:label "Cl0.15+ FruitSeeds"@en .


###  http://w3.id.org/def/BiomassOntology#Cl0.15+OliveResidues
<http://w3.id.org/def/BiomassOntology#Cl0.15+OliveResidues> rdf:type owl:NamedIndividual ,
                                                                     :OliveResiduesResult ;
                                                            rdfs:comment "> 0,15 % in mass of chlorine in olive residues of dry basis"@en ;
                                                            rdfs:label "Cl0.15+ OliveResidues"@en .


###  http://w3.id.org/def/BiomassOntology#Cl0.3+Briquette
<http://w3.id.org/def/BiomassOntology#Cl0.3+Briquette> rdf:type owl:NamedIndividual ,
                                                                :BriquetteResult ;
                                                       rdfs:comment "> 0,30 % in mass of chlorine in briquettes of dry basis"@en ;
                                                       rdfs:label "Cl0.30+ Briquette"@en .


###  http://w3.id.org/def/BiomassOntology#Cl0.3+Pellet
<http://w3.id.org/def/BiomassOntology#Cl0.3+Pellet> rdf:type owl:NamedIndividual ,
                                                             :PelletResult ;
                                                    rdfs:comment "> 0,30 % in mass of chlorine in pellets of dry basis"@en ;
                                                    rdfs:label "Cl0.30+ Pellet"@en .


###  http://w3.id.org/def/BiomassOntology#D10+FruitSeeds
<http://w3.id.org/def/BiomassOntology#D10+FruitSeeds> rdf:type owl:NamedIndividual ,
                                                               :FruitSeedsResult ;
                                                      rdfs:comment "≥ 10 mm diameter of fruit seeds, (5 % in mass may have diameter over the class)"@en ;
                                                      rdfs:label "D10+ FruitSeeds"@en .


###  http://w3.id.org/def/BiomassOntology#D10+OliveResidues
<http://w3.id.org/def/BiomassOntology#D10+OliveResidues> rdf:type owl:NamedIndividual ,
                                                                  :OliveResiduesResult ;
                                                         rdfs:comment "≥ 10 mm diameter of olive residues"@en ;
                                                         rdfs:label "D10+ OliveResidues"@en .


###  http://w3.id.org/def/BiomassOntology#DE1.2+Briquette
<http://w3.id.org/def/BiomassOntology#DE1.2+Briquette> rdf:type owl:NamedIndividual ,
                                                                :BriquetteResult ;
                                                       rdfs:comment "> 1,2 g/cm3 briquette density as received"@en ;
                                                       rdfs:label "DE1.2+ Briquette"@en .


###  http://w3.id.org/def/BiomassOntology#F1+EnergyGrain
<http://w3.id.org/def/BiomassOntology#F1+EnergyGrain> rdf:type owl:NamedIndividual ,
                                                               :EnergyGrainResult ;
                                                      rdfs:comment "> 1,0 % in mass of  fines in energy grain,  fines < 3,15 mm for D 10"@en ;
                                                      rdfs:label "F1.0+ EnergyGrain"@en .


###  http://w3.id.org/def/BiomassOntology#F1+OliveResidues
<http://w3.id.org/def/BiomassOntology#F1+OliveResidues> rdf:type owl:NamedIndividual ,
                                                                 :OliveResiduesResult ;
                                                        rdfs:comment "> 1,0 % in mass of  fines in olive residues, fines < 3,15 mm for D 10 and D10+"@en ;
                                                        rdfs:label "F1.0+ OliveResidues"@en .


###  http://w3.id.org/def/BiomassOntology#F30+WoodChipsHogFuel
<http://w3.id.org/def/BiomassOntology#F30+WoodChipsHogFuel> rdf:type owl:NamedIndividual ,
                                                                     :WoodChipsHogFuelResult ;
                                                            rdfs:comment "> 30 % in mass of fines, < 3,15 mm particles"@en ;
                                                            rdfs:label "F30+ Wood Chips/Hog Fuel"@en .


###  http://w3.id.org/def/BiomassOntology#F6+Pellet
<http://w3.id.org/def/BiomassOntology#F6+Pellet> rdf:type owl:NamedIndividual ,
                                                          :PelletResult ;
                                                 rdfs:comment "> 6,0 % in mass of fines, particles < 3,15 mm. after production when loaded or packed"@en ;
                                                 rdfs:label "F6.0+ Pellet"@en .


###  http://w3.id.org/def/BiomassOntology#Fs1+EnergyGrain
<http://w3.id.org/def/BiomassOntology#Fs1+EnergyGrain> rdf:type owl:NamedIndividual ,
                                                                :EnergyGrainResult ;
                                                       rdfs:comment "> 1,0 % in mass of small fines in energy grain, small fines (Fs)< 1 mm for D 05"@en ;
                                                       rdfs:label "Fs1.0+ EnergyGrain"@en .


###  http://w3.id.org/def/BiomassOntology#Fs1+FruitSeeds
<http://w3.id.org/def/BiomassOntology#Fs1+FruitSeeds> rdf:type owl:NamedIndividual ,
                                                               :FruitSeedsResult ;
                                                      rdfs:comment "> 1,0 % in mass of small fines in fruit seeds, small fines < 1 mm"@en ;
                                                      rdfs:label "Fs1.0+ FruitSeeds"@en .


###  http://w3.id.org/def/BiomassOntology#Fs1+OliveResidues
<http://w3.id.org/def/BiomassOntology#Fs1+OliveResidues> rdf:type owl:NamedIndividual ,
                                                                  :OliveResiduesResult ;
                                                         rdfs:comment "> 1,0 % in mass of small fines in olive residues, small fines < 1 mm for for D 03 and D 05"@en ;
                                                         rdfs:label "Fs1.0+ OliveResidues"@en .


###  http://w3.id.org/def/BiomassOntology#L100+LogFirewood
<http://w3.id.org/def/BiomassOntology#L100+LogFirewood> rdf:type owl:NamedIndividual ,
                                                                 :LogFirewoodResult ;
                                                        rdfs:comment "> 100 cm maximum length of a single piece of log wood/ firewood"@en ;
                                                        rdfs:label "L100+ Log wood/Firewood"@en .


###  http://w3.id.org/def/BiomassOntology#M30+Bale
<http://w3.id.org/def/BiomassOntology#M30+Bale> rdf:type owl:NamedIndividual ,
                                                         :BaleResult ;
                                                rdfs:comment "> 30 % in mass of moisture in bale as received"@en ;
                                                rdfs:label "M30+ Bale"@en .


###  http://w3.id.org/def/BiomassOntology#M30+Shavings
<http://w3.id.org/def/BiomassOntology#M30+Shavings> rdf:type owl:NamedIndividual ,
                                                             :ShavingsResult ;
                                                    rdfs:comment "> 30 % in mass of moisture in shavings as received"@en ;
                                                    rdfs:label "M30+ Shavings"@en .


###  http://w3.id.org/def/BiomassOntology#M55+LogFirewood
<http://w3.id.org/def/BiomassOntology#M55+LogFirewood> rdf:type owl:NamedIndividual ,
                                                                :LogFirewoodResult ;
                                                       rdfs:comment "> 55% in mass of moisture as received on wet basis of log wood/ firewood"@en ;
                                                       rdfs:label "M55+ Log wood/Firewood"@en .


###  http://w3.id.org/def/BiomassOntology#M55+WoodChipsHogFuel
<http://w3.id.org/def/BiomassOntology#M55+WoodChipsHogFuel> rdf:type owl:NamedIndividual ,
                                                                     :WoodChipsHogFuelResult ;
                                                            rdfs:comment "> 55 % in mass of moisture in wood chips/hog fuel as received"@en ;
                                                            rdfs:label "M55+ Wood Chips/Hog Fuel"@en .


###  http://w3.id.org/def/BiomassOntology#M65+Bark
<http://w3.id.org/def/BiomassOntology#M65+Bark> rdf:type owl:NamedIndividual ,
                                                         :BarkResult ;
                                                rdfs:comment "> 65 % in mass of moisture in bark as received"@en ;
                                                rdfs:label "M65+ Bark"@en .


###  http://w3.id.org/def/BiomassOntology#M65+Sawdust
<http://w3.id.org/def/BiomassOntology#M65+Sawdust> rdf:type owl:NamedIndividual ,
                                                            :SawdustResult ;
                                                   rdfs:comment "> 65 % in mass of moisture in sawdust as received"@en ;
                                                   rdfs:label "M65+ Sawdust"@en .


###  http://w3.id.org/def/BiomassOntology#N2+Bale
<http://w3.id.org/def/BiomassOntology#N2+Bale> rdf:type owl:NamedIndividual ,
                                                        :BaleResult ;
                                               rdfs:comment "> 2,0 % in mass of nitrogen of dry basis in bale"@en ;
                                               rdfs:label "N2.0+ Bale"@en .


###  http://w3.id.org/def/BiomassOntology#N2+EnergyGrain
<http://w3.id.org/def/BiomassOntology#N2+EnergyGrain> rdf:type owl:NamedIndividual ,
                                                               :EnergyGrainResult ;
                                                      rdfs:comment "> 2,0 % in mass of nitrogen in energy grain of dry basis"@en ;
                                                      rdfs:label "N2.0+ EnergyGrain"@en .


###  http://w3.id.org/def/BiomassOntology#N3+Bark
<http://w3.id.org/def/BiomassOntology#N3+Bark> rdf:type owl:NamedIndividual ,
                                                        :BarkResult ;
                                               rdfs:comment "> 3,0 % in mass of nitrogen of dry basis in bark"@en ;
                                               rdfs:label "N3.0+ Bark"@en .


###  http://w3.id.org/def/BiomassOntology#N3+Briquette
<http://w3.id.org/def/BiomassOntology#N3+Briquette> rdf:type owl:NamedIndividual ,
                                                             :BriquetteResult ;
                                                    rdfs:comment "> 3,0 % in mass of nitrogen in briquettes of dry basis"@en ;
                                                    rdfs:label "N3.0+ Briquette"@en .


###  http://w3.id.org/def/BiomassOntology#N3+FruitSeeds
<http://w3.id.org/def/BiomassOntology#N3+FruitSeeds> rdf:type owl:NamedIndividual ,
                                                              :FruitSeedsResult ;
                                                     rdfs:comment "> 3,0 % in mass of nitrogen in fruit seeds of dry basis"@en ;
                                                     rdfs:label "N3.0+ FruitSeeds"@en .


###  http://w3.id.org/def/BiomassOntology#N3+OliveResidues
<http://w3.id.org/def/BiomassOntology#N3+OliveResidues> rdf:type owl:NamedIndividual ,
                                                                 :OliveResiduesResult ;
                                                        rdfs:comment "> 3,0 % in mass of nitrogen in olive residues of dry basis"@en ;
                                                        rdfs:label "N3.0+ OliveResidues"@en .


###  http://w3.id.org/def/BiomassOntology#N3+Pellet
<http://w3.id.org/def/BiomassOntology#N3+Pellet> rdf:type owl:NamedIndividual ,
                                                          :PelletResult ;
                                                 rdfs:comment "> 3,0 % in mass of nitrogen in pellets of dry basis"@en ;
                                                 rdfs:label "N3.0+ Pellet"@en .


###  http://w3.id.org/def/BiomassOntology#N3+Sawdust
<http://w3.id.org/def/BiomassOntology#N3+Sawdust> rdf:type owl:NamedIndividual ,
                                                           :SawdustResult ;
                                                  rdfs:comment "> 3,0 % in mass of nitrogen of dry basis in sawdust"@en ;
                                                  rdfs:label "N3.0+ Sawdust"@en .


###  http://w3.id.org/def/BiomassOntology#N3+Shavings
<http://w3.id.org/def/BiomassOntology#N3+Shavings> rdf:type owl:NamedIndividual ,
                                                            :ShavingsResult ;
                                                   rdfs:comment "> 3,0 % in mass of nitrogen in shavings of dry basis"@en ;
                                                   rdfs:label "N3.0+ Shavings"@en .


###  http://w3.id.org/def/BiomassOntology#N3+WoodChipsHogFuel
<http://w3.id.org/def/BiomassOntology#N3+WoodChipsHogFuel> rdf:type owl:NamedIndividual ,
                                                                    :WoodChipsHogFuelResult ;
                                                           rdfs:comment "> 3,0 % in mass of nitrogen in wood chips/hog fuel of dry basis"@en ;
                                                           rdfs:label "N3.0+ Wood Chips/Hog Fuel"@en .


###  http://w3.id.org/def/BiomassOntology#P3+Bale
<http://w3.id.org/def/BiomassOntology#P3+Bale> rdf:type owl:NamedIndividual ,
                                                        :BaleResult ;
                                               rdfs:comment "Square bale; Length (L 1) > 3 m (value to be stated); Width (L 2) > 1,2 m (value to be stated); Height (L 3) > 3 m (value to be stated)"@en ;
                                               rdfs:label "P3+ Bale"@en .


###  http://w3.id.org/def/BiomassOntology#PL30+WoodChipsHogFuel
<http://w3.id.org/def/BiomassOntology#PL30+WoodChipsHogFuel> rdf:type owl:NamedIndividual ,
                                                                      :WoodChipsHogFuelResult ;
                                                             rdfs:comment "Dimensions of wood chips or hog fuel. Mass of long particles (100 mm ≤ m ≤ maximum length of particle), m > 30 % (value to be stated) in mass"@en ;
                                                             rdfs:label "PL30+ Wood Chip/Hog Fuel"@en .


###  http://w3.id.org/def/BiomassOntology#S0.1+WoodChipsHogFuel
<http://w3.id.org/def/BiomassOntology#S0.1+WoodChipsHogFuel> rdf:type owl:NamedIndividual ,
                                                                      :WoodChipsHogFuelResult ;
                                                             rdfs:comment "> 0,10 % in mass of sulfur in wood chips/hog fuel of dry basis"@en ;
                                                             rdfs:label "S0.10+ Wood Chips/Hog Fuel"@en .


###  http://w3.id.org/def/BiomassOntology#S0.2+EnergyGrain
<http://w3.id.org/def/BiomassOntology#S0.2+EnergyGrain> rdf:type owl:NamedIndividual ,
                                                                 :EnergyGrainResult ;
                                                        rdfs:comment "> 0,20 % in mass of sulfur in energy grain of dry basis"@en ;
                                                        rdfs:label "S0.2+ EnergyGrain"@en .


###  http://w3.id.org/def/BiomassOntology#S0.2+FruitSeeds
<http://w3.id.org/def/BiomassOntology#S0.2+FruitSeeds> rdf:type owl:NamedIndividual ,
                                                                :FruitSeedsResult ;
                                                       rdfs:comment "> 0,20 % in mass of sulfur in fruit seeds of dry basis"@en ;
                                                       rdfs:label "S0.20+ FruitSeeds"@en .


###  http://w3.id.org/def/BiomassOntology#S0.2+OliveResidues
<http://w3.id.org/def/BiomassOntology#S0.2+OliveResidues> rdf:type owl:NamedIndividual ,
                                                                   :OliveResiduesResult ;
                                                          rdfs:comment "> 0,20 % in mass of sulfur in olive residues of dry basis"@en ;
                                                          rdfs:label "S0.20+ OliveResidues"@en .


###  http://w3.id.org/def/BiomassOntology#S0.3+Briquette
<http://w3.id.org/def/BiomassOntology#S0.3+Briquette> rdf:type owl:NamedIndividual ,
                                                               :BriquetteResult ;
                                                      rdfs:comment "> 0,30 % in mass of sulfur in briquettes of dry basis"@en ;
                                                      rdfs:label "S0.30+ Briquette"@en .


###  http://w3.id.org/def/BiomassOntology#S0.3+Pellet
<http://w3.id.org/def/BiomassOntology#S0.3+Pellet> rdf:type owl:NamedIndividual ,
                                                            :PelletResult ;
                                                   rdfs:comment "> 0,30 % in mass of sulfur in pellets of dry basis"@en ;
                                                   rdfs:label "S0.30+ Pellet"@en .


###  Generated by the OWL API (version 5.1.18) https://github.com/owlcs/owlapi/
